<?xml version="1.0"?>
<rdf:RDF xmlns="http://www.ontologylibrary.mil/OperationalEnvironment/Mid/OEFutureWarfareOntology#"
     xml:base="http://www.ontologylibrary.mil/OperationalEnvironment/Mid/OEFutureWarfareOntology"
     xmlns:dc="http://purl.org/dc/elements/1.1/"
     xmlns:obo="http://purl.obolibrary.org/obo/"
     xmlns:owl="http://www.w3.org/2002/07/owl#"
     xmlns:rdf="http://www.w3.org/1999/02/22-rdf-syntax-ns#"
     xmlns:xml="http://www.w3.org/XML/1998/namespace"
     xmlns:xsd="http://www.w3.org/2001/XMLSchema#"
     xmlns:foaf="http://xmlns.com/foaf/0.1/"
     xmlns:rdfs="http://www.w3.org/2000/01/rdf-schema#"
     xmlns:CommonCoreOntologies="http://www.ontologyrepository.com/CommonCoreOntologies/">
    <owl:Ontology rdf:about="http://www.ontologylibrary.mil/OperationalEnvironment/Mid/OEFutureWarfareOntology">
        <owl:imports rdf:resource="http://purl.obolibrary.org/obo/bfo/2.0/bfo.owl"/>
        <owl:imports rdf:resource="http://www.obofoundry.org/ro/ro.owl"/>
        <owl:imports rdf:resource="http://www.ontologyrepository.com/CommonCoreOntologies/Mid/InformationEntityOntology"/>
        <owl:imports rdf:resource="http://www.ontologyrepository.com/CommonCoreOntologies/Upper/ExtendedRelationOntology"/>
        <owl:versionInfo xml:lang="mail.mil, (757) 878-9547)">DISTRIBUTION A: Approved for public release; distribution is unlimited.  For more information contact United States Army TRADOC G-27 at usarmy.jble.tradoc.list.tboc-operations@mail.mil (or Kaye Darone, Data Science Branch Chief, DSMS, Kaye.t.darone.civ</owl:versionInfo>
    </owl:Ontology>
    


    <!-- 
    ///////////////////////////////////////////////////////////////////////////////////////
    //
    // Annotation properties
    //
    ///////////////////////////////////////////////////////////////////////////////////////
     -->

    


    <!-- http://www.ontologyrepository.com/CommonCoreOntologies/definition -->

    <owl:AnnotationProperty rdf:about="http://www.ontologyrepository.com/CommonCoreOntologies/definition"/>
    


    <!-- 
    ///////////////////////////////////////////////////////////////////////////////////////
    //
    // Object Properties
    //
    ///////////////////////////////////////////////////////////////////////////////////////
     -->

    


    <!-- http://www.ontologylibrary.mil/OperationalEnvironment/Mid/OEFutureWarfareOntology#hasCategoryOfEffort -->

    <owl:ObjectProperty rdf:about="http://www.ontologylibrary.mil/OperationalEnvironment/Mid/OEFutureWarfareOntology#hasCategoryOfEffort"/>
    


    <!-- http://www.ontologylibrary.mil/OperationalEnvironment/Mid/OEFutureWarfareOntology#hasCombatApplication -->

    <owl:ObjectProperty rdf:about="http://www.ontologylibrary.mil/OperationalEnvironment/Mid/OEFutureWarfareOntology#hasCombatApplication">
        <rdfs:subPropertyOf rdf:resource="http://www.w3.org/2002/07/owl#topObjectProperty"/>
    </owl:ObjectProperty>
    


    <!-- 
    ///////////////////////////////////////////////////////////////////////////////////////
    //
    // Data properties
    //
    ///////////////////////////////////////////////////////////////////////////////////////
     -->

    


    <!-- http://www.ontologylibrary.mil/OperationalEnvironment/Mid/OEFutureWarfareOntology#EmergesInYear -->

    <owl:DatatypeProperty rdf:about="http://www.ontologylibrary.mil/OperationalEnvironment/Mid/OEFutureWarfareOntology#EmergesInYear">
        <rdfs:subPropertyOf rdf:resource="http://www.w3.org/2002/07/owl#topDataProperty"/>
        <rdfs:range rdf:resource="http://www.w3.org/2001/XMLSchema#int"/>
    </owl:DatatypeProperty>
    


    <!-- 
    ///////////////////////////////////////////////////////////////////////////////////////
    //
    // Classes
    //
    ///////////////////////////////////////////////////////////////////////////////////////
     -->

    


    <!-- http://www.ontologylibrary.mil/OperationalEnvironment/Mid/OEFutureWarfareOntology#AbilityToPrintMaterial -->

    <owl:Class rdf:about="http://www.ontologylibrary.mil/OperationalEnvironment/Mid/OEFutureWarfareOntology#AbilityToPrintMaterial">
        <rdfs:subClassOf rdf:resource="http://www.ontologylibrary.mil/OperationalEnvironment/Mid/OEFutureWarfareOntology#SystemsThatSupply"/>
        <obo:IAO_0000115>Ability to print materiel, in theater, on an as-needed basis. Example: Print a small drone with specific capabilities for a mission in 24 hours. [SOURCE: TRADOC G-2 Potential Game Changers, May 2018]

In-theater on-demand manufacturing of platform and weapon parts using high performance printable alloys and other materials, with significant performance gains using new structures and materials [SOURCE: ARL ERP documents]</obo:IAO_0000115>
        <obo:IAO_0000119>Technology Environment of Ground Warfare in 2035-2050

Projections made in 2018 by ARL and TRADOC

[This is a draft outline of a potential document; prepared by Alexander Kott, the US Army Research Laboratory; July 2018]</obo:IAO_0000119>
    </owl:Class>
    


    <!-- http://www.ontologylibrary.mil/OperationalEnvironment/Mid/OEFutureWarfareOntology#AccessControl -->

    <owl:Class rdf:about="http://www.ontologylibrary.mil/OperationalEnvironment/Mid/OEFutureWarfareOntology#AccessControl">
        <rdfs:subClassOf rdf:resource="http://www.ontologylibrary.mil/OperationalEnvironment/Mid/OEFutureWarfareOntology#CyberSecurityControlledVocabulary"/>
        <obo:IAO_0000115>means to ensure that access to assets is authorized and restricted based on business and security requirements</obo:IAO_0000115>
        <obo:IAO_0000119>International Organization for Standardization/International Electrotechnical Commission 27000:2018

Security techniques — Information security management systems — Overview and vocabulary

Publication date : 2018-02

5th Edition</obo:IAO_0000119>
    </owl:Class>
    


    <!-- http://www.ontologylibrary.mil/OperationalEnvironment/Mid/OEFutureWarfareOntology#ActiveDenialSystems -->

    <owl:Class rdf:about="http://www.ontologylibrary.mil/OperationalEnvironment/Mid/OEFutureWarfareOntology#ActiveDenialSystems">
        <rdfs:subClassOf rdf:resource="http://www.ontologylibrary.mil/OperationalEnvironment/Mid/OEFutureWarfareOntology#CombatApplication"/>
        <rdfs:subClassOf>
            <owl:Restriction>
                <owl:onProperty rdf:resource="http://www.ontologylibrary.mil/OperationalEnvironment/Mid/OEFutureWarfareOntology#hasCategoryOfEffort"/>
                <owl:someValuesFrom rdf:resource="http://www.ontologylibrary.mil/OperationalEnvironment/Mid/OEFutureWarfareOntology#SystemsThatProtect"/>
            </owl:Restriction>
        </rdfs:subClassOf>
    </owl:Class>
    


    <!-- http://www.ontologylibrary.mil/OperationalEnvironment/Mid/OEFutureWarfareOntology#ActiveProtectionSystem -->

    <owl:Class rdf:about="http://www.ontologylibrary.mil/OperationalEnvironment/Mid/OEFutureWarfareOntology#ActiveProtectionSystem">
        <rdfs:subClassOf rdf:resource="http://www.ontologylibrary.mil/OperationalEnvironment/Mid/OEFutureWarfareOntology#SystemsThatProtect"/>
        <obo:IAO_0000115>Intelligent and adaptive protective systems must alter in real time its adaptive properties depending on threats, resulting in lightweight and flexible armor that can sense impending danger, react at the “speed of the fight” to mitigate a broad range  of near peer lethal mechanisms, including Multi-hit [SOURCE: ARL ERP documents]</obo:IAO_0000115>
        <obo:IAO_0000119>Technology Environment of Ground Warfare in 2035-2050

Projections made in 2018 by ARL and TRADOC

[This is a draft outline of a potential document; prepared by Alexander Kott, the US Army Research Laboratory; July 2018]</obo:IAO_0000119>
    </owl:Class>
    


    <!-- http://www.ontologylibrary.mil/OperationalEnvironment/Mid/OEFutureWarfareOntology#AdaptiveProtectiveSystems -->

    <owl:Class rdf:about="http://www.ontologylibrary.mil/OperationalEnvironment/Mid/OEFutureWarfareOntology#AdaptiveProtectiveSystems">
        <rdfs:subClassOf rdf:resource="http://www.ontologylibrary.mil/OperationalEnvironment/Mid/OEFutureWarfareOntology#SystemsThatProtect"/>
        <obo:IAO_0000115>Intelligent and adaptive protective systems must alter in real time its adaptive properties depending on threats, resulting in lightweight and flexible armor that can sense impending danger, react at the “speed of the fight” to mitigate a broad range  of near peer lethal mechanisms, including Multi-hit [SOURCE: ARL ERP documents]</obo:IAO_0000115>
        <obo:IAO_0000119>Technology Environment of Ground Warfare in 2035-2050

Projections made in 2018 by ARL and TRADOC

[This is a draft outline of a potential document; prepared by Alexander Kott, the US Army Research Laboratory; July 2018]</obo:IAO_0000119>
    </owl:Class>
    


    <!-- http://www.ontologylibrary.mil/OperationalEnvironment/Mid/OEFutureWarfareOntology#AdvancedAirToGroundMissiles -->

    <owl:Class rdf:about="http://www.ontologylibrary.mil/OperationalEnvironment/Mid/OEFutureWarfareOntology#AdvancedAirToGroundMissiles">
        <rdfs:subClassOf rdf:resource="http://www.ontologylibrary.mil/OperationalEnvironment/Mid/OEFutureWarfareOntology#SystemsThatShoot"/>
        <obo:IAO_0000115>Extended range. Proliferate more rapidly than Active Protection systems develop, putting armored vehicles and helicopters at risk. [SOURCE: TRADOC G-2 Potential Game Changers, May 2018]</obo:IAO_0000115>
        <obo:IAO_0000119>Technology Environment of Ground Warfare in 2035-2050

Projections made in 2018 by ARL and TRADOC

[This is a draft outline of a potential document; prepared by Alexander Kott, the US Army Research Laboratory; July 2018]</obo:IAO_0000119>
    </owl:Class>
    


    <!-- http://www.ontologylibrary.mil/OperationalEnvironment/Mid/OEFutureWarfareOntology#AdvancedManPortableAirDefenseSystems -->

    <owl:Class rdf:about="http://www.ontologylibrary.mil/OperationalEnvironment/Mid/OEFutureWarfareOntology#AdvancedManPortableAirDefenseSystems">
        <rdfs:subClassOf rdf:resource="http://www.ontologylibrary.mil/OperationalEnvironment/Mid/OEFutureWarfareOntology#SystemsThatShoot"/>
        <obo:IAO_0000115>Extended range. Proliferate more rapidly than Active Protection systems develop, putting armored vehicles and helicopters at risk. [SOURCE: TRADOC G-2 Potential Game Changers, May 2018]</obo:IAO_0000115>
        <obo:IAO_0000119>Technology Environment of Ground Warfare in 2035-2050

Projections made in 2018 by ARL and TRADOC

[This is a draft outline of a potential document; prepared by Alexander Kott, the US Army Research Laboratory; July 2018]</obo:IAO_0000119>
    </owl:Class>
    


    <!-- http://www.ontologylibrary.mil/OperationalEnvironment/Mid/OEFutureWarfareOntology#AgingPopulation -->

    <owl:Class rdf:about="http://www.ontologylibrary.mil/OperationalEnvironment/Mid/OEFutureWarfareOntology#AgingPopulation">
        <rdfs:subClassOf rdf:resource="http://www.ontologylibrary.mil/OperationalEnvironment/Mid/OEFutureWarfareOntology#Demographics"/>
        <obo:IAO_0000119>(1)

&quot;Population Ageing&quot;, Wikipedia

March 25, 2019

https://en.wikipedia.org/wiki/Population_ageing</obo:IAO_0000119>
        <obo:IAO_0000119>(2)

Population Reference Bureau, &quot;Featured Graphic:  Many Countries&apos; Populations are Again&quot;, Population Reference Bureau

October 2, 2018

https://www.prb.org/insight/featured-graphic-many-countries-populations-are-aging/</obo:IAO_0000119>
        <CommonCoreOntologies:definition>(1)

Population aging is a shift in the distribution of a country&apos;s population towards older ages. This is usually reflected in an increase in the population&apos;s mean and median ages, a decline in the proportion of the population composed of children, and a rise in the proportion of the population composed of elderly.</CommonCoreOntologies:definition>
        <CommonCoreOntologies:definition>(2)

Shifts in a country’s age structure over time can have important implications for a country’s economic and social trajectory, as well as its resource allocations and policy agendas. For example, many countries in the world are experiencing—and will continue to experience—steady increases in the number of older adults, both in absolute terms and as a percentage of the total population. This trend poses challenges for countries in balancing the pension, health, and other benefits that older adults typically receive with investments in the well-being of younger generations. In addition, some countries may choose to incentivize older adults to remain in the work force longer.</CommonCoreOntologies:definition>
        <rdfs:label>Aging Population</rdfs:label>
    </owl:Class>
    


    <!-- http://www.ontologylibrary.mil/OperationalEnvironment/Mid/OEFutureWarfareOntology#Agriculture -->

    <owl:Class rdf:about="http://www.ontologylibrary.mil/OperationalEnvironment/Mid/OEFutureWarfareOntology#Agriculture">
        <rdfs:subClassOf rdf:resource="http://www.ontologylibrary.mil/OperationalEnvironment/Mid/OEFutureWarfareOntology#EconomicActivity"/>
        <obo:IAO_0000119>&quot;Agriculture&quot;, Wikipedia

March 13, 2019

https://en.wikipedia.org/wiki/Agriculture</obo:IAO_0000119>
        <CommonCoreOntologies:definition>Modern agronomy, plant breeding, agrochemicals such as pesticides and fertilizers, and technological developments have sharply increased yields, while causing widespread ecological and environmental damage. Selective breeding and modern practices in animal husbandry have similarly increased the output of meat, but have raised concerns about animal welfare and environmental damage. Environmental issues include contributions to global warming, depletion of aquifers, deforestation, antibiotic resistance, and growth hormones in industrial meat production. Genetically modified organisms are widely used, although some are banned in certain countries.

The major agricultural products can be broadly grouped into foods, fibers, fuels and raw materials (such as rubber). Food classes include cereals (grains), vegetables, fruits, oils, meat, milk, fungi and eggs.

...

From the twentieth century, intensive agriculture increased productivity. It substituted synthetic fertilizers and pesticides for labor, but caused increased water pollution, and often involved farm subsidies. In recent years there has been a backlash against the environmental effects of conventional agriculture, resulting in the organic, regenerative, and sustainable agriculture movements.</CommonCoreOntologies:definition>
        <rdfs:label>Agriculture</rdfs:label>
    </owl:Class>
    


    <!-- http://www.ontologylibrary.mil/OperationalEnvironment/Mid/OEFutureWarfareOntology#Algorithms -->

    <owl:Class rdf:about="http://www.ontologylibrary.mil/OperationalEnvironment/Mid/OEFutureWarfareOntology#Algorithms">
        <rdfs:subClassOf rdf:resource="http://www.ontologylibrary.mil/OperationalEnvironment/Mid/OEFutureWarfareOntology#SystemsThatSeeThinkCommunicate"/>
        <obo:IAO_0000115>Projected breakthroughs in algorithms that combine images to produce a coherent aperture in near real time will enable creation of “seeing skins” for high-resolution, 3-D imaging in the visible and IR bands over a large field of view. [SOURCE: ARL-TR-8283]</obo:IAO_0000115>
        <obo:IAO_0000119>Technology Environment of Ground Warfare in 2035-2050

Projections made in 2018 by ARL and TRADOC

[This is a draft outline of a potential document; prepared by Alexander Kott, the US Army Research Laboratory; July 2018]</obo:IAO_0000119>
    </owl:Class>
    


    <!-- http://www.ontologylibrary.mil/OperationalEnvironment/Mid/OEFutureWarfareOntology#AnthropogenicBiogenicGreenhouseGasEmission -->

    <owl:Class rdf:about="http://www.ontologylibrary.mil/OperationalEnvironment/Mid/OEFutureWarfareOntology#AnthropogenicBiogenicGreenhouseGasEmission">
        <rdfs:subClassOf rdf:resource="http://www.ontologylibrary.mil/OperationalEnvironment/Mid/OEFutureWarfareOntology#ClimateChangeAndResourceCompetitionControlledVocabulary"/>
        <obo:IAO_0000115>GHG emission (3.1.5) from biogenic material as a result of human activities</obo:IAO_0000115>
        <obo:IAO_0000119>International Organization for Standardization/International Electrotechnical Commission 27000:2018

Technical Committee : ISO/TC 207/SC 7  Greenhouse gas management and related activities

ICS :  13.020.40  Pollution, pollution control and conservation

Greenhouse gases -- Part 1: Specification with guidance at the organization level for quantification and reporting of greenhouse gas emissions and removals 

Publication date : 2018-12

2nd Edition</obo:IAO_0000119>
    </owl:Class>
    


    <!-- http://www.ontologylibrary.mil/OperationalEnvironment/Mid/OEFutureWarfareOntology#Anti-immigrantOpinion -->

    <owl:Class rdf:about="http://www.ontologylibrary.mil/OperationalEnvironment/Mid/OEFutureWarfareOntology#Anti-immigrantOpinion">
        <rdfs:subClassOf rdf:resource="http://www.ontologylibrary.mil/OperationalEnvironment/Mid/OEFutureWarfareOntology#Migration"/>
        <obo:IAO_0000119>&quot;Immigration and Populism&quot;, Stanford Workshop, Freeman Spogli Institute for International Studies, Stanford University

March 25, 2019

https://fsi.stanford.edu/populism-and-immigration</obo:IAO_0000119>
        <CommonCoreOntologies:definition>Critics of immigration, populist and otherwise, view it as posing unfair economic competition: whether [skilled workers], undocumented domestic and service workers, or the undercutting of wages and job availability. In addition, populist parties (among others) often charge that immigrants overuse and strain the welfare states of recipient countries.

...

One of the critical concerns of populist parties is protecting “the people” or “the nation,” defined in historical and homogenous terms. Populist parties frequently criticize immigrant and minority populations for diluting and undermining “the people” and their  well-being: in other words, these populations are a cultural threat to historical identities. At the same time, there is a broader concern with the integration of immigration populations.

...

[Electoral] data shows that the rise in immigration flows and the surge in electoral support for populist parties are closely aligned.</CommonCoreOntologies:definition>
        <rdfs:label>Anti-immigrant Opinion</rdfs:label>
    </owl:Class>
    


    <!-- http://www.ontologylibrary.mil/OperationalEnvironment/Mid/OEFutureWarfareOntology#AntiSatellite -->

    <owl:Class rdf:about="http://www.ontologylibrary.mil/OperationalEnvironment/Mid/OEFutureWarfareOntology#AntiSatellite">
        <rdfs:subClassOf rdf:resource="http://www.ontologylibrary.mil/OperationalEnvironment/Mid/OEFutureWarfareOntology#ActiveDenialSystems"/>
    </owl:Class>
    


    <!-- http://www.ontologylibrary.mil/OperationalEnvironment/Mid/OEFutureWarfareOntology#Arms -->

    <owl:Class rdf:about="http://www.ontologylibrary.mil/OperationalEnvironment/Mid/OEFutureWarfareOntology#Arms">
        <rdfs:subClassOf rdf:resource="http://www.ontologylibrary.mil/OperationalEnvironment/Mid/OEFutureWarfareOntology#SecurityAndViolentConflict"/>
    </owl:Class>
    


    <!-- http://www.ontologylibrary.mil/OperationalEnvironment/Mid/OEFutureWarfareOntology#ArmsRaces -->

    <owl:Class rdf:about="http://www.ontologylibrary.mil/OperationalEnvironment/Mid/OEFutureWarfareOntology#ArmsRaces">
        <rdfs:subClassOf rdf:resource="http://www.ontologylibrary.mil/OperationalEnvironment/Mid/OEFutureWarfareOntology#Arms"/>
    </owl:Class>
    


    <!-- http://www.ontologylibrary.mil/OperationalEnvironment/Mid/OEFutureWarfareOntology#ArtificialCells -->

    <owl:Class rdf:about="http://www.ontologylibrary.mil/OperationalEnvironment/Mid/OEFutureWarfareOntology#ArtificialCells">
        <rdfs:subClassOf rdf:resource="http://www.ontologylibrary.mil/OperationalEnvironment/Mid/OEFutureWarfareOntology#SystemsThatSupply"/>
        <obo:IAO_0000115>Projected breakthroughs in creation of artificial cells will enable on-demand, on-base production of high-value molecules, significantly reducing the logistics tail and associated transport and storage costs. [SOURCE: ARL-TR-8283]</obo:IAO_0000115>
        <obo:IAO_0000119>Technology Environment of Ground Warfare in 2035-2050

Projections made in 2018 by ARL and TRADOC

[This is a draft outline of a potential document; prepared by Alexander Kott, the US Army Research Laboratory; July 2018]</obo:IAO_0000119>
    </owl:Class>
    


    <!-- http://www.ontologylibrary.mil/OperationalEnvironment/Mid/OEFutureWarfareOntology#ArtificialIntelligenceControlledVocabulary -->

    <owl:Class rdf:about="http://www.ontologylibrary.mil/OperationalEnvironment/Mid/OEFutureWarfareOntology#ArtificialIntelligenceControlledVocabulary">
        <rdfs:subClassOf rdf:resource="http://www.ontologylibrary.mil/OperationalEnvironment/Mid/OEFutureWarfareOntology#ControlledVocabulary"/>
    </owl:Class>
    


    <!-- http://www.ontologylibrary.mil/OperationalEnvironment/Mid/OEFutureWarfareOntology#ArtificialIntelligenceTrend -->

    <owl:Class rdf:about="http://www.ontologylibrary.mil/OperationalEnvironment/Mid/OEFutureWarfareOntology#ArtificialIntelligenceTrend">
        <rdfs:subClassOf rdf:resource="http://www.ontologylibrary.mil/OperationalEnvironment/Mid/OEFutureWarfareOntology#Trend"/>
        <obo:IAO_0000115>Artificial Intelligence (AI) may be the most disruptive technology of our time: much of today’s “thought” is artificial, vice human.  Breakthroughs in AI and deep learning enable reasoning intelligent systems that, though not sentient, administer and optimize a great many aspects of modern life.  Advanced physio-mechanical interfaces enable humanmachine integration to include optimized searching of massive indexes of data, direct access to large-scale computing power, and life-like experiences through virtual reality. The revolutionary impact of “trans-humanism” challenges the very definition of “human” – with profound ethical dilemmas that remain unresolved. Big data techniques interrogate massive databases to discover hidden patterns and correlations that form the basis of modern advertising – and are continually leveraged for intelligence and security purposes by nation states and non-state entities alike.  Quantum computing, first applied to encryption functions, is now a key computing enabler, especially for artificial intelligence.9  A mature Internet of Things connects and integrates the devices of the information realm with formerly inert objects – structures, motors, or appliances -- of the physical realm.  Neuroscience has enhanced our understanding of brain function, including neural plasticity, and has enabled advanced techniques for human-machine interfacing. A better understanding of the machinery of the mind has found commercial application in the acceleration of speed and retention in learning.  In the most connected and wealthy parts of the world, cell phones and computers will all but disappear as physical, hand held devices.  Select individuals will directly connect to cyberspace through neural implants or augmented reality systems painted directly on a retina.  If we have not yet reached the “singularity”, where AI and machines are capable of outperforming the human mind, we will nonetheless have reached a point where AI, machines, and man-machine teaming open new possibilities in this realm.</obo:IAO_0000115>
        <obo:IAO_0000115>Singularity is the point at which artificial intelligence (AI) exceeds the collective intelligence of mankind, which will radically and irrevocably change the relationship between man and machine.  There are several divergent possibilities regarding the singularity: 

 As optimistic singularity advocates, such as Ray Kurzweil have suggested, AI improves human life in every way, from healthcare, to emotional evolution, to intergalactic space travel. 

 While not entirely apocalyptic, unboxed general artificial superintelligence improves and evolves at such an exponential rate it escapes human restrictions, perspectives, and morality.  It threatens the very existence of humanity. 

 Humans evolve their own cognitive abilities through learning developments, brain implants, artificial stimulants, and non-AI high performance computing to match, or at least keep pace with AI. 

AI has the capacity to change paradigms, revolutionize everyday life, and take mankind to exciting new horizons.  However, it also may be capable of incredible destruction, malice, and lines of thinking and decision-making that are dangerous to mankind.  This duality will be critical as actors develop military applications for AI.</obo:IAO_0000115>
        <obo:IAO_0000119>The Operational Environment and the Changing Character of Future Warfare</obo:IAO_0000119>
    </owl:Class>
    


    <!-- http://www.ontologylibrary.mil/OperationalEnvironment/Mid/OEFutureWarfareOntology#ArtificialLife -->

    <owl:Class rdf:about="http://www.ontologylibrary.mil/OperationalEnvironment/Mid/OEFutureWarfareOntology#ArtificialLife">
        <rdfs:subClassOf rdf:resource="http://www.ontologylibrary.mil/OperationalEnvironment/Mid/OEFutureWarfareOntology#ArtificialIntelligenceControlledVocabulary"/>
        <obo:IAO_0000115>An interdisciplinary field of research that aims to create artificial systems inspired by living systems, in the form of computer programmes or robots.</obo:IAO_0000115>
        <obo:IAO_0000119>United Nations Educational, Scientific, and Cultural Organization Courier 

March 2018

https://en.unesco.org/courier/2018-3/lexicon-artificial-intelligence</obo:IAO_0000119>
    </owl:Class>
    


    <!-- http://www.ontologylibrary.mil/OperationalEnvironment/Mid/OEFutureWarfareOntology#AssessExperts -->

    <owl:Class rdf:about="http://www.ontologylibrary.mil/OperationalEnvironment/Mid/OEFutureWarfareOntology#AssessExperts">
        <rdfs:subClassOf rdf:resource="http://www.ontologylibrary.mil/OperationalEnvironment/Mid/OEFutureWarfareOntology#FaultLineMethodology"/>
        <obo:IAO_0000115>Identify, contact, and leverage SMEs in the OE. Identify, make contact and develop a professional relationship with an expert(s) in the OE from academia, government or industry that can help guide the early research stages with baseline understanding and resource assistance.  The researcher presents the SME with their research questions and requests their expertise, understanding and research guidance to answer these questions. GCKN has a curated repository of cultural experts available to the Army to enable OE analysis.</obo:IAO_0000115>
        <obo:IAO_0000119>Fault Lines Methodology Infographic</obo:IAO_0000119>
    </owl:Class>
    


    <!-- http://www.ontologylibrary.mil/OperationalEnvironment/Mid/OEFutureWarfareOntology#Attack -->

    <owl:Class rdf:about="http://www.ontologylibrary.mil/OperationalEnvironment/Mid/OEFutureWarfareOntology#Attack">
        <rdfs:subClassOf rdf:resource="http://www.ontologylibrary.mil/OperationalEnvironment/Mid/OEFutureWarfareOntology#CyberSecurityControlledVocabulary"/>
        <obo:IAO_0000115>attempt to destroy, expose, alter, disable, steal or gain unauthorized access to or make unauthorized use of an asset</obo:IAO_0000115>
        <obo:IAO_0000119>International Organization for Standardization/International Electrotechnical Commission 27000:2018

Security techniques — Information security management systems — Overview and vocabulary

Publication date : 2018-02

5th Edition</obo:IAO_0000119>
    </owl:Class>
    


    <!-- http://www.ontologylibrary.mil/OperationalEnvironment/Mid/OEFutureWarfareOntology#Audit -->

    <owl:Class rdf:about="http://www.ontologylibrary.mil/OperationalEnvironment/Mid/OEFutureWarfareOntology#Audit">
        <rdfs:subClassOf rdf:resource="http://www.ontologylibrary.mil/OperationalEnvironment/Mid/OEFutureWarfareOntology#CyberSecurityControlledVocabulary"/>
        <obo:IAO_0000115>systematic, independent and documented process (3.54) for obtaining audit evidence and evaluating it objectively to determine the extent to which the audit criteria are fulfilled

Note 1 to entry: An audit can be an internal audit (first party) or an external audit (second party or third party), and it can be a combined audit (combining two or more disciplines).

Note 2 to entry: An internal audit is conducted by the organization itself, or by an external party on its behalf.

Note 3 to entry: “Audit evidence” and “audit criteria” are defined in ISO 19011.</obo:IAO_0000115>
        <obo:IAO_0000119>International Organization for Standardization/International Electrotechnical Commission 27000:2018

Security techniques — Information security management systems — Overview and vocabulary

Publication date : 2018-02

5th Edition</obo:IAO_0000119>
    </owl:Class>
    


    <!-- http://www.ontologylibrary.mil/OperationalEnvironment/Mid/OEFutureWarfareOntology#AuditScope -->

    <owl:Class rdf:about="http://www.ontologylibrary.mil/OperationalEnvironment/Mid/OEFutureWarfareOntology#AuditScope">
        <rdfs:subClassOf rdf:resource="http://www.ontologylibrary.mil/OperationalEnvironment/Mid/OEFutureWarfareOntology#CyberSecurityControlledVocabulary"/>
        <obo:IAO_0000115>extent and boundaries of an audit (3.3)</obo:IAO_0000115>
        <obo:IAO_0000119>International Organization for Standardization/International Electrotechnical Commission 27000:2018

Security techniques — Information security management systems — Overview and vocabulary

Publication date : 2018-02

5th Edition</obo:IAO_0000119>
    </owl:Class>
    


    <!-- http://www.ontologylibrary.mil/OperationalEnvironment/Mid/OEFutureWarfareOntology#AugmentedMan -->

    <owl:Class rdf:about="http://www.ontologylibrary.mil/OperationalEnvironment/Mid/OEFutureWarfareOntology#AugmentedMan">
        <rdfs:subClassOf rdf:resource="http://www.ontologylibrary.mil/OperationalEnvironment/Mid/OEFutureWarfareOntology#ArtificialIntelligenceControlledVocabulary"/>
        <obo:IAO_0000115>A transhumanist* ideal, the augmented man is an individual who has been subjected to modifications aimed at enhancing his performance, thanks to interventions on the body based on scientific or technological principles. Part-man, part-machine, the individual would be able to run faster, see well in the dark, withstand pain, possess enhanced intellectual abilities, resist illness or death, etc. The “repaired man” already exists and “connected” prostheses are getting better every day. The augmented man is gradually becoming a reality, with the development of artificial external skeletons used for military purposes.</obo:IAO_0000115>
        <obo:IAO_0000119>United Nations Educational, Scientific, and Cultural Organization Courier 

March 2018

https://en.unesco.org/courier/2018-3/lexicon-artificial-intelligence</obo:IAO_0000119>
    </owl:Class>
    


    <!-- http://www.ontologylibrary.mil/OperationalEnvironment/Mid/OEFutureWarfareOntology#AugmentedReality -->

    <owl:Class rdf:about="http://www.ontologylibrary.mil/OperationalEnvironment/Mid/OEFutureWarfareOntology#AugmentedReality">
        <rdfs:subClassOf rdf:resource="http://www.ontologylibrary.mil/OperationalEnvironment/Mid/OEFutureWarfareOntology#ArtificialIntelligenceControlledVocabulary"/>
        <obo:IAO_0000115>The superimposition of virtual elements onto reality, calculated by a computer system in real time (such as sounds, 2D and 3D video images, etc.). This technique is used in video games and cinema, where the spectator interacts with virtual objects through sensors. It is also used for geolocation and  heritage applications. For instance, the Cluny Abbey in France uses augmented reality screens, so visitors can visualize the town as it was in the fifteenth century.</obo:IAO_0000115>
        <obo:IAO_0000119>United Nations Educational, Scientific, and Cultural Organization Courier 

March 2018

https://en.unesco.org/courier/2018-3/lexicon-artificial-intelligence</obo:IAO_0000119>
    </owl:Class>
    


    <!-- http://www.ontologylibrary.mil/OperationalEnvironment/Mid/OEFutureWarfareOntology#Authentication -->

    <owl:Class rdf:about="http://www.ontologylibrary.mil/OperationalEnvironment/Mid/OEFutureWarfareOntology#Authentication">
        <rdfs:subClassOf rdf:resource="http://www.ontologylibrary.mil/OperationalEnvironment/Mid/OEFutureWarfareOntology#CyberSecurityControlledVocabulary"/>
        <obo:IAO_0000115>provision of assurance that a claimed characteristic of an entity is correct</obo:IAO_0000115>
        <obo:IAO_0000119>International Organization for Standardization/International Electrotechnical Commission 27000:2018

Security techniques — Information security management systems — Overview and vocabulary

Publication date : 2018-02

5th Edition</obo:IAO_0000119>
    </owl:Class>
    


    <!-- http://www.ontologylibrary.mil/OperationalEnvironment/Mid/OEFutureWarfareOntology#Authenticity -->

    <owl:Class rdf:about="http://www.ontologylibrary.mil/OperationalEnvironment/Mid/OEFutureWarfareOntology#Authenticity">
        <rdfs:subClassOf rdf:resource="http://www.ontologylibrary.mil/OperationalEnvironment/Mid/OEFutureWarfareOntology#CyberSecurityControlledVocabulary"/>
        <obo:IAO_0000115>property that an entity is what it claims to be</obo:IAO_0000115>
        <obo:IAO_0000119>International Organization for Standardization/International Electrotechnical Commission 27000:2018

Security techniques — Information security management systems — Overview and vocabulary

Publication date : 2018-02

5th Edition</obo:IAO_0000119>
    </owl:Class>
    


    <!-- http://www.ontologylibrary.mil/OperationalEnvironment/Mid/OEFutureWarfareOntology#Authoritariansim -->

    <owl:Class rdf:about="http://www.ontologylibrary.mil/OperationalEnvironment/Mid/OEFutureWarfareOntology#Authoritariansim">
        <rdfs:subClassOf rdf:resource="http://www.ontologylibrary.mil/OperationalEnvironment/Mid/OEFutureWarfareOntology#Government"/>
        <obo:IAO_0000115>Authoritarianism [is the] principle of blind submission to authority, as opposed to individual freedom of thought and action. In government, authoritarianism denotes any political system that concentrates power in the hands of a leader or a small elite that is not constitutionally responsible to the body of the people. Authoritarian leaders often exercise power arbitrarily and without regard to existing bodies of law, and they usually cannot be replaced by citizens choosing freely among various competitors in elections. The freedom to create opposition political parties or other alternative political groupings with which to compete for power with the ruling group is either limited or nonexistent in authoritarian regimes.</obo:IAO_0000115>
        <obo:IAO_0000115>Editors of Encyclopaedia Britannica &amp; Amy Tikkanen, &quot;Authoritarianism&quot;, Encyclopaedia Britannica

March 12, 2019

https://www.britannica.com/topic/authoritarianism</obo:IAO_0000115>
        <rdfs:label>Authoritarianism</rdfs:label>
    </owl:Class>
    


    <!-- http://www.ontologylibrary.mil/OperationalEnvironment/Mid/OEFutureWarfareOntology#AutonomousIntelligentMunitions -->

    <owl:Class rdf:about="http://www.ontologylibrary.mil/OperationalEnvironment/Mid/OEFutureWarfareOntology#AutonomousIntelligentMunitions">
        <rdfs:subClassOf rdf:resource="http://www.ontologylibrary.mil/OperationalEnvironment/Mid/OEFutureWarfareOntology#SystemsThatMove"/>
        <obo:IAO_0000115>Autonomous intelligent munitions will fly and navigate in highly contested environments, avoiding effects of the OPFOR countermeasures [SOURCE: ARL ERP documents]

Autonomous intelligent munitions will collaborate to synchronize lethal effects -- which enables dispersed engagements by multiple smaller weapons -- to destroy targets that change (move, hide, deploy soldiers) during the flight time [SOURCE: ARL ERP documents]</obo:IAO_0000115>
        <obo:IAO_0000119>Technology Environment of Ground Warfare in 2035-2050

Projections made in 2018 by ARL and TRADOC

[This is a draft outline of a potential document; prepared by Alexander Kott, the US Army Research Laboratory; July 2018]</obo:IAO_0000119>
    </owl:Class>
    


    <!-- http://www.ontologylibrary.mil/OperationalEnvironment/Mid/OEFutureWarfareOntology#AutonomousNanoWeapons -->

    <owl:Class rdf:about="http://www.ontologylibrary.mil/OperationalEnvironment/Mid/OEFutureWarfareOntology#AutonomousNanoWeapons">
        <rdfs:subClassOf rdf:resource="http://www.ontologylibrary.mil/OperationalEnvironment/Mid/OEFutureWarfareOntology#SystemsThatShoot"/>
    </owl:Class>
    


    <!-- http://www.ontologylibrary.mil/OperationalEnvironment/Mid/OEFutureWarfareOntology#Availability -->

    <owl:Class rdf:about="http://www.ontologylibrary.mil/OperationalEnvironment/Mid/OEFutureWarfareOntology#Availability">
        <rdfs:subClassOf rdf:resource="http://www.ontologylibrary.mil/OperationalEnvironment/Mid/OEFutureWarfareOntology#CyberSecurityControlledVocabulary"/>
        <obo:IAO_0000115>property of being accessible and usable on demand by an authorized entity</obo:IAO_0000115>
        <obo:IAO_0000119>International Organization for Standardization/International Electrotechnical Commission 27000:2018

Security techniques — Information security management systems — Overview and vocabulary

Publication date : 2018-02

5th Edition</obo:IAO_0000119>
    </owl:Class>
    


    <!-- http://www.ontologylibrary.mil/OperationalEnvironment/Mid/OEFutureWarfareOntology#BaseMeasure -->

    <owl:Class rdf:about="http://www.ontologylibrary.mil/OperationalEnvironment/Mid/OEFutureWarfareOntology#BaseMeasure">
        <rdfs:subClassOf rdf:resource="http://www.ontologylibrary.mil/OperationalEnvironment/Mid/OEFutureWarfareOntology#CyberSecurityControlledVocabulary"/>
        <obo:IAO_0000115>measure (3.42) defined in terms of an attribute and the method for quantifying it

Note 1 to entry: A base measure is functionally independent of other measures.</obo:IAO_0000115>
        <obo:IAO_0000119>International Organization for Standardization/International Electrotechnical Commission 27000:2018

Security techniques — Information security management systems — Overview and vocabulary

Publication date : 2018-02

5th Edition</obo:IAO_0000119>
    </owl:Class>
    


    <!-- http://www.ontologylibrary.mil/OperationalEnvironment/Mid/OEFutureWarfareOntology#BaseYear -->

    <owl:Class rdf:about="http://www.ontologylibrary.mil/OperationalEnvironment/Mid/OEFutureWarfareOntology#BaseYear">
        <rdfs:subClassOf rdf:resource="http://www.ontologylibrary.mil/OperationalEnvironment/Mid/OEFutureWarfareOntology#ClimateChangeAndResourceCompetitionControlledVocabulary"/>
        <obo:IAO_0000115>specific, historical period identified for the purpose of comparing GHGemissions (3.1.5) or GHGremovals (3.1.6) or other GHG-related information over time</obo:IAO_0000115>
        <obo:IAO_0000119>International Organization for Standardization/International Electrotechnical Commission 27000:2018

Technical Committee : ISO/TC 207/SC 7  Greenhouse gas management and related activities

ICS :  13.020.40  Pollution, pollution control and conservation

Greenhouse gases -- Part 1: Specification with guidance at the organization level for quantification and reporting of greenhouse gas emissions and removals 

Publication date : 2018-12

2nd Edition</obo:IAO_0000119>
    </owl:Class>
    


    <!-- http://www.ontologylibrary.mil/OperationalEnvironment/Mid/OEFutureWarfareOntology#Benefit -->

    <owl:Class rdf:about="http://www.ontologylibrary.mil/OperationalEnvironment/Mid/OEFutureWarfareOntology#Benefit">
        <rdfs:subClassOf rdf:resource="http://www.ontologylibrary.mil/OperationalEnvironment/Mid/OEFutureWarfareOntology#BigDataControlledVocabulary"/>
        <obo:IAO_0000115>Benefit refers to the extent that the application outcome meets the goals for those building the big data processing system.</obo:IAO_0000115>
        <obo:IAO_0000115>advantage to the organization of the actionable knowledge derived from an analytic system

Note 1 to entry: Benefit is often ascribed to big data due to the understanding that data has potential value that was typically not considered previously.</obo:IAO_0000115>
        <obo:IAO_0000119>Information technology — Big data — Overview and vocabulary

https://www.iso.org/jtc1</obo:IAO_0000119>
    </owl:Class>
    


    <!-- http://www.ontologylibrary.mil/OperationalEnvironment/Mid/OEFutureWarfareOntology#BigData -->

    <owl:Class rdf:about="http://www.ontologylibrary.mil/OperationalEnvironment/Mid/OEFutureWarfareOntology#BigData">
        <rdfs:subClassOf rdf:resource="http://www.ontologylibrary.mil/OperationalEnvironment/Mid/OEFutureWarfareOntology#ArtificialIntelligenceControlledVocabulary"/>
        <rdfs:subClassOf rdf:resource="http://www.ontologylibrary.mil/OperationalEnvironment/Mid/OEFutureWarfareOntology#BigDataControlledVocabulary"/>
        <obo:IAO_0000115>(1)

extensive datasets (3.1.13) — primarily in the data (3.1.5) characteristics of volume, variety, velocity, and/or variability — that require a scalable technology for efficient storage, manipulation, management, and analysis

Note 1 to entry: Big data is commonly used in many different ways, for example as the name of the scalable technology used to handle big data extensive datasets.</obo:IAO_0000115>
        <obo:IAO_0000115>(2) 

A set of digital data that, through its volume, surpasses human intuition and analytical abilities. We generate some 2.5 trillion bytes of data every day on the internet, through emails, videos, weather information, GPS signals, online transactions, etc. No traditional computerized database management tool can process this mass of data – it has required the development of new algorithms* to store, classify and analyse it.</obo:IAO_0000115>
        <obo:IAO_0000119>(1)

Information technology — Big data — Overview and vocabulary

https://www.iso.org/jtc1</obo:IAO_0000119>
        <obo:IAO_0000119>(2)

United Nations Educational, Scientific, and Cultural Organization Courier 

March 2018

https://en.unesco.org/courier/2018-3/lexicon-artificial-intelligence</obo:IAO_0000119>
    </owl:Class>
    


    <!-- http://www.ontologylibrary.mil/OperationalEnvironment/Mid/OEFutureWarfareOntology#BigDataApplicationProvider -->

    <owl:Class rdf:about="http://www.ontologylibrary.mil/OperationalEnvironment/Mid/OEFutureWarfareOntology#BigDataApplicationProvider">
        <rdfs:subClassOf rdf:resource="http://www.ontologylibrary.mil/OperationalEnvironment/Mid/OEFutureWarfareOntology#BigDataRole"/>
        <obo:IAO_0000115>The Big Data Application Provider executes the manipulations of the data life cycle to meet requirements established by the System Orchestrator. This is where the general capabilities within the Big Data framework are combined to produce the specific data system. While the activities of an application provider are the same whether the solution being built concerns Big Data or not, the methods and techniques have changed because the data and data processing is parallelized across resources.

The Big Data Application Provider role executes a specific set of operations along the data life cycle to meet the requirements established by the System Orchestrator, as well as meeting security and privacy requirements. The Big Data Application Provider is the architecture component that encapsulates the business logic and functionality to be executed by the architecture. The Big Data Application Provider activities include the following:
- Collection
- Preparation
- Analytics
- Visualization
- Access</obo:IAO_0000115>
        <obo:IAO_0000119>NIST Big Data Interoperability Framework: Volume 6, Reference Architecture

Final Version 1 

NIST Big Data Public Working Group (NBD-PWG) Reference Architecture Subgroup Information Technology Laboratory</obo:IAO_0000119>
        <rdfs:comment>In general, the collection activity of the Big Data Application Provider handles the interface with the Data Provider. This may be a general service, such as a file server or web server configured by the System Orchestrator to accept or perform specific collections of data, or it may be an application-specific service designed to pull data or receive pushes of data from the Data Provider. Since this activity is receiving data at a minimum, it must store/buffer the received data until it is persisted through the Big Data Framework Provider. This persistence need not be to physical media but may simply be to an in-memory queue or other service provided by the processing frameworks of the Big Data Framework Provider. The collection activity is likely where the extraction portion of the Extract, Transform, Load (ETL)/Extract, Load, Transform (ELT) cycle is performed. At the initial collection stage, sets of data (e.g., data records) of similar structure are collected (and combined), resulting in uniform security, policy, and other considerations. Initial metadata is created (e.g., subjects with keys are identified) to facilitate subsequent aggregation or look-up methods. 

The preparation activity is where the transformation portion of the ETL/ELT cycle is likely performed, although analytics activity will also likely perform advanced parts of the transformation. Tasks performed by this activity could include data validation (e.g., checksums/hashes, format checks), cleansing (e.g., eliminating bad records/fields), outlier removal, standardization, reformatting, or encapsulating. This activity is also where source data will frequently be persisted to archive storage in the Big Data Framework Provider and provenance data will be verified or attached/associated. Verification or attachment may include optimization of data through manipulations (e.g., deduplication) and indexing to optimize the analytics process. This activity may also aggregate data from different Data Providers, leveraging metadata keys to create an expanded and enhanced data set. 

The analytics activity of the Big Data Application Provider includes the encoding of the low-level business logic of the Big Data system (with higher-level business process logic being encoded by the System Orchestrator). The activity implements the techniques to extract knowledge from the data based
on the requirements of the vertical application. The requirements specify the data processing algorithms for processing the data to produce new insights that will address the technical goal. The analytics activity will leverage the processing frameworks to implement the associated logic. This typically involves the
activity providing software that implements the analytic logic to the batch and/or streaming elements of  the processing framework for execution. The messaging/communication framework of the Big Data Framework Provider may be used to pass data or control functions to the application logic running in the
processing frameworks. The analytic logic may be broken up into multiple modules to be executed by the processing frameworks which communicate, through the messaging/communication framework, with each other and other functions instantiated by the Big Data Application Provider. 

The visualization activity of the Big Data Application Provider prepares elements of the processed data and the output of the analytic activity for presentation to the Data Consumer. The objective of this activity is to format and present data in such a way as to optimally communicate meaning and knowledge. The visualization preparation may involve producing a text-based report or rendering the analytic results as some form of graphic. The resulting output may be a static visualization and may simply be stored through the Big Data Framework Provider for later access. However, the visualization activity frequently interacts with the access activity, the analytics activity, and the Big Data Framework Provider (processing and platform) to provide interactive visualization of the data to the Data Consumer based on parameters provided to the access activity by the Data Consumer. The visualization activity may be completely application-implemented, leverage one or more application libraries, or may use specialized visualization processing frameworks within the Big Data Framework Provider.

The access activity within the Big Data Application Provider is focused on the communication/interaction with the Data Consumer. Similar to the collection activity, the access activity may be a generic service such as a web server or application server that is configured by the System Orchestrator to handle specific
requests from the Data Consumer. This activity would interface with the visualization and analytic activities to respond to requests from the Data Consumer (who may be a person) and uses the processing and platform frameworks to retrieve data to respond to Data Consumer requests. In addition, the access
activity confirms that descriptive and administrative metadata and metadata schemes are captured and maintained for access by the Data Consumer and as data is transferred to the Data Consumer. The interface with the Data Consumer may be synchronous or asynchronous in nature and may use a pull or
push paradigm for data transfer.</rdfs:comment>
    </owl:Class>
    


    <!-- http://www.ontologylibrary.mil/OperationalEnvironment/Mid/OEFutureWarfareOntology#BigDataControlledVocabulary -->

    <owl:Class rdf:about="http://www.ontologylibrary.mil/OperationalEnvironment/Mid/OEFutureWarfareOntology#BigDataControlledVocabulary">
        <rdfs:subClassOf rdf:resource="http://www.ontologylibrary.mil/OperationalEnvironment/Mid/OEFutureWarfareOntology#ControlledVocabulary"/>
    </owl:Class>
    


    <!-- http://www.ontologylibrary.mil/OperationalEnvironment/Mid/OEFutureWarfareOntology#BigDataFrameworkProvider -->

    <owl:Class rdf:about="http://www.ontologylibrary.mil/OperationalEnvironment/Mid/OEFutureWarfareOntology#BigDataFrameworkProvider">
        <rdfs:subClassOf rdf:resource="http://www.ontologylibrary.mil/OperationalEnvironment/Mid/OEFutureWarfareOntology#BigDataRole"/>
        <obo:IAO_0000115>The Big Data Framework Provider has general resources or services to be used by the Big Data Application Provider in the creation of the specific application. There are many new components from which the Big Data Application Provider can choose in using these resources and the network to build the specific system. This is the role that has seen the most significant changes because of Big Data. The Big
Data Framework Provider consists of one or more instances of the three subcomponents: infrastructure frameworks, data platforms, and processing frameworks. There is no requirement that all instances at a given level in the hierarchy be of the same technology and, in fact, most Big Data implementations are hybrids combining multiple technology approaches. These provide flexibility and can meet the complete range of requirements that are driven from the Big Data Application Provider. Due to the rapid emergence of new techniques, this is an area that will continue to need discussion.</obo:IAO_0000115>
        <obo:IAO_0000119>NIST Big Data Interoperability Framework: Volume 6, Reference Architecture

Final Version 1 

NIST Big Data Public Working Group (NBD-PWG) Reference Architecture Subgroup Information Technology Laboratory</obo:IAO_0000119>
    </owl:Class>
    


    <!-- http://www.ontologylibrary.mil/OperationalEnvironment/Mid/OEFutureWarfareOntology#BigDataRole -->

    <owl:Class rdf:about="http://www.ontologylibrary.mil/OperationalEnvironment/Mid/OEFutureWarfareOntology#BigDataRole">
        <rdfs:subClassOf rdf:resource="http://purl.obolibrary.org/obo/BFO_0000023"/>
    </owl:Class>
    


    <!-- http://www.ontologylibrary.mil/OperationalEnvironment/Mid/OEFutureWarfareOntology#BigDataTrend -->

    <owl:Class rdf:about="http://www.ontologylibrary.mil/OperationalEnvironment/Mid/OEFutureWarfareOntology#BigDataTrend">
        <rdfs:subClassOf rdf:resource="http://www.ontologylibrary.mil/OperationalEnvironment/Mid/OEFutureWarfareOntology#Trend"/>
        <obo:IAO_0000115>Artificial Intelligence (AI) may be the most disruptive technology of our time: much of today’s “thought” is artificial, vice human.  Breakthroughs in AI and deep learning enable reasoning intelligent systems that, though not sentient, administer and optimize a great many aspects of modern life.  Advanced physio-mechanical interfaces enable humanmachine integration to include optimized searching of massive indexes of data, direct access to large-scale computing power, and life-like experiences through virtual reality. The revolutionary impact of “trans-humanism” challenges the very definition of “human” – with profound ethical dilemmas that remain unresolved. Big data techniques interrogate massive databases to discover hidden patterns and correlations that form the basis of modern advertising – and are continually leveraged for intelligence and security purposes by nation states and non-state entities alike.  Quantum computing, first applied to encryption functions, is now a key computing enabler, especially for artificial intelligence.9  A mature Internet of Things connects and integrates the devices of the information realm with formerly inert objects – structures, motors, or appliances -- of the physical realm.  Neuroscience has enhanced our understanding of brain function, including neural plasticity, and has enabled advanced techniques for human-machine interfacing. A better understanding of the machinery of the mind has found commercial application in the acceleration of speed and retention in learning.  In the most connected and wealthy parts of the world, cell phones and computers will all but disappear as physical, hand held devices.  Select individuals will directly connect to cyberspace through neural implants or augmented reality systems painted directly on a retina.  If we have not yet reached the “singularity”, where AI and machines are capable of outperforming the human mind, we will nonetheless have reached a point where AI, machines, and man-machine teaming open new possibilities in this realm.</obo:IAO_0000115>
        <obo:IAO_0000119>The Operational Environment and the Changing Character of Future Warfare</obo:IAO_0000119>
    </owl:Class>
    


    <!-- http://www.ontologylibrary.mil/OperationalEnvironment/Mid/OEFutureWarfareOntology#Bioconservative -->

    <owl:Class rdf:about="http://www.ontologylibrary.mil/OperationalEnvironment/Mid/OEFutureWarfareOntology#Bioconservative">
        <rdfs:subClassOf rdf:resource="http://www.ontologylibrary.mil/OperationalEnvironment/Mid/OEFutureWarfareOntology#ArtificialIntelligenceControlledVocabulary"/>
        <obo:IAO_0000115>For transhumanists,* people who criticize their ideal, augmented man are bioconservatives – regressive individuals who refuse to change the laws of life and nature, even though technology makes it possible to do so.</obo:IAO_0000115>
        <obo:IAO_0000119>United Nations Educational, Scientific, and Cultural Organization Courier 

March 2018

https://en.unesco.org/courier/2018-3/lexicon-artificial-intelligence</obo:IAO_0000119>
    </owl:Class>
    


    <!-- http://www.ontologylibrary.mil/OperationalEnvironment/Mid/OEFutureWarfareOntology#BiogenicCarbon -->

    <owl:Class rdf:about="http://www.ontologylibrary.mil/OperationalEnvironment/Mid/OEFutureWarfareOntology#BiogenicCarbon">
        <rdfs:subClassOf rdf:resource="http://www.ontologylibrary.mil/OperationalEnvironment/Mid/OEFutureWarfareOntology#ClimateChangeAndResourceCompetitionControlledVocabulary"/>
        <obo:IAO_0000115>carbon derived from biomass (3.3.1)</obo:IAO_0000115>
        <obo:IAO_0000119>International Organization for Standardization/International Electrotechnical Commission 27000:2018

Technical Committee : ISO/TC 207/SC 7  Greenhouse gas management and related activities

ICS :  13.020.40  Pollution, pollution control and conservation

Greenhouse gases -- Part 1: Specification with guidance at the organization level for quantification and reporting of greenhouse gas emissions and removals 

Publication date : 2018-12

2nd Edition</obo:IAO_0000119>
    </owl:Class>
    


    <!-- http://www.ontologylibrary.mil/OperationalEnvironment/Mid/OEFutureWarfareOntology#BiogenicCarbonDioxide -->

    <owl:Class rdf:about="http://www.ontologylibrary.mil/OperationalEnvironment/Mid/OEFutureWarfareOntology#BiogenicCarbonDioxide">
        <rdfs:subClassOf rdf:resource="http://www.ontologylibrary.mil/OperationalEnvironment/Mid/OEFutureWarfareOntology#ClimateChangeAndResourceCompetitionControlledVocabulary"/>
        <obo:IAO_0000115>CO2 obtained by the oxidation of biogenic carbon (3.3.2)</obo:IAO_0000115>
        <obo:IAO_0000119>International Organization for Standardization/International Electrotechnical Commission 27000:2018

Technical Committee : ISO/TC 207/SC 7  Greenhouse gas management and related activities

ICS :  13.020.40  Pollution, pollution control and conservation

Greenhouse gases -- Part 1: Specification with guidance at the organization level for quantification and reporting of greenhouse gas emissions and removals 

Publication date : 2018-12

2nd Edition</obo:IAO_0000119>
    </owl:Class>
    


    <!-- http://www.ontologylibrary.mil/OperationalEnvironment/Mid/OEFutureWarfareOntology#Biomass -->

    <owl:Class rdf:about="http://www.ontologylibrary.mil/OperationalEnvironment/Mid/OEFutureWarfareOntology#Biomass">
        <rdfs:subClassOf rdf:resource="http://www.ontologylibrary.mil/OperationalEnvironment/Mid/OEFutureWarfareOntology#ClimateChangeAndResourceCompetitionControlledVocabulary"/>
        <obo:IAO_0000115>material of biological origin, excluding material embedded in geological formations and material transformed to fossilized material

Note 1 to entry: Biomass includes organic material (both living and dead), e.g. trees, crops, grasses, tree litter, algae, animals, manure and waste of biological origin.</obo:IAO_0000115>
        <obo:IAO_0000119>International Organization for Standardization/International Electrotechnical Commission 27000:2018

Technical Committee : ISO/TC 207/SC 7  Greenhouse gas management and related activities

ICS :  13.020.40  Pollution, pollution control and conservation

Greenhouse gases -- Part 1: Specification with guidance at the organization level for quantification and reporting of greenhouse gas emissions and removals 

Publication date : 2018-12

2nd Edition</obo:IAO_0000119>
    </owl:Class>
    


    <!-- http://www.ontologylibrary.mil/OperationalEnvironment/Mid/OEFutureWarfareOntology#BrainToBrainInterfaces -->

    <owl:Class rdf:about="http://www.ontologylibrary.mil/OperationalEnvironment/Mid/OEFutureWarfareOntology#BrainToBrainInterfaces">
        <rdfs:subClassOf rdf:resource="http://www.ontologylibrary.mil/OperationalEnvironment/Mid/OEFutureWarfareOntology#SystemsThatSoldier"/>
        <obo:IAO_0000115>Projected breakthrough in brain-to-brain and brain-to-artificial-intelligence (AI) interfaces will enable high-performance warfighting teams that understand each other in complex operations, nearly instantly, without any verbal communications and even with little training. [SOURCE: ARL-TR-8283]</obo:IAO_0000115>
        <obo:IAO_0000119>Technology Environment of Ground Warfare in 2035-2050

Projections made in 2018 by ARL and TRADOC

[This is a draft outline of a potential document; prepared by Alexander Kott, the US Army Research Laboratory; July 2018]</obo:IAO_0000119>
    </owl:Class>
    


    <!-- http://www.ontologylibrary.mil/OperationalEnvironment/Mid/OEFutureWarfareOntology#BrittleMaterial -->

    <owl:Class rdf:about="http://www.ontologylibrary.mil/OperationalEnvironment/Mid/OEFutureWarfareOntology#BrittleMaterial">
        <rdfs:subClassOf rdf:resource="http://www.ontologylibrary.mil/OperationalEnvironment/Mid/OEFutureWarfareOntology#SpaceSystems"/>
        <obo:IAO_0000115>material that breaks due to a propagation defect under the action of a stress</obo:IAO_0000115>
        <obo:IAO_0000119>International Organization for Standardization/International Electrotechnical Commission 11227:2012

Space systems — Test procedure to evaluate spacecraft material ejecta upon hypervelocity impact

Publication Date: 2012-09

1st Edition</obo:IAO_0000119>
    </owl:Class>
    


    <!-- http://www.ontologylibrary.mil/OperationalEnvironment/Mid/OEFutureWarfareOntology#Bureaucracy -->

    <owl:Class rdf:about="http://www.ontologylibrary.mil/OperationalEnvironment/Mid/OEFutureWarfareOntology#Bureaucracy">
        <rdfs:subClassOf rdf:resource="http://www.ontologylibrary.mil/OperationalEnvironment/Mid/OEFutureWarfareOntology#Executive"/>
        <obo:IAO_0000115>Bureaucracy...refers to both a body of non-elective government officials and an administrative policy-making group.  [A bureaucracy is] a government administration managed by departments staffed with non-elected officials. Today, bureaucracy is the administrative system governing any large institution.... The public administration in many countries is an example of a bureaucracy.</obo:IAO_0000115>
        <obo:IAO_0000119>&quot;Bureaucracy&quot;, Wikipedia

March 12, 2019

https://en.wikipedia.org/wiki/Bureaucracy</obo:IAO_0000119>
        <rdfs:label>Bureaucracy</rdfs:label>
    </owl:Class>
    


    <!-- http://www.ontologylibrary.mil/OperationalEnvironment/Mid/OEFutureWarfareOntology#BusinessCycle -->

    <owl:Class rdf:about="http://www.ontologylibrary.mil/OperationalEnvironment/Mid/OEFutureWarfareOntology#BusinessCycle">
        <rdfs:subClassOf rdf:resource="http://www.ontologylibrary.mil/OperationalEnvironment/Mid/OEFutureWarfareOntology#MacroeconomicPolicy"/>
        <obo:IAO_0000119>Christina D. Romer, &quot;Business Cycles&quot;, The Library of Economics and LIberty

March 21, 2019

https://www.econlib.org/library/Enc/BusinessCycles.html</obo:IAO_0000119>
        <CommonCoreOntologies:definition>The United States and all other modern industrial economies experience significant swings in economic activity. In some years, most industries are booming and unemployment is low; in other years, most industries are operating well below capacity and unemployment is high. Periods of economic prosperity are typically called expansions or booms; periods of economic decline are called recessions or depressions. The combination of expansions and recessions, the ebb and flow of economic activity, is called the business cycle.</CommonCoreOntologies:definition>
        <rdfs:label>Business Cycle</rdfs:label>
    </owl:Class>
    


    <!-- http://www.ontologylibrary.mil/OperationalEnvironment/Mid/OEFutureWarfareOntology#Cabinet -->

    <owl:Class rdf:about="http://www.ontologylibrary.mil/OperationalEnvironment/Mid/OEFutureWarfareOntology#Cabinet">
        <rdfs:subClassOf rdf:resource="http://www.ontologylibrary.mil/OperationalEnvironment/Mid/OEFutureWarfareOntology#Executive"/>
        <obo:IAO_0000115>A Cabinet is a body of high-ranking state officials, typically consisting of the top leaders of the executive branch. Members of a cabinet are usually called Cabinet ministers or secretaries. The function of a Cabinet varies: in some countries it is a collegiate decision-making body with collective responsibility, while in others it may function either as a purely advisory body or an assisting institution to a decision making head of state or head of government. Cabinets are typically the body responsible for the day-to-day management of the government and response to sudden events, whereas the legislative and judicial branches work in a measured pace, in sessions according to lengthy procedures.

In some countries, particularly those that use a parliamentary system...the Cabinet collectively decides the government&apos;s direction, especially in regard to legislation passed by the parliament. In countries with a presidential system...the Cabinet does not function as a collective legislative influence; rather, their primary role is as an official advisory council to the head of government. In this way, the President obtains opinions and advice relating to forthcoming decisions.

...

The second role of cabinet officials is to administer executive branches, government agencies, or departments....Cabinets are also important originators for legislation. Cabinets and ministers are usually in charge of the preparation of proposed legislation in the ministries before it is passed to the parliament. Thus, often the majority of new legislation actually originates from the cabinet and its ministries.</obo:IAO_0000115>
        <obo:IAO_0000119>&quot;Cabinent (government)&quot;, Wikipedia

March 12, 2019

https://en.wikipedia.org/wiki/Cabinet_(government)</obo:IAO_0000119>
        <rdfs:label>Cabinet</rdfs:label>
    </owl:Class>
    


    <!-- http://www.ontologylibrary.mil/OperationalEnvironment/Mid/OEFutureWarfareOntology#CarbonDioxideEquivalent -->

    <owl:Class rdf:about="http://www.ontologylibrary.mil/OperationalEnvironment/Mid/OEFutureWarfareOntology#CarbonDioxideEquivalent">
        <rdfs:subClassOf rdf:resource="http://www.ontologylibrary.mil/OperationalEnvironment/Mid/OEFutureWarfareOntology#ClimateChangeAndResourceCompetitionControlledVocabulary"/>
        <obo:IAO_0000115>unit for comparing the radiative forcing of a greenhouse gas to that of carbon dioxide

Note 1 to entry: The carbon dioxide equivalent is calculated using the mass of a given greenhouse gas multiplied by its global warming potential</obo:IAO_0000115>
        <obo:IAO_0000119>International Organization for Standardization/International Electrotechnical Commission 27000:2018

Technical Committee : ISO/TC 207/SC 7  Greenhouse gas management and related activities

ICS :  13.020.40  Pollution, pollution control and conservation

Greenhouse gases -- Part 1: Specification with guidance at the organization level for quantification and reporting of greenhouse gas emissions and removals 

Publication date : 2018-12

2nd Edition</obo:IAO_0000119>
    </owl:Class>
    


    <!-- http://www.ontologylibrary.mil/OperationalEnvironment/Mid/OEFutureWarfareOntology#ChemicalWeapons -->

    <owl:Class rdf:about="http://www.ontologylibrary.mil/OperationalEnvironment/Mid/OEFutureWarfareOntology#ChemicalWeapons">
        <rdfs:subClassOf rdf:resource="http://www.ontologylibrary.mil/OperationalEnvironment/Mid/OEFutureWarfareOntology#SystemsThatShoot"/>
        <obo:IAO_0000115>Non-traditional agents developed to defeat detection and protection capabilities. [SOURCE: TRADOC G-2 Potential Game Changers, May 2018]</obo:IAO_0000115>
        <obo:IAO_0000119>Technology Environment of Ground Warfare in 2035-2050

Projections made in 2018 by ARL and TRADOC

[This is a draft outline of a potential document; prepared by Alexander Kott, the US Army Research Laboratory; July 2018]</obo:IAO_0000119>
    </owl:Class>
    


    <!-- http://www.ontologylibrary.mil/OperationalEnvironment/Mid/OEFutureWarfareOntology#CivilLaw -->

    <owl:Class rdf:about="http://www.ontologylibrary.mil/OperationalEnvironment/Mid/OEFutureWarfareOntology#CivilLaw">
        <rdfs:subClassOf rdf:resource="http://www.ontologylibrary.mil/OperationalEnvironment/Mid/OEFutureWarfareOntology#JudicialSystem"/>
        <obo:IAO_0000115>The law relating to civil wrongs and quasi-contracts is part of the civil law, as is law of property.... The rights and duties of persons (natural persons and legal persons) amongst themselves is the primary concern of civil law. It is often suggested that civil proceedings are taken for the purpose of obtaining compensation for injury, and may thus be distinguished from criminal proceedings, whose purpose is to inflict punishment. However, exemplary damages or punitive damages may be awarded in civil proceedings.</obo:IAO_0000115>
        <obo:IAO_0000119>&quot;Civil Law (Common Law)&quot;, Wikipedia

March 12, 2019

https://en.wikipedia.org/wiki/Civil_law_(common_law)</obo:IAO_0000119>
        <rdfs:label>Civil Law</rdfs:label>
    </owl:Class>
    


    <!-- http://www.ontologylibrary.mil/OperationalEnvironment/Mid/OEFutureWarfareOntology#CivilWar -->

    <owl:Class rdf:about="http://www.ontologylibrary.mil/OperationalEnvironment/Mid/OEFutureWarfareOntology#CivilWar">
        <rdfs:subClassOf rdf:resource="http://www.ontologylibrary.mil/OperationalEnvironment/Mid/OEFutureWarfareOntology#SubstateConflict"/>
    </owl:Class>
    


    <!-- http://www.ontologylibrary.mil/OperationalEnvironment/Mid/OEFutureWarfareOntology#Class -->

    <owl:Class rdf:about="http://www.ontologylibrary.mil/OperationalEnvironment/Mid/OEFutureWarfareOntology#Class">
        <rdfs:subClassOf rdf:resource="http://www.ontologylibrary.mil/OperationalEnvironment/Mid/OEFutureWarfareOntology#Identity"/>
    </owl:Class>
    


    <!-- http://www.ontologylibrary.mil/OperationalEnvironment/Mid/OEFutureWarfareOntology#CleanRenewableEnergy -->

    <owl:Class rdf:about="http://www.ontologylibrary.mil/OperationalEnvironment/Mid/OEFutureWarfareOntology#CleanRenewableEnergy">
        <rdfs:subClassOf rdf:resource="http://www.ontologylibrary.mil/OperationalEnvironment/Mid/OEFutureWarfareOntology#PowerGenerationAndStorageControlledVocabulary"/>
        <obo:IAO_0000115>renewable energy (3.38) whose direct or indirect emissions of greenhouse gases, other gases with adverse impacts on human health, water pollutants, or other toxic releases, and whose impacts on ecosystems are substantially lower than those of conventional alternatives such as gas-fired generation

Note 1 to entry: Geothermal energy that releases high-SO2 gases to the atmosphere does not qualify under this definition

Note 2 to entry: Wood pellet or solid wood combustion does not qualify if the greenhouse gas emissions associated with producing the wood are similar to those of coal on the basis of a megajoule of fuel.</obo:IAO_0000115>
        <obo:IAO_0000119>International Organization for Standardization/International ISO 50007:2017

Technical Committee : ISO/TC 301  Energy management and energy savings

ICS :  27.015  Energy efficiency. Energy conservation in general

Energy services -- Guidelines for the assessment and improvement of the energy service to users

Publication date : 2017-06

1st Edition</obo:IAO_0000119>
    </owl:Class>
    


    <!-- http://www.ontologylibrary.mil/OperationalEnvironment/Mid/OEFutureWarfareOntology#Client -->

    <owl:Class rdf:about="http://www.ontologylibrary.mil/OperationalEnvironment/Mid/OEFutureWarfareOntology#Client">
        <rdfs:subClassOf rdf:resource="http://www.ontologylibrary.mil/OperationalEnvironment/Mid/OEFutureWarfareOntology#ClimateChangeAndResourceCompetitionControlledVocabulary"/>
        <obo:IAO_0000115>organization (3.4.2) or person requesting verification (3.4.9) or validation (3.4.10)</obo:IAO_0000115>
        <obo:IAO_0000119>International Organization for Standardization/International Electrotechnical Commission 27000:2018

Technical Committee : ISO/TC 207/SC 7  Greenhouse gas management and related activities

ICS :  13.020.40  Pollution, pollution control and conservation

Greenhouse gases -- Part 1: Specification with guidance at the organization level for quantification and reporting of greenhouse gas emissions and removals 

Publication date : 2018-12

2nd Edition</obo:IAO_0000119>
    </owl:Class>
    


    <!-- http://www.ontologylibrary.mil/OperationalEnvironment/Mid/OEFutureWarfareOntology#ClimateChangeAndResourceCompetitionControlledVocabulary -->

    <owl:Class rdf:about="http://www.ontologylibrary.mil/OperationalEnvironment/Mid/OEFutureWarfareOntology#ClimateChangeAndResourceCompetitionControlledVocabulary">
        <rdfs:subClassOf rdf:resource="http://www.ontologylibrary.mil/OperationalEnvironment/Mid/OEFutureWarfareOntology#ControlledVocabulary"/>
        <obo:IAO_0000115>index, based on radiative properties of greenhouse gases, measuring the radiative forcing following a pulse emission of a unit mass of a given greenhouse gas in the present-day atmosphere integrated over a chosen time horizon, relative to that of carbon dioxide (CO2)</obo:IAO_0000115>
    </owl:Class>
    


    <!-- http://www.ontologylibrary.mil/OperationalEnvironment/Mid/OEFutureWarfareOntology#ClimateChangeAndResourceCompetitionTrend -->

    <owl:Class rdf:about="http://www.ontologylibrary.mil/OperationalEnvironment/Mid/OEFutureWarfareOntology#ClimateChangeAndResourceCompetitionTrend">
        <rdfs:subClassOf rdf:resource="http://www.ontologylibrary.mil/OperationalEnvironment/Mid/OEFutureWarfareOntology#Trend"/>
        <obo:IAO_0000115>Humanity will become richer, older, more urban, and better educated, but the uneven distribution of this progress will accelerate tension and conflict.  The convergence of more information and more people with fewer state resources will constrain governments’ efforts to address rampant poverty, violence, and pollution, and create a breeding ground for dissatisfaction among increasingly aware, yet still disempowered populations. These factors will be attenuated by a changing climate, which has the potential to create additional crises and discontent.  The addition of over seven billion people over the last century has altered geography itself, and cities now sprawl over large areas of the globe and contain almost two-thirds of the world’s population. These numbers will only increase.  Some megacities will become more important politically and economically than the nationstate in which they reside.  Life will become both easier and more complex, with those able to take advantage of the leading edge of technological advancement increasingly exploiting those who cannot.  New social stresses and fractures will lead to strife and population migrations, which in turn create further challenges for urbanized areas.  Furthermore, the move of large numbers of people to large urban areas and megacities will strain resources, as these area will become increasingly reliant on rural areas for food, water, and even additional power.  From a military perspective, cities represent challenges, opportunities, and unique vulnerabilities.</obo:IAO_0000115>
        <obo:IAO_0000119>The Operational Environment and the Changing Character of Future Warfare</obo:IAO_0000119>
    </owl:Class>
    


    <!-- http://www.ontologylibrary.mil/OperationalEnvironment/Mid/OEFutureWarfareOntology#ClimateRefugees -->

    <owl:Class rdf:about="http://www.ontologylibrary.mil/OperationalEnvironment/Mid/OEFutureWarfareOntology#ClimateRefugees">
        <rdfs:subClassOf rdf:resource="http://www.ontologylibrary.mil/OperationalEnvironment/Mid/OEFutureWarfareOntology#Migration"/>
        <obo:IAO_0000119>&quot;Environmental Migrant&quot;, Wikipedia

March 26, 2019

https://en.wikipedia.org/wiki/Environmental_migrant</obo:IAO_0000119>
        <CommonCoreOntologies:definition>Environmental migrants are people who are forced to leave their home region due to sudden or long-term changes to their local environment. These are changes which compromise their well-being or secure livelihood. Such changes are held to include increased droughts, desertification, sea level rise, and disruption of seasonal weather patterns (i.e. monsoons). Climate refugees may choose to flee to or migrate to another country, or they may migrate internally within their own country.

The term &quot;environmental migrant&quot; is used somewhat interchangeably with a range of similar terms, such as ecological refugee, environmental refugee, climate refugee, forced environmental migrant, environmentally motivated migrant, climate change refugee, environmentally displaced person (EDP), disaster refugee, environmental displacee, eco-refugee, ecologically displaced person, or environmental-refugee-to-be (ERTB)</CommonCoreOntologies:definition>
        <rdfs:label>Climate Refugees</rdfs:label>
    </owl:Class>
    


    <!-- http://www.ontologylibrary.mil/OperationalEnvironment/Mid/OEFutureWarfareOntology#Cloud -->

    <owl:Class rdf:about="http://www.ontologylibrary.mil/OperationalEnvironment/Mid/OEFutureWarfareOntology#Cloud">
        <rdfs:subClassOf rdf:resource="http://www.ontologylibrary.mil/OperationalEnvironment/Mid/OEFutureWarfareOntology#ArtificialIntelligenceControlledVocabulary"/>
        <obo:IAO_0000115>Different computer systems involving a large number of computers connected to each other, and exchanging messages in real time over the internet. A calculation or the storage of information launched by one computer can therefore be carried out by a network of interconnected computers – thus creating a cloud.</obo:IAO_0000115>
        <obo:IAO_0000119>United Nations Educational, Scientific, and Cultural Organization Courier 

March 2018

https://en.unesco.org/courier/2018-3/lexicon-artificial-intelligence</obo:IAO_0000119>
    </owl:Class>
    


    <!-- http://www.ontologylibrary.mil/OperationalEnvironment/Mid/OEFutureWarfareOntology#CloudComputing -->

    <owl:Class rdf:about="http://www.ontologylibrary.mil/OperationalEnvironment/Mid/OEFutureWarfareOntology#CloudComputing">
        <rdfs:subClassOf rdf:resource="http://www.ontologylibrary.mil/OperationalEnvironment/Mid/OEFutureWarfareOntology#BigDataControlledVocabulary"/>
        <obo:IAO_0000115>paradigm for enabling network access to a scalable and elastic pool of shareable physical or virtual resources with self-service provisioning and administration on-demand

Note 1 to entry: Examples of resources include servers, operating systems, networks, software, applications, and storage equipment.</obo:IAO_0000115>
        <obo:IAO_0000119>Information technology — Big data — Overview and vocabulary

https://www.iso.org/jtc1</obo:IAO_0000119>
    </owl:Class>
    


    <!-- http://www.ontologylibrary.mil/OperationalEnvironment/Mid/OEFutureWarfareOntology#Cluster -->

    <owl:Class rdf:about="http://www.ontologylibrary.mil/OperationalEnvironment/Mid/OEFutureWarfareOntology#Cluster">
        <rdfs:subClassOf rdf:resource="http://www.ontologylibrary.mil/OperationalEnvironment/Mid/OEFutureWarfareOntology#BigDataControlledVocabulary"/>
        <obo:IAO_0000115>&lt;distributed data processing&gt; set of functional units under common control</obo:IAO_0000115>
        <obo:IAO_0000119>Information technology — Big data — Overview and vocabulary

https://www.iso.org/jtc1</obo:IAO_0000119>
        <obo:IAO_0000119>[SOURCE: ISO/IEC 2382:2015, 18.05.06]</obo:IAO_0000119>
    </owl:Class>
    


    <!-- http://www.ontologylibrary.mil/OperationalEnvironment/Mid/OEFutureWarfareOntology#CollectiveIntelligenceControlledVocabulary -->

    <owl:Class rdf:about="http://www.ontologylibrary.mil/OperationalEnvironment/Mid/OEFutureWarfareOntology#CollectiveIntelligenceControlledVocabulary">
        <rdfs:subClassOf rdf:resource="http://www.ontologylibrary.mil/OperationalEnvironment/Mid/OEFutureWarfareOntology#ControlledVocabulary"/>
    </owl:Class>
    


    <!-- http://www.ontologylibrary.mil/OperationalEnvironment/Mid/OEFutureWarfareOntology#CollectiveIntelligenceTrend -->

    <owl:Class rdf:about="http://www.ontologylibrary.mil/OperationalEnvironment/Mid/OEFutureWarfareOntology#CollectiveIntelligenceTrend">
        <rdfs:subClassOf rdf:resource="http://www.ontologylibrary.mil/OperationalEnvironment/Mid/OEFutureWarfareOntology#Trend"/>
        <obo:IAO_0000115>Singularity is the point at which artificial intelligence (AI) exceeds the collective intelligence of mankind, which will radically and irrevocably change the relationship between man and machine.  There are several divergent possibilities regarding the singularity: 

 As optimistic singularity advocates, such as Ray Kurzweil have suggested, AI improves human life in every way, from healthcare, to emotional evolution, to intergalactic space travel. 

 While not entirely apocalyptic, unboxed general artificial superintelligence improves and evolves at such an exponential rate it escapes human restrictions, perspectives, and morality.  It threatens the very existence of humanity. 

 Humans evolve their own cognitive abilities through learning developments, brain implants, artificial stimulants, and non-AI high performance computing to match, or at least keep pace with AI. 

AI has the capacity to change paradigms, revolutionize everyday life, and take mankind to exciting new horizons.  However, it also may be capable of incredible destruction, malice, and lines of thinking and decision-making that are dangerous to mankind.  This duality will be critical as actors develop military applications for AI.</obo:IAO_0000115>
        <obo:IAO_0000119>The Operational Environment and the Changing Character of Future Warfare</obo:IAO_0000119>
    </owl:Class>
    


    <!-- http://www.ontologylibrary.mil/OperationalEnvironment/Mid/OEFutureWarfareOntology#CombatApplication -->

    <owl:Class rdf:about="http://www.ontologylibrary.mil/OperationalEnvironment/Mid/OEFutureWarfareOntology#CombatApplication">
        <rdfs:subClassOf rdf:resource="http://purl.obolibrary.org/obo/BFO_0000019"/>
    </owl:Class>
    


    <!-- http://www.ontologylibrary.mil/OperationalEnvironment/Mid/OEFutureWarfareOntology#CombinedCycle -->

    <owl:Class rdf:about="http://www.ontologylibrary.mil/OperationalEnvironment/Mid/OEFutureWarfareOntology#CombinedCycle">
        <rdfs:subClassOf rdf:resource="http://www.ontologylibrary.mil/OperationalEnvironment/Mid/OEFutureWarfareOntology#GasEnergyGeneration"/>
        <obo:IAO_0000115>thermodynamic cycle employing the combination of a gas turbine cycle with a steam or other fluid Rankine cycle

Note 1 to entry: In a common example, the gas turbine exhaust heat is used to generate steam for the Rankine cycle.

Note 2 to entry: The superior thermal performance of this cycle is due to a combination of the best thermodynamic attributes of each cycle, namely the addition of thermal energy at higher temperatures in the gas turbine cycle and the rejection of thermal energy at lower temperatures in the Rankine cycle.
[SOURCE: ISO 11086:1996, 1.12]</obo:IAO_0000115>
        <obo:IAO_0000119>International Organization for Standardization/International ISO 19859:2016

Technical Committee : ISO/TC 192  Gas turbines

ICS :  29.160.99  Other standards related to rotating machinery 27.040  Gas and steam turbines. Steam engines

Gas turbine applications -- Requirements for power generation

Publication date : 2016-08

1st Edition</obo:IAO_0000119>
    </owl:Class>
    


    <!-- http://www.ontologylibrary.mil/OperationalEnvironment/Mid/OEFutureWarfareOntology#Competence -->

    <owl:Class rdf:about="http://www.ontologylibrary.mil/OperationalEnvironment/Mid/OEFutureWarfareOntology#Competence">
        <rdfs:subClassOf rdf:resource="http://www.ontologylibrary.mil/OperationalEnvironment/Mid/OEFutureWarfareOntology#CyberSecurityControlledVocabulary"/>
        <obo:IAO_0000115>ability to apply knowledge and skills to achieve intended results</obo:IAO_0000115>
        <obo:IAO_0000119>International Organization for Standardization/International Electrotechnical Commission 27000:2018

Security techniques — Information security management systems — Overview and vocabulary

Publication date : 2018-02

5th Edition</obo:IAO_0000119>
    </owl:Class>
    


    <!-- http://www.ontologylibrary.mil/OperationalEnvironment/Mid/OEFutureWarfareOntology#ComplexityScience -->

    <owl:Class rdf:about="http://www.ontologylibrary.mil/OperationalEnvironment/Mid/OEFutureWarfareOntology#ComplexityScience">
        <rdfs:subClassOf rdf:resource="http://www.ontologylibrary.mil/OperationalEnvironment/Mid/OEFutureWarfareOntology#SystemsThatSeeThinkCommunicate"/>
        <obo:IAO_0000119>Projected breakthroughs in Complexity Science, particularly in Fractional Calculus, will enable new methods to anticipate and mitigate failures in planning exceptionally complex operations like interventions in megacities. [SOURCE: ARL-TR-8283]</obo:IAO_0000119>
        <obo:IAO_0000119>Technology Environment of Ground Warfare in 2035-2050

Projections made in 2018 by ARL and TRADOC

[This is a draft outline of a potential document; prepared by Alexander Kott, the US Army Research Laboratory; July 2018]</obo:IAO_0000119>
    </owl:Class>
    


    <!-- http://www.ontologylibrary.mil/OperationalEnvironment/Mid/OEFutureWarfareOntology#Confidentiality -->

    <owl:Class rdf:about="http://www.ontologylibrary.mil/OperationalEnvironment/Mid/OEFutureWarfareOntology#Confidentiality">
        <rdfs:subClassOf rdf:resource="http://www.ontologylibrary.mil/OperationalEnvironment/Mid/OEFutureWarfareOntology#CyberSecurityControlledVocabulary"/>
        <obo:IAO_0000115>property that information is not made available or disclosed to unauthorized individuals, entities, or processes (3.54)</obo:IAO_0000115>
        <obo:IAO_0000119>International Organization for Standardization/International Electrotechnical Commission 27000:2018

Security techniques — Information security management systems — Overview and vocabulary

Publication date : 2018-02

5th Edition</obo:IAO_0000119>
    </owl:Class>
    


    <!-- http://www.ontologylibrary.mil/OperationalEnvironment/Mid/OEFutureWarfareOntology#Conformity -->

    <owl:Class rdf:about="http://www.ontologylibrary.mil/OperationalEnvironment/Mid/OEFutureWarfareOntology#Conformity">
        <rdfs:subClassOf rdf:resource="http://www.ontologylibrary.mil/OperationalEnvironment/Mid/OEFutureWarfareOntology#CyberSecurityControlledVocabulary"/>
        <obo:IAO_0000115>fulfilment of a requirement (3.56)</obo:IAO_0000115>
        <obo:IAO_0000119>International Organization for Standardization/International Electrotechnical Commission 27000:2018

Security techniques — Information security management systems — Overview and vocabulary

Publication date : 2018-02

5th Edition</obo:IAO_0000119>
    </owl:Class>
    


    <!-- http://www.ontologylibrary.mil/OperationalEnvironment/Mid/OEFutureWarfareOntology#Consequence -->

    <owl:Class rdf:about="http://www.ontologylibrary.mil/OperationalEnvironment/Mid/OEFutureWarfareOntology#Consequence">
        <rdfs:subClassOf rdf:resource="http://www.ontologylibrary.mil/OperationalEnvironment/Mid/OEFutureWarfareOntology#CyberSecurityControlledVocabulary"/>
        <obo:IAO_0000115>outcome of an event (3.21) affecting objectives (3.49)

Note 1 to entry: An event can lead to a range of consequences.

Note 2 to entry: A consequence can be certain or uncertain and, in the context of information security, is usually negative.

Note 3 to entry: Consequences can be expressed qualitatively or quantitatively.

Note 4 to entry: Initial consequences can escalate through knock-on effects.</obo:IAO_0000115>
        <obo:IAO_0000119>International Organization for Standardization/International Electrotechnical Commission 27000:2018

Security techniques — Information security management systems — Overview and vocabulary

Publication date : 2018-02

5th Edition</obo:IAO_0000119>
    </owl:Class>
    


    <!-- http://www.ontologylibrary.mil/OperationalEnvironment/Mid/OEFutureWarfareOntology#ContinualImprovement -->

    <owl:Class rdf:about="http://www.ontologylibrary.mil/OperationalEnvironment/Mid/OEFutureWarfareOntology#ContinualImprovement">
        <rdfs:subClassOf rdf:resource="http://www.ontologylibrary.mil/OperationalEnvironment/Mid/OEFutureWarfareOntology#CyberSecurityControlledVocabulary"/>
        <obo:IAO_0000115>recurring activity to enhance performance (3.52)</obo:IAO_0000115>
        <obo:IAO_0000119>International Organization for Standardization/International Electrotechnical Commission 27000:2018

Security techniques — Information security management systems — Overview and vocabulary

Publication date : 2018-02

5th Edition</obo:IAO_0000119>
    </owl:Class>
    


    <!-- http://www.ontologylibrary.mil/OperationalEnvironment/Mid/OEFutureWarfareOntology#Control -->

    <owl:Class rdf:about="http://www.ontologylibrary.mil/OperationalEnvironment/Mid/OEFutureWarfareOntology#Control">
        <rdfs:subClassOf rdf:resource="http://www.ontologylibrary.mil/OperationalEnvironment/Mid/OEFutureWarfareOntology#CyberSecurityControlledVocabulary"/>
        <obo:IAO_0000115>measure that is modifying risk (3.61)

Note 1 to entry: Controls include any process (3.54), policy (3.53), device, practice, or other actions which modify risk (3.61).

Note 2 to entry: It is possible that controls not always exert the intended or assumed modifying effect.</obo:IAO_0000115>
        <obo:IAO_0000119>International Organization for Standardization/International Electrotechnical Commission 27000:2018

Security techniques — Information security management systems — Overview and vocabulary

Publication date : 2018-02

5th Edition</obo:IAO_0000119>
    </owl:Class>
    


    <!-- http://www.ontologylibrary.mil/OperationalEnvironment/Mid/OEFutureWarfareOntology#ControlObjective -->

    <owl:Class rdf:about="http://www.ontologylibrary.mil/OperationalEnvironment/Mid/OEFutureWarfareOntology#ControlObjective">
        <rdfs:subClassOf rdf:resource="http://www.ontologylibrary.mil/OperationalEnvironment/Mid/OEFutureWarfareOntology#CyberSecurityControlledVocabulary"/>
        <obo:IAO_0000115>statement describing what is to be achieved as a result of implementing controls (3.14)</obo:IAO_0000115>
        <obo:IAO_0000119>International Organization for Standardization/International Electrotechnical Commission 27000:2018

Security techniques — Information security management systems — Overview and vocabulary

Publication date : 2018-02

5th Edition</obo:IAO_0000119>
    </owl:Class>
    


    <!-- http://www.ontologylibrary.mil/OperationalEnvironment/Mid/OEFutureWarfareOntology#ControlledVocabulary -->

    <owl:Class rdf:about="http://www.ontologylibrary.mil/OperationalEnvironment/Mid/OEFutureWarfareOntology#ControlledVocabulary">
        <rdfs:subClassOf rdf:resource="http://www.ontologyrepository.com/CommonCoreOntologies/DescriptiveInformationContentEntity"/>
    </owl:Class>
    


    <!-- http://www.ontologylibrary.mil/OperationalEnvironment/Mid/OEFutureWarfareOntology#Correction -->

    <owl:Class rdf:about="http://www.ontologylibrary.mil/OperationalEnvironment/Mid/OEFutureWarfareOntology#Correction">
        <rdfs:subClassOf rdf:resource="http://www.ontologylibrary.mil/OperationalEnvironment/Mid/OEFutureWarfareOntology#CyberSecurityControlledVocabulary"/>
        <obo:IAO_0000115>action to eliminate a detected nonconformity (3.47)</obo:IAO_0000115>
        <obo:IAO_0000119>International Organization for Standardization/International Electrotechnical Commission 27000:2018

Security techniques — Information security management systems — Overview and vocabulary

Publication date : 2018-02

5th Edition</obo:IAO_0000119>
    </owl:Class>
    


    <!-- http://www.ontologylibrary.mil/OperationalEnvironment/Mid/OEFutureWarfareOntology#CorrectiveAction -->

    <owl:Class rdf:about="http://www.ontologylibrary.mil/OperationalEnvironment/Mid/OEFutureWarfareOntology#CorrectiveAction">
        <rdfs:subClassOf rdf:resource="http://www.ontologylibrary.mil/OperationalEnvironment/Mid/OEFutureWarfareOntology#CyberSecurityControlledVocabulary"/>
        <obo:IAO_0000115>action to eliminate the cause of a nonconformity (3.47) and to prevent recurrence</obo:IAO_0000115>
        <obo:IAO_0000119>International Organization for Standardization/International Electrotechnical Commission 27000:2018

Security techniques — Information security management systems — Overview and vocabulary

Publication date : 2018-02

5th Edition</obo:IAO_0000119>
    </owl:Class>
    


    <!-- http://www.ontologylibrary.mil/OperationalEnvironment/Mid/OEFutureWarfareOntology#Corruption -->

    <owl:Class rdf:about="http://www.ontologylibrary.mil/OperationalEnvironment/Mid/OEFutureWarfareOntology#Corruption">
        <rdfs:subClassOf rdf:resource="http://www.ontologylibrary.mil/OperationalEnvironment/Mid/OEFutureWarfareOntology#InformalInstitutions"/>
        <obo:IAO_0000115>In general, corruption is a form of dishonesty or criminal activity undertaken by a person or organization entrusted with a position of authority, often to acquire illicit benefit. Corruption may include many activities including bribery and embezzlement, though it may also involve practices that are legal in many countries. Political corruption occurs when an office-holder or other governmental employee acts in an official capacity for personal gain. Corruption is most commonplace in kleptocracies, oligarchies, narco-states and mafia states.

Corruption can occur on different scales. Corruption ranges from small favors between a small number of people (petty corruption), to corruption that affects the government on a large scale (grand corruption), and corruption that is so prevalent that it is part of the everyday structure of society, including corruption as one of the symptoms of organized crime.</obo:IAO_0000115>
        <obo:IAO_0000119>&quot;Corruption&quot;, Wikiepedia

March 12, 2019

https://en.wikipedia.org/wiki/Corruption</obo:IAO_0000119>
        <rdfs:label>Corruption</rdfs:label>
    </owl:Class>
    


    <!-- http://www.ontologylibrary.mil/OperationalEnvironment/Mid/OEFutureWarfareOntology#Coup -->

    <owl:Class rdf:about="http://www.ontologylibrary.mil/OperationalEnvironment/Mid/OEFutureWarfareOntology#Coup">
        <rdfs:subClassOf rdf:resource="http://www.ontologylibrary.mil/OperationalEnvironment/Mid/OEFutureWarfareOntology#SubstateConflict"/>
    </owl:Class>
    


    <!-- http://www.ontologylibrary.mil/OperationalEnvironment/Mid/OEFutureWarfareOntology#Crime -->

    <owl:Class rdf:about="http://www.ontologylibrary.mil/OperationalEnvironment/Mid/OEFutureWarfareOntology#Crime">
        <rdfs:subClassOf rdf:resource="http://www.ontologylibrary.mil/OperationalEnvironment/Mid/OEFutureWarfareOntology#SecurityAndViolentConflict"/>
    </owl:Class>
    


    <!-- http://www.ontologylibrary.mil/OperationalEnvironment/Mid/OEFutureWarfareOntology#CriminalLaw -->

    <owl:Class rdf:about="http://www.ontologylibrary.mil/OperationalEnvironment/Mid/OEFutureWarfareOntology#CriminalLaw">
        <rdfs:subClassOf rdf:resource="http://www.ontologylibrary.mil/OperationalEnvironment/Mid/OEFutureWarfareOntology#JudicialSystem"/>
        <obo:IAO_0000115>Criminal law is the body of law that relates to crime. It proscribes conduct perceived as threatening, harmful, or otherwise endangering to the property, health, safety, and moral welfare of people inclusive of one&apos;s self. Most criminal law is established by statute, which is to say that the laws are enacted by a legislature. Criminal law includes the punishment and rehabilitation of people who violate such laws.</obo:IAO_0000115>
        <obo:IAO_0000119>&quot;Criminal Law&quot;, Wikipedia

March 12, 2019

https://en.wikipedia.org/wiki/Criminal_law</obo:IAO_0000119>
        <rdfs:label>Criminal Law</rdfs:label>
    </owl:Class>
    


    <!-- http://www.ontologylibrary.mil/OperationalEnvironment/Mid/OEFutureWarfareOntology#CyberAndSpaceControlledVocabulary -->

    <owl:Class rdf:about="http://www.ontologylibrary.mil/OperationalEnvironment/Mid/OEFutureWarfareOntology#CyberAndSpaceControlledVocabulary">
        <rdfs:subClassOf rdf:resource="http://www.ontologylibrary.mil/OperationalEnvironment/Mid/OEFutureWarfareOntology#ControlledVocabulary"/>
    </owl:Class>
    


    <!-- http://www.ontologylibrary.mil/OperationalEnvironment/Mid/OEFutureWarfareOntology#CyberAndSpaceTrend -->

    <owl:Class rdf:about="http://www.ontologylibrary.mil/OperationalEnvironment/Mid/OEFutureWarfareOntology#CyberAndSpaceTrend">
        <rdfs:subClassOf rdf:resource="http://www.ontologylibrary.mil/OperationalEnvironment/Mid/OEFutureWarfareOntology#Trend"/>
        <obo:IAO_0000115>Our adversaries will rely on strategic capabilities, such as weapons of mass destruction, information operations, and direct cyber-attacks designed to give us pause in responding to their actions and provide them the strategic space they need to operate.  Space will become a contested domain, as our enemies will enhance their ability to operate in that domain while working to deny us what was once a key area of advantage</obo:IAO_0000115>
        <obo:IAO_0000119>The Operational Environment and the Changing Character of Future Warfare</obo:IAO_0000119>
    </owl:Class>
    


    <!-- http://www.ontologylibrary.mil/OperationalEnvironment/Mid/OEFutureWarfareOntology#CyberSecurityControlledVocabulary -->

    <owl:Class rdf:about="http://www.ontologylibrary.mil/OperationalEnvironment/Mid/OEFutureWarfareOntology#CyberSecurityControlledVocabulary">
        <rdfs:subClassOf rdf:resource="http://www.ontologylibrary.mil/OperationalEnvironment/Mid/OEFutureWarfareOntology#CyberAndSpaceControlledVocabulary"/>
    </owl:Class>
    


    <!-- http://www.ontologylibrary.mil/OperationalEnvironment/Mid/OEFutureWarfareOntology#Data -->

    <owl:Class rdf:about="http://www.ontologylibrary.mil/OperationalEnvironment/Mid/OEFutureWarfareOntology#Data">
        <rdfs:subClassOf rdf:resource="http://www.ontologylibrary.mil/OperationalEnvironment/Mid/OEFutureWarfareOntology#BigDataControlledVocabulary"/>
        <obo:IAO_0000115>reinterpretable representation of information in a formalized manner suitable for communication, interpretation, or processing

Note 1 to entry:	data can be processed by humans or by automatic means.</obo:IAO_0000115>
        <obo:IAO_0000119>Information technology — Big data — Overview and vocabulary

https://www.iso.org/jtc1</obo:IAO_0000119>
        <obo:IAO_0000119>[SOURCE: ISO/IEC 2382:2015, 2122101]</obo:IAO_0000119>
    </owl:Class>
    


    <!-- http://www.ontologylibrary.mil/OperationalEnvironment/Mid/OEFutureWarfareOntology#DataAnalytics -->

    <owl:Class rdf:about="http://www.ontologylibrary.mil/OperationalEnvironment/Mid/OEFutureWarfareOntology#DataAnalytics">
        <rdfs:subClassOf rdf:resource="http://www.ontologylibrary.mil/OperationalEnvironment/Mid/OEFutureWarfareOntology#BigDataControlledVocabulary"/>
        <obo:IAO_0000115>composite concept consisting of data acquisition, data collection, data validation, data processing (3.1.11), including data quantification, data visualization, and data interpretation

Note 1 to entry: Data analytics is used to understand objects represented by data (3.1.5), to make predictions for a given situation, and to recommend on steps to achieve objectives. The insights obtained from analytics are used for various purposes such as decision-making, research, sustainable development, design, planning, etc.</obo:IAO_0000115>
        <obo:IAO_0000119>Information technology — Big data — Overview and vocabulary

https://www.iso.org/jtc1</obo:IAO_0000119>
    </owl:Class>
    


    <!-- http://www.ontologylibrary.mil/OperationalEnvironment/Mid/OEFutureWarfareOntology#DataConsumer -->

    <owl:Class rdf:about="http://www.ontologylibrary.mil/OperationalEnvironment/Mid/OEFutureWarfareOntology#DataConsumer">
        <rdfs:subClassOf rdf:resource="http://www.ontologylibrary.mil/OperationalEnvironment/Mid/OEFutureWarfareOntology#BigDataRole"/>
        <obo:IAO_0000115>The Data Consumer receives the value output of the Big Data system. In many respects, it is the recipient of the same type of functional interfaces that the Data Provider exposes to the Big Data Application Provider. After the system adds value to the original data sources, the Big Data Application Provider then exposes that same type of functional interfaces to the Data Consumer.</obo:IAO_0000115>
        <obo:IAO_0000119>NIST Big Data Interoperability Framework: Volume 6, Reference Architecture

Final Version 1 

NIST Big Data Public Working Group (NBD-PWG) Reference Architecture Subgroup Information Technology Laboratory</obo:IAO_0000119>
    </owl:Class>
    


    <!-- http://www.ontologylibrary.mil/OperationalEnvironment/Mid/OEFutureWarfareOntology#DataEngineering -->

    <owl:Class rdf:about="http://www.ontologylibrary.mil/OperationalEnvironment/Mid/OEFutureWarfareOntology#DataEngineering">
        <rdfs:subClassOf rdf:resource="http://www.ontologylibrary.mil/OperationalEnvironment/Mid/OEFutureWarfareOntology#BigDataControlledVocabulary"/>
        <obo:IAO_0000115>discipline which is related to the engineering aspects of systems, processing, models and management of data (3.1.5), including but not limited to big data (3.1.2).</obo:IAO_0000115>
        <obo:IAO_0000119>Information technology — Big data — Overview and vocabulary

https://www.iso.org/jtc1</obo:IAO_0000119>
    </owl:Class>
    


    <!-- http://www.ontologylibrary.mil/OperationalEnvironment/Mid/OEFutureWarfareOntology#DataModel -->

    <owl:Class rdf:about="http://www.ontologylibrary.mil/OperationalEnvironment/Mid/OEFutureWarfareOntology#DataModel">
        <rdfs:subClassOf rdf:resource="http://www.ontologylibrary.mil/OperationalEnvironment/Mid/OEFutureWarfareOntology#BigDataControlledVocabulary"/>
        <obo:IAO_0000115>pattern of structuring data (3.1.5) in a database (3.1.7) according to the formal descriptions in its information system and according to the requirements of the database management system to be applied</obo:IAO_0000115>
        <obo:IAO_0000119>Information technology — Big data — Overview and vocabulary

https://www.iso.org/jtc1</obo:IAO_0000119>
        <obo:IAO_0000119>[SOURCE: ISO/IEC 2382:2015, 17.01.07]</obo:IAO_0000119>
    </owl:Class>
    


    <!-- http://www.ontologylibrary.mil/OperationalEnvironment/Mid/OEFutureWarfareOntology#DataMonetaryValue -->

    <owl:Class rdf:about="http://www.ontologylibrary.mil/OperationalEnvironment/Mid/OEFutureWarfareOntology#DataMonetaryValue">
        <rdfs:subClassOf rdf:resource="http://www.ontologylibrary.mil/OperationalEnvironment/Mid/OEFutureWarfareOntology#BigDataControlledVocabulary"/>
        <obo:IAO_0000115>excess return on investment over the cost of acquiring, processing, and maintaining the data (3.1.5)</obo:IAO_0000115>
        <obo:IAO_0000119>Information technology — Big data — Overview and vocabulary

https://www.iso.org/jtc1</obo:IAO_0000119>
    </owl:Class>
    


    <!-- http://www.ontologylibrary.mil/OperationalEnvironment/Mid/OEFutureWarfareOntology#DataProcessing -->

    <owl:Class rdf:about="http://www.ontologylibrary.mil/OperationalEnvironment/Mid/OEFutureWarfareOntology#DataProcessing">
        <rdfs:subClassOf rdf:resource="http://www.ontologylibrary.mil/OperationalEnvironment/Mid/OEFutureWarfareOntology#BigDataControlledVocabulary"/>
        <obo:IAO_0000115>systematic performance of operations upon data(3.1.5)

Note 1 to entry: Example: Arithmetic or logic operations upon data, merging or sorting of data, or operations on text, such as editing, sorting, merging, storing, retrieving, displaying, or printing.

Note 2 to entry: The term data processing should not be used as a synonym for information processing.</obo:IAO_0000115>
        <obo:IAO_0000119>Information technology — Big data — Overview and vocabulary

https://www.iso.org/jtc1</obo:IAO_0000119>
        <obo:IAO_0000119>[SOURCE: ISO/IEC 2382:2015, 01.01.06]</obo:IAO_0000119>
    </owl:Class>
    


    <!-- http://www.ontologylibrary.mil/OperationalEnvironment/Mid/OEFutureWarfareOntology#DataProvider -->

    <owl:Class rdf:about="http://www.ontologylibrary.mil/OperationalEnvironment/Mid/OEFutureWarfareOntology#DataProvider">
        <rdfs:subClassOf rdf:resource="http://www.ontologylibrary.mil/OperationalEnvironment/Mid/OEFutureWarfareOntology#BigDataRole"/>
        <obo:IAO_0000115>A Data Provider makes data available to itself or to others. In fulfilling its role, the Data Provider creates an abstraction of various types of data sources (such as raw data or data previously transformed by another system) and makes them available through different functional interfaces. The actor fulfilling this role can be part of the Big Data system, internal to the organization in another system, or external to the organization orchestrating the system. While the concept of a Data Provider is not new, the greater data collection and analytics capabilities have opened up new possibilities for providing valuable data.

The Data Provider role introduces new data or information feeds into the Big Data system for discovery, access, and transformation by the Big Data system. New data feeds are distinct from the data already in use by the system and residing in the various system repositories. Similar technologies can be used to access both new data feeds and existing data. The Data Provider actors can be anything from a sensor, to a human inputting data manually, to another Big Data system.

The Data Provider exposes a collection of interfaces (or services) for discovering and accessing the data. These interfaces would typically include a registry so that applications can locate a Data Provider, identify the data of interest it contains, understand the types of access allowed, understand the types of analysis supported, locate the data source, determine data access methods, identify the data security requirements, identify the data privacy requirements, and other pertinent information. Therefore, the interface would provide the means to register the data source, query the registry, and identify a standard set of data contained by the registry.</obo:IAO_0000115>
        <obo:IAO_0000119>NIST Big Data Interoperability Framework: Volume 6, Reference Architecture

Final Version 1 

NIST Big Data Public Working Group (NBD-PWG) Reference Architecture Subgroup Information Technology Laboratory</obo:IAO_0000119>
    </owl:Class>
    


    <!-- http://www.ontologylibrary.mil/OperationalEnvironment/Mid/OEFutureWarfareOntology#DataScience -->

    <owl:Class rdf:about="http://www.ontologylibrary.mil/OperationalEnvironment/Mid/OEFutureWarfareOntology#DataScience">
        <rdfs:subClassOf rdf:resource="http://www.ontologylibrary.mil/OperationalEnvironment/Mid/OEFutureWarfareOntology#BigDataControlledVocabulary"/>
        <obo:IAO_0000115>Data science refers to the process for extracting knowledge from data – the approach can be either through exploration or by hypothesis testing. Data Science refers to the complete data analytics lifecycle where data analytics is understood</obo:IAO_0000115>
        <obo:IAO_0000115>extraction of actionable knowledge from data (3.1.5) through a process of discovery, or hypothesis and hypothesis testing</obo:IAO_0000115>
        <obo:IAO_0000119>Information technology — Big data — Overview and vocabulary

https://www.iso.org/jtc1</obo:IAO_0000119>
    </owl:Class>
    


    <!-- http://www.ontologylibrary.mil/OperationalEnvironment/Mid/OEFutureWarfareOntology#DataSet -->

    <owl:Class rdf:about="http://www.ontologylibrary.mil/OperationalEnvironment/Mid/OEFutureWarfareOntology#DataSet">
        <rdfs:subClassOf rdf:resource="http://www.ontologylibrary.mil/OperationalEnvironment/Mid/OEFutureWarfareOntology#BigDataControlledVocabulary"/>
        <obo:IAO_0000115>identifiable collection of data (3.1.5) available for access or download in one or more formats</obo:IAO_0000115>
        <obo:IAO_0000119>Information technology — Big data — Overview and vocabulary

https://www.iso.org/jtc1</obo:IAO_0000119>
        <obo:IAO_0000119>[SOURCE: Adapted from ISO 19115-2:2009 (en), 4.7]</obo:IAO_0000119>
    </owl:Class>
    


    <!-- http://www.ontologylibrary.mil/OperationalEnvironment/Mid/OEFutureWarfareOntology#DataType -->

    <owl:Class rdf:about="http://www.ontologylibrary.mil/OperationalEnvironment/Mid/OEFutureWarfareOntology#DataType">
        <rdfs:subClassOf rdf:resource="http://www.ontologylibrary.mil/OperationalEnvironment/Mid/OEFutureWarfareOntology#BigDataControlledVocabulary"/>
        <obo:IAO_0000115>defined set of data (3.1.5) objects of a specified data structure and a set of permissible operations, such that these data objects act as operands in the execution of any one of these operations

Note 1 to entry: Example: An integer type has a very simple structure, each occurrence of which, usually called value, is a representation of a member of a specified range of whole numbers and the permissible operations include the usual arithmetic operations on these integers.

Note 2 to entry: The term &quot;type&quot; may be used instead of &quot;data type&quot; when there is no ambiguity.

Note 3 to entry: data type; datatype: terms and definition standardized by ISO/IEC [ISO/IEC 2382-15:1999].</obo:IAO_0000115>
        <obo:IAO_0000119>Information technology — Big data — Overview and vocabulary

https://www.iso.org/jtc1</obo:IAO_0000119>
        <obo:IAO_0000119>[SOURCE: ISO/IEC 2382:2015, 2122374]</obo:IAO_0000119>
    </owl:Class>
    


    <!-- http://www.ontologylibrary.mil/OperationalEnvironment/Mid/OEFutureWarfareOntology#DataVariability -->

    <owl:Class rdf:about="http://www.ontologylibrary.mil/OperationalEnvironment/Mid/OEFutureWarfareOntology#DataVariability">
        <rdfs:subClassOf rdf:resource="http://www.ontologylibrary.mil/OperationalEnvironment/Mid/OEFutureWarfareOntology#BigDataControlledVocabulary"/>
        <obo:IAO_0000115>Data variability refers to changes in data rate, format/structure, semantics, and/or quality that impact the supported application, analytic, or problem. Impacts can include the need to refactor architectures, interfaces, processing/algorithms, integration/fusion, storage, applicability, or use of the data. In addition, a variability in data volumes implies the need to scale-up or scale-down virtualized resources to efficiently handle the additional processing load.</obo:IAO_0000115>
        <obo:IAO_0000115>changes in transmission rate, format or structure, semantics, or quality of datasets (3.1.12)</obo:IAO_0000115>
        <obo:IAO_0000119>Information technology — Big data — Overview and vocabulary

https://www.iso.org/jtc1</obo:IAO_0000119>
    </owl:Class>
    


    <!-- http://www.ontologylibrary.mil/OperationalEnvironment/Mid/OEFutureWarfareOntology#DataVariety -->

    <owl:Class rdf:about="http://www.ontologylibrary.mil/OperationalEnvironment/Mid/OEFutureWarfareOntology#DataVariety">
        <rdfs:subClassOf rdf:resource="http://www.ontologylibrary.mil/OperationalEnvironment/Mid/OEFutureWarfareOntology#BigDataControlledVocabulary"/>
        <obo:IAO_0000115>Data variety represents the need to analyse data from a number of domains and a number of data types. The variety of data was handled through transformations or pre-analytics to identify features that would allow integration with other data. The wider range of data formats, logical models, timescales, and semantics, which is desirous to be used in data analytics, complicates the integration of the variety of data. Metadata is increasingly used to aid in the integration. Impacts of variety on big data include that it requires the semantics of the data to be machine readable.</obo:IAO_0000115>
        <obo:IAO_0000115>range of formats, logical models, timescales, and semantics of a dataset (3.1.12)

Note 1 to entry: Data variety refers to irregular or heterogeneous data structures, their navigation, query, and data typing.</obo:IAO_0000115>
        <obo:IAO_0000119>Information technology — Big data — Overview and vocabulary

https://www.iso.org/jtc1</obo:IAO_0000119>
    </owl:Class>
    


    <!-- http://www.ontologylibrary.mil/OperationalEnvironment/Mid/OEFutureWarfareOntology#DataVelocity -->

    <owl:Class rdf:about="http://www.ontologylibrary.mil/OperationalEnvironment/Mid/OEFutureWarfareOntology#DataVelocity">
        <rdfs:subClassOf rdf:resource="http://www.ontologylibrary.mil/OperationalEnvironment/Mid/OEFutureWarfareOntology#BigDataControlledVocabulary"/>
        <obo:IAO_0000115>Data velocity is the rate of flow at which the data is created, stored, analysed or visualized. Big data velocity means a large quantity of data needs to be processed in a short amount of time. An example of dealing with high velocity data is commonly referred to as techniques for streaming data.</obo:IAO_0000115>
        <obo:IAO_0000115>rate of flow at which data (3.1.5) is created, transmitted, stored, analysed or visualised</obo:IAO_0000115>
        <obo:IAO_0000119>Information technology — Big data — Overview and vocabulary

https://www.iso.org/jtc1</obo:IAO_0000119>
    </owl:Class>
    


    <!-- http://www.ontologylibrary.mil/OperationalEnvironment/Mid/OEFutureWarfareOntology#DataVeracity -->

    <owl:Class rdf:about="http://www.ontologylibrary.mil/OperationalEnvironment/Mid/OEFutureWarfareOntology#DataVeracity">
        <rdfs:subClassOf rdf:resource="http://www.ontologylibrary.mil/OperationalEnvironment/Mid/OEFutureWarfareOntology#BigDataControlledVocabulary"/>
        <obo:IAO_0000115>Data veracity refers to the completeness and accuracy of the data and relates to the vernacular “garbage-in, garbage-out” description for data quality issues in existence for a long time. If the data analytics are causal, then the quality of every data element is extremely important. If the data analytics are correlations or trending over massive volume datasets, then individual bad elements could be lost in the overall counts and the trend could still be accurate.</obo:IAO_0000115>
        <obo:IAO_0000115>completeness and/or accuracy of data (3.1.5)

Note 1 to entry: Data veracity refers to descriptive data and self-inquiry about objects to support real-time decision-making.</obo:IAO_0000115>
        <obo:IAO_0000119>Information technology — Big data — Overview and vocabulary

https://www.iso.org/jtc1</obo:IAO_0000119>
    </owl:Class>
    


    <!-- http://www.ontologylibrary.mil/OperationalEnvironment/Mid/OEFutureWarfareOntology#DataVisualization -->

    <owl:Class rdf:about="http://www.ontologylibrary.mil/OperationalEnvironment/Mid/OEFutureWarfareOntology#DataVisualization">
        <rdfs:subClassOf rdf:resource="http://www.ontologylibrary.mil/OperationalEnvironment/Mid/OEFutureWarfareOntology#BigDataControlledVocabulary"/>
        <obo:IAO_0000115>Data visualization refers to the presentation of data to allow the viewer to discern information about the data being displayed. Big data has required new techniques for large volume datasets, including aggregation and summarization to make the data more accessible visually. Big data also requires more attention to the visual presentation to decision-makers – to convey easily understood results while also communicating the complexity, accuracy, and probabilistic error range on the results.</obo:IAO_0000115>
        <obo:IAO_0000119>Information technology — Big data — Overview and vocabulary

https://www.iso.org/jtc1</obo:IAO_0000119>
    </owl:Class>
    


    <!-- http://www.ontologylibrary.mil/OperationalEnvironment/Mid/OEFutureWarfareOntology#DataVolatility -->

    <owl:Class rdf:about="http://www.ontologylibrary.mil/OperationalEnvironment/Mid/OEFutureWarfareOntology#DataVolatility">
        <rdfs:subClassOf rdf:resource="http://www.ontologylibrary.mil/OperationalEnvironment/Mid/OEFutureWarfareOntology#BigDataControlledVocabulary"/>
        <obo:IAO_0000115>Data volatility refers to a limited time span in which data values remain relevant for a particular analysis, expressed as a rate of change over time. In real-time data analytics situations, it is critical to operate on data immediately for decision-making. This is most evident in high velocity situations such as stock markets or telecommunications. However,  data that is no longer valid for a particular time sensitive analytic due to time decay may still be valid for other non-time sensitive analytics.</obo:IAO_0000115>
        <obo:IAO_0000115>characteristic of data (3.1.5) pertaining to the rate of change of these data over time</obo:IAO_0000115>
        <obo:IAO_0000119>Information technology — Big data — Overview and vocabulary

https://www.iso.org/jtc1</obo:IAO_0000119>
        <obo:IAO_0000119>[SOURCE: ISO/IEC 2382:2015, 17.06.06]</obo:IAO_0000119>
    </owl:Class>
    


    <!-- http://www.ontologylibrary.mil/OperationalEnvironment/Mid/OEFutureWarfareOntology#DataVolume -->

    <owl:Class rdf:about="http://www.ontologylibrary.mil/OperationalEnvironment/Mid/OEFutureWarfareOntology#DataVolume">
        <rdfs:subClassOf rdf:resource="http://www.ontologylibrary.mil/OperationalEnvironment/Mid/OEFutureWarfareOntology#BigDataControlledVocabulary"/>
        <obo:IAO_0000115>Data volume represents the extensive amount of data available for analysis to extract valuable information. The massive amounts of data generated through internet activity was one of the primary drivers for the development of the big data processing techniques.</obo:IAO_0000115>
        <obo:IAO_0000115>Extent of the amount of data (3.1.5) relevant to impacting computation and storage resources and their management during data processing

Note 1 to entry: Data volume becomes important in dealing with large datasets (3.1.13), including their</obo:IAO_0000115>
        <obo:IAO_0000119>Information technology — Big data — Overview and vocabulary

https://www.iso.org/jtc1</obo:IAO_0000119>
    </owl:Class>
    


    <!-- http://www.ontologylibrary.mil/OperationalEnvironment/Mid/OEFutureWarfareOntology#Database -->

    <owl:Class rdf:about="http://www.ontologylibrary.mil/OperationalEnvironment/Mid/OEFutureWarfareOntology#Database">
        <rdfs:subClassOf rdf:resource="http://www.ontologylibrary.mil/OperationalEnvironment/Mid/OEFutureWarfareOntology#BigDataControlledVocabulary"/>
        <obo:IAO_0000115>collection of data (3.1.5) organized according to a conceptual structure describing the characteristics of these data and the relationships among their corresponding entities, supporting one or more application areas</obo:IAO_0000115>
        <obo:IAO_0000119>Information technology — Big data — Overview and vocabulary

https://www.iso.org/jtc1</obo:IAO_0000119>
        <obo:IAO_0000119>[SOURCE: ISO/IEC 2382:2015, 01.08.05]</obo:IAO_0000119>
    </owl:Class>
    


    <!-- http://www.ontologylibrary.mil/OperationalEnvironment/Mid/OEFutureWarfareOntology#DecliningFertilityRate -->

    <owl:Class rdf:about="http://www.ontologylibrary.mil/OperationalEnvironment/Mid/OEFutureWarfareOntology#DecliningFertilityRate">
        <rdfs:subClassOf rdf:resource="http://www.ontologylibrary.mil/OperationalEnvironment/Mid/OEFutureWarfareOntology#AgingPopulation"/>
        <obo:IAO_0000119>Nicola Davis, &quot;Falling Total Fertility Rate Should Be Welcomed, Population Expert Says&quot;, The Guardian

December 26, 2018

https://www.theguardian.com/world/2018/dec/26/falling-total-fertility-rate-should-be-welcomed-population-expert-says</obo:IAO_0000119>
        <CommonCoreOntologies:definition>Declines in total fertility rate have been seen time and again after national economies develop, public health improves, and infant mortality falls, and women find themselves raising larger families. ...[Drivers] for such declines included huge strides in family planning and women’s education – with girls staying at school and entering the workforce - allowing women to delay childbearing and choose how many children to have – if any.</CommonCoreOntologies:definition>
        <rdfs:label>Declining Fertility Rate</rdfs:label>
    </owl:Class>
    


    <!-- http://www.ontologylibrary.mil/OperationalEnvironment/Mid/OEFutureWarfareOntology#Decoys -->

    <owl:Class rdf:about="http://www.ontologylibrary.mil/OperationalEnvironment/Mid/OEFutureWarfareOntology#Decoys">
        <rdfs:subClassOf rdf:resource="http://www.ontologylibrary.mil/OperationalEnvironment/Mid/OEFutureWarfareOntology#SystemsThatProtect"/>
        <obo:IAO_0000115>Must deceive multi-disciplined intelligence. [SOURCE: TRADOC G-2 Potential Game Changers, May 2018]</obo:IAO_0000115>
        <obo:IAO_0000119>Technology Environment of Ground Warfare in 2035-2050

Projections made in 2018 by ARL and TRADOC

[This is a draft outline of a potential document; prepared by Alexander Kott, the US Army Research Laboratory; July 2018]</obo:IAO_0000119>
    </owl:Class>
    


    <!-- http://www.ontologylibrary.mil/OperationalEnvironment/Mid/OEFutureWarfareOntology#DeepLearning -->

    <owl:Class rdf:about="http://www.ontologylibrary.mil/OperationalEnvironment/Mid/OEFutureWarfareOntology#DeepLearning">
        <rdfs:subClassOf rdf:resource="http://www.ontologylibrary.mil/OperationalEnvironment/Mid/OEFutureWarfareOntology#ArtificialIntelligenceControlledVocabulary"/>
        <obo:IAO_0000115>At the cutting edge of machine learning*, this technique enables a machine to independently recognize complex concepts such as faces, human bodies, or images of cats. This is done by scouring millions of images picked from the internet – images that have not been labelled by humans. The result of a combination of learning algorithms and formal neural networks* and the use of mass data, deep learning has revolutionized artificial intelligence. It has countless applications, including search engines, medical diagnosis, autonomous cars, etc. In 2015, the AlphaGo computer used deep learning to beat humans at Go, the ancient Chinese board game.</obo:IAO_0000115>
        <obo:IAO_0000115>United Nations Educational, Scientific, and Cultural Organization Courier 

March 2018

https://en.unesco.org/courier/2018-3/lexicon-artificial-intelligence</obo:IAO_0000115>
    </owl:Class>
    


    <!-- http://www.ontologylibrary.mil/OperationalEnvironment/Mid/OEFutureWarfareOntology#Democracy -->

    <owl:Class rdf:about="http://www.ontologylibrary.mil/OperationalEnvironment/Mid/OEFutureWarfareOntology#Democracy">
        <rdfs:subClassOf rdf:resource="http://www.ontologylibrary.mil/OperationalEnvironment/Mid/OEFutureWarfareOntology#Government"/>
        <obo:IAO_0000115>Democracy...is a system of government where the citizens exercise power by voting.... In a representative democracy the citizens elect representatives from among themselves. These representatives meet to form a governing body, such as a legislature. In a constitutional democracy the powers of the majority are exercised within the framework of a representative democracy, but the constitution limits the majority and protects the minority, usually through the enjoyment by all of certain individual rights, e.g. freedom of speech, or freedom of association. &quot;Rule of the majority&quot; is sometimes referred to as democracy

...

...[Democracy] consists of four key elements: a political system for choosing and replacing the government through free and fair elections; the active participation of the people, as citizens, in politics and civic life; protection of the human rights of all citizens; a rule of law, in which the laws and procedures apply equally to all citizens.</obo:IAO_0000115>
        <obo:IAO_0000119>&quot;Democracy&quot;, Wikipedia

March 12, 2019

https://en.wikipedia.org/wiki/Democracy</obo:IAO_0000119>
        <rdfs:label>Democracy</rdfs:label>
    </owl:Class>
    


    <!-- http://www.ontologylibrary.mil/OperationalEnvironment/Mid/OEFutureWarfareOntology#Demographics -->

    <owl:Class rdf:about="http://www.ontologylibrary.mil/OperationalEnvironment/Mid/OEFutureWarfareOntology#Demographics">
        <rdfs:subClassOf rdf:resource="http://www.ontologylibrary.mil/OperationalEnvironment/Mid/OEFutureWarfareOntology#HumanFactorsControlledVocabulary"/>
        <rdfs:label>Demographics</rdfs:label>
    </owl:Class>
    


    <!-- http://www.ontologylibrary.mil/OperationalEnvironment/Mid/OEFutureWarfareOntology#DemographicsAndUrbanizationControlledVocabulary -->

    <owl:Class rdf:about="http://www.ontologylibrary.mil/OperationalEnvironment/Mid/OEFutureWarfareOntology#DemographicsAndUrbanizationControlledVocabulary">
        <rdfs:subClassOf rdf:resource="http://www.ontologylibrary.mil/OperationalEnvironment/Mid/OEFutureWarfareOntology#ControlledVocabulary"/>
    </owl:Class>
    


    <!-- http://www.ontologylibrary.mil/OperationalEnvironment/Mid/OEFutureWarfareOntology#DemographicsAndUrbanizationTrend -->

    <owl:Class rdf:about="http://www.ontologylibrary.mil/OperationalEnvironment/Mid/OEFutureWarfareOntology#DemographicsAndUrbanizationTrend">
        <rdfs:subClassOf rdf:resource="http://www.ontologylibrary.mil/OperationalEnvironment/Mid/OEFutureWarfareOntology#Trend"/>
        <obo:IAO_0000115>Humanity will become richer, older, more urban, and better educated, but the uneven distribution of this progress will accelerate tension and conflict.  The convergence of more information and more people with fewer state resources will constrain governments’ efforts to address rampant poverty, violence, and pollution, and create a breeding ground for dissatisfaction among increasingly aware, yet still disempowered populations. These factors will be attenuated by a changing climate, which has the potential to create additional crises and discontent.  The addition of over seven billion people over the last century has altered geography itself, and cities now sprawl over large areas of the globe and contain almost two-thirds of the world’s population. These numbers will only increase.  Some megacities will become more important politically and economically than the nationstate in which they reside.  Life will become both easier and more complex, with those able to take advantage of the leading edge of technological advancement increasingly exploiting those who cannot.  New social stresses and fractures will lead to strife and population migrations, which in turn create further challenges for urbanized areas.  Furthermore, the move of large numbers of people to large urban areas and megacities will strain resources, as these area will become increasingly reliant on rural areas for food, water, and even additional power.  From a military perspective, cities represent challenges, opportunities, and unique vulnerabilities.</obo:IAO_0000115>
        <obo:IAO_0000115>Our adversaries will operate in and among populations and in complex terrain, and endeavor to mitigate many of our own traditional technological advantages and force us to operate with degraded capabilities and take advantage of the infrastructure and other resources cities offer.</obo:IAO_0000115>
        <obo:IAO_0000119>The Operational Environment and the Changing Character of Future Warfare</obo:IAO_0000119>
    </owl:Class>
    


    <!-- http://www.ontologylibrary.mil/OperationalEnvironment/Mid/OEFutureWarfareOntology#DenseUrbanArea -->

    <owl:Class rdf:about="http://www.ontologylibrary.mil/OperationalEnvironment/Mid/OEFutureWarfareOntology#DenseUrbanArea">
        <rdfs:subClassOf rdf:resource="http://www.ontologylibrary.mil/OperationalEnvironment/Mid/OEFutureWarfareOntology#Urbanization"/>
        <obo:IAO_0000232>There&apos;s essentially nothing in the public discourse that addresses the Army&apos;s concerns about dense urban areas:  whereas the Army sees these areas as posing unusual operational challenges (that is, making operations more difficult), most social scientists and commentators focus on the ways in which dense urban areas make commerce, culture, and the provision of services easier.</obo:IAO_0000232>
        <rdfs:label>Dense Urban Area</rdfs:label>
    </owl:Class>
    


    <!-- http://www.ontologylibrary.mil/OperationalEnvironment/Mid/OEFutureWarfareOntology#DerivedMeasure -->

    <owl:Class rdf:about="http://www.ontologylibrary.mil/OperationalEnvironment/Mid/OEFutureWarfareOntology#DerivedMeasure">
        <rdfs:subClassOf rdf:resource="http://www.ontologylibrary.mil/OperationalEnvironment/Mid/OEFutureWarfareOntology#CyberSecurityControlledVocabulary"/>
        <obo:IAO_0000115>measure (3.42) that is defined as a function of two or more values of base measures (3.8)</obo:IAO_0000115>
        <obo:IAO_0000119>International Organization for Standardization/International Electrotechnical Commission 27000:2018

Security techniques — Information security management systems — Overview and vocabulary

Publication date : 2018-02

5th Edition</obo:IAO_0000119>
    </owl:Class>
    


    <!-- http://www.ontologylibrary.mil/OperationalEnvironment/Mid/OEFutureWarfareOntology#Dictatorship -->

    <owl:Class rdf:about="http://www.ontologylibrary.mil/OperationalEnvironment/Mid/OEFutureWarfareOntology#Dictatorship">
        <rdfs:subClassOf rdf:resource="http://www.ontologylibrary.mil/OperationalEnvironment/Mid/OEFutureWarfareOntology#Authoritariansim"/>
        <obo:IAO_0000115>(1)

A dictatorship is an authoritarian form of government, characterized by a single leader or group of leaders with either no party or a weak party, little mass mobilization, and limited political pluralism....A common aspect that characterized dictators is taking advantage of their strong personality, usually by suppressing freedom of thought and speech of the masses, in order to maintain complete political and social supremacy and stability. Dictatorships and totalitarian societies generally employ political propaganda to decrease the influence of proponents of alternative governing systems.</obo:IAO_0000115>
        <obo:IAO_0000115>(2)

A dictator is a political leader who possesses absolute power. A state which is ruled by a dictator is called a dictatorship

...

...[The] term &quot;dictator&quot; is generally used to describe a leader who holds or abuses an extraordinary amount of personal power. Dictatorships are often characterised by some of the following: suspension of elections and civil liberties; proclamation of a state of emergency; rule by decree; repression of political opponents; not abiding by the rule of law procedures, and cult of personality. Dictatorships are often one-party or dominant-party states.

A wide variety of leaders coming to power in different kinds of regimes, such as military juntas, one-party states, dominant-party states, and civilian governments under a personal rule, have been described as dictators. They may hold left or right-wing views, or may be apolitical.</obo:IAO_0000115>
        <obo:IAO_0000119>(1)

&quot;Dictatorship&quot;, Wikipedia

March 12, 2019

https://en.wikipedia.org/wiki/Dictatorship</obo:IAO_0000119>
        <obo:IAO_0000119>(2)

&quot;Dictator&quot;, Wikipedia

March 12, 2019

https://en.wikipedia.org/wiki/Dictator</obo:IAO_0000119>
        <rdfs:label>Dictatorship</rdfs:label>
    </owl:Class>
    


    <!-- http://www.ontologylibrary.mil/OperationalEnvironment/Mid/OEFutureWarfareOntology#DirectGreenhouseGasEmission -->

    <owl:Class rdf:about="http://www.ontologylibrary.mil/OperationalEnvironment/Mid/OEFutureWarfareOntology#DirectGreenhouseGasEmission">
        <rdfs:subClassOf rdf:resource="http://www.ontologylibrary.mil/OperationalEnvironment/Mid/OEFutureWarfareOntology#ClimateChangeAndResourceCompetitionControlledVocabulary"/>
        <obo:IAO_0000115>Greenhouse gas emission from greenhouse gas sources owned or controlled by the organization

Note 1 to entry: This document uses the concepts of equity share or control (financial or operational control) to establish organizational boundaries.</obo:IAO_0000115>
        <obo:IAO_0000119>International Organization for Standardization/International Electrotechnical Commission 27000:2018

Technical Committee : ISO/TC 207/SC 7  Greenhouse gas management and related activities

ICS :  13.020.40  Pollution, pollution control and conservation

Greenhouse gases -- Part 1: Specification with guidance at the organization level for quantification and reporting of greenhouse gas emissions and removals 

Publication date : 2018-12

2nd Edition</obo:IAO_0000119>
    </owl:Class>
    


    <!-- http://www.ontologylibrary.mil/OperationalEnvironment/Mid/OEFutureWarfareOntology#DirectGreenhouseGasRemoval -->

    <owl:Class rdf:about="http://www.ontologylibrary.mil/OperationalEnvironment/Mid/OEFutureWarfareOntology#DirectGreenhouseGasRemoval">
        <rdfs:subClassOf rdf:resource="http://www.ontologylibrary.mil/OperationalEnvironment/Mid/OEFutureWarfareOntology#ClimateChangeAndResourceCompetitionControlledVocabulary"/>
        <obo:IAO_0000115>Greenhouse gas removal (3.1.6) from greenhouse gas sinks (3.1.3) owned or controlled by the organization (3.4.2)</obo:IAO_0000115>
        <obo:IAO_0000119>International Organization for Standardization/International Electrotechnical Commission 27000:2018

Technical Committee : ISO/TC 207/SC 7  Greenhouse gas management and related activities

ICS :  13.020.40  Pollution, pollution control and conservation

Greenhouse gases -- Part 1: Specification with guidance at the organization level for quantification and reporting of greenhouse gas emissions and removals 

Publication date : 2018-12

2nd Edition</obo:IAO_0000119>
    </owl:Class>
    


    <!-- http://www.ontologylibrary.mil/OperationalEnvironment/Mid/OEFutureWarfareOntology#DirectLandUseChange -->

    <owl:Class rdf:about="http://www.ontologylibrary.mil/OperationalEnvironment/Mid/OEFutureWarfareOntology#DirectLandUseChange">
        <rdfs:subClassOf rdf:resource="http://www.ontologylibrary.mil/OperationalEnvironment/Mid/OEFutureWarfareOntology#ClimateChangeAndResourceCompetitionControlledVocabulary"/>
        <obo:IAO_0000115>change in the human use of land within the relevant boundary

Note 1 to entry: Relevant boundary is the reporting boundary (3.4.8).</obo:IAO_0000115>
        <obo:IAO_0000119>International Organization for Standardization/International Electrotechnical Commission 27000:2018

Technical Committee : ISO/TC 207/SC 7  Greenhouse gas management and related activities

ICS :  13.020.40  Pollution, pollution control and conservation

Greenhouse gases -- Part 1: Specification with guidance at the organization level for quantification and reporting of greenhouse gas emissions and removals 

Publication date : 2018-12

2nd Edition</obo:IAO_0000119>
    </owl:Class>
    


    <!-- http://www.ontologylibrary.mil/OperationalEnvironment/Mid/OEFutureWarfareOntology#DirectedEnergyWeapons -->

    <owl:Class rdf:about="http://www.ontologylibrary.mil/OperationalEnvironment/Mid/OEFutureWarfareOntology#DirectedEnergyWeapons">
        <rdfs:subClassOf rdf:resource="http://www.ontologylibrary.mil/OperationalEnvironment/Mid/OEFutureWarfareOntology#SystemsThatShoot"/>
        <rdfs:subClassOf>
            <owl:Restriction>
                <owl:onProperty rdf:resource="http://www.ontologylibrary.mil/OperationalEnvironment/Mid/OEFutureWarfareOntology#hasCombatApplication"/>
                <owl:someValuesFrom rdf:resource="http://www.ontologylibrary.mil/OperationalEnvironment/Mid/OEFutureWarfareOntology#ActiveDenialSystems"/>
            </owl:Restriction>
        </rdfs:subClassOf>
    </owl:Class>
    


    <!-- http://www.ontologylibrary.mil/OperationalEnvironment/Mid/OEFutureWarfareOntology#DistributedDataProcessing -->

    <owl:Class rdf:about="http://www.ontologylibrary.mil/OperationalEnvironment/Mid/OEFutureWarfareOntology#DistributedDataProcessing">
        <rdfs:subClassOf rdf:resource="http://www.ontologylibrary.mil/OperationalEnvironment/Mid/OEFutureWarfareOntology#BigDataControlledVocabulary"/>
        <obo:IAO_0000115>The popular framework for distributed computing consists of a storage layer and processing layer combination that implements a multiple-class, algorithm-programming model. Low-cost commodity servers supporting the distributed file system that stores the data can dramatically lower the storage costs of computing on a large scale of data (e.g., web indexing). In distributed data processing a query is scattered across the processors and the results are gathered into a central processor. Processing results are typically then loaded into an analysis environment. Multiple nodes (e.g. client nodes, data nodes, replica nodes) are arranged in a master-slave architecture to achieve efficiency, reliability, high availability, and fault-tolerance of the system.</obo:IAO_0000115>
        <obo:IAO_0000115>data processing (3.1.11) in which the performance of operations is dispersed among the nodes in a computer network</obo:IAO_0000115>
        <obo:IAO_0000119>Information technology — Big data — Overview and vocabulary

https://www.iso.org/jtc1</obo:IAO_0000119>
        <obo:IAO_0000119>[SOURCE: ISO/IEC 2382:2015, 18.01.08]</obo:IAO_0000119>
    </owl:Class>
    


    <!-- http://www.ontologylibrary.mil/OperationalEnvironment/Mid/OEFutureWarfareOntology#DistributedFileSystem -->

    <owl:Class rdf:about="http://www.ontologylibrary.mil/OperationalEnvironment/Mid/OEFutureWarfareOntology#DistributedFileSystem">
        <rdfs:subClassOf rdf:resource="http://www.ontologylibrary.mil/OperationalEnvironment/Mid/OEFutureWarfareOntology#BigDataControlledVocabulary"/>
        <obo:IAO_0000115>In distributed file systems, multi-structured (object) datasets are distributed across the computing nodes of the server cluster(s). The data may be distributed at the file/dataset level, or more commonly, at the block level, allowing multiple nodes in the cluster to interact with different parts of a large file/dataset simultaneously. Big data systems are frequently designed to take advantage of data locality to each node when distributing the processing, which avoids any need to move the data between nodes. In addition, many distributed file systems also implement file/block level replication where each file/block is stored multiple times on different machines nodes for both reliability/recovery (data is not lost if a node in the cluster fails), as well as enhanced data locality. Any type of data and many sizes of files can be handled without formal extract, transformation, and load conversions, with some technologies performing markedly better for large file sizes</obo:IAO_0000115>
        <obo:IAO_0000115>system which manages files and folders across multiple networked systems</obo:IAO_0000115>
        <obo:IAO_0000119>Information technology — Big data — Overview and vocabulary

https://www.iso.org/jtc1</obo:IAO_0000119>
    </owl:Class>
    


    <!-- http://www.ontologylibrary.mil/OperationalEnvironment/Mid/OEFutureWarfareOntology#DocumentedInformation -->

    <owl:Class rdf:about="http://www.ontologylibrary.mil/OperationalEnvironment/Mid/OEFutureWarfareOntology#DocumentedInformation">
        <rdfs:subClassOf rdf:resource="http://www.ontologylibrary.mil/OperationalEnvironment/Mid/OEFutureWarfareOntology#CyberSecurityControlledVocabulary"/>
        <obo:IAO_0000115>information required to be controlled and maintained by an organization (3.50) and the medium on which it is contained

Note 1 to entry: Documented information can be in any format and media and from any source.

Note 2 to entry: Documented information can refer to
— the management system (3.41), including related processes (3.54);
— information created in order for the organization (3.50) to operate (documentation);
— evidence of results achieved (records).</obo:IAO_0000115>
        <obo:IAO_0000119>International Organization for Standardization/International Electrotechnical Commission 27000:2018

Security techniques — Information security management systems — Overview and vocabulary

Publication date : 2018-02

5th Edition</obo:IAO_0000119>
    </owl:Class>
    


    <!-- http://www.ontologylibrary.mil/OperationalEnvironment/Mid/OEFutureWarfareOntology#DuctileMaterial -->

    <owl:Class rdf:about="http://www.ontologylibrary.mil/OperationalEnvironment/Mid/OEFutureWarfareOntology#DuctileMaterial">
        <rdfs:subClassOf rdf:resource="http://www.ontologylibrary.mil/OperationalEnvironment/Mid/OEFutureWarfareOntology#SpaceSystems"/>
        <obo:IAO_0000115>material that can be plastically deformed without breaking under the action of a stress</obo:IAO_0000115>
        <obo:IAO_0000119>International Organization for Standardization/International Electrotechnical Commission 11227:2012

Space systems — Test procedure to evaluate spacecraft material ejecta upon hypervelocity impact

Publication Date: 2012-09

1st Edition</obo:IAO_0000119>
    </owl:Class>
    


    <!-- http://www.ontologylibrary.mil/OperationalEnvironment/Mid/OEFutureWarfareOntology#DurabilityCriteria -->

    <owl:Class rdf:about="http://www.ontologylibrary.mil/OperationalEnvironment/Mid/OEFutureWarfareOntology#DurabilityCriteria">
        <rdfs:subClassOf rdf:resource="http://www.ontologylibrary.mil/OperationalEnvironment/Mid/OEFutureWarfareOntology#SpaceEnvironmentControlledVocabulary"/>
        <obo:IAO_0000115>maximum permissible changes in operational parameters of spacecraft materials and equipment causing by the impact of primary and secondary space environment factors when a material or an equipment element can perform the given function
— radiation hardness
— durability to surface and internal charge accumulation
— mass losses and surface erosion
— surface contamination
— thermal stability

Note 1 to entry: In determining durability criteria, mechanical, thermal, electrical and optical properties of materials are to be considered.</obo:IAO_0000115>
    </owl:Class>
    


    <!-- http://www.ontologylibrary.mil/OperationalEnvironment/Mid/OEFutureWarfareOntology#EarthsIonosphere -->

    <owl:Class rdf:about="http://www.ontologylibrary.mil/OperationalEnvironment/Mid/OEFutureWarfareOntology#EarthsIonosphere">
        <rdfs:subClassOf rdf:resource="http://www.ontologylibrary.mil/OperationalEnvironment/Mid/OEFutureWarfareOntology#SpaceEnvironmentControlledVocabulary"/>
        <obo:IAO_0000115>region of the Earth’s atmosphere at 50 km to 1 500 km height containing partially ionized cold plasma</obo:IAO_0000115>
        <obo:IAO_0000119>International Organization for Standardization/International Electrotechnical Commission 17851:2016

Space systems -- Space environment simulation for material tests -- General principles and criteria

Publication Date: 2016-09

1st Edition</obo:IAO_0000119>
    </owl:Class>
    


    <!-- http://www.ontologylibrary.mil/OperationalEnvironment/Mid/OEFutureWarfareOntology#EarthsMagnetosphere -->

    <owl:Class rdf:about="http://www.ontologylibrary.mil/OperationalEnvironment/Mid/OEFutureWarfareOntology#EarthsMagnetosphere">
        <rdfs:subClassOf rdf:resource="http://www.ontologylibrary.mil/OperationalEnvironment/Mid/OEFutureWarfareOntology#SpaceEnvironmentControlledVocabulary"/>
        <obo:IAO_0000115>region of the near-Earth space occupied by the Earth’s magnetic field where physical conditions are determined by its interaction with solar wind</obo:IAO_0000115>
        <obo:IAO_0000119>International Organization for Standardization/International Electrotechnical Commission 17851:2016

Space systems -- Space environment simulation for material tests -- General principles and criteria

Publication Date: 2016-09

1st Edition</obo:IAO_0000119>
    </owl:Class>
    


    <!-- http://www.ontologylibrary.mil/OperationalEnvironment/Mid/OEFutureWarfareOntology#EconomicActivity -->

    <owl:Class rdf:about="http://www.ontologylibrary.mil/OperationalEnvironment/Mid/OEFutureWarfareOntology#EconomicActivity">
        <rdfs:subClassOf rdf:resource="http://www.ontologylibrary.mil/OperationalEnvironment/Mid/OEFutureWarfareOntology#EconomicsAndTrade"/>
        <obo:IAO_0000119>(1)

&quot;Economy&quot;, Wikipedia

March 13, 2019

https://en.wikipedia.org/wiki/Economy</obo:IAO_0000119>
        <obo:IAO_0000119>(2)

&quot;Economic Activity&quot;, BusinessDictionary.com

March 13, 2019

http://www.businessdictionary.com/definition/economic-activity.html</obo:IAO_0000119>
        <CommonCoreOntologies:definition>(1)

Economic activity is spurred by production which uses natural resources, labor, and capital. It has changed over time due to technology (automation, accelerator of process, reduction of cost functions), innovation (new products, services, processes, expanding markets, diversification of markets, niche markets, increases revenue functions) such as, that which produces intellectual property and changes in industrial relations....</CommonCoreOntologies:definition>
        <CommonCoreOntologies:definition>(2)

Actions that involve the production, distribution and consumption of goods and services at all levels within a society. Gross domestic product or GDP is one way of assessing economic activity, and the degree of current economic activity and forecasts for its future level can significantly impact business activity and profits, as well as inflation and interest rates.</CommonCoreOntologies:definition>
        <rdfs:label>Economic Activity</rdfs:label>
    </owl:Class>
    


    <!-- http://www.ontologylibrary.mil/OperationalEnvironment/Mid/OEFutureWarfareOntology#EconomicDevelopment -->

    <owl:Class rdf:about="http://www.ontologylibrary.mil/OperationalEnvironment/Mid/OEFutureWarfareOntology#EconomicDevelopment">
        <rdfs:subClassOf rdf:resource="http://www.ontologylibrary.mil/OperationalEnvironment/Mid/OEFutureWarfareOntology#EconomicsAndTrade"/>
        <obo:IAO_0000119>&quot;Economic Development&quot;, Wikipedia

March 19, 2019

https://en.wikipedia.org/wiki/Economic_development</obo:IAO_0000119>
        <CommonCoreOntologies:definition>Economic development was concerned with the expansion of people&apos;s entitlements and their corresponding capabilities, morbidity, nourishment, literacy, education, and other socio-economic indicators.

...

Economic growth deals with increase in the level of output, but economic development is related to increase in output coupled with improvement in social and political welfare of people within a country. Therefore, economic development encompasses both growth and welfare values. 

...

[E]conomic development is typically associated with improvements in a variety of areas or indicators (such as literacy rates, life expectancy, and poverty rates), that may be causes of economic development rather than consequences of specific economic development programs.</CommonCoreOntologies:definition>
        <rdfs:label>Economic Development</rdfs:label>
    </owl:Class>
    


    <!-- http://www.ontologylibrary.mil/OperationalEnvironment/Mid/OEFutureWarfareOntology#EconomicGrowth -->

    <owl:Class rdf:about="http://www.ontologylibrary.mil/OperationalEnvironment/Mid/OEFutureWarfareOntology#EconomicGrowth">
        <rdfs:subClassOf rdf:resource="http://www.ontologylibrary.mil/OperationalEnvironment/Mid/OEFutureWarfareOntology#EconomicDevelopment"/>
        <obo:IAO_0000119>&quot;Economic Growth&quot;, Wikipedia

March 19, 2019

https://en.wikipedia.org/wiki/Economic_growth</obo:IAO_0000119>
        <CommonCoreOntologies:definition>Economic growth is the increase in the inflation-adjusted market value of the goods and services produced by an economy over time. It is conventionally measured as the percent rate of increase in real gross domestic product, or real GDP.

Growth is usually calculated in real terms - i.e., inflation-adjusted terms – to eliminate the distorting effect of inflation on the price of goods produced. Measurement of economic growth uses national income accounting. Since economic growth is measured as the annual percent change of gross domestic product (GDP), it has all the advantages and drawbacks of that measure. The economic growth rates of nations are commonly compared using the ratio of the GDP to population or per-capita income.</CommonCoreOntologies:definition>
        <rdfs:label>Economic Growth</rdfs:label>
    </owl:Class>
    


    <!-- http://www.ontologylibrary.mil/OperationalEnvironment/Mid/OEFutureWarfareOntology#EconomicRebalancingControlledVocabulary -->

    <owl:Class rdf:about="http://www.ontologylibrary.mil/OperationalEnvironment/Mid/OEFutureWarfareOntology#EconomicRebalancingControlledVocabulary">
        <rdfs:subClassOf rdf:resource="http://www.ontologylibrary.mil/OperationalEnvironment/Mid/OEFutureWarfareOntology#ControlledVocabulary"/>
    </owl:Class>
    


    <!-- http://www.ontologylibrary.mil/OperationalEnvironment/Mid/OEFutureWarfareOntology#EconomicRebalancingTrend -->

    <owl:Class rdf:about="http://www.ontologylibrary.mil/OperationalEnvironment/Mid/OEFutureWarfareOntology#EconomicRebalancingTrend">
        <rdfs:subClassOf rdf:resource="http://www.ontologylibrary.mil/OperationalEnvironment/Mid/OEFutureWarfareOntology#Trend"/>
        <obo:IAO_0000115>Although AI and its associated technologies will shatter many industries and livelihoods, a wide range of advances continue to create new sources of wealth and economic development – while also significantly impacting the strategic security environment. Robotics and autonomous systems will underpin the smooth functioning of advanced societies.  Additive manufacturing, computer-aided design and millions of industrial robots will dislocate significant portions of the global supply chain.  Virtually anyone in the world with access to a computer system and 3D printer will be able to “print” anything from drones to weapons.  Encrypted blockchains will be massively disruptive to commerce functions. Together with robotics, autonomy, and AI they comprise a perfect storm for “blue collar” and “white collars” alike, causing vast economic displacement as formerly high-quality information technology and management jobs follow the previous path of agricultural and manufacturing labor.  Militaries, paramilitaries, mercenary groups, criminal elements, and even extremists groups all will be able to take advantage of this potential pool of manpower.  Biotechnology will see major advances, with many chemical and materials industry being replaced or augmented by a “bio-based economy” in which precision genetic engineering allows for bulk chemical production.  Individualized genetics enable precise performance enhancements for cognition, health, longevity, and fitness.</obo:IAO_0000115>
        <obo:IAO_0000119>The Operational Environment and the Changing Character of Future Warfare</obo:IAO_0000119>
    </owl:Class>
    


    <!-- http://www.ontologylibrary.mil/OperationalEnvironment/Mid/OEFutureWarfareOntology#EconomicsAndTrade -->

    <owl:Class rdf:about="http://www.ontologylibrary.mil/OperationalEnvironment/Mid/OEFutureWarfareOntology#EconomicsAndTrade">
        <rdfs:subClassOf rdf:resource="http://www.ontologylibrary.mil/OperationalEnvironment/Mid/OEFutureWarfareOntology#HumanFactorsControlledVocabulary"/>
        <rdfs:label>Economics and Trade</rdfs:label>
    </owl:Class>
    


    <!-- http://www.ontologylibrary.mil/OperationalEnvironment/Mid/OEFutureWarfareOntology#Education -->

    <owl:Class rdf:about="http://www.ontologylibrary.mil/OperationalEnvironment/Mid/OEFutureWarfareOntology#Education">
        <rdfs:subClassOf rdf:resource="http://www.ontologylibrary.mil/OperationalEnvironment/Mid/OEFutureWarfareOntology#WelfareState"/>
        <obo:IAO_0000119>&quot;State School&quot;, Wikipedia

March 23, 2019

https://en.wikipedia.org/wiki/State_school</obo:IAO_0000119>
        <CommonCoreOntologies:definition>State schools (known as public schools in some parts of the world) are generally primary or secondary schools mandated for or offered to all children without charge, funded in whole or in part by taxation. These schools are generally inclusive (non-selective) in admitting all students within the geographical area that they serve.

While such schools are to be found in virtually every country, there are significant variations in their structure and educational programs. State education generally encompasses primary and secondary education (kindergarten to twelfth grade, or equivalent), as well as post-secondary educational institutions such as universities, colleges, and technical schools that are funded and overseen by government rather than by private entities.</CommonCoreOntologies:definition>
        <rdfs:label>Education</rdfs:label>
    </owl:Class>
    


    <!-- http://www.ontologylibrary.mil/OperationalEnvironment/Mid/OEFutureWarfareOntology#Effectiveness -->

    <owl:Class rdf:about="http://www.ontologylibrary.mil/OperationalEnvironment/Mid/OEFutureWarfareOntology#Effectiveness">
        <rdfs:subClassOf rdf:resource="http://www.ontologylibrary.mil/OperationalEnvironment/Mid/OEFutureWarfareOntology#CyberSecurityControlledVocabulary"/>
        <obo:IAO_0000115>extent to which planned activities are realized and planned results achieved</obo:IAO_0000115>
        <obo:IAO_0000119>International Organization for Standardization/International Electrotechnical Commission 27000:2018

Security techniques — Information security management systems — Overview and vocabulary

Publication date : 2018-02

5th Edition</obo:IAO_0000119>
    </owl:Class>
    


    <!-- http://www.ontologylibrary.mil/OperationalEnvironment/Mid/OEFutureWarfareOntology#EjectaCone -->

    <owl:Class rdf:about="http://www.ontologylibrary.mil/OperationalEnvironment/Mid/OEFutureWarfareOntology#EjectaCone">
        <rdfs:subClassOf rdf:resource="http://www.ontologylibrary.mil/OperationalEnvironment/Mid/OEFutureWarfareOntology#SpaceSystems"/>
        <obo:IAO_0000115>shaped spray of fine particles, comprising fragments and spalls that are released during a high-velocity impact.</obo:IAO_0000115>
        <obo:IAO_0000119>International Organization for Standardization/International Electrotechnical Commission 11227:2012

Space systems — Test procedure to evaluate spacecraft material ejecta upon hypervelocity impact

Publication Date: 2012-09

1st Edition</obo:IAO_0000119>
    </owl:Class>
    


    <!-- http://www.ontologylibrary.mil/OperationalEnvironment/Mid/OEFutureWarfareOntology#Election -->

    <owl:Class rdf:about="http://www.ontologylibrary.mil/OperationalEnvironment/Mid/OEFutureWarfareOntology#Election">
        <rdfs:subClassOf rdf:resource="http://www.ontologylibrary.mil/OperationalEnvironment/Mid/OEFutureWarfareOntology#Democracy"/>
        <obo:IAO_0000115>Electoral systems are the detailed constitutional arrangements and voting systems that convert the vote into a political decision. The first step is to tally the votes, for which various vote counting systems and ballot types are used. Voting systems then determine the result on the basis of the tally. Most systems can be categorized as either proportional or majoritarian. Among the former are party-list proportional representation and additional member system. Among the latter are First Past the Post electoral system (relative majority) and absolute majority. Many countries have growing electoral reform movements, which advocate systems such as approval voting, single transferable vote, instant runoff voting or a Condorcet method; these methods are also gaining popularity for lesser elections in some countries where more important elections still use more traditional counting methods.

While openness and accountability are usually considered cornerstones of a democratic system, the act of casting a vote and the content of a voter&apos;s ballot are usually an important exception. The secret ballot is a relatively modern development, but it is now considered crucial in most free and fair elections, as it limits the effectiveness of intimidation.</obo:IAO_0000115>
        <obo:IAO_0000119>&quot;Election&quot;, Wikipedia

March 12, 2019

https://en.wikipedia.org/wiki/Election#Electoral_systems</obo:IAO_0000119>
        <rdfs:label>Election</rdfs:label>
    </owl:Class>
    


    <!-- http://www.ontologylibrary.mil/OperationalEnvironment/Mid/OEFutureWarfareOntology#ElectroDynamicKineticEnergyWeaponsPrecisionWeaponPointDefense -->

    <owl:Class rdf:about="http://www.ontologylibrary.mil/OperationalEnvironment/Mid/OEFutureWarfareOntology#ElectroDynamicKineticEnergyWeaponsPrecisionWeaponPointDefense">
        <rdfs:subClassOf rdf:resource="http://www.ontologylibrary.mil/OperationalEnvironment/Mid/OEFutureWarfareOntology#CombatApplication"/>
        <rdfs:subClassOf>
            <owl:Restriction>
                <owl:onProperty rdf:resource="http://www.ontologylibrary.mil/OperationalEnvironment/Mid/OEFutureWarfareOntology#hasCategoryOfEffort"/>
                <owl:someValuesFrom rdf:resource="http://www.ontologylibrary.mil/OperationalEnvironment/Mid/OEFutureWarfareOntology#SystemsThatProtect"/>
            </owl:Restriction>
        </rdfs:subClassOf>
    </owl:Class>
    


    <!-- http://www.ontologylibrary.mil/OperationalEnvironment/Mid/OEFutureWarfareOntology#Enclosure -->

    <owl:Class rdf:about="http://www.ontologylibrary.mil/OperationalEnvironment/Mid/OEFutureWarfareOntology#Enclosure">
        <rdfs:subClassOf rdf:resource="http://www.ontologylibrary.mil/OperationalEnvironment/Mid/OEFutureWarfareOntology#GasEnergyGeneration"/>
        <obo:IAO_0000115>structure enveloping/enclosing sections of equipment for the applicable requirements of —weather protection (all applicable types), — noise attenuation, —ventilation for removal of hazardous gases and vapours, —ventilation for temperature control, —control of radiated heat, and —contamination due to local environment conditions.</obo:IAO_0000115>
        <obo:IAO_0000119>International Organization for Standardization/International ISO 19859:2016

Technical Committee : ISO/TC 192  Gas turbines

ICS :  29.160.99  Other standards related to rotating machinery 27.040  Gas and steam turbines. Steam engines

Gas turbine applications -- Requirements for power generation

Publication date : 2016-08

1st Edition</obo:IAO_0000119>
    </owl:Class>
    


    <!-- http://www.ontologylibrary.mil/OperationalEnvironment/Mid/OEFutureWarfareOntology#Energy -->

    <owl:Class rdf:about="http://www.ontologylibrary.mil/OperationalEnvironment/Mid/OEFutureWarfareOntology#Energy">
        <rdfs:subClassOf rdf:resource="http://www.ontologylibrary.mil/OperationalEnvironment/Mid/OEFutureWarfareOntology#PowerGenerationAndStorageControlledVocabulary"/>
        <obo:IAO_0000115>electricity, fuels, steam, heat, compressed air and other similar media

Note 1 to entry: For the purposes of this document, energy refers to the various types of energy, including renewable, which can be purchased, stored, treated, used in an equipment or in a process, or recovered.</obo:IAO_0000115>
        <obo:IAO_0000119>International Organization for Standardization/International ISO 50001:2018

Technical Committee : ISO/TC 301  Energy management and energy savings

ICS :  27.015  Energy efficiency. Energy conservation in general 03.100.70 Management systems

Energy management systems -- Requirements with guidance for use

Publication date : 2018-08

2nd Edition</obo:IAO_0000119>
    </owl:Class>
    


    <!-- http://www.ontologylibrary.mil/OperationalEnvironment/Mid/OEFutureWarfareOntology#EnergyBaseline -->

    <owl:Class rdf:about="http://www.ontologylibrary.mil/OperationalEnvironment/Mid/OEFutureWarfareOntology#EnergyBaseline">
        <rdfs:subClassOf rdf:resource="http://www.ontologylibrary.mil/OperationalEnvironment/Mid/OEFutureWarfareOntology#PowerGenerationAndStorageControlledVocabulary"/>
        <obo:IAO_0000115>quantitative reference(s) providing a basis for comparison of energy performance (3.4.3)

Note 1 to entry: An energy baseline is based on data from a specified period of time and/or conditions, as defined by the organization (3.1.1).

Note 2 to entry: One or more energy baselines are used for determination of energy performance improvement (3.4.6), as a reference before and after, or with and without implementation of energy performance improvement actions.

Note 3 to entry: See ISO 50015 for additional information on measurement and verification of energy performance.

Note 4 to entry: See ISO 50006 for additional information on EnPIs and EnBs.</obo:IAO_0000115>
        <obo:IAO_0000119>International Organization for Standardization/International ISO 50001:2018

Technical Committee : ISO/TC 301  Energy management and energy savings

ICS :  27.015  Energy efficiency. Energy conservation in general 03.100.70 Management systems

Energy management systems -- Requirements with guidance for use

Publication date : 2018-08

2nd Edition</obo:IAO_0000119>
    </owl:Class>
    


    <!-- http://www.ontologylibrary.mil/OperationalEnvironment/Mid/OEFutureWarfareOntology#EnergyConsumption -->

    <owl:Class rdf:about="http://www.ontologylibrary.mil/OperationalEnvironment/Mid/OEFutureWarfareOntology#EnergyConsumption">
        <rdfs:subClassOf rdf:resource="http://www.ontologylibrary.mil/OperationalEnvironment/Mid/OEFutureWarfareOntology#PowerGenerationAndStorageControlledVocabulary"/>
        <obo:IAO_0000115>quantity of energy (3.5.1) applied</obo:IAO_0000115>
        <obo:IAO_0000119>International Organization for Standardization/International ISO 50001:2018

Technical Committee : ISO/TC 301  Energy management and energy savings

ICS :  27.015  Energy efficiency. Energy conservation in general 03.100.70 Management systems

Energy management systems -- Requirements with guidance for use

Publication date : 2018-08

2nd Edition</obo:IAO_0000119>
    </owl:Class>
    


    <!-- http://www.ontologylibrary.mil/OperationalEnvironment/Mid/OEFutureWarfareOntology#EnergyEfficiency -->

    <owl:Class rdf:about="http://www.ontologylibrary.mil/OperationalEnvironment/Mid/OEFutureWarfareOntology#EnergyEfficiency">
        <rdfs:subClassOf rdf:resource="http://www.ontologylibrary.mil/OperationalEnvironment/Mid/OEFutureWarfareOntology#PowerGenerationAndStorageControlledVocabulary"/>
        <obo:IAO_0000115>ratio or other quantitative relationship between an output of performance (3.4.2), service, goods, commodities, or energy (3.5.1), and an input of energy

EXAMPLE:Conversion efficiency; energy required/energy consumed.

Note 1 to entry: Both input and output should be clearly specified in terms of quantity and quality and be measurable.</obo:IAO_0000115>
        <obo:IAO_0000119>International Organization for Standardization/International ISO 50001:2018

Technical Committee : ISO/TC 301  Energy management and energy savings

ICS :  27.015  Energy efficiency. Energy conservation in general 03.100.70 Management systems

Energy management systems -- Requirements with guidance for use

Publication date : 2018-08

2nd Edition</obo:IAO_0000119>
    </owl:Class>
    


    <!-- http://www.ontologylibrary.mil/OperationalEnvironment/Mid/OEFutureWarfareOntology#EnergyManagementSystem -->

    <owl:Class rdf:about="http://www.ontologylibrary.mil/OperationalEnvironment/Mid/OEFutureWarfareOntology#EnergyManagementSystem">
        <rdfs:subClassOf rdf:resource="http://www.ontologylibrary.mil/OperationalEnvironment/Mid/OEFutureWarfareOntology#PowerGenerationAndStorageControlledVocabulary"/>
        <obo:IAO_0000115>management system (3.2.1) to establish an energy policy (3.2.4), objectives (3.4.13), energy targets (3.4.15), action plans and process(es) (3.3.6) to achieve the objectives and energy targets</obo:IAO_0000115>
        <obo:IAO_0000119>International Organization for Standardization/International ISO 50001:2018

Technical Committee : ISO/TC 301  Energy management and energy savings

ICS :  27.015  Energy efficiency. Energy conservation in general 03.100.70 Management systems

Energy management systems -- Requirements with guidance for use

Publication date : 2018-08

2nd Edition</obo:IAO_0000119>
    </owl:Class>
    


    <!-- http://www.ontologylibrary.mil/OperationalEnvironment/Mid/OEFutureWarfareOntology#EnergyManagementTeam -->

    <owl:Class rdf:about="http://www.ontologylibrary.mil/OperationalEnvironment/Mid/OEFutureWarfareOntology#EnergyManagementTeam">
        <rdfs:subClassOf rdf:resource="http://www.ontologylibrary.mil/OperationalEnvironment/Mid/OEFutureWarfareOntology#PowerGenerationAndStorageControlledVocabulary"/>
        <obo:IAO_0000115>person(s) with responsibility and authority for effective implementation of an energy managementsystem (3.2.2) and for delivering energy performance improvement (3.4.6)

Note 1 to entry: The size and nature of an organization (3.1.1) and available resources are taken into account when determining the size of an energy management team. A single person can perform the role of the team.</obo:IAO_0000115>
        <obo:IAO_0000119>International Organization for Standardization/International ISO 50001:2018

Technical Committee : ISO/TC 301  Energy management and energy savings

ICS :  27.015  Energy efficiency. Energy conservation in general 03.100.70 Management systems

Energy management systems -- Requirements with guidance for use

Publication date : 2018-08

2nd Edition</obo:IAO_0000119>
    </owl:Class>
    


    <!-- http://www.ontologylibrary.mil/OperationalEnvironment/Mid/OEFutureWarfareOntology#EnergyPerformance -->

    <owl:Class rdf:about="http://www.ontologylibrary.mil/OperationalEnvironment/Mid/OEFutureWarfareOntology#EnergyPerformance">
        <rdfs:subClassOf rdf:resource="http://www.ontologylibrary.mil/OperationalEnvironment/Mid/OEFutureWarfareOntology#PowerGenerationAndStorageControlledVocabulary"/>
        <obo:IAO_0000115>measurable result(s) related to energy efficiency (3.5.3), energy use (3.5.4) and energy consumption (3.5.2)

Note 1 to entry: Energy performance can be measured against the organization’s (3.1.1)objectives (3.4.13), energy targets (3.4.15) and other energy performance requirements.

Note 2 to entry: Energy performance is one component of the performance (3.4.2) of the energy managementsystem (3.2.2).</obo:IAO_0000115>
        <obo:IAO_0000119>International Organization for Standardization/International ISO 50001:2018

Technical Committee : ISO/TC 301  Energy management and energy savings

ICS :  27.015  Energy efficiency. Energy conservation in general 03.100.70 Management systems

Energy management systems -- Requirements with guidance for use

Publication date : 2018-08

2nd Edition</obo:IAO_0000119>
    </owl:Class>
    


    <!-- http://www.ontologylibrary.mil/OperationalEnvironment/Mid/OEFutureWarfareOntology#EnergyPerformanceImprovement -->

    <owl:Class rdf:about="http://www.ontologylibrary.mil/OperationalEnvironment/Mid/OEFutureWarfareOntology#EnergyPerformanceImprovement">
        <rdfs:subClassOf rdf:resource="http://www.ontologylibrary.mil/OperationalEnvironment/Mid/OEFutureWarfareOntology#PowerGenerationAndStorageControlledVocabulary"/>
        <obo:IAO_0000115>improvement in measurable results of energy efficiency (3.5.3), or energy consumption (3.5.2) related to energy use (3.5.4), compared to the energy baseline (3.4.7)</obo:IAO_0000115>
        <obo:IAO_0000119>International Organization for Standardization/International ISO 50001:2018

Technical Committee : ISO/TC 301  Energy management and energy savings

ICS :  27.015  Energy efficiency. Energy conservation in general 03.100.70 Management systems

Energy management systems -- Requirements with guidance for use

Publication date : 2018-08

2nd Edition</obo:IAO_0000119>
    </owl:Class>
    


    <!-- http://www.ontologylibrary.mil/OperationalEnvironment/Mid/OEFutureWarfareOntology#EnergyPerformanceIndicator -->

    <owl:Class rdf:about="http://www.ontologylibrary.mil/OperationalEnvironment/Mid/OEFutureWarfareOntology#EnergyPerformanceIndicator">
        <rdfs:subClassOf rdf:resource="http://www.ontologylibrary.mil/OperationalEnvironment/Mid/OEFutureWarfareOntology#PowerGenerationAndStorageControlledVocabulary"/>
        <obo:IAO_0000115>measure or unit of energy performance (3.4.3), as defined by the organization (3.1.1)

Note 1 to entry: EnPI(s) can be expressed by using a simple metric, ratio, or a model, depending on the nature of the activities being measured.

Note 2 to entry: See ISO 50006 for additional information on EnPI(s).</obo:IAO_0000115>
        <obo:IAO_0000119>International Organization for Standardization/International ISO 50001:2018

Technical Committee : ISO/TC 301  Energy management and energy savings

ICS :  27.015  Energy efficiency. Energy conservation in general 03.100.70 Management systems

Energy management systems -- Requirements with guidance for use

Publication date : 2018-08

2nd Edition</obo:IAO_0000119>
    </owl:Class>
    


    <!-- http://www.ontologylibrary.mil/OperationalEnvironment/Mid/OEFutureWarfareOntology#EnergyPerformanceIndicatorValue -->

    <owl:Class rdf:about="http://www.ontologylibrary.mil/OperationalEnvironment/Mid/OEFutureWarfareOntology#EnergyPerformanceIndicatorValue">
        <rdfs:subClassOf rdf:resource="http://www.ontologylibrary.mil/OperationalEnvironment/Mid/OEFutureWarfareOntology#PowerGenerationAndStorageControlledVocabulary"/>
        <obo:IAO_0000115>quantification of the EnPI (3.4.4) at a point in or over a specified period of time</obo:IAO_0000115>
        <obo:IAO_0000119>International Organization for Standardization/International ISO 50001:2018

Technical Committee : ISO/TC 301  Energy management and energy savings

ICS :  27.015  Energy efficiency. Energy conservation in general 03.100.70 Management systems

Energy management systems -- Requirements with guidance for use

Publication date : 2018-08

2nd Edition</obo:IAO_0000119>
    </owl:Class>
    


    <!-- http://www.ontologylibrary.mil/OperationalEnvironment/Mid/OEFutureWarfareOntology#EnergyPolicy -->

    <owl:Class rdf:about="http://www.ontologylibrary.mil/OperationalEnvironment/Mid/OEFutureWarfareOntology#EnergyPolicy">
        <rdfs:subClassOf rdf:resource="http://www.ontologylibrary.mil/OperationalEnvironment/Mid/OEFutureWarfareOntology#PowerGenerationAndStorageControlledVocabulary"/>
        <obo:IAO_0000115>statement by the organization (3.1.1) of its overall intention(s), direction(s), and commitment(s) related to its energy performance (3.4.3), as formally expressed by top management (3.1.2)</obo:IAO_0000115>
        <obo:IAO_0000119>International Organization for Standardization/International ISO 50001:2018

Technical Committee : ISO/TC 301  Energy management and energy savings

ICS :  27.015  Energy efficiency. Energy conservation in general 03.100.70 Management systems

Energy management systems -- Requirements with guidance for use

Publication date : 2018-08

2nd Edition</obo:IAO_0000119>
    </owl:Class>
    


    <!-- http://www.ontologylibrary.mil/OperationalEnvironment/Mid/OEFutureWarfareOntology#EnergyReview -->

    <owl:Class rdf:about="http://www.ontologylibrary.mil/OperationalEnvironment/Mid/OEFutureWarfareOntology#EnergyReview">
        <rdfs:subClassOf rdf:resource="http://www.ontologylibrary.mil/OperationalEnvironment/Mid/OEFutureWarfareOntology#PowerGenerationAndStorageControlledVocabulary"/>
        <obo:IAO_0000115>analysis of energy efficiency (3.5.3), energy use (3.5.4) and energy consumption (3.5.2) based on data and other information, leading to identification of SEUs (3.5.6) and opportunities for energy performance improvement (3.4.6)</obo:IAO_0000115>
        <obo:IAO_0000119>International Organization for Standardization/International ISO 50001:2018

Technical Committee : ISO/TC 301  Energy management and energy savings

ICS :  27.015  Energy efficiency. Energy conservation in general 03.100.70 Management systems

Energy management systems -- Requirements with guidance for use

Publication date : 2018-08

2nd Edition</obo:IAO_0000119>
    </owl:Class>
    


    <!-- http://www.ontologylibrary.mil/OperationalEnvironment/Mid/OEFutureWarfareOntology#EnergyScavengingFromTheEnvironment -->

    <owl:Class rdf:about="http://www.ontologylibrary.mil/OperationalEnvironment/Mid/OEFutureWarfareOntology#EnergyScavengingFromTheEnvironment">
        <rdfs:subClassOf rdf:resource="http://www.ontologylibrary.mil/OperationalEnvironment/Mid/OEFutureWarfareOntology#SystemsThatMove"/>
    </owl:Class>
    


    <!-- http://www.ontologylibrary.mil/OperationalEnvironment/Mid/OEFutureWarfareOntology#EnergyService -->

    <owl:Class rdf:about="http://www.ontologylibrary.mil/OperationalEnvironment/Mid/OEFutureWarfareOntology#EnergyService">
        <rdfs:subClassOf rdf:resource="http://www.ontologylibrary.mil/OperationalEnvironment/Mid/OEFutureWarfareOntology#PowerGenerationAndStorageControlledVocabulary"/>
        <obo:IAO_0000115>set of organization, processes (3.31), activities, means and resources necessary for production, transmission, distribution and supply of energy and for providing a physical benefit, utility or goods, which are derived from a combination of energy with energy-efficient technology or with action, which can include the operations, maintenance (3.21) and control necessary to deliver the service (3.44)

Note 1 to entry: Key features for an energy service include: —   its mission to provide an energy service; —   its physical area of responsibility and the population within this area; —   its responsible body (3.42); —   the general organization, with the function of operator (3.25) being carried out by the responsible body; —   the scope of the energy service offered by the energy service provider (3.14), or by other organizations operating in the same geographic area; —   the type of physical or information technology systems used to provide the services, with various degrees of centralization.

Note 2 to entry: When it is not necessary or it is difficult to make a distinction between responsible body and operator, the term “energy service provider” covers both.

Note 3 to entry: In this document, the term “energy services (3.15)” (plural) refers to generic activities or energy uses such as heating or lighting or supply of natural gas, whereas the term “energy service” (singular) is used to refer to the activity by an organization (an energy service provider) to a user (3.50) or consumer to provide energy services in the best way, such as offering incentives for energy efficient air conditioning systems or financing for consumer-provided solar energy generating systems.</obo:IAO_0000115>
        <obo:IAO_0000119>International Organization for Standardization/International ISO 50007:2017

Technical Committee : ISO/TC 301  Energy management and energy savings

ICS :  27.015  Energy efficiency. Energy conservation in general

Energy services -- Guidelines for the assessment and improvement of the energy service to users

Publication date : 2017-06

1st Edition</obo:IAO_0000119>
    </owl:Class>
    


    <!-- http://www.ontologylibrary.mil/OperationalEnvironment/Mid/OEFutureWarfareOntology#EnergyServiceProvider -->

    <owl:Class rdf:about="http://www.ontologylibrary.mil/OperationalEnvironment/Mid/OEFutureWarfareOntology#EnergyServiceProvider">
        <rdfs:subClassOf rdf:resource="http://www.ontologylibrary.mil/OperationalEnvironment/Mid/OEFutureWarfareOntology#PowerGenerationAndStorageControlledVocabulary"/>
        <obo:IAO_0000115>energy entity or person that provides service (3.44) to a retail or end-use customer</obo:IAO_0000115>
        <obo:IAO_0000119>International Organization for Standardization/International ISO 50007:2017

Technical Committee : ISO/TC 301  Energy management and energy savings

ICS :  27.015  Energy efficiency. Energy conservation in general

Energy services -- Guidelines for the assessment and improvement of the energy service to users

Publication date : 2017-06

1st Edition</obo:IAO_0000119>
    </owl:Class>
    


    <!-- http://www.ontologylibrary.mil/OperationalEnvironment/Mid/OEFutureWarfareOntology#EnergyTarget -->

    <owl:Class rdf:about="http://www.ontologylibrary.mil/OperationalEnvironment/Mid/OEFutureWarfareOntology#EnergyTarget">
        <rdfs:subClassOf rdf:resource="http://www.ontologylibrary.mil/OperationalEnvironment/Mid/OEFutureWarfareOntology#PowerGenerationAndStorageControlledVocabulary"/>
        <obo:IAO_0000115>quantifiable objective (3.4.13) of energyperformance improvement (3.4.6)

Note 1 to entry: An energy target can be included within an objective.</obo:IAO_0000115>
        <obo:IAO_0000119>International Organization for Standardization/International ISO 50001:2018

Technical Committee : ISO/TC 301  Energy management and energy savings

ICS :  27.015  Energy efficiency. Energy conservation in general 03.100.70 Management systems

Energy management systems -- Requirements with guidance for use

Publication date : 2018-08

2nd Edition</obo:IAO_0000119>
    </owl:Class>
    


    <!-- http://www.ontologylibrary.mil/OperationalEnvironment/Mid/OEFutureWarfareOntology#EnergyUse -->

    <owl:Class rdf:about="http://www.ontologylibrary.mil/OperationalEnvironment/Mid/OEFutureWarfareOntology#EnergyUse">
        <rdfs:subClassOf rdf:resource="http://www.ontologylibrary.mil/OperationalEnvironment/Mid/OEFutureWarfareOntology#PowerGenerationAndStorageControlledVocabulary"/>
        <obo:IAO_0000115>application of energy (3.5.1)

EXAMPLE:Ventilation; lighting; heating; cooling; transportation; data storage; production process.

Note 1 to entry: Energy use is sometimes referred to as “energy end-use”.</obo:IAO_0000115>
        <obo:IAO_0000119>International Organization for Standardization/International ISO 50001:2018

Technical Committee : ISO/TC 301  Energy management and energy savings

ICS :  27.015  Energy efficiency. Energy conservation in general 03.100.70 Management systems

Energy management systems -- Requirements with guidance for use

Publication date : 2018-08

2nd Edition</obo:IAO_0000119>
    </owl:Class>
    


    <!-- http://www.ontologylibrary.mil/OperationalEnvironment/Mid/OEFutureWarfareOntology#EthnicRegionalReligiousAndRacialIdentities -->

    <owl:Class rdf:about="http://www.ontologylibrary.mil/OperationalEnvironment/Mid/OEFutureWarfareOntology#EthnicRegionalReligiousAndRacialIdentities">
        <rdfs:subClassOf rdf:resource="http://www.ontologylibrary.mil/OperationalEnvironment/Mid/OEFutureWarfareOntology#Identity"/>
    </owl:Class>
    


    <!-- http://www.ontologylibrary.mil/OperationalEnvironment/Mid/OEFutureWarfareOntology#EvaluateWithSubjectMatterExperts -->

    <owl:Class rdf:about="http://www.ontologylibrary.mil/OperationalEnvironment/Mid/OEFutureWarfareOntology#EvaluateWithSubjectMatterExperts">
        <rdfs:subClassOf rdf:resource="http://www.ontologylibrary.mil/OperationalEnvironment/Mid/OEFutureWarfareOntology#FaultLineMethodology"/>
        <obo:IAO_0000115>Test the OE assumptions/research hypotheses with a pool of relevant SMEs.  The researcher sends the fault line hypotheses to a pool of SMEs in the OE and requests their ratings on 5 variables (probability of exploitation, consequence(s) of exploitation, pervasiveness of the condition, importance of the condition, and speed of recovery if exploited).   The aggregate ratings of the variables become a risk assessment from a SME perspective. SME qualitative feedback may assist in refining fault line hypotheses better understand the sources of instability and any implications.  GCKN can provide an online survey template to distribute and a process for collating and analyzing the data from survey collection.</obo:IAO_0000115>
        <obo:IAO_0000119>Fault Lines Methodology Infographic</obo:IAO_0000119>
    </owl:Class>
    


    <!-- http://www.ontologylibrary.mil/OperationalEnvironment/Mid/OEFutureWarfareOntology#Event -->

    <owl:Class rdf:about="http://www.ontologylibrary.mil/OperationalEnvironment/Mid/OEFutureWarfareOntology#Event">
        <rdfs:subClassOf rdf:resource="http://www.ontologylibrary.mil/OperationalEnvironment/Mid/OEFutureWarfareOntology#CyberSecurityControlledVocabulary"/>
        <obo:IAO_0000115>occurrence or change of a particular set of circumstances

Note 1 to entry: An event can be one or more occurrences, and can have several causes.

Note 2 to entry: An event can consist of something not happening.

Note 3 to entry: An event can sometimes be referred to as an “incident” or “accident”.</obo:IAO_0000115>
        <obo:IAO_0000119>International Organization for Standardization/International Electrotechnical Commission 27000:2018

Security techniques — Information security management systems — Overview and vocabulary

Publication date : 2018-02

5th Edition</obo:IAO_0000119>
    </owl:Class>
    


    <!-- http://www.ontologylibrary.mil/OperationalEnvironment/Mid/OEFutureWarfareOntology#Executive -->

    <owl:Class rdf:about="http://www.ontologylibrary.mil/OperationalEnvironment/Mid/OEFutureWarfareOntology#Executive">
        <rdfs:subClassOf rdf:resource="http://www.ontologylibrary.mil/OperationalEnvironment/Mid/OEFutureWarfareOntology#Government"/>
        <obo:IAO_0000115>[The executive is] a person or persons constituting the branch of government charged with executing or carrying out the laws and appointing officials, formulating and instituting foreign policy, and providing diplomatic representation.</obo:IAO_0000115>
        <obo:IAO_0000119>Editors of Encyclopaedia Brittanica, &quot;Executive, Government&quot;, Encyclopaedia Britannica

March 12, 2019

https://www.britannica.com/topic/executive-government</obo:IAO_0000119>
        <rdfs:label>Executive</rdfs:label>
    </owl:Class>
    


    <!-- http://www.ontologylibrary.mil/OperationalEnvironment/Mid/OEFutureWarfareOntology#ExploitingPrinciplesOfQuantumMechanics -->

    <owl:Class rdf:about="http://www.ontologylibrary.mil/OperationalEnvironment/Mid/OEFutureWarfareOntology#ExploitingPrinciplesOfQuantumMechanics">
        <rdfs:subClassOf rdf:resource="http://www.ontologylibrary.mil/OperationalEnvironment/Mid/OEFutureWarfareOntology#SystemsThatProtect"/>
        <rdfs:subClassOf>
            <owl:Restriction>
                <owl:onProperty rdf:resource="http://www.ontologylibrary.mil/OperationalEnvironment/Mid/OEFutureWarfareOntology#hasCombatApplication"/>
                <owl:someValuesFrom rdf:resource="http://www.ontologylibrary.mil/OperationalEnvironment/Mid/OEFutureWarfareOntology#QuantumCommunications"/>
            </owl:Restriction>
        </rdfs:subClassOf>
        <rdfs:subClassOf>
            <owl:Restriction>
                <owl:onProperty rdf:resource="http://www.ontologylibrary.mil/OperationalEnvironment/Mid/OEFutureWarfareOntology#hasCombatApplication"/>
                <owl:someValuesFrom rdf:resource="http://www.ontologylibrary.mil/OperationalEnvironment/Mid/OEFutureWarfareOntology#QuantumComputing"/>
            </owl:Restriction>
        </rdfs:subClassOf>
        <rdfs:subClassOf>
            <owl:Restriction>
                <owl:onProperty rdf:resource="http://www.ontologylibrary.mil/OperationalEnvironment/Mid/OEFutureWarfareOntology#hasCombatApplication"/>
                <owl:someValuesFrom rdf:resource="http://www.ontologylibrary.mil/OperationalEnvironment/Mid/OEFutureWarfareOntology#QuantumCryptography"/>
            </owl:Restriction>
        </rdfs:subClassOf>
        <rdfs:subClassOf>
            <owl:Restriction>
                <owl:onProperty rdf:resource="http://www.ontologylibrary.mil/OperationalEnvironment/Mid/OEFutureWarfareOntology#hasCombatApplication"/>
                <owl:someValuesFrom rdf:resource="http://www.ontologylibrary.mil/OperationalEnvironment/Mid/OEFutureWarfareOntology#QuantumNavigation"/>
            </owl:Restriction>
        </rdfs:subClassOf>
        <rdfs:subClassOf>
            <owl:Restriction>
                <owl:onProperty rdf:resource="http://www.ontologylibrary.mil/OperationalEnvironment/Mid/OEFutureWarfareOntology#hasCombatApplication"/>
                <owl:someValuesFrom rdf:resource="http://www.ontologylibrary.mil/OperationalEnvironment/Mid/OEFutureWarfareOntology#QuantumSensing"/>
            </owl:Restriction>
        </rdfs:subClassOf>
    </owl:Class>
    


    <!-- http://www.ontologylibrary.mil/OperationalEnvironment/Mid/OEFutureWarfareOntology#ExternalContext -->

    <owl:Class rdf:about="http://www.ontologylibrary.mil/OperationalEnvironment/Mid/OEFutureWarfareOntology#ExternalContext">
        <rdfs:subClassOf rdf:resource="http://www.ontologylibrary.mil/OperationalEnvironment/Mid/OEFutureWarfareOntology#CyberSecurityControlledVocabulary"/>
        <obo:IAO_0000115>external environment in which the organization seeks to achieve its objectives (3.49)

Note 1 to entry: External context can include the following:

— the cultural, social, political, legal, regulatory, financial, technological, economic, natural and competitive environment, whether international, national, regional or local;
— key drivers and trends having impact on the objectives of the organization (3.50);
— relationships with, and perceptions and values of, external stakeholders (3.37).</obo:IAO_0000115>
        <obo:IAO_0000119>International Organization for Standardization/International Electrotechnical Commission 27000:2018

Security techniques — Information security management systems — Overview and vocabulary

Publication date : 2018-02

5th Edition</obo:IAO_0000119>
    </owl:Class>
    


    <!-- http://www.ontologylibrary.mil/OperationalEnvironment/Mid/OEFutureWarfareOntology#ExtrajudicialViolence -->

    <owl:Class rdf:about="http://www.ontologylibrary.mil/OperationalEnvironment/Mid/OEFutureWarfareOntology#ExtrajudicialViolence">
        <rdfs:subClassOf rdf:resource="http://www.ontologylibrary.mil/OperationalEnvironment/Mid/OEFutureWarfareOntology#InformalInstitutions"/>
        <obo:IAO_0000115>(1)

Extrajudicial punishment is punishment for an alleged crime or offense carried out without legal process or supervision from a court or tribunal through a legal proceeding. Such actions are carried out by state actors.</obo:IAO_0000115>
        <obo:IAO_0000115>(2)

Extrajudicial punishment consists of various actions to imprison, relocate, harm, torture, or kill someone outside of the legal system, without legal process, and without supervision from a court and its systems of recourse.</obo:IAO_0000115>
        <obo:IAO_0000119>(1)

&quot;Extrajudcial punishment&quot;, Wikipedia

March 12, 2019

https://en.wikipedia.org/wiki/Extrajudicial_punishment</obo:IAO_0000119>
        <obo:IAO_0000119>(2)

&quot;Extrajudicial punishment&quot;, RationalWiki

March 12th, 2019

https://rationalwiki.org/wiki/Extrajudicial_punishment</obo:IAO_0000119>
        <obo:IAO_0000232>The articles in source #2 are, on the the whole, tendentious and of uneven quality.  However, this particular definition is correct, and, usually for topic modeling, written in everyday language.</obo:IAO_0000232>
        <rdfs:label>Extrajudicial Violence</rdfs:label>
    </owl:Class>
    


    <!-- http://www.ontologylibrary.mil/OperationalEnvironment/Mid/OEFutureWarfareOntology#Facility -->

    <owl:Class rdf:about="http://www.ontologylibrary.mil/OperationalEnvironment/Mid/OEFutureWarfareOntology#Facility">
        <rdfs:subClassOf rdf:resource="http://www.ontologylibrary.mil/OperationalEnvironment/Mid/OEFutureWarfareOntology#ClimateChangeAndResourceCompetitionControlledVocabulary"/>
        <obo:IAO_0000115>single installation, set of installations or production processes (stationary or mobile), which can be defined within a single geographical boundary, organizational unit or production process</obo:IAO_0000115>
        <obo:IAO_0000119>International Organization for Standardization/International Electrotechnical Commission 27000:2018

Technical Committee : ISO/TC 207/SC 7  Greenhouse gas management and related activities

ICS :  13.020.40  Pollution, pollution control and conservation

Greenhouse gases -- Part 1: Specification with guidance at the organization level for quantification and reporting of greenhouse gas emissions and removals 

Publication date : 2018-12

2nd Edition</obo:IAO_0000119>
    </owl:Class>
    


    <!-- http://www.ontologylibrary.mil/OperationalEnvironment/Mid/OEFutureWarfareOntology#FaultLine -->

    <owl:Class rdf:about="http://www.ontologylibrary.mil/OperationalEnvironment/Mid/OEFutureWarfareOntology#FaultLine">
        <rdfs:subClassOf rdf:resource="http://purl.obolibrary.org/obo/BFO_0000016"/>
        <obo:IAO_0000115>A fault line is an exploitable source of instability in the human domain—it can be real or perceived</obo:IAO_0000115>
        <obo:IAO_0000119>Fault Lines Methodology Infographic</obo:IAO_0000119>
    </owl:Class>
    


    <!-- http://www.ontologylibrary.mil/OperationalEnvironment/Mid/OEFutureWarfareOntology#FaultLineMethodology -->

    <owl:Class rdf:about="http://www.ontologylibrary.mil/OperationalEnvironment/Mid/OEFutureWarfareOntology#FaultLineMethodology">
        <rdfs:subClassOf rdf:resource="http://purl.obolibrary.org/obo/BFO_0000015"/>
        <obo:IAO_0000115>A Fault Line Methodology is a methodology that is used to reduce risk &amp; increase confidence of analysis with utilization of both social science methods and expert knowledge</obo:IAO_0000115>
        <obo:IAO_0000119>Fault Lines Methodology Infographic</obo:IAO_0000119>
    </owl:Class>
    


    <!-- http://www.ontologylibrary.mil/OperationalEnvironment/Mid/OEFutureWarfareOntology#FemaleNeglect -->

    <owl:Class rdf:about="http://www.ontologylibrary.mil/OperationalEnvironment/Mid/OEFutureWarfareOntology#FemaleNeglect">
        <rdfs:subClassOf rdf:resource="http://www.ontologylibrary.mil/OperationalEnvironment/Mid/OEFutureWarfareOntology#SkewedSexRatio"/>
        <CommonCoreOntologies:definition>&quot;Sex-selective Abortion&quot;, Wikipedia

March 25, 2019

https://en.wikipedia.org/wiki/Sex-selective_abortion#Disparate_gendered_access_to_resources</CommonCoreOntologies:definition>
        <CommonCoreOntologies:definition>[Some] of the variation in global sex ratios is due to disparate access to resources. ...[There] can be significant differences in gender violence and access to food, healthcare, immunizations between male and female children. This leads to high infant and childhood mortality among girls, which causes changes in sex ratio.</CommonCoreOntologies:definition>
        <rdfs:label>Female Neglect</rdfs:label>
    </owl:Class>
    


    <!-- http://www.ontologylibrary.mil/OperationalEnvironment/Mid/OEFutureWarfareOntology#File -->

    <owl:Class rdf:about="http://www.ontologylibrary.mil/OperationalEnvironment/Mid/OEFutureWarfareOntology#File">
        <rdfs:subClassOf rdf:resource="http://www.ontologylibrary.mil/OperationalEnvironment/Mid/OEFutureWarfareOntology#BigDataControlledVocabulary"/>
        <obo:IAO_0000115>named set of records treated as a unit</obo:IAO_0000115>
        <obo:IAO_0000119>Information technology — Big data — Overview and vocabulary

https://www.iso.org/jtc1</obo:IAO_0000119>
        <obo:IAO_0000119>[SOURCE: ISO/IEC 2382:2015, 04.07.10]</obo:IAO_0000119>
    </owl:Class>
    


    <!-- http://www.ontologylibrary.mil/OperationalEnvironment/Mid/OEFutureWarfareOntology#Finance -->

    <owl:Class rdf:about="http://www.ontologylibrary.mil/OperationalEnvironment/Mid/OEFutureWarfareOntology#Finance">
        <rdfs:subClassOf rdf:resource="http://www.ontologylibrary.mil/OperationalEnvironment/Mid/OEFutureWarfareOntology#EconomicActivity"/>
        <obo:IAO_0000119>Will Kenton (ed.), &quot;Financial Sector&quot;, Investopedia

March 13, 2019

https://www.investopedia.com/terms/f/financial_sector.asp</obo:IAO_0000119>
        <CommonCoreOntologies:definition>The financial sector is a section of the economy made up of firms and institutions that provide financial services to commercial and retail customers. This sector comprises a broad range of industries including banks, investment companies, insurance companies, and real estate firms.

...

In order for an economy to remain stable, it needs to have a healthy financial sector. This sector advances loans for businesses so they can expand, grants mortgages to homeowners, and issues insurance policies to protect people, companies, and their assets. It also helps build up savings for retirement....

The financial sector generates a good portion of its revenue from loans and mortgages. These gain value in an environment where interest rates drop. When rates are low, the economic conditions open up the doors for more capital projects and investment. When this happens, the financial sector benefits, meaning more economic growth.</CommonCoreOntologies:definition>
        <rdfs:label>Finance</rdfs:label>
    </owl:Class>
    


    <!-- http://www.ontologylibrary.mil/OperationalEnvironment/Mid/OEFutureWarfareOntology#FiscalPolicy -->

    <owl:Class rdf:about="http://www.ontologylibrary.mil/OperationalEnvironment/Mid/OEFutureWarfareOntology#FiscalPolicy">
        <rdfs:subClassOf rdf:resource="http://www.ontologylibrary.mil/OperationalEnvironment/Mid/OEFutureWarfareOntology#MacroeconomicPolicy"/>
        <obo:IAO_0000119>Will Kenton (ed.), &quot;Fiscal Policy&quot;, Investopedia

Nov 2, 2017

https://www.investopedia.com/terms/f/fiscalpolicy.asp</obo:IAO_0000119>
        <CommonCoreOntologies:definition>To illustrate how the government could try to use fiscal policy to affect the economy, consider an economy that&apos;s experiencing recession. The government might lower tax rates to increase aggregate demand and fuel economic growth; this is known as expansionary fiscal policy.

...

Rather than lowering taxes, the government might decide to increase spending. 

...

Expansionary fiscal policy is usually characterized by deficit spending, when government expenditures exceed receipts from taxes and other sources. In practice, deficit spending tends to result from a combination of tax cuts and higher spending.</CommonCoreOntologies:definition>
        <rdfs:label>Fiscal Policy</rdfs:label>
    </owl:Class>
    


    <!-- http://www.ontologylibrary.mil/OperationalEnvironment/Mid/OEFutureWarfareOntology#FormalNeuralNetworks -->

    <owl:Class rdf:about="http://www.ontologylibrary.mil/OperationalEnvironment/Mid/OEFutureWarfareOntology#FormalNeuralNetworks">
        <rdfs:subClassOf rdf:resource="http://www.ontologylibrary.mil/OperationalEnvironment/Mid/OEFutureWarfareOntology#ArtificialIntelligenceControlledVocabulary"/>
        <obo:IAO_0000115>These are algorithms designed to be implemented by a computer, which aims to replicate the neural connections of the brain. Existing systems are much more limited than human intelligence. But they are still capable of estimating the speed of a vehicle according to movements of the accelerator pedal and the slope of the road; the hardness of a material as a function of its chemical composition and its processing temperature; or the solvency of a business according to its turnover, etc.</obo:IAO_0000115>
        <obo:IAO_0000119>United Nations Educational, Scientific, and Cultural Organization Courier 

March 2018

https://en.unesco.org/courier/2018-3/lexicon-artificial-intelligence</obo:IAO_0000119>
    </owl:Class>
    


    <!-- http://www.ontologylibrary.mil/OperationalEnvironment/Mid/OEFutureWarfareOntology#Fragmentation -->

    <owl:Class rdf:about="http://www.ontologylibrary.mil/OperationalEnvironment/Mid/OEFutureWarfareOntology#Fragmentation">
        <rdfs:subClassOf rdf:resource="http://www.ontologylibrary.mil/OperationalEnvironment/Mid/OEFutureWarfareOntology#SpaceSystems"/>
        <obo:IAO_0000115>process by which an orbiting space object dissociates and produces debris, such as break-up, exposure to space environment, and ageing</obo:IAO_0000115>
        <obo:IAO_0000119>International Organization for Standardization/International Electrotechnical Commission 11227:2012

Space systems — Test procedure to evaluate spacecraft material ejecta upon hypervelocity impact

Publication Date: 2012-09

1st Edition</obo:IAO_0000119>
    </owl:Class>
    


    <!-- http://www.ontologylibrary.mil/OperationalEnvironment/Mid/OEFutureWarfareOntology#FreeSpeech -->

    <owl:Class rdf:about="http://www.ontologylibrary.mil/OperationalEnvironment/Mid/OEFutureWarfareOntology#FreeSpeech">
        <rdfs:subClassOf rdf:resource="http://www.ontologylibrary.mil/OperationalEnvironment/Mid/OEFutureWarfareOntology#Democracy"/>
        <obo:IAO_0000115>Freedom of speech is a principle that supports the freedom of an individual or a community to articulate their opinions and ideas without fear of retaliation, censorship, or legal sanction. The term &quot;freedom of expression&quot; is sometimes used synonymously but includes any act of seeking, receiving, and imparting information or ideas, regardless of the medium used.

Freedom of expression is recognized as a human right under article 19 of the Universal Declaration of Human Rights (UDHR) and recognized in international human rights law in the International Covenant on Civil and Political Rights (ICCPR). Article 19 of the UDHR states that &quot;everyone shall have the right to hold opinions without interference&quot; and &quot;everyone shall have the right to freedom of expression; this right shall include freedom to seek, receive and impart information and ideas of all kinds, regardless of frontiers, either orally, in writing or in print, in the form of art, or through any other media of his choice&quot;.</obo:IAO_0000115>
        <obo:IAO_0000119>&quot;Freedom of Speech&quot;, Wikipedia

March 12, 2019

https://en.wikipedia.org/wiki/Freedom_of_speech</obo:IAO_0000119>
        <rdfs:label>Free Speech</rdfs:label>
    </owl:Class>
    


    <!-- http://www.ontologylibrary.mil/OperationalEnvironment/Mid/OEFutureWarfareOntology#FunctionalSystem -->

    <owl:Class rdf:about="http://www.ontologylibrary.mil/OperationalEnvironment/Mid/OEFutureWarfareOntology#FunctionalSystem">
        <rdfs:subClassOf rdf:resource="http://www.ontologylibrary.mil/OperationalEnvironment/Mid/OEFutureWarfareOntology#System"/>
        <rdfs:subClassOf>
            <owl:Restriction>
                <owl:onProperty rdf:resource="http://www.ontologylibrary.mil/OperationalEnvironment/Mid/OEFutureWarfareOntology#hasCombatApplication"/>
                <owl:someValuesFrom rdf:resource="http://www.ontologylibrary.mil/OperationalEnvironment/Mid/OEFutureWarfareOntology#HighEnergyLaserPrecisionWeaponPointDefense"/>
            </owl:Restriction>
        </rdfs:subClassOf>
        <rdfs:subClassOf>
            <owl:Restriction>
                <owl:onProperty rdf:resource="http://www.ontologylibrary.mil/OperationalEnvironment/Mid/OEFutureWarfareOntology#hasCombatApplication"/>
                <owl:someValuesFrom rdf:resource="http://www.ontologylibrary.mil/OperationalEnvironment/Mid/OEFutureWarfareOntology#HighPowerMicrowavePrecisionWeaponPointDefense"/>
            </owl:Restriction>
        </rdfs:subClassOf>
    </owl:Class>
    


    <!-- http://www.ontologylibrary.mil/OperationalEnvironment/Mid/OEFutureWarfareOntology#GasEnergyGeneration -->

    <owl:Class rdf:about="http://www.ontologylibrary.mil/OperationalEnvironment/Mid/OEFutureWarfareOntology#GasEnergyGeneration">
        <rdfs:subClassOf rdf:resource="http://www.ontologylibrary.mil/OperationalEnvironment/Mid/OEFutureWarfareOntology#PowerGenerationAndStorageControlledVocabulary"/>
    </owl:Class>
    


    <!-- http://www.ontologylibrary.mil/OperationalEnvironment/Mid/OEFutureWarfareOntology#GasTurbineCore -->

    <owl:Class rdf:about="http://www.ontologylibrary.mil/OperationalEnvironment/Mid/OEFutureWarfareOntology#GasTurbineCore">
        <rdfs:subClassOf rdf:resource="http://www.ontologylibrary.mil/OperationalEnvironment/Mid/OEFutureWarfareOntology#GasEnergyGeneration"/>
        <obo:IAO_0000115>assembly that includes the gas turbine compressor, combustion system, power turbine and integral equipment</obo:IAO_0000115>
        <obo:IAO_0000119>International Organization for Standardization/International ISO 19859:2016

Technical Committee : ISO/TC 192  Gas turbines

ICS :  29.160.99  Other standards related to rotating machinery 27.040  Gas and steam turbines. Steam engines

Gas turbine applications -- Requirements for power generation

Publication date : 2016-08

1st Edition</obo:IAO_0000119>
    </owl:Class>
    


    <!-- http://www.ontologylibrary.mil/OperationalEnvironment/Mid/OEFutureWarfareOntology#GasTurbineEnclosure -->

    <owl:Class rdf:about="http://www.ontologylibrary.mil/OperationalEnvironment/Mid/OEFutureWarfareOntology#GasTurbineEnclosure">
        <rdfs:subClassOf rdf:resource="http://www.ontologylibrary.mil/OperationalEnvironment/Mid/OEFutureWarfareOntology#GasEnergyGeneration"/>
        <obo:IAO_0000115>local enclosure (3.4) covering a single gas turbine</obo:IAO_0000115>
        <obo:IAO_0000119>International Organization for Standardization/International ISO 19859:2016

Technical Committee : ISO/TC 192  Gas turbines

ICS :  29.160.99  Other standards related to rotating machinery 27.040  Gas and steam turbines. Steam engines

Gas turbine applications -- Requirements for power generation

Publication date : 2016-08

1st Edition</obo:IAO_0000119>
    </owl:Class>
    


    <!-- http://www.ontologylibrary.mil/OperationalEnvironment/Mid/OEFutureWarfareOntology#GasTurbineHall -->

    <owl:Class rdf:about="http://www.ontologylibrary.mil/OperationalEnvironment/Mid/OEFutureWarfareOntology#GasTurbineHall">
        <rdfs:subClassOf rdf:resource="http://www.ontologylibrary.mil/OperationalEnvironment/Mid/OEFutureWarfareOntology#GasEnergyGeneration"/>
        <obo:IAO_0000115>arge structure that may enclose one or more gas turbine packages, each of which may have their own local enclosure(s) (3.4)</obo:IAO_0000115>
        <obo:IAO_0000119>International Organization for Standardization/International ISO 19859:2016

Technical Committee : ISO/TC 192  Gas turbines

ICS :  29.160.99  Other standards related to rotating machinery 27.040  Gas and steam turbines. Steam engines

Gas turbine applications -- Requirements for power generation

Publication date : 2016-08

1st Edition</obo:IAO_0000119>
    </owl:Class>
    


    <!-- http://www.ontologylibrary.mil/OperationalEnvironment/Mid/OEFutureWarfareOntology#GasTurbinePackage -->

    <owl:Class rdf:about="http://www.ontologylibrary.mil/OperationalEnvironment/Mid/OEFutureWarfareOntology#GasTurbinePackage">
        <rdfs:subClassOf rdf:resource="http://www.ontologylibrary.mil/OperationalEnvironment/Mid/OEFutureWarfareOntology#GasEnergyGeneration"/>
        <obo:IAO_0000115>assembly that includes the gas turbine core (3.5), gas turbine load and auxiliary gearboxes, core integral equipment, applicable auxiliary systems and enclosure (3.4)</obo:IAO_0000115>
        <obo:IAO_0000119>International Organization for Standardization/International ISO 19859:2016

Technical Committee : ISO/TC 192  Gas turbines

ICS :  29.160.99  Other standards related to rotating machinery 27.040  Gas and steam turbines. Steam engines

Gas turbine applications -- Requirements for power generation

Publication date : 2016-08

1st Edition</obo:IAO_0000119>
    </owl:Class>
    


    <!-- http://www.ontologylibrary.mil/OperationalEnvironment/Mid/OEFutureWarfareOntology#Gather -->

    <owl:Class rdf:about="http://www.ontologylibrary.mil/OperationalEnvironment/Mid/OEFutureWarfareOntology#Gather">
        <rdfs:subClassOf rdf:resource="http://www.ontologylibrary.mil/OperationalEnvironment/Mid/OEFutureWarfareOntology#BigDataControlledVocabulary"/>
        <obo:IAO_0000115>consolidation of results from multiple nodes in a cluster</obo:IAO_0000115>
        <obo:IAO_0000119>Information technology — Big data — Overview and vocabulary

https://www.iso.org/jtc1</obo:IAO_0000119>
    </owl:Class>
    


    <!-- http://www.ontologylibrary.mil/OperationalEnvironment/Mid/OEFutureWarfareOntology#GenderAndSexualIdentities -->

    <owl:Class rdf:about="http://www.ontologylibrary.mil/OperationalEnvironment/Mid/OEFutureWarfareOntology#GenderAndSexualIdentities">
        <rdfs:subClassOf rdf:resource="http://www.ontologylibrary.mil/OperationalEnvironment/Mid/OEFutureWarfareOntology#Identity"/>
    </owl:Class>
    


    <!-- http://www.ontologylibrary.mil/OperationalEnvironment/Mid/OEFutureWarfareOntology#GeneticModification -->

    <owl:Class rdf:about="http://www.ontologylibrary.mil/OperationalEnvironment/Mid/OEFutureWarfareOntology#GeneticModification">
        <rdfs:subClassOf rdf:resource="http://www.ontologylibrary.mil/OperationalEnvironment/Mid/OEFutureWarfareOntology#SystemsThatSoldier"/>
        <obo:IAO_0000115>Genetic Modification: Disease resistant, potentially designer babies and super athletes/soldiers.. CRISPR: Genome editing. [SOURCE: TRADOC G-2 Potential Game Changers, May 2018]</obo:IAO_0000115>
        <obo:IAO_0000119>Technology Environment of Ground Warfare in 2035-2050

Projections made in 2018 by ARL and TRADOC

[This is a draft outline of a potential document; prepared by Alexander Kott, the US Army Research Laboratory; July 2018]</obo:IAO_0000119>
    </owl:Class>
    


    <!-- http://www.ontologylibrary.mil/OperationalEnvironment/Mid/OEFutureWarfareOntology#GeoStationaryOrbit -->

    <owl:Class rdf:about="http://www.ontologylibrary.mil/OperationalEnvironment/Mid/OEFutureWarfareOntology#GeoStationaryOrbit">
        <rdfs:subClassOf rdf:resource="http://www.ontologylibrary.mil/OperationalEnvironment/Mid/OEFutureWarfareOntology#SpaceEnvironmentControlledVocabulary"/>
        <obo:IAO_0000115>circular orbit with the altitude of ~36 000 km in the Earth’s equatorial plane. Geostationary orbit is a special case of a geosynchronous orbit</obo:IAO_0000115>
        <obo:IAO_0000119>International Organization for Standardization/International Electrotechnical Commission 17851:2016

Space systems -- Space environment simulation for material tests -- General principles and criteria

Publication Date: 2016-09

1st Edition</obo:IAO_0000119>
    </owl:Class>
    


    <!-- http://www.ontologylibrary.mil/OperationalEnvironment/Mid/OEFutureWarfareOntology#GeosynchronousOrbit -->

    <owl:Class rdf:about="http://www.ontologylibrary.mil/OperationalEnvironment/Mid/OEFutureWarfareOntology#GeosynchronousOrbit">
        <rdfs:subClassOf rdf:resource="http://www.ontologylibrary.mil/OperationalEnvironment/Mid/OEFutureWarfareOntology#SpaceEnvironmentControlledVocabulary"/>
        <obo:IAO_0000115>orbit around the Earth with an orbital period of one sidereal day, matching the Earth&apos;s sidereal rotation period</obo:IAO_0000115>
        <obo:IAO_0000119>International Organization for Standardization/International Electrotechnical Commission 17851:2016

Space systems -- Space environment simulation for material tests -- General principles and criteria

Publication Date: 2016-09

1st Edition</obo:IAO_0000119>
    </owl:Class>
    


    <!-- http://www.ontologylibrary.mil/OperationalEnvironment/Mid/OEFutureWarfareOntology#GlobalWarmingPotential -->

    <owl:Class rdf:about="http://www.ontologylibrary.mil/OperationalEnvironment/Mid/OEFutureWarfareOntology#GlobalWarmingPotential">
        <rdfs:subClassOf rdf:resource="http://www.ontologylibrary.mil/OperationalEnvironment/Mid/OEFutureWarfareOntology#ClimateChangeAndResourceCompetitionControlledVocabulary"/>
        <obo:IAO_0000115>index, based on radiative properties of greenhouse gases, measuring the radiative forcing following a pulse emission of a unit mass of a given greenhouse gas in the present-day atmosphere integrated over a chosen time horizon, relative to that of carbon dioxide (CO2)</obo:IAO_0000115>
        <obo:IAO_0000119>International Organization for Standardization/International Electrotechnical Commission 27000:2018

Technical Committee : ISO/TC 207/SC 7  Greenhouse gas management and related activities

ICS :  13.020.40  Pollution, pollution control and conservation

Greenhouse gases -- Part 1: Specification with guidance at the organization level for quantification and reporting of greenhouse gas emissions and removals 

Publication date : 2018-12

2nd Edition</obo:IAO_0000119>
    </owl:Class>
    


    <!-- http://www.ontologylibrary.mil/OperationalEnvironment/Mid/OEFutureWarfareOntology#GovernanceOfInformationSecurity -->

    <owl:Class rdf:about="http://www.ontologylibrary.mil/OperationalEnvironment/Mid/OEFutureWarfareOntology#GovernanceOfInformationSecurity">
        <rdfs:subClassOf rdf:resource="http://www.ontologylibrary.mil/OperationalEnvironment/Mid/OEFutureWarfareOntology#CyberSecurityControlledVocabulary"/>
        <obo:IAO_0000115>system by which an organization’s (3.50)information security (3.28) activities are directed and controlled</obo:IAO_0000115>
        <obo:IAO_0000119>International Organization for Standardization/International Electrotechnical Commission 27000:2018

Security techniques — Information security management systems — Overview and vocabulary

Publication date : 2018-02

5th Edition</obo:IAO_0000119>
    </owl:Class>
    


    <!-- http://www.ontologylibrary.mil/OperationalEnvironment/Mid/OEFutureWarfareOntology#GoverningBody -->

    <owl:Class rdf:about="http://www.ontologylibrary.mil/OperationalEnvironment/Mid/OEFutureWarfareOntology#GoverningBody">
        <rdfs:subClassOf rdf:resource="http://www.ontologylibrary.mil/OperationalEnvironment/Mid/OEFutureWarfareOntology#CyberSecurityControlledVocabulary"/>
        <obo:IAO_0000115>person or group of people who are accountable for the performance (3.52) and conformity of the organization (3.50)

Note 1 to entry: The governing body can, in some jurisdictions, be a board of directors.</obo:IAO_0000115>
        <obo:IAO_0000119>International Organization for Standardization/International Electrotechnical Commission 27000:2018

Security techniques — Information security management systems — Overview and vocabulary

Publication date : 2018-02

5th Edition</obo:IAO_0000119>
    </owl:Class>
    


    <!-- http://www.ontologylibrary.mil/OperationalEnvironment/Mid/OEFutureWarfareOntology#Government -->

    <owl:Class rdf:about="http://www.ontologylibrary.mil/OperationalEnvironment/Mid/OEFutureWarfareOntology#Government">
        <rdfs:subClassOf rdf:resource="http://www.ontologylibrary.mil/OperationalEnvironment/Mid/OEFutureWarfareOntology#HumanFactorsControlledVocabulary"/>
        <rdfs:label>Government</rdfs:label>
    </owl:Class>
    


    <!-- http://www.ontologylibrary.mil/OperationalEnvironment/Mid/OEFutureWarfareOntology#GreehouseGasEmission -->

    <owl:Class rdf:about="http://www.ontologylibrary.mil/OperationalEnvironment/Mid/OEFutureWarfareOntology#GreehouseGasEmission">
        <rdfs:subClassOf rdf:resource="http://www.ontologylibrary.mil/OperationalEnvironment/Mid/OEFutureWarfareOntology#ClimateChangeAndResourceCompetitionControlledVocabulary"/>
        <obo:IAO_0000115>release of a greehouse gas into the atmosphere</obo:IAO_0000115>
        <obo:IAO_0000119>International Organization for Standardization/International Electrotechnical Commission 27000:2018

Technical Committee : ISO/TC 207/SC 7  Greenhouse gas management and related activities

ICS :  13.020.40  Pollution, pollution control and conservation

Greenhouse gases -- Part 1: Specification with guidance at the organization level for quantification and reporting of greenhouse gas emissions and removals 

Publication date : 2018-12

2nd Edition</obo:IAO_0000119>
    </owl:Class>
    


    <!-- http://www.ontologylibrary.mil/OperationalEnvironment/Mid/OEFutureWarfareOntology#GreenhouseGas -->

    <owl:Class rdf:about="http://www.ontologylibrary.mil/OperationalEnvironment/Mid/OEFutureWarfareOntology#GreenhouseGas">
        <rdfs:subClassOf rdf:resource="http://www.ontologylibrary.mil/OperationalEnvironment/Mid/OEFutureWarfareOntology#ClimateChangeAndResourceCompetitionControlledVocabulary"/>
        <obo:IAO_0000115>gaseous constituent of the atmosphere, both natural and anthropogenic, that absorbs and emits radiation at specific wavelengths within the spectrum of infrared radiation emitted by the Earth’s surface, the atmosphere and clouds

Note 1 to entry: For a list of GHGs, see the latest Intergovernmental Panel on Climate Change (IPCC) Assessment Report.

Note 2 to entry: Water vapour and ozone are anthropogenic as well as natural GHGs, but are not included as recognized GHGs due to difficulties, in most cases, in isolating the human-induced component of global warming attributable to their presence in the atmosphere.</obo:IAO_0000115>
        <obo:IAO_0000119>International Organization for Standardization/International Electrotechnical Commission 27000:2018

Technical Committee : ISO/TC 207/SC 7  Greenhouse gas management and related activities

ICS :  13.020.40  Pollution, pollution control and conservation

Greenhouse gases -- Part 1: Specification with guidance at the organization level for quantification and reporting of greenhouse gas emissions and removals 

Publication date : 2018-12

2nd Edition</obo:IAO_0000119>
    </owl:Class>
    


    <!-- http://www.ontologylibrary.mil/OperationalEnvironment/Mid/OEFutureWarfareOntology#GreenhouseGasActivityData -->

    <owl:Class rdf:about="http://www.ontologylibrary.mil/OperationalEnvironment/Mid/OEFutureWarfareOntology#GreenhouseGasActivityData">
        <rdfs:subClassOf rdf:resource="http://www.ontologylibrary.mil/OperationalEnvironment/Mid/OEFutureWarfareOntology#ClimateChangeAndResourceCompetitionControlledVocabulary"/>
        <obo:IAO_0000115>quantitative measure of activity that results in a greenhouse gas emission (3.1.5) or greenhouse gas removal (3.1.6)

EXAMPLE:Amount of energy, fuels or electricity consumed, material produced, service provided, area of land affected.</obo:IAO_0000115>
        <obo:IAO_0000119>International Organization for Standardization/International Electrotechnical Commission 27000:2018

Technical Committee : ISO/TC 207/SC 7  Greenhouse gas management and related activities

ICS :  13.020.40  Pollution, pollution control and conservation

Greenhouse gases -- Part 1: Specification with guidance at the organization level for quantification and reporting of greenhouse gas emissions and removals 

Publication date : 2018-12

2nd Edition</obo:IAO_0000119>
    </owl:Class>
    


    <!-- http://www.ontologylibrary.mil/OperationalEnvironment/Mid/OEFutureWarfareOntology#GreenhouseGasAssertion -->

    <owl:Class rdf:about="http://www.ontologylibrary.mil/OperationalEnvironment/Mid/OEFutureWarfareOntology#GreenhouseGasAssertion">
        <rdfs:subClassOf rdf:resource="http://www.ontologylibrary.mil/OperationalEnvironment/Mid/OEFutureWarfareOntology#ClimateChangeAndResourceCompetitionControlledVocabulary"/>
        <obo:IAO_0000115>factual and objective declaration that provides the subject matter for the verification (3.4.9) or validation (3.4.10)

Note 1 to entry: The GHG statement could be presented at a point in time or could cover a period of time.

Note 2 to entry: The GHG statement provided by the responsible party (3.4.3) should be clearly identifiable, capable of consistent evaluation or measurement against suitable criteria by a verifier (3.4.11) or validator (3.4.12).

Note 3 to entry: The GHG statement could be provided in a GHG report (3.2.9) or GHG project (3.2.7) plan.</obo:IAO_0000115>
        <obo:IAO_0000119>International Organization for Standardization/International Electrotechnical Commission 27000:2018

Technical Committee : ISO/TC 207/SC 7  Greenhouse gas management and related activities

ICS :  13.020.40  Pollution, pollution control and conservation

Greenhouse gases -- Part 1: Specification with guidance at the organization level for quantification and reporting of greenhouse gas emissions and removals 

Publication date : 2018-12

2nd Edition</obo:IAO_0000119>
    </owl:Class>
    


    <!-- http://www.ontologylibrary.mil/OperationalEnvironment/Mid/OEFutureWarfareOntology#GreenhouseGasEmissionFactor -->

    <owl:Class rdf:about="http://www.ontologylibrary.mil/OperationalEnvironment/Mid/OEFutureWarfareOntology#GreenhouseGasEmissionFactor">
        <rdfs:subClassOf rdf:resource="http://www.ontologylibrary.mil/OperationalEnvironment/Mid/OEFutureWarfareOntology#ClimateChangeAndResourceCompetitionControlledVocabulary"/>
        <obo:IAO_0000115>coefficient relating greenhouse gas activity data (3.2.1) with the greenhouse gas emission (3.1.5)

Note 1 to entry: A GHG emission factor could include an oxidation component.</obo:IAO_0000115>
        <obo:IAO_0000119>International Organization for Standardization/International Electrotechnical Commission 27000:2018

Technical Committee : ISO/TC 207/SC 7  Greenhouse gas management and related activities

ICS :  13.020.40  Pollution, pollution control and conservation

Greenhouse gases -- Part 1: Specification with guidance at the organization level for quantification and reporting of greenhouse gas emissions and removals 

Publication date : 2018-12

2nd Edition</obo:IAO_0000119>
    </owl:Class>
    


    <!-- http://www.ontologylibrary.mil/OperationalEnvironment/Mid/OEFutureWarfareOntology#GreenhouseGasInventory -->

    <owl:Class rdf:about="http://www.ontologylibrary.mil/OperationalEnvironment/Mid/OEFutureWarfareOntology#GreenhouseGasInventory">
        <rdfs:subClassOf rdf:resource="http://www.ontologylibrary.mil/OperationalEnvironment/Mid/OEFutureWarfareOntology#ClimateChangeAndResourceCompetitionControlledVocabulary"/>
        <obo:IAO_0000115>list of greenhouse gas sources (3.1.2) and greenhouse gas sinks (3.1.3), and their quantified greenhouse gas emissions (3.1.5) and greenhouse gas removals (3.1.6)</obo:IAO_0000115>
        <obo:IAO_0000119>International Organization for Standardization/International Electrotechnical Commission 27000:2018

Technical Committee : ISO/TC 207/SC 7  Greenhouse gas management and related activities

ICS :  13.020.40  Pollution, pollution control and conservation

Greenhouse gases -- Part 1: Specification with guidance at the organization level for quantification and reporting of greenhouse gas emissions and removals 

Publication date : 2018-12

2nd Edition</obo:IAO_0000119>
    </owl:Class>
    


    <!-- http://www.ontologylibrary.mil/OperationalEnvironment/Mid/OEFutureWarfareOntology#GreenhouseGasProgram -->

    <owl:Class rdf:about="http://www.ontologylibrary.mil/OperationalEnvironment/Mid/OEFutureWarfareOntology#GreenhouseGasProgram">
        <rdfs:subClassOf rdf:resource="http://www.ontologylibrary.mil/OperationalEnvironment/Mid/OEFutureWarfareOntology#ClimateChangeAndResourceCompetitionControlledVocabulary"/>
        <obo:IAO_0000115>voluntary or mandatory international, national or subnational system or scheme that registers, accounts or manages greenhouse gas emissions (3.1.5), greenhouse gas removals (3.1.6), greenhouse gas emission reductions or greenhouse gas removal enhancements outside the organization (3.4.2) or greenhouse gas project (3.2.7)</obo:IAO_0000115>
        <obo:IAO_0000119>International Organization for Standardization/International Electrotechnical Commission 27000:2018

Technical Committee : ISO/TC 207/SC 7  Greenhouse gas management and related activities

ICS :  13.020.40  Pollution, pollution control and conservation

Greenhouse gases -- Part 1: Specification with guidance at the organization level for quantification and reporting of greenhouse gas emissions and removals 

Publication date : 2018-12

2nd Edition</obo:IAO_0000119>
    </owl:Class>
    


    <!-- http://www.ontologylibrary.mil/OperationalEnvironment/Mid/OEFutureWarfareOntology#GreenhouseGasProject -->

    <owl:Class rdf:about="http://www.ontologylibrary.mil/OperationalEnvironment/Mid/OEFutureWarfareOntology#GreenhouseGasProject">
        <rdfs:subClassOf rdf:resource="http://www.ontologylibrary.mil/OperationalEnvironment/Mid/OEFutureWarfareOntology#ClimateChangeAndResourceCompetitionControlledVocabulary"/>
        <obo:IAO_0000115>activity or activities that alter the conditions of a greenhouse gas baseline and which cause greenhouse gas emission (3.1.5) reductions or greenhouse gas removal (3.1.6) enhancements

Note 1 to entry: ISO 14064-2 provides information on how to determine and use greenhouse gas baselines.</obo:IAO_0000115>
        <obo:IAO_0000119>International Organization for Standardization/International Electrotechnical Commission 27000:2018

Technical Committee : ISO/TC 207/SC 7  Greenhouse gas management and related activities

ICS :  13.020.40  Pollution, pollution control and conservation

Greenhouse gases -- Part 1: Specification with guidance at the organization level for quantification and reporting of greenhouse gas emissions and removals 

Publication date : 2018-12

2nd Edition</obo:IAO_0000119>
    </owl:Class>
    


    <!-- http://www.ontologylibrary.mil/OperationalEnvironment/Mid/OEFutureWarfareOntology#GreenhouseGasReductionInitiative -->

    <owl:Class rdf:about="http://www.ontologylibrary.mil/OperationalEnvironment/Mid/OEFutureWarfareOntology#GreenhouseGasReductionInitiative">
        <rdfs:subClassOf rdf:resource="http://www.ontologylibrary.mil/OperationalEnvironment/Mid/OEFutureWarfareOntology#ClimateChangeAndResourceCompetitionControlledVocabulary"/>
        <obo:IAO_0000115>specific activity or initiative, not organized as a GHG project (3.2.7), implemented by an organization (3.4.2) on a discrete or continuous basis, to reduce or prevent direct or indirect GHGemissions (3.1.5) or enhance direct or indirect GHGremovals (3.1.6)</obo:IAO_0000115>
        <obo:IAO_0000119>International Organization for Standardization/International Electrotechnical Commission 27000:2018

Technical Committee : ISO/TC 207/SC 7  Greenhouse gas management and related activities

ICS :  13.020.40  Pollution, pollution control and conservation

Greenhouse gases -- Part 1: Specification with guidance at the organization level for quantification and reporting of greenhouse gas emissions and removals 

Publication date : 2018-12

2nd Edition</obo:IAO_0000119>
    </owl:Class>
    


    <!-- http://www.ontologylibrary.mil/OperationalEnvironment/Mid/OEFutureWarfareOntology#GreenhouseGasRemoval -->

    <owl:Class rdf:about="http://www.ontologylibrary.mil/OperationalEnvironment/Mid/OEFutureWarfareOntology#GreenhouseGasRemoval">
        <rdfs:subClassOf rdf:resource="http://www.ontologylibrary.mil/OperationalEnvironment/Mid/OEFutureWarfareOntology#ClimateChangeAndResourceCompetitionControlledVocabulary"/>
        <obo:IAO_0000115>withdrawal of a greenhouse gas from the atmosphere by greenhouse gas sinks</obo:IAO_0000115>
        <obo:IAO_0000119>International Organization for Standardization/International Electrotechnical Commission 27000:2018

Technical Committee : ISO/TC 207/SC 7  Greenhouse gas management and related activities

ICS :  13.020.40  Pollution, pollution control and conservation

Greenhouse gases -- Part 1: Specification with guidance at the organization level for quantification and reporting of greenhouse gas emissions and removals 

Publication date : 2018-12

2nd Edition</obo:IAO_0000119>
    </owl:Class>
    


    <!-- http://www.ontologylibrary.mil/OperationalEnvironment/Mid/OEFutureWarfareOntology#GreenhouseGasRemovalFactor -->

    <owl:Class rdf:about="http://www.ontologylibrary.mil/OperationalEnvironment/Mid/OEFutureWarfareOntology#GreenhouseGasRemovalFactor">
        <rdfs:subClassOf rdf:resource="http://www.ontologylibrary.mil/OperationalEnvironment/Mid/OEFutureWarfareOntology#ClimateChangeAndResourceCompetitionControlledVocabulary"/>
        <obo:IAO_0000115>coefficient relating greenhouse gas activity data (3.2.1) with the greenhouse gas removal (3.1.6)

Note 1 to entry: A GHG removal factor could include an oxidation component.</obo:IAO_0000115>
        <obo:IAO_0000119>International Organization for Standardization/International Electrotechnical Commission 27000:2018

Technical Committee : ISO/TC 207/SC 7  Greenhouse gas management and related activities

ICS :  13.020.40  Pollution, pollution control and conservation

Greenhouse gases -- Part 1: Specification with guidance at the organization level for quantification and reporting of greenhouse gas emissions and removals 

Publication date : 2018-12

2nd Edition</obo:IAO_0000119>
    </owl:Class>
    


    <!-- http://www.ontologylibrary.mil/OperationalEnvironment/Mid/OEFutureWarfareOntology#GreenhouseGasReport -->

    <owl:Class rdf:about="http://www.ontologylibrary.mil/OperationalEnvironment/Mid/OEFutureWarfareOntology#GreenhouseGasReport">
        <rdfs:subClassOf rdf:resource="http://www.ontologylibrary.mil/OperationalEnvironment/Mid/OEFutureWarfareOntology#ClimateChangeAndResourceCompetitionControlledVocabulary"/>
        <obo:IAO_0000115>standalone document intended to communicate an organization’s (3.4.2) or GHG project’s (3.2.7) GHG-related information to its intended users (3.4.4)

Note 1 to entry: A GHG report can include a GHG statement (3.2.5).</obo:IAO_0000115>
        <obo:IAO_0000119>International Organization for Standardization/International Electrotechnical Commission 27000:2018

Technical Committee : ISO/TC 207/SC 7  Greenhouse gas management and related activities

ICS :  13.020.40  Pollution, pollution control and conservation

Greenhouse gases -- Part 1: Specification with guidance at the organization level for quantification and reporting of greenhouse gas emissions and removals 

Publication date : 2018-12

2nd Edition</obo:IAO_0000119>
    </owl:Class>
    


    <!-- http://www.ontologylibrary.mil/OperationalEnvironment/Mid/OEFutureWarfareOntology#GreenhouseGasReservoir -->

    <owl:Class rdf:about="http://www.ontologylibrary.mil/OperationalEnvironment/Mid/OEFutureWarfareOntology#GreenhouseGasReservoir">
        <rdfs:subClassOf rdf:resource="http://www.ontologylibrary.mil/OperationalEnvironment/Mid/OEFutureWarfareOntology#ClimateChangeAndResourceCompetitionControlledVocabulary"/>
        <obo:IAO_0000115>component, other than the atmosphere, that has the capacity to accumulate greenhouse gases, and to store and release them

Note 1 to entry: Oceans, soils and forests are examples of components that can act as reservoirs.

Note 2 to entry: GHG capture and storage is one of the processes that results in a GHG reservoir.</obo:IAO_0000115>
        <obo:IAO_0000119>International Organization for Standardization/International Electrotechnical Commission 27000:2018

Technical Committee : ISO/TC 207/SC 7  Greenhouse gas management and related activities

ICS :  13.020.40  Pollution, pollution control and conservation

Greenhouse gases -- Part 1: Specification with guidance at the organization level for quantification and reporting of greenhouse gas emissions and removals 

Publication date : 2018-12

2nd Edition</obo:IAO_0000119>
    </owl:Class>
    


    <!-- http://www.ontologylibrary.mil/OperationalEnvironment/Mid/OEFutureWarfareOntology#GreenhouseGasSink -->

    <owl:Class rdf:about="http://www.ontologylibrary.mil/OperationalEnvironment/Mid/OEFutureWarfareOntology#GreenhouseGasSink">
        <rdfs:subClassOf rdf:resource="http://www.ontologylibrary.mil/OperationalEnvironment/Mid/OEFutureWarfareOntology#ClimateChangeAndResourceCompetitionControlledVocabulary"/>
        <obo:IAO_0000115>process that removes a greenhouse gas from the atmosphere</obo:IAO_0000115>
        <obo:IAO_0000119>International Organization for Standardization/International Electrotechnical Commission 27000:2018

Technical Committee : ISO/TC 207/SC 7  Greenhouse gas management and related activities

ICS :  13.020.40  Pollution, pollution control and conservation

Greenhouse gases -- Part 1: Specification with guidance at the organization level for quantification and reporting of greenhouse gas emissions and removals 

Publication date : 2018-12

2nd Edition</obo:IAO_0000119>
    </owl:Class>
    


    <!-- http://www.ontologylibrary.mil/OperationalEnvironment/Mid/OEFutureWarfareOntology#GreenhouseGasSource -->

    <owl:Class rdf:about="http://www.ontologylibrary.mil/OperationalEnvironment/Mid/OEFutureWarfareOntology#GreenhouseGasSource">
        <rdfs:subClassOf rdf:resource="http://www.ontologylibrary.mil/OperationalEnvironment/Mid/OEFutureWarfareOntology#ClimateChangeAndResourceCompetitionControlledVocabulary"/>
        <obo:IAO_0000115>process that releases a greenhouse gas into the atmosphere</obo:IAO_0000115>
        <obo:IAO_0000119>International Organization for Standardization/International Electrotechnical Commission 27000:2018

Technical Committee : ISO/TC 207/SC 7  Greenhouse gas management and related activities

ICS :  13.020.40  Pollution, pollution control and conservation

Greenhouse gases -- Part 1: Specification with guidance at the organization level for quantification and reporting of greenhouse gas emissions and removals 

Publication date : 2018-12

2nd Edition</obo:IAO_0000119>
    </owl:Class>
    


    <!-- http://www.ontologylibrary.mil/OperationalEnvironment/Mid/OEFutureWarfareOntology#HardenedMunitions -->

    <owl:Class rdf:about="http://www.ontologylibrary.mil/OperationalEnvironment/Mid/OEFutureWarfareOntology#HardenedMunitions">
        <rdfs:subClassOf rdf:resource="http://www.ontologylibrary.mil/OperationalEnvironment/Mid/OEFutureWarfareOntology#SystemsThatShoot"/>
    </owl:Class>
    


    <!-- http://www.ontologylibrary.mil/OperationalEnvironment/Mid/OEFutureWarfareOntology#Healthcare -->

    <owl:Class rdf:about="http://www.ontologylibrary.mil/OperationalEnvironment/Mid/OEFutureWarfareOntology#Healthcare">
        <rdfs:subClassOf rdf:resource="http://www.ontologylibrary.mil/OperationalEnvironment/Mid/OEFutureWarfareOntology#WelfareState"/>
        <obo:IAO_0000119>&quot;Health Care&quot;, Wikipedia

March 23, 2019

https://en.wikipedia.org/wiki/Health_care</obo:IAO_0000119>
        <CommonCoreOntologies:definition>Health care or healthcare is the maintenance or improvement of health via the prevention, diagnosis, and treatment of disease, illness, injury, and other physical and mental impairments in people. Health care is delivered by health professionals (providers or practitioners) in allied health fields. Physicians and physician associates are a part of these health professionals. Dentistry, midwifery, nursing, medicine, optometry, audiology, pharmacy, psychology, occupational therapy, physical therapy and other health professions are all part of health care. It includes work done in providing primary care, secondary care, and tertiary care, as well as in public health.

Access to health care may vary across countries, communities, and individuals, largely influenced by social and economic conditions as well as health policies. Health care systems are organizations established to meet the health needs of targeted populations. According to the World Health Organization (WHO), a well-functioning health care system requires a financing mechanism, a well-trained and adequately paid workforce, reliable information on which to base decisions and policies, and well maintained health facilities to deliver quality medicines and technologies.</CommonCoreOntologies:definition>
        <rdfs:label>Healthcare</rdfs:label>
    </owl:Class>
    


    <!-- http://www.ontologylibrary.mil/OperationalEnvironment/Mid/OEFutureWarfareOntology#HighEllipticalOrbits -->

    <owl:Class rdf:about="http://www.ontologylibrary.mil/OperationalEnvironment/Mid/OEFutureWarfareOntology#HighEllipticalOrbits">
        <rdfs:subClassOf rdf:resource="http://www.ontologylibrary.mil/OperationalEnvironment/Mid/OEFutureWarfareOntology#SpaceEnvironmentControlledVocabulary"/>
        <obo:IAO_0000115>perigee of approximately 1 000 km and apogee of approximately 36 000 km</obo:IAO_0000115>
        <obo:IAO_0000119>International Organization for Standardization/International Electrotechnical Commission 17851:2016

Space systems -- Space environment simulation for material tests -- General principles and criteria

Publication Date: 2016-09

1st Edition</obo:IAO_0000119>
    </owl:Class>
    


    <!-- http://www.ontologylibrary.mil/OperationalEnvironment/Mid/OEFutureWarfareOntology#HighEnergyLaserPrecisionWeaponPointDefense -->

    <owl:Class rdf:about="http://www.ontologylibrary.mil/OperationalEnvironment/Mid/OEFutureWarfareOntology#HighEnergyLaserPrecisionWeaponPointDefense">
        <rdfs:subClassOf rdf:resource="http://www.ontologylibrary.mil/OperationalEnvironment/Mid/OEFutureWarfareOntology#CombatApplication"/>
        <rdfs:subClassOf>
            <owl:Restriction>
                <owl:onProperty rdf:resource="http://www.ontologylibrary.mil/OperationalEnvironment/Mid/OEFutureWarfareOntology#hasCategoryOfEffort"/>
                <owl:someValuesFrom rdf:resource="http://www.ontologylibrary.mil/OperationalEnvironment/Mid/OEFutureWarfareOntology#SystemsThatProtect"/>
            </owl:Restriction>
        </rdfs:subClassOf>
    </owl:Class>
    


    <!-- http://www.ontologylibrary.mil/OperationalEnvironment/Mid/OEFutureWarfareOntology#HighPowerMicrowavePrecisionWeaponPointDefense -->

    <owl:Class rdf:about="http://www.ontologylibrary.mil/OperationalEnvironment/Mid/OEFutureWarfareOntology#HighPowerMicrowavePrecisionWeaponPointDefense">
        <rdfs:subClassOf rdf:resource="http://www.ontologylibrary.mil/OperationalEnvironment/Mid/OEFutureWarfareOntology#CombatApplication"/>
        <rdfs:subClassOf>
            <owl:Restriction>
                <owl:onProperty rdf:resource="http://www.ontologylibrary.mil/OperationalEnvironment/Mid/OEFutureWarfareOntology#hasCategoryOfEffort"/>
                <owl:someValuesFrom rdf:resource="http://www.ontologylibrary.mil/OperationalEnvironment/Mid/OEFutureWarfareOntology#SystemsThatProtect"/>
            </owl:Restriction>
        </rdfs:subClassOf>
        <obo:IAO_0000119>High Power Microwaves

Strategic and Operational Implications for Warfare

Eileen M. Walling, Colonel, UASF

May 2000

Occasional Paper No. 11

Center for Strategy and Technology
Air War College

Air University

Maxwell Air Force Base

http://www.dtic.mil/dtic/tr/fulltext/u2/a425472.pdf</obo:IAO_0000119>
        <obo:IAO_0000119>The military research laboratories have demonstrated that high power
microwave technologies can produce significant effects, ranging from upsetting
to destroying the electronics within military and commercial systems.
The Air Force has led this technology development, and various operational
communities, including the Air Combat Command and U.S. Strategic
Command, have identified numerous offensive and defensive requirements
that can be satisfied by high power microwave weapons.

Several high power microwave technologies have matured to the point
where they are now ready for the transition from engineering and manufacturing
development to deployment as operational weapons. The conclusion
of this study is that high power microwave technology is ready for the transition
to active weapons in the U.S. military. It reviews various applications of high power microwave weapons in strategic and operational missions for
the Air Force, considers the implications of the integration of microwave
technology into operational weapons, and examines numerous constraints
and challenges associated with the transition of new technologies and systems
into the Air Force inventory.</obo:IAO_0000119>
    </owl:Class>
    


    <!-- http://www.ontologylibrary.mil/OperationalEnvironment/Mid/OEFutureWarfareOntology#HorizontalScaling -->

    <owl:Class rdf:about="http://www.ontologylibrary.mil/OperationalEnvironment/Mid/OEFutureWarfareOntology#HorizontalScaling">
        <rdfs:subClassOf rdf:resource="http://www.ontologylibrary.mil/OperationalEnvironment/Mid/OEFutureWarfareOntology#BigDataControlledVocabulary"/>
        <obo:IAO_0000115>providing a single logical unit through the connection of multiple hardware and software

Note 1 to entry: The example of horizontal scaling is increasing the performance of distributed data processing through the addition of nodes in the cluster for additional resources.

Note 2 to entry: Horizontal scaling for increasing performance is also referred to as scale-out.</obo:IAO_0000115>
        <obo:IAO_0000119>Information technology — Big data — Overview and vocabulary

https://www.iso.org/jtc1</obo:IAO_0000119>
    </owl:Class>
    


    <!-- http://www.ontologylibrary.mil/OperationalEnvironment/Mid/OEFutureWarfareOntology#HumanAgentTeaming -->

    <owl:Class rdf:about="http://www.ontologylibrary.mil/OperationalEnvironment/Mid/OEFutureWarfareOntology#HumanAgentTeaming">
        <rdfs:subClassOf rdf:resource="http://www.ontologylibrary.mil/OperationalEnvironment/Mid/OEFutureWarfareOntology#SystemsThatSoldier"/>
        <obo:IAO_0000115>Human-Agent Teaming, i.e., where humans and intelligent systems work together to achieve either a physical or mental task. Human and the intelligent system will trade off cognitive and physical loads in a collaborative fashion. [SOURCE: TRADOC G-2 Potential Game Changers, May 2018]

Interface: From mouse/keyboard/wearables to digital telepathy, centaur systems. [SOURCE: TRADOC G-2 Potential Game Changers, May 2018]</obo:IAO_0000115>
        <obo:IAO_0000119>Technology Environment of Ground Warfare in 2035-2050

Projections made in 2018 by ARL and TRADOC

[This is a draft outline of a potential document; prepared by Alexander Kott, the US Army Research Laboratory; July 2018]</obo:IAO_0000119>
    </owl:Class>
    


    <!-- http://www.ontologylibrary.mil/OperationalEnvironment/Mid/OEFutureWarfareOntology#HumanComputerInteractionControlledVocabulary -->

    <owl:Class rdf:about="http://www.ontologylibrary.mil/OperationalEnvironment/Mid/OEFutureWarfareOntology#HumanComputerInteractionControlledVocabulary">
        <rdfs:subClassOf rdf:resource="http://www.ontologylibrary.mil/OperationalEnvironment/Mid/OEFutureWarfareOntology#ControlledVocabulary"/>
    </owl:Class>
    


    <!-- http://www.ontologylibrary.mil/OperationalEnvironment/Mid/OEFutureWarfareOntology#HumanComputerInteractionTrend -->

    <owl:Class rdf:about="http://www.ontologylibrary.mil/OperationalEnvironment/Mid/OEFutureWarfareOntology#HumanComputerInteractionTrend">
        <rdfs:subClassOf rdf:resource="http://www.ontologylibrary.mil/OperationalEnvironment/Mid/OEFutureWarfareOntology#Trend"/>
        <obo:IAO_0000115>Although more human beings stress available resources, population growth has also compounded the rate of innovation and technology development.  Human creativity is now clearly the most transformative force in the world, both enhancing human life, but also upending it, and – at times – precipitating catastrophic, disruptive events.  Information technology will continue to improve exponentially, and most of the developed world already is instrumented in some way.  Nearly every person on Earth has access to a connected, mobile device.  Advanced material capabilities have, and will continue to extend the trend of reduced size, weight, and power requirements, as nanomaterials, metamaterials, and bespoke structures allow multifunctional assemblies, vastly improving overall systems integration, reliability, and performance.  Advanced materials also foster increases in battery power and performance, allowing large amounts of power to be stored across a distributed grid, and miniaturized storage powers mobile robotics and vehicles of all types</obo:IAO_0000115>
        <obo:IAO_0000115>Singularity is the point at which artificial intelligence (AI) exceeds the collective intelligence of mankind, which will radically and irrevocably change the relationship between man and machine.  There are several divergent possibilities regarding the singularity: 

 As optimistic singularity advocates, such as Ray Kurzweil have suggested, AI improves human life in every way, from healthcare, to emotional evolution, to intergalactic space travel. 

 While not entirely apocalyptic, unboxed general artificial superintelligence improves and evolves at such an exponential rate it escapes human restrictions, perspectives, and morality.  It threatens the very existence of humanity. 

 Humans evolve their own cognitive abilities through learning developments, brain implants, artificial stimulants, and non-AI high performance computing to match, or at least keep pace with AI. 

AI has the capacity to change paradigms, revolutionize everyday life, and take mankind to exciting new horizons.  However, it also may be capable of incredible destruction, malice, and lines of thinking and decision-making that are dangerous to mankind.  This duality will be critical as actors develop military applications for AI.</obo:IAO_0000115>
        <obo:IAO_0000119>The Operational Environment and the Changing Character of Future Warfare</obo:IAO_0000119>
    </owl:Class>
    


    <!-- http://www.ontologylibrary.mil/OperationalEnvironment/Mid/OEFutureWarfareOntology#HumanCryogenics -->

    <owl:Class rdf:about="http://www.ontologylibrary.mil/OperationalEnvironment/Mid/OEFutureWarfareOntology#HumanCryogenics">
        <rdfs:subClassOf rdf:resource="http://www.ontologylibrary.mil/OperationalEnvironment/Mid/OEFutureWarfareOntology#ArtificialIntelligenceControlledVocabulary"/>
        <obo:IAO_0000115>The technique for the conservation of a human body or head in liquid nitrogen, after an individual’s death, with the aim of resuscitating it one day.</obo:IAO_0000115>
        <obo:IAO_0000119>United Nations Educational, Scientific, and Cultural Organization Courier 

March 2018

https://en.unesco.org/courier/2018-3/lexicon-artificial-intelligence</obo:IAO_0000119>
    </owl:Class>
    


    <!-- http://www.ontologylibrary.mil/OperationalEnvironment/Mid/OEFutureWarfareOntology#HumanFactorsControlledVocabulary -->

    <owl:Class rdf:about="http://www.ontologylibrary.mil/OperationalEnvironment/Mid/OEFutureWarfareOntology#HumanFactorsControlledVocabulary">
        <rdfs:subClassOf rdf:resource="http://www.ontologylibrary.mil/OperationalEnvironment/Mid/OEFutureWarfareOntology#ControlledVocabulary"/>
        <rdfs:label>Human Factors Controlled Vocabulary</rdfs:label>
    </owl:Class>
    


    <!-- http://www.ontologylibrary.mil/OperationalEnvironment/Mid/OEFutureWarfareOntology#HunterKillerSwarm -->

    <owl:Class rdf:about="http://www.ontologylibrary.mil/OperationalEnvironment/Mid/OEFutureWarfareOntology#HunterKillerSwarm">
        <rdfs:subClassOf rdf:resource="http://www.ontologylibrary.mil/OperationalEnvironment/Mid/OEFutureWarfareOntology#UnmannedAirVehicles"/>
        <obo:IAO_0000115>Massed, coordinated, fast, collaborative, small, stand-off. Overwhelm target systems. Mass or disaggregate. [SOURCE: TRADOC G-2 Potential Game Changers, May 2018]</obo:IAO_0000115>
        <obo:IAO_0000119>Technology Environment of Ground Warfare in 2035-2050

Projections made in 2018 by ARL and TRADOC

[This is a draft outline of a potential document; prepared by Alexander Kott, the US Army Research Laboratory; July 2018]</obo:IAO_0000119>
    </owl:Class>
    


    <!-- http://www.ontologylibrary.mil/OperationalEnvironment/Mid/OEFutureWarfareOntology#HybridizationBetweenHumansAndMachines -->

    <owl:Class rdf:about="http://www.ontologylibrary.mil/OperationalEnvironment/Mid/OEFutureWarfareOntology#HybridizationBetweenHumansAndMachines">
        <rdfs:subClassOf rdf:resource="http://www.ontologylibrary.mil/OperationalEnvironment/Mid/OEFutureWarfareOntology#ArtificialIntelligenceControlledVocabulary"/>
        <obo:IAO_0000115>This process allows a connection between the human body and a technological system. The connection can be physical, like a mind-controlled prosthetic arm, or virtual, like Google glasses, which are voice-controlled and which display information or images in a corner of the lenses that are superimposed on our usual vision.</obo:IAO_0000115>
        <obo:IAO_0000119>United Nations Educational, Scientific, and Cultural Organization Courier 

March 2018

https://en.unesco.org/courier/2018-3/lexicon-artificial-intelligence</obo:IAO_0000119>
    </owl:Class>
    


    <!-- http://www.ontologylibrary.mil/OperationalEnvironment/Mid/OEFutureWarfareOntology#HyperGlideVehicles -->

    <owl:Class rdf:about="http://www.ontologylibrary.mil/OperationalEnvironment/Mid/OEFutureWarfareOntology#HyperGlideVehicles">
        <rdfs:subClassOf rdf:resource="http://www.ontologylibrary.mil/OperationalEnvironment/Mid/OEFutureWarfareOntology#SystemsThatMove"/>
        <obo:IAO_0000115>Less susceptible to anti ballistic missile countermeasures. [SOURCE: TRADOC G-2 Potential Game Changers, May 2018]</obo:IAO_0000115>
        <obo:IAO_0000119>Technology Environment of Ground Warfare in 2035-2050

Projections made in 2018 by ARL and TRADOC

[This is a draft outline of a potential document; prepared by Alexander Kott, the US Army Research Laboratory; July 2018]</obo:IAO_0000119>
    </owl:Class>
    


    <!-- http://www.ontologylibrary.mil/OperationalEnvironment/Mid/OEFutureWarfareOntology#HypersonicGlideVehicleDefense -->

    <owl:Class rdf:about="http://www.ontologylibrary.mil/OperationalEnvironment/Mid/OEFutureWarfareOntology#HypersonicGlideVehicleDefense">
        <rdfs:subClassOf rdf:resource="http://www.ontologylibrary.mil/OperationalEnvironment/Mid/OEFutureWarfareOntology#CombatApplication"/>
        <rdfs:subClassOf>
            <owl:Restriction>
                <owl:onProperty rdf:resource="http://www.ontologylibrary.mil/OperationalEnvironment/Mid/OEFutureWarfareOntology#hasCategoryOfEffort"/>
                <owl:someValuesFrom rdf:resource="http://www.ontologylibrary.mil/OperationalEnvironment/Mid/OEFutureWarfareOntology#SystemsThatProtect"/>
            </owl:Restriction>
        </rdfs:subClassOf>
    </owl:Class>
    


    <!-- http://www.ontologylibrary.mil/OperationalEnvironment/Mid/OEFutureWarfareOntology#HypervelocityImpact -->

    <owl:Class rdf:about="http://www.ontologylibrary.mil/OperationalEnvironment/Mid/OEFutureWarfareOntology#HypervelocityImpact">
        <rdfs:subClassOf rdf:resource="http://www.ontologylibrary.mil/OperationalEnvironment/Mid/OEFutureWarfareOntology#SpaceSystems"/>
        <obo:IAO_0000115>impact occurring with a velocity greater than the velocity of sound in any given material</obo:IAO_0000115>
        <obo:IAO_0000119>International Organization for Standardization/International Electrotechnical Commission 11227:2012

Space systems — Test procedure to evaluate spacecraft material ejecta upon hypervelocity impact

Publication Date: 2012-09

1st Edition</obo:IAO_0000119>
    </owl:Class>
    


    <!-- http://www.ontologylibrary.mil/OperationalEnvironment/Mid/OEFutureWarfareOntology#Identity -->

    <owl:Class rdf:about="http://www.ontologylibrary.mil/OperationalEnvironment/Mid/OEFutureWarfareOntology#Identity">
        <rdfs:subClassOf rdf:resource="http://www.ontologylibrary.mil/OperationalEnvironment/Mid/OEFutureWarfareOntology#HumanFactorsControlledVocabulary"/>
    </owl:Class>
    


    <!-- http://www.ontologylibrary.mil/OperationalEnvironment/Mid/OEFutureWarfareOntology#ImmersiveVirtualReality -->

    <owl:Class rdf:about="http://www.ontologylibrary.mil/OperationalEnvironment/Mid/OEFutureWarfareOntology#ImmersiveVirtualReality">
        <rdfs:subClassOf rdf:resource="http://www.ontologylibrary.mil/OperationalEnvironment/Mid/OEFutureWarfareOntology#ArtificialIntelligenceControlledVocabulary"/>
        <obo:IAO_0000115>A virtual, computer-generated universe, into which the user is immersed via various sensors or objects (glasses, sensory feedback suits, etc.). Immersion in virtual reality may involve the player of a video game or an aircraft pilot in training.</obo:IAO_0000115>
        <obo:IAO_0000119>United Nations Educational, Scientific, and Cultural Organization Courier 

March 2018

https://en.unesco.org/courier/2018-3/lexicon-artificial-intelligence</obo:IAO_0000119>
    </owl:Class>
    


    <!-- http://www.ontologylibrary.mil/OperationalEnvironment/Mid/OEFutureWarfareOntology#ImpactCrater -->

    <owl:Class rdf:about="http://www.ontologylibrary.mil/OperationalEnvironment/Mid/OEFutureWarfareOntology#ImpactCrater">
        <rdfs:subClassOf rdf:resource="http://www.ontologylibrary.mil/OperationalEnvironment/Mid/OEFutureWarfareOntology#SpaceSystems"/>
        <obo:IAO_0000115>damage left on a material, generally hemispherical in shape, after a projectile has hit its surface without going throughout the material</obo:IAO_0000115>
        <obo:IAO_0000119>International Organization for Standardization/International Electrotechnical Commission 11227:2012

Space systems — Test procedure to evaluate spacecraft material ejecta upon hypervelocity impact

Publication Date: 2012-09

1st Edition</obo:IAO_0000119>
    </owl:Class>
    


    <!-- http://www.ontologylibrary.mil/OperationalEnvironment/Mid/OEFutureWarfareOntology#IncreasedLevelOfHumanPerformanceControlledVocabulary -->

    <owl:Class rdf:about="http://www.ontologylibrary.mil/OperationalEnvironment/Mid/OEFutureWarfareOntology#IncreasedLevelOfHumanPerformanceControlledVocabulary">
        <rdfs:subClassOf rdf:resource="http://www.ontologylibrary.mil/OperationalEnvironment/Mid/OEFutureWarfareOntology#ControlledVocabulary"/>
    </owl:Class>
    


    <!-- http://www.ontologylibrary.mil/OperationalEnvironment/Mid/OEFutureWarfareOntology#IncreasedLevelOfHumanPerformanceTrend -->

    <owl:Class rdf:about="http://www.ontologylibrary.mil/OperationalEnvironment/Mid/OEFutureWarfareOntology#IncreasedLevelOfHumanPerformanceTrend">
        <rdfs:subClassOf rdf:resource="http://www.ontologylibrary.mil/OperationalEnvironment/Mid/OEFutureWarfareOntology#Trend"/>
        <obo:IAO_0000115>Although more human beings stress available resources, population growth has also compounded the rate of innovation and technology development.  Human creativity is now clearly the most transformative force in the world, both enhancing human life, but also upending it, and – at times – precipitating catastrophic, disruptive events.  Information technology will continue to improve exponentially, and most of the developed world already is instrumented in some way.  Nearly every person on Earth has access to a connected, mobile device.  Advanced material capabilities have, and will continue to extend the trend of reduced size, weight, and power requirements, as nanomaterials, metamaterials, and bespoke structures allow multifunctional assemblies, vastly improving overall systems integration, reliability, and performance.  Advanced materials also foster increases in battery power and performance, allowing large amounts of power to be stored across a distributed grid, and miniaturized storage powers mobile robotics and vehicles of all types</obo:IAO_0000115>
        <obo:IAO_0000119>The Operational Environment and the Changing Character of Future Warfare</obo:IAO_0000119>
    </owl:Class>
    


    <!-- http://www.ontologylibrary.mil/OperationalEnvironment/Mid/OEFutureWarfareOntology#IncreasingLongevity -->

    <owl:Class rdf:about="http://www.ontologylibrary.mil/OperationalEnvironment/Mid/OEFutureWarfareOntology#IncreasingLongevity">
        <rdfs:subClassOf rdf:resource="http://www.ontologylibrary.mil/OperationalEnvironment/Mid/OEFutureWarfareOntology#AgingPopulation"/>
        <obo:IAO_0000119>&quot;Life Expectancy around the World Has Increased Steadily for Nearly 200 Years&quot;, Scitable

2014

https://www.nature.com/scitable/content/life-expectancy-around-the-world-has-increased-19786</obo:IAO_0000119>
        <CommonCoreOntologies:definition>During the nineteenth and early twentieth centuries, an increase in life expectancy was driven mainly by improvements in sanitation, housing, and education, causing a steady decline in early and mid-life mortality, which was chiefly due to infections. This trend continued with the development of vaccines and then antibiotics. By the latter half of the twentieth century, there was little room for further reduction in early and mid-life mortality. The continuing increase is due almost entirely to a new phenomenon: the decline in late-life mortality.</CommonCoreOntologies:definition>
        <rdfs:label>Increasing Longevity</rdfs:label>
    </owl:Class>
    


    <!-- http://www.ontologylibrary.mil/OperationalEnvironment/Mid/OEFutureWarfareOntology#Indicator -->

    <owl:Class rdf:about="http://www.ontologylibrary.mil/OperationalEnvironment/Mid/OEFutureWarfareOntology#Indicator">
        <rdfs:subClassOf rdf:resource="http://www.ontologylibrary.mil/OperationalEnvironment/Mid/OEFutureWarfareOntology#CyberSecurityControlledVocabulary"/>
        <obo:IAO_0000115>measure (3.42) that provides an estimate or evaluation</obo:IAO_0000115>
        <obo:IAO_0000119>International Organization for Standardization/International Electrotechnical Commission 27000:2018

Security techniques — Information security management systems — Overview and vocabulary

Publication date : 2018-02

5th Edition</obo:IAO_0000119>
    </owl:Class>
    


    <!-- http://www.ontologylibrary.mil/OperationalEnvironment/Mid/OEFutureWarfareOntology#IndirectGreenhouseGasEmission -->

    <owl:Class rdf:about="http://www.ontologylibrary.mil/OperationalEnvironment/Mid/OEFutureWarfareOntology#IndirectGreenhouseGasEmission">
        <rdfs:subClassOf rdf:resource="http://www.ontologylibrary.mil/OperationalEnvironment/Mid/OEFutureWarfareOntology#ClimateChangeAndResourceCompetitionControlledVocabulary"/>
        <obo:IAO_0000115>Greenhouse gas emission that is a consequence of an organization’s operations and activities, but that arises from greenhouse gas sources that are not owned or controlled by the organization

Note 1 to entry: These emissions occur generally in the upstream and/or downstream chain.</obo:IAO_0000115>
        <obo:IAO_0000119>International Organization for Standardization/International Electrotechnical Commission 27000:2018

Technical Committee : ISO/TC 207/SC 7  Greenhouse gas management and related activities

ICS :  13.020.40  Pollution, pollution control and conservation

Greenhouse gases -- Part 1: Specification with guidance at the organization level for quantification and reporting of greenhouse gas emissions and removals 

Publication date : 2018-12

2nd Edition</obo:IAO_0000119>
    </owl:Class>
    


    <!-- http://www.ontologylibrary.mil/OperationalEnvironment/Mid/OEFutureWarfareOntology#Industrialization -->

    <owl:Class rdf:about="http://www.ontologylibrary.mil/OperationalEnvironment/Mid/OEFutureWarfareOntology#Industrialization">
        <rdfs:subClassOf rdf:resource="http://www.ontologylibrary.mil/OperationalEnvironment/Mid/OEFutureWarfareOntology#EconomicDevelopment"/>
        <obo:IAO_0000119>Will Kenton (ed.), &quot;Industrialization&quot;, Investopedia

April 7, 2018

https://www.investopedia.com/terms/i/industrialization.asp</obo:IAO_0000119>
        <CommonCoreOntologies:definition>Industrialization is the process by which an economy is transformed from primarily agricultural to one based on the manufacturing of goods. Individual manual labor is often replaced by mechanized mass production, and craftsmen are replaced by assembly lines. Characteristics of industrialization include economic growth, more efficient division of labor, and the use of technological innovation to solve problems as opposed to dependency on conditions outside human control.</CommonCoreOntologies:definition>
        <rdfs:label>Industrialization</rdfs:label>
    </owl:Class>
    


    <!-- http://www.ontologylibrary.mil/OperationalEnvironment/Mid/OEFutureWarfareOntology#InformalEconomy -->

    <owl:Class rdf:about="http://www.ontologylibrary.mil/OperationalEnvironment/Mid/OEFutureWarfareOntology#InformalEconomy">
        <rdfs:subClassOf rdf:resource="http://www.ontologylibrary.mil/OperationalEnvironment/Mid/OEFutureWarfareOntology#EconomicActivity"/>
        <obo:IAO_0000119>Diana Farrell, &quot;The Hidden Dangers of the Informal Economy&quot;, McKinsey Quarterly

July, 2004

https://www.mckinsey.com/featured-insights/employment-and-growth/the-hidden-dangers-of-the-informal-economy</obo:IAO_0000119>
        <CommonCoreOntologies:definition>The informal economy refers to companies that are engaged in legitimate business activities but don&apos;t fully comply with tax, labor market obligations, or product market regulations.

...

Around the world, these informal players operate at just half the average productivity level of formal companies in the same sectors and at a small fraction of the productivity of the best companies. As a result, informal companies persistently drag down a country&apos;s overall productivity and standard of living.

MGI&apos;s investigation also found that the substantial cost advantage that informal companies gain by avoiding taxes and regulations more than offsets their low productivity and small scale. Competition is therefore distorted because inefficient informal players stay in business and prevent more productive, formal companies from gaining market share.</CommonCoreOntologies:definition>
        <rdfs:label>Informal Economy</rdfs:label>
    </owl:Class>
    


    <!-- http://www.ontologylibrary.mil/OperationalEnvironment/Mid/OEFutureWarfareOntology#InformalInstitutions -->

    <owl:Class rdf:about="http://www.ontologylibrary.mil/OperationalEnvironment/Mid/OEFutureWarfareOntology#InformalInstitutions">
        <rdfs:subClassOf rdf:resource="http://www.ontologylibrary.mil/OperationalEnvironment/Mid/OEFutureWarfareOntology#Government"/>
        <obo:IAO_0000115>To understand the political behaviour in a country it is important to look at how that behaviour is enabled or constrained by informal institutions, and how this affects how formal institutions are run. For example, if there are high levels of extrajudicial killings in a country, it might be that while it is prohibited by the state the police are actually enabled to carry out such killings and informally encouraged to prop up an inefficient formal state police institution. An informal institution tends to have socially shared rules, which are unwritten and yet are often known by all inhabitants of a certain country, as such they are often referred to as being an inherent part of the culture of a given country. Informal practices are often referred to as &quot;cultural&quot;, for example clientelism or corruption is sometimes stated as a part of the political culture in a certain place, but an informal institution itself is not cultural, it may be shaped by culture or behaviour of a given political landscape, but they should be looked at in the same way as formal institutions to understand their role in a given country. Informal institutions might be particularly used to pursue a political agenda, or a course of action that might not be publicly popular, or even legal, and can be seen as an effective way of making up for lack of efficiency in a formal institution. For example, in countries where formal institutions are particularly inefficient, an informal institution may be the most cost effective way or actually carrying out a given task, and this ensures that there is little pressure on the formal institutions to become more efficient.The relationship between formal and informal institutions is often closely aligned and informal institutions step in to prop up inefficient institutions.</obo:IAO_0000115>
        <obo:IAO_0000119>&quot;Institution&quot;, Wikipedia

March 12, 2019

https://en.wikipedia.org/wiki/Institution#Informal_institutions</obo:IAO_0000119>
        <rdfs:label>Informal Institutions</rdfs:label>
    </owl:Class>
    


    <!-- http://www.ontologylibrary.mil/OperationalEnvironment/Mid/OEFutureWarfareOntology#InformationNeed -->

    <owl:Class rdf:about="http://www.ontologylibrary.mil/OperationalEnvironment/Mid/OEFutureWarfareOntology#InformationNeed">
        <rdfs:subClassOf rdf:resource="http://www.ontologylibrary.mil/OperationalEnvironment/Mid/OEFutureWarfareOntology#CyberSecurityControlledVocabulary"/>
        <obo:IAO_0000115>insight necessary to manage objectives (3.49), goals, risks and problems</obo:IAO_0000115>
        <obo:IAO_0000119>International Organization for Standardization/International Electrotechnical Commission 27000:2018

Security techniques — Information security management systems — Overview and vocabulary

Publication date : 2018-02

5th Edition</obo:IAO_0000119>
    </owl:Class>
    


    <!-- http://www.ontologylibrary.mil/OperationalEnvironment/Mid/OEFutureWarfareOntology#InformationProcessingFacilities -->

    <owl:Class rdf:about="http://www.ontologylibrary.mil/OperationalEnvironment/Mid/OEFutureWarfareOntology#InformationProcessingFacilities">
        <rdfs:subClassOf rdf:resource="http://www.ontologylibrary.mil/OperationalEnvironment/Mid/OEFutureWarfareOntology#CyberSecurityControlledVocabulary"/>
        <obo:IAO_0000115>any information processing system, service or infrastructure, or the physical location housing it</obo:IAO_0000115>
        <obo:IAO_0000119>International Organization for Standardization/International Electrotechnical Commission 27000:2018

Security techniques — Information security management systems — Overview and vocabulary

Publication date : 2018-02

5th Edition</obo:IAO_0000119>
    </owl:Class>
    


    <!-- http://www.ontologylibrary.mil/OperationalEnvironment/Mid/OEFutureWarfareOntology#InformationSecurity -->

    <owl:Class rdf:about="http://www.ontologylibrary.mil/OperationalEnvironment/Mid/OEFutureWarfareOntology#InformationSecurity">
        <rdfs:subClassOf rdf:resource="http://www.ontologylibrary.mil/OperationalEnvironment/Mid/OEFutureWarfareOntology#CyberSecurityControlledVocabulary"/>
        <obo:IAO_0000115>preservation of confidentiality (3.10), integrity (3.36) and availability (3.7) of information

Note 1 to entry: In addition, other properties, such as authenticity (3.6), accountability, non-repudiation (3.48), and reliability (3.55) can also be involved.</obo:IAO_0000115>
        <obo:IAO_0000119>International Organization for Standardization/International Electrotechnical Commission 27000:2018

Security techniques — Information security management systems — Overview and vocabulary

Publication date : 2018-02

5th Edition</obo:IAO_0000119>
    </owl:Class>
    


    <!-- http://www.ontologylibrary.mil/OperationalEnvironment/Mid/OEFutureWarfareOntology#InformationSecurityContinuity -->

    <owl:Class rdf:about="http://www.ontologylibrary.mil/OperationalEnvironment/Mid/OEFutureWarfareOntology#InformationSecurityContinuity">
        <rdfs:subClassOf rdf:resource="http://www.ontologylibrary.mil/OperationalEnvironment/Mid/OEFutureWarfareOntology#CyberSecurityControlledVocabulary"/>
        <obo:IAO_0000115>processes (3.54) and procedures for ensuring continued information security (3.28) operations</obo:IAO_0000115>
        <obo:IAO_0000119>International Organization for Standardization/International Electrotechnical Commission 27000:2018

Security techniques — Information security management systems — Overview and vocabulary

Publication date : 2018-02

5th Edition</obo:IAO_0000119>
    </owl:Class>
    


    <!-- http://www.ontologylibrary.mil/OperationalEnvironment/Mid/OEFutureWarfareOntology#InformationSecurityEvent -->

    <owl:Class rdf:about="http://www.ontologylibrary.mil/OperationalEnvironment/Mid/OEFutureWarfareOntology#InformationSecurityEvent">
        <rdfs:subClassOf rdf:resource="http://www.ontologylibrary.mil/OperationalEnvironment/Mid/OEFutureWarfareOntology#CyberSecurityControlledVocabulary"/>
        <obo:IAO_0000115>identified occurrence of a system, service or network state indicating a possible breach of information security (3.28) policy (3.53) or failure of controls (3.14), or a previously unknown situation that can be security relevant</obo:IAO_0000115>
        <obo:IAO_0000119>International Organization for Standardization/International Electrotechnical Commission 27000:2018

Security techniques — Information security management systems — Overview and vocabulary

Publication date : 2018-02

5th Edition</obo:IAO_0000119>
    </owl:Class>
    


    <!-- http://www.ontologylibrary.mil/OperationalEnvironment/Mid/OEFutureWarfareOntology#InformationSecurityIncident -->

    <owl:Class rdf:about="http://www.ontologylibrary.mil/OperationalEnvironment/Mid/OEFutureWarfareOntology#InformationSecurityIncident">
        <rdfs:subClassOf rdf:resource="http://www.ontologylibrary.mil/OperationalEnvironment/Mid/OEFutureWarfareOntology#CyberSecurityControlledVocabulary"/>
        <obo:IAO_0000115>single or a series of unwanted or unexpected information security events (3.30) that have a significant probability of compromising business operations and threatening information security (3.28)</obo:IAO_0000115>
        <obo:IAO_0000119>International Organization for Standardization/International Electrotechnical Commission 27000:2018

Security techniques — Information security management systems — Overview and vocabulary

Publication date : 2018-02

5th Edition</obo:IAO_0000119>
    </owl:Class>
    


    <!-- http://www.ontologylibrary.mil/OperationalEnvironment/Mid/OEFutureWarfareOntology#InformationSecurityIncidentManagement -->

    <owl:Class rdf:about="http://www.ontologylibrary.mil/OperationalEnvironment/Mid/OEFutureWarfareOntology#InformationSecurityIncidentManagement">
        <rdfs:subClassOf rdf:resource="http://www.ontologylibrary.mil/OperationalEnvironment/Mid/OEFutureWarfareOntology#CyberSecurityControlledVocabulary"/>
        <obo:IAO_0000115>set ofprocesses (3.54) for detecting, reporting, assessing, responding to, dealing with, and learning from information security incidents (3.31)</obo:IAO_0000115>
        <obo:IAO_0000119>International Organization for Standardization/International Electrotechnical Commission 27000:2018

Security techniques — Information security management systems — Overview and vocabulary

Publication date : 2018-02

5th Edition</obo:IAO_0000119>
    </owl:Class>
    


    <!-- http://www.ontologylibrary.mil/OperationalEnvironment/Mid/OEFutureWarfareOntology#InformationSecurityManagementSystemProfessional -->

    <owl:Class rdf:about="http://www.ontologylibrary.mil/OperationalEnvironment/Mid/OEFutureWarfareOntology#InformationSecurityManagementSystemProfessional">
        <rdfs:subClassOf rdf:resource="http://www.ontologylibrary.mil/OperationalEnvironment/Mid/OEFutureWarfareOntology#CyberSecurityControlledVocabulary"/>
        <obo:IAO_0000115>person who establishes, implements, maintains and continuously improves one or more information security management system processes (3.54)</obo:IAO_0000115>
        <obo:IAO_0000119>International Organization for Standardization/International Electrotechnical Commission 27000:2018

Security techniques — Information security management systems — Overview and vocabulary

Publication date : 2018-02

5th Edition</obo:IAO_0000119>
    </owl:Class>
    


    <!-- http://www.ontologylibrary.mil/OperationalEnvironment/Mid/OEFutureWarfareOntology#InformationSharingCommunity -->

    <owl:Class rdf:about="http://www.ontologylibrary.mil/OperationalEnvironment/Mid/OEFutureWarfareOntology#InformationSharingCommunity">
        <rdfs:subClassOf rdf:resource="http://www.ontologylibrary.mil/OperationalEnvironment/Mid/OEFutureWarfareOntology#CyberSecurityControlledVocabulary"/>
        <obo:IAO_0000115>group of organizations (3.50) that agree to share information

Note 1 to entry: An organization can be an individual.</obo:IAO_0000115>
        <obo:IAO_0000119>International Organization for Standardization/International Electrotechnical Commission 27000:2018

Security techniques — Information security management systems — Overview and vocabulary

Publication date : 2018-02

5th Edition</obo:IAO_0000119>
    </owl:Class>
    


    <!-- http://www.ontologylibrary.mil/OperationalEnvironment/Mid/OEFutureWarfareOntology#InformationSystem -->

    <owl:Class rdf:about="http://www.ontologylibrary.mil/OperationalEnvironment/Mid/OEFutureWarfareOntology#InformationSystem">
        <rdfs:subClassOf rdf:resource="http://www.ontologylibrary.mil/OperationalEnvironment/Mid/OEFutureWarfareOntology#CyberSecurityControlledVocabulary"/>
        <obo:IAO_0000115>set of applications, services, information technology assets, or other information-handling components</obo:IAO_0000115>
        <obo:IAO_0000119>International Organization for Standardization/International Electrotechnical Commission 27000:2018

Security techniques — Information security management systems — Overview and vocabulary

Publication date : 2018-02

5th Edition</obo:IAO_0000119>
    </owl:Class>
    


    <!-- http://www.ontologylibrary.mil/OperationalEnvironment/Mid/OEFutureWarfareOntology#InsensitiveMunitions -->

    <owl:Class rdf:about="http://www.ontologylibrary.mil/OperationalEnvironment/Mid/OEFutureWarfareOntology#InsensitiveMunitions">
        <rdfs:subClassOf rdf:resource="http://www.ontologylibrary.mil/OperationalEnvironment/Mid/OEFutureWarfareOntology#SystemsThatShoot"/>
        <obo:IAO_0000115>Chemically stable munitions withstand shock, fire, projectiles; yet explode as intended. [SOURCE: TRADOC G-2 Potential Game Changers, May 2018]</obo:IAO_0000115>
        <obo:IAO_0000119>Technology Environment of Ground Warfare in 2035-2050

Projections made in 2018 by ARL and TRADOC

[This is a draft outline of a potential document; prepared by Alexander Kott, the US Army Research Laboratory; July 2018]</obo:IAO_0000119>
    </owl:Class>
    


    <!-- http://www.ontologylibrary.mil/OperationalEnvironment/Mid/OEFutureWarfareOntology#Insurgency -->

    <owl:Class rdf:about="http://www.ontologylibrary.mil/OperationalEnvironment/Mid/OEFutureWarfareOntology#Insurgency">
        <rdfs:subClassOf rdf:resource="http://www.ontologylibrary.mil/OperationalEnvironment/Mid/OEFutureWarfareOntology#SubstateConflict"/>
    </owl:Class>
    


    <!-- http://www.ontologylibrary.mil/OperationalEnvironment/Mid/OEFutureWarfareOntology#IntegrationOfNeuroscienceIntoAI -->

    <owl:Class rdf:about="http://www.ontologylibrary.mil/OperationalEnvironment/Mid/OEFutureWarfareOntology#IntegrationOfNeuroscienceIntoAI">
        <rdfs:subClassOf rdf:resource="http://www.ontologylibrary.mil/OperationalEnvironment/Mid/OEFutureWarfareOntology#SystemsThatSoldier"/>
        <obo:IAO_0000115>Projected breakthroughs in integration of neuroscience and conventional computing into AI will lead to omnipresent, highly distributed machine intelligence embedded within a multitude of physical objects surrounding and teaming with the warfighters. [SOURCE: ARL-TR-8283]</obo:IAO_0000115>
        <obo:IAO_0000119>Technology Environment of Ground Warfare in 2035-2050

Projections made in 2018 by ARL and TRADOC

[This is a draft outline of a potential document; prepared by Alexander Kott, the US Army Research Laboratory; July 2018]</obo:IAO_0000119>
    </owl:Class>
    


    <!-- http://www.ontologylibrary.mil/OperationalEnvironment/Mid/OEFutureWarfareOntology#Integrity -->

    <owl:Class rdf:about="http://www.ontologylibrary.mil/OperationalEnvironment/Mid/OEFutureWarfareOntology#Integrity">
        <rdfs:subClassOf rdf:resource="http://www.ontologylibrary.mil/OperationalEnvironment/Mid/OEFutureWarfareOntology#CyberSecurityControlledVocabulary"/>
        <obo:IAO_0000115>property of accuracy and completeness</obo:IAO_0000115>
        <obo:IAO_0000119>International Organization for Standardization/International Electrotechnical Commission 27000:2018

Security techniques — Information security management systems — Overview and vocabulary

Publication date : 2018-02

5th Edition</obo:IAO_0000119>
    </owl:Class>
    


    <!-- http://www.ontologylibrary.mil/OperationalEnvironment/Mid/OEFutureWarfareOntology#IntendedUseOfTheGreenhouseGasInventory -->

    <owl:Class rdf:about="http://www.ontologylibrary.mil/OperationalEnvironment/Mid/OEFutureWarfareOntology#IntendedUseOfTheGreenhouseGasInventory">
        <rdfs:subClassOf rdf:resource="http://www.ontologylibrary.mil/OperationalEnvironment/Mid/OEFutureWarfareOntology#ClimateChangeAndResourceCompetitionControlledVocabulary"/>
        <obo:IAO_0000115>main purpose set by the organization (3.4.2), or a programme, to quantify its GHGemissions (3.1.5) and GHGremovals (3.1.6) consistent with the needs of the intended user (3.4.4)</obo:IAO_0000115>
        <obo:IAO_0000119>International Organization for Standardization/International Electrotechnical Commission 27000:2018

Technical Committee : ISO/TC 207/SC 7  Greenhouse gas management and related activities

ICS :  13.020.40  Pollution, pollution control and conservation

Greenhouse gases -- Part 1: Specification with guidance at the organization level for quantification and reporting of greenhouse gas emissions and removals 

Publication date : 2018-12

2nd Edition</obo:IAO_0000119>
    </owl:Class>
    


    <!-- http://www.ontologylibrary.mil/OperationalEnvironment/Mid/OEFutureWarfareOntology#IntendedUser -->

    <owl:Class rdf:about="http://www.ontologylibrary.mil/OperationalEnvironment/Mid/OEFutureWarfareOntology#IntendedUser">
        <rdfs:subClassOf rdf:resource="http://www.ontologylibrary.mil/OperationalEnvironment/Mid/OEFutureWarfareOntology#ClimateChangeAndResourceCompetitionControlledVocabulary"/>
        <obo:IAO_0000115>individual or organization (3.4.2) identified by those reporting GHG-related information as being the one who relies on that information to make decisions

Note 1 to entry: The intended user can be the client (3.4.5), the responsible party (3.4.3), the organization itself, GHG programme (3.2.8) administrators, regulators, the financial community or other affected interested parties, such as local communities, government departments, general public or non-governmental organizations.</obo:IAO_0000115>
        <obo:IAO_0000119>International Organization for Standardization/International Electrotechnical Commission 27000:2018

Technical Committee : ISO/TC 207/SC 7  Greenhouse gas management and related activities

ICS :  13.020.40  Pollution, pollution control and conservation

Greenhouse gases -- Part 1: Specification with guidance at the organization level for quantification and reporting of greenhouse gas emissions and removals 

Publication date : 2018-12

2nd Edition</obo:IAO_0000119>
    </owl:Class>
    


    <!-- http://www.ontologylibrary.mil/OperationalEnvironment/Mid/OEFutureWarfareOntology#InterestedParty -->

    <owl:Class rdf:about="http://www.ontologylibrary.mil/OperationalEnvironment/Mid/OEFutureWarfareOntology#InterestedParty">
        <rdfs:subClassOf rdf:resource="http://www.ontologylibrary.mil/OperationalEnvironment/Mid/OEFutureWarfareOntology#CyberSecurityControlledVocabulary"/>
        <obo:IAO_0000115>person or organization (3.50) that can affect, be affected by, or perceive itself to be affected by a decision or activity</obo:IAO_0000115>
        <obo:IAO_0000119>International Organization for Standardization/International Electrotechnical Commission 27000:2018

Security techniques — Information security management systems — Overview and vocabulary

Publication date : 2018-02

5th Edition</obo:IAO_0000119>
    </owl:Class>
    


    <!-- http://www.ontologylibrary.mil/OperationalEnvironment/Mid/OEFutureWarfareOntology#IntergovernmentalOrganization -->

    <owl:Class rdf:about="http://www.ontologylibrary.mil/OperationalEnvironment/Mid/OEFutureWarfareOntology#IntergovernmentalOrganization">
        <rdfs:subClassOf rdf:resource="http://www.ontologylibrary.mil/OperationalEnvironment/Mid/OEFutureWarfareOntology#InternationalSystem"/>
        <obo:IAO_0000119>&quot;Intergovernment Organization&quot;, Wikipedia

March 13, 2019

https://en.wikipedia.org/wiki/Intergovernmental_organization#Types_and_purpose</obo:IAO_0000119>
        <CommonCoreOntologies:definition>[Intergovernmental organizations] have various goals and scopes, often outlined in the treaty or charter. Some IGOs developed to fulfill a need for a neutral forum for debate or negotiation to resolve disputes. Others developed to carry out mutual interests with unified aims to preserve peace through conflict resolution and better international relations, promote international cooperation on matters such as environmental protection, to promote human rights, to promote social development (education, health care), to render humanitarian aid, and to economic development. Some are more general in scope (the United Nations) while others may have subject-specific missions (such as Interpol or the International Organization for Standardization and other standards organizations).</CommonCoreOntologies:definition>
        <rdfs:label>Intergovernment Organization</rdfs:label>
    </owl:Class>
    


    <!-- http://www.ontologylibrary.mil/OperationalEnvironment/Mid/OEFutureWarfareOntology#InternalContext -->

    <owl:Class rdf:about="http://www.ontologylibrary.mil/OperationalEnvironment/Mid/OEFutureWarfareOntology#InternalContext">
        <rdfs:subClassOf rdf:resource="http://www.ontologylibrary.mil/OperationalEnvironment/Mid/OEFutureWarfareOntology#CyberSecurityControlledVocabulary"/>
        <obo:IAO_0000115>internal environment in which the organization (3.50) seeks to achieve its objectives

Note 1 to entry: Internal context can include:

— governance, organizational structure, roles and accountabilities;
— policies (3.53), objectives (3.49), and the strategies that are in place to achieve them;
— the capabilities, understood in terms of resources and knowledge (e.g. capital, time, people, processes (3.54), systems and technologies);
— information systems (3.35), information flows and decision-making processes (both formal and informal);
— relationships with, and perceptions and values of, internal stakeholders (3.37);
— the organization&apos;s culture;
— standards, guidelines and models adopted by the organization;
— form and extent of contractual relationships.</obo:IAO_0000115>
        <obo:IAO_0000119>International Organization for Standardization/International Electrotechnical Commission 27000:2018

Security techniques — Information security management systems — Overview and vocabulary

Publication date : 2018-02

5th Edition</obo:IAO_0000119>
        <obo:IAO_0000119>[SOURCE: ISO Guide 73:2009, 3.3.1.2]</obo:IAO_0000119>
    </owl:Class>
    


    <!-- http://www.ontologylibrary.mil/OperationalEnvironment/Mid/OEFutureWarfareOntology#InternationalAlliances -->

    <owl:Class rdf:about="http://www.ontologylibrary.mil/OperationalEnvironment/Mid/OEFutureWarfareOntology#InternationalAlliances">
        <rdfs:subClassOf rdf:resource="http://www.ontologylibrary.mil/OperationalEnvironment/Mid/OEFutureWarfareOntology#SecurityAndViolentConflict"/>
    </owl:Class>
    


    <!-- http://www.ontologylibrary.mil/OperationalEnvironment/Mid/OEFutureWarfareOntology#InternationalMigration -->

    <owl:Class rdf:about="http://www.ontologylibrary.mil/OperationalEnvironment/Mid/OEFutureWarfareOntology#InternationalMigration">
        <rdfs:subClassOf rdf:resource="http://www.ontologylibrary.mil/OperationalEnvironment/Mid/OEFutureWarfareOntology#Migration"/>
        <obo:IAO_0000119>&quot;International Migration&quot;, Wikipedia

March 26, 2019

https://en.wikipedia.org/wiki/International_migration</obo:IAO_0000119>
        <CommonCoreOntologies:definition>nternational migration occurs when people cross state boundaries and stay in the host state for some minimum length of time. Migration occurs for many reasons. Many people leave their home countries in order to look for economic opportunities in another country. Others migrate to be with family members who have migrated or because of political conditions in their countries. Education is another reason for international migration, as students pursue their studies abroad. While there are several different potential systems for categorizing international migrants, one system organizes them into nine groups: temporary labour migrants; irregular, illegal, or undocumented migrants; highly skilled and business migrants; refugees; asylum seekers; forced migration; family members; return migrants; and long-term, low-skilled migrants. These migrants can also be divided into two large groups, permanent and temporary. Permanent migrants intend to establish their permanent residence in a new country and possibly obtain that country’s citizenship. Temporary migrants intend only to stay for a limited periods of time; perhaps until the end of a particular program of study or for the duration of a their work contract or a certain work season. Both types of migrants have a significant effect on the economies and societies of the chosen destination country and the country of origin.</CommonCoreOntologies:definition>
        <rdfs:label>International Migration</rdfs:label>
    </owl:Class>
    


    <!-- http://www.ontologylibrary.mil/OperationalEnvironment/Mid/OEFutureWarfareOntology#InternationalSystem -->

    <owl:Class rdf:about="http://www.ontologylibrary.mil/OperationalEnvironment/Mid/OEFutureWarfareOntology#InternationalSystem">
        <rdfs:subClassOf rdf:resource="http://www.ontologylibrary.mil/OperationalEnvironment/Mid/OEFutureWarfareOntology#Government"/>
        <obo:IAO_0000115>(1)

An international organization is an organization with an international membership, scope, or presence.</obo:IAO_0000115>
        <obo:IAO_0000115>(2)

International organizations serve many diverse functions, including collecting information and monitoring trends...delivering services and aid...and providing forums for bargaining...and settling disputes.... By providing political institutions through which states can work together to achieve common objectives, international organizations can help to foster cooperative behaviour. IGOs also serve useful purposes for individual states, which often use them as instruments of foreign policy to legitimate their actions and to constrain the behaviour of other states.</obo:IAO_0000115>
        <obo:IAO_0000119>(1)

&quot;International Organiztion&quot;, Wikipedia

March 12, 2019

https://en.wikipedia.org/wiki/International_organization</obo:IAO_0000119>
        <obo:IAO_0000119>(2)

Karen Mingst, &quot;International Organization&quot;, Encyclopaedia Britannica

March 12, 2019

https://www.britannica.com/topic/international-organization</obo:IAO_0000119>
        <rdfs:label>International System</rdfs:label>
    </owl:Class>
    


    <!-- http://www.ontologylibrary.mil/OperationalEnvironment/Mid/OEFutureWarfareOntology#InternationalTrade -->

    <owl:Class rdf:about="http://www.ontologylibrary.mil/OperationalEnvironment/Mid/OEFutureWarfareOntology#InternationalTrade">
        <rdfs:subClassOf rdf:resource="http://www.ontologylibrary.mil/OperationalEnvironment/Mid/OEFutureWarfareOntology#EconomicsAndTrade"/>
        <obo:IAO_0000119>Reem Heakal, &quot;What Is International Trade?&quot;, Investopedia

Jan 12, 2018

https://www.investopedia.com/insights/what-is-international-trade/</obo:IAO_0000119>
        <CommonCoreOntologies:definition>International trade is the exchange of goods and services between countries. This type of trade gives rise to a world economy, in which prices, or supply and demand, affect and are affected by global events.

...

Trading globally gives consumers and countries the opportunity to be exposed to goods and services not available in their own countries..... A product that is sold to the global market is an export, and a product that is bought from the global market is an import. Imports and exports are accounted for in a country&apos;s current account in the balance of payments.</CommonCoreOntologies:definition>
        <rdfs:label>International Trade</rdfs:label>
    </owl:Class>
    


    <!-- http://www.ontologylibrary.mil/OperationalEnvironment/Mid/OEFutureWarfareOntology#InternetOfThings -->

    <owl:Class rdf:about="http://www.ontologylibrary.mil/OperationalEnvironment/Mid/OEFutureWarfareOntology#InternetOfThings">
        <rdfs:subClassOf rdf:resource="http://www.ontologylibrary.mil/OperationalEnvironment/Mid/OEFutureWarfareOntology#ArtificialIntelligenceControlledVocabulary"/>
        <obo:IAO_0000115>A computing concept that describes the idea of everyday objects or places in the physical world that are connected to the internet, and are able to identify themselves to other devices. A connected object gathers data (temperature, speed, humidity, etc.) through sensors, and sends it, via the internet, for computer analysis. The object might be a vehicle, a watch, an industrial machine or even a parking space.</obo:IAO_0000115>
        <obo:IAO_0000119>United Nations Educational, Scientific, and Cultural Organization Courier 

March 2018

https://en.unesco.org/courier/2018-3/lexicon-artificial-intelligence</obo:IAO_0000119>
    </owl:Class>
    


    <!-- http://www.ontologylibrary.mil/OperationalEnvironment/Mid/OEFutureWarfareOntology#InterplanetarySpace -->

    <owl:Class rdf:about="http://www.ontologylibrary.mil/OperationalEnvironment/Mid/OEFutureWarfareOntology#InterplanetarySpace">
        <rdfs:subClassOf rdf:resource="http://www.ontologylibrary.mil/OperationalEnvironment/Mid/OEFutureWarfareOntology#SpaceEnvironmentControlledVocabulary"/>
        <obo:IAO_0000115>region of space limited by sphere with radius equal to average distance of the most remote from the Sun planet</obo:IAO_0000115>
        <obo:IAO_0000119>International Organization for Standardization/International Electrotechnical Commission 17851:2016

Space systems -- Space environment simulation for material tests -- General principles and criteria

Publication Date: 2016-09

1st Edition</obo:IAO_0000119>
    </owl:Class>
    


    <!-- http://www.ontologylibrary.mil/OperationalEnvironment/Mid/OEFutureWarfareOntology#InterstateConflict -->

    <owl:Class rdf:about="http://www.ontologylibrary.mil/OperationalEnvironment/Mid/OEFutureWarfareOntology#InterstateConflict">
        <rdfs:subClassOf rdf:resource="http://www.ontologylibrary.mil/OperationalEnvironment/Mid/OEFutureWarfareOntology#SecurityAndViolentConflict"/>
    </owl:Class>
    


    <!-- http://www.ontologylibrary.mil/OperationalEnvironment/Mid/OEFutureWarfareOntology#JudicialSystem -->

    <owl:Class rdf:about="http://www.ontologylibrary.mil/OperationalEnvironment/Mid/OEFutureWarfareOntology#JudicialSystem">
        <rdfs:subClassOf rdf:resource="http://www.ontologylibrary.mil/OperationalEnvironment/Mid/OEFutureWarfareOntology#Government"/>
        <obo:IAO_0000115>The judiciary (also known as the judicial system, judicial branch or court system) is the system of courts that interprets and applies the law in the name of the state. Under the doctrine of the separation of powers, the judiciary generally does not make statutory law (which is the responsibility of the legislature) or enforce law (which is the responsibility of the executive), but rather interprets law and applies it to the facts of each case. However, in some countries the judiciary does make common law, setting precedent for other courts to follow. This branch of the state is often tasked with ensuring equal justice under law. 

In many jurisdictions the judicial branch has the power to change laws through the process of judicial review. Courts with judicial review power may annul the laws and rules of the state when it finds them incompatible with a higher norm, such as primary legislation, the provisions of the constitution or international law. Judges constitute a critical force for interpretation and implementation of a constitution, thus de facto in common law countries creating the body of constitutional law.</obo:IAO_0000115>
        <obo:IAO_0000119>&quot;Judiciary&quot;, Wikipedia

March 12, 2019

https://en.wikipedia.org/wiki/Judiciary</obo:IAO_0000119>
        <rdfs:label>Judicial System</rdfs:label>
    </owl:Class>
    


    <!-- http://www.ontologylibrary.mil/OperationalEnvironment/Mid/OEFutureWarfareOntology#LandUse -->

    <owl:Class rdf:about="http://www.ontologylibrary.mil/OperationalEnvironment/Mid/OEFutureWarfareOntology#LandUse">
        <rdfs:subClassOf rdf:resource="http://www.ontologylibrary.mil/OperationalEnvironment/Mid/OEFutureWarfareOntology#ClimateChangeAndResourceCompetitionControlledVocabulary"/>
        <obo:IAO_0000115>human use or management of land within the relevant boundary

Note 1 to entry: Relevant boundary is the reporting boundary (3.4.8).</obo:IAO_0000115>
        <obo:IAO_0000119>International Organization for Standardization/International Electrotechnical Commission 27000:2018

Technical Committee : ISO/TC 207/SC 7  Greenhouse gas management and related activities

ICS :  13.020.40  Pollution, pollution control and conservation

Greenhouse gases -- Part 1: Specification with guidance at the organization level for quantification and reporting of greenhouse gas emissions and removals 

Publication date : 2018-12

2nd Edition</obo:IAO_0000119>
    </owl:Class>
    


    <!-- http://www.ontologylibrary.mil/OperationalEnvironment/Mid/OEFutureWarfareOntology#Laser -->

    <owl:Class rdf:about="http://www.ontologylibrary.mil/OperationalEnvironment/Mid/OEFutureWarfareOntology#Laser">
        <rdfs:subClassOf rdf:resource="http://www.ontologylibrary.mil/OperationalEnvironment/Mid/OEFutureWarfareOntology#SystemsThatShoot"/>
        <obo:IAO_0000115>Directed energy damages intended target. Targets: Counter Aircraft, UAS, Missiles, Projectiles, Sensors, Swarms. [SOURCE: TRADOC G-2 Potential Game Changers, May 2018]</obo:IAO_0000115>
        <obo:IAO_0000119>Technology Environment of Ground Warfare in 2035-2050

Projections made in 2018 by ARL and TRADOC

[This is a draft outline of a potential document; prepared by Alexander Kott, the US Army Research Laboratory; July 2018]</obo:IAO_0000119>
    </owl:Class>
    


    <!-- http://www.ontologylibrary.mil/OperationalEnvironment/Mid/OEFutureWarfareOntology#Legislature -->

    <owl:Class rdf:about="http://www.ontologylibrary.mil/OperationalEnvironment/Mid/OEFutureWarfareOntology#Legislature">
        <rdfs:subClassOf rdf:resource="http://www.ontologylibrary.mil/OperationalEnvironment/Mid/OEFutureWarfareOntology#Democracy"/>
        <obo:IAO_0000115>(1)

A legislature is a deliberative assembly with the authority to make laws for a political entity such as a country or city. Legislatures form important parts of most governments.

...

Laws enacted by legislatures are known as primary legislation. Legislatures observe and steer governing actions and usually have exclusive authority to amend the budget or budgets involved in the process.

The members of a legislature are called legislators. In a democracy, legislators are most commonly popularly elected, although indirect election and appointment by the executive are also used, particularly for bicameral legislatures featuring an upper chamber.</obo:IAO_0000115>
        <obo:IAO_0000119>(1)

&quot;Legislature&quot;, Wikipedia

March 12, 2019

https://en.wikipedia.org/wiki/Legislature</obo:IAO_0000119>
        <obo:IAO_0000119>(2)

&quot;Legislation&quot;, Wikipedia

March 12, 2019

https://en.wikipedia.org/wiki/Legislation</obo:IAO_0000119>
        <obo:IAO_0000232>&quot;Legislature&quot; is placed under &quot;DemocraticPolitics&quot; rather than constituting a category of it&apos;s own, like the other two branches of government, because the legislature has little importance outside a democracy.</obo:IAO_0000232>
        <CommonCoreOntologies:definition>(2)

Legislation (or &quot;statutory law&quot;) is law which has been promulgated (or &quot;enacted&quot;) by a legislature or other governing body or the process of making it. Before an item of legislation becomes law it may be known as a bill, and may be broadly referred to as &quot;legislation&quot;, while it remains under consideration to distinguish it from other business. Legislation can have many purposes: to regulate, to authorize, to outlaw, to provide (funds), to sanction, to grant, to declare or to restrict.

...

Legislation is usually proposed by a member of the legislature (e.g. a member of Congress or Parliament), or by the executive, where upon it is debated by members of the legislature and is often amended before passage. Most large legislatures enact only a small fraction of the bills proposed in a given session. Whether a given bill will be proposed and is generally a matter of the legislative priorities of government.

Legislation is regarded as one of the three main functions of government. Those who have the formal power to create legislation are known as legislators.</CommonCoreOntologies:definition>
        <rdfs:label>Legislature</rdfs:label>
    </owl:Class>
    


    <!-- http://www.ontologylibrary.mil/OperationalEnvironment/Mid/OEFutureWarfareOntology#LevelOfAssurance -->

    <owl:Class rdf:about="http://www.ontologylibrary.mil/OperationalEnvironment/Mid/OEFutureWarfareOntology#LevelOfAssurance">
        <rdfs:subClassOf rdf:resource="http://www.ontologylibrary.mil/OperationalEnvironment/Mid/OEFutureWarfareOntology#ClimateChangeAndResourceCompetitionControlledVocabulary"/>
        <obo:IAO_0000115>degree of confidence in the GHG statement (3.2.5)</obo:IAO_0000115>
        <obo:IAO_0000119>International Organization for Standardization/International Electrotechnical Commission 27000:2018

Technical Committee : ISO/TC 207/SC 7  Greenhouse gas management and related activities

ICS :  13.020.40  Pollution, pollution control and conservation

Greenhouse gases -- Part 1: Specification with guidance at the organization level for quantification and reporting of greenhouse gas emissions and removals 

Publication date : 2018-12

2nd Edition</obo:IAO_0000119>
    </owl:Class>
    


    <!-- http://www.ontologylibrary.mil/OperationalEnvironment/Mid/OEFutureWarfareOntology#LevelOfRisk -->

    <owl:Class rdf:about="http://www.ontologylibrary.mil/OperationalEnvironment/Mid/OEFutureWarfareOntology#LevelOfRisk">
        <rdfs:subClassOf rdf:resource="http://www.ontologylibrary.mil/OperationalEnvironment/Mid/OEFutureWarfareOntology#CyberSecurityControlledVocabulary"/>
        <obo:IAO_0000115>magnitude of a risk (3.61) expressed in terms of the combination of consequences (3.12) and their likelihood (3.40)</obo:IAO_0000115>
        <obo:IAO_0000119>International Organization for Standardization/International Electrotechnical Commission 27000:2018

Security techniques — Information security management systems — Overview and vocabulary

Publication date : 2018-02

5th Edition</obo:IAO_0000119>
        <obo:IAO_0000119>[SOURCE: ISO Guide 73:2009, 3.6.1.8, modified — “or combination of risks” has been deleted in the definition.]</obo:IAO_0000119>
    </owl:Class>
    


    <!-- http://www.ontologylibrary.mil/OperationalEnvironment/Mid/OEFutureWarfareOntology#LightGasGun -->

    <owl:Class rdf:about="http://www.ontologylibrary.mil/OperationalEnvironment/Mid/OEFutureWarfareOntology#LightGasGun">
        <rdfs:subClassOf rdf:resource="http://www.ontologylibrary.mil/OperationalEnvironment/Mid/OEFutureWarfareOntology#SpaceSystems"/>
        <obo:IAO_0000115>experimental device consisting of a powder gun that compresses a low-density gas to accelerate a projectile up to hypervelocities</obo:IAO_0000115>
        <obo:IAO_0000119>International Organization for Standardization/International Electrotechnical Commission 11227:2012

Space systems — Test procedure to evaluate spacecraft material ejecta upon hypervelocity impact

Publication Date: 2012-09

1st Edition</obo:IAO_0000119>
    </owl:Class>
    


    <!-- http://www.ontologylibrary.mil/OperationalEnvironment/Mid/OEFutureWarfareOntology#Likelihood -->

    <owl:Class rdf:about="http://www.ontologylibrary.mil/OperationalEnvironment/Mid/OEFutureWarfareOntology#Likelihood">
        <rdfs:subClassOf rdf:resource="http://www.ontologylibrary.mil/OperationalEnvironment/Mid/OEFutureWarfareOntology#CyberSecurityControlledVocabulary"/>
        <obo:IAO_0000115>chance of something happening</obo:IAO_0000115>
        <obo:IAO_0000119>International Organization for Standardization/International Electrotechnical Commission 27000:2018

Security techniques — Information security management systems — Overview and vocabulary

Publication date : 2018-02

5th Edition</obo:IAO_0000119>
        <obo:IAO_0000119>[SOURCE: ISO Guide 73:2009, 3.6.1.1, modified — Notes 1 and 2 to entry have been deleted.]</obo:IAO_0000119>
    </owl:Class>
    


    <!-- http://www.ontologylibrary.mil/OperationalEnvironment/Mid/OEFutureWarfareOntology#LogisticsManufacturing -->

    <owl:Class rdf:about="http://www.ontologylibrary.mil/OperationalEnvironment/Mid/OEFutureWarfareOntology#LogisticsManufacturing">
        <rdfs:subClassOf rdf:resource="http://www.ontologylibrary.mil/OperationalEnvironment/Mid/OEFutureWarfareOntology#CombatApplication"/>
        <obo:IAO_0000115>Ability to print materiel, in theater, on an as-needed basis. 

Example: Print a small drone with specific capabilities for a mission in 24 hours.</obo:IAO_0000115>
        <obo:IAO_0000119>Potential Game Changers Infographic

7/11/2018</obo:IAO_0000119>
    </owl:Class>
    


    <!-- http://www.ontologylibrary.mil/OperationalEnvironment/Mid/OEFutureWarfareOntology#LongRangePrecisionFires -->

    <owl:Class rdf:about="http://www.ontologylibrary.mil/OperationalEnvironment/Mid/OEFutureWarfareOntology#LongRangePrecisionFires">
        <rdfs:subClassOf rdf:resource="http://www.ontologylibrary.mil/OperationalEnvironment/Mid/OEFutureWarfareOntology#ElectroDynamicKineticEnergyWeaponsPrecisionWeaponPointDefense"/>
        <rdfs:subClassOf>
            <owl:Restriction>
                <owl:onProperty rdf:resource="http://www.ontologylibrary.mil/OperationalEnvironment/Mid/OEFutureWarfareOntology#hasCategoryOfEffort"/>
                <owl:someValuesFrom rdf:resource="http://www.ontologylibrary.mil/OperationalEnvironment/Mid/OEFutureWarfareOntology#SystemsThatShoot"/>
            </owl:Restriction>
        </rdfs:subClassOf>
        <obo:IAO_0000115>The mission of the Long Range Precision Fires (LRPF) Missile is to attack, neutralize, suppress and destroy targets using missile-delivered indirect precision fires. LRPF provides field artillery units with long-range and deep-strike capability while supporting brigade, division, corps, Army, theater, Joint and Coalition forces and Marine Corps air-to-ground task forces in full, limited or expeditionary operations. The LRPF will replace the Army Tactical Missile System (ATACMS) capability, which is impacted by the age of the ATACMS inventory and the cluster munition policy that removes all M39 and M39A1 ATACMS from the inventory after 2018.</obo:IAO_0000115>
        <obo:IAO_0000119>https://asc.army.mil/web/portfolio-item/long-range-precision-fires-lrpf/</obo:IAO_0000119>
    </owl:Class>
    


    <!-- http://www.ontologylibrary.mil/OperationalEnvironment/Mid/OEFutureWarfareOntology#LongRangedMilitary -->

    <owl:Class rdf:about="http://www.ontologylibrary.mil/OperationalEnvironment/Mid/OEFutureWarfareOntology#LongRangedMilitary">
        <rdfs:subClassOf rdf:resource="http://www.ontologylibrary.mil/OperationalEnvironment/Mid/OEFutureWarfareOntology#SystemsThatShoot"/>
    </owl:Class>
    


    <!-- http://www.ontologylibrary.mil/OperationalEnvironment/Mid/OEFutureWarfareOntology#LowEarthOrbits -->

    <owl:Class rdf:about="http://www.ontologylibrary.mil/OperationalEnvironment/Mid/OEFutureWarfareOntology#LowEarthOrbits">
        <rdfs:subClassOf rdf:resource="http://www.ontologylibrary.mil/OperationalEnvironment/Mid/OEFutureWarfareOntology#SpaceEnvironmentControlledVocabulary"/>
        <obo:IAO_0000115>orbits with altitude up to 2 000 km</obo:IAO_0000115>
        <obo:IAO_0000119>International Organization for Standardization/International Electrotechnical Commission 17851:2016

Space systems -- Space environment simulation for material tests -- General principles and criteria

Publication Date: 2016-09

1st Edition</obo:IAO_0000119>
    </owl:Class>
    


    <!-- http://www.ontologylibrary.mil/OperationalEnvironment/Mid/OEFutureWarfareOntology#LowEnergyNuclearReactions -->

    <owl:Class rdf:about="http://www.ontologylibrary.mil/OperationalEnvironment/Mid/OEFutureWarfareOntology#LowEnergyNuclearReactions">
        <rdfs:subClassOf rdf:resource="http://www.ontologylibrary.mil/OperationalEnvironment/Mid/OEFutureWarfareOntology#SystemsThatShoot"/>
    </owl:Class>
    


    <!-- http://www.ontologylibrary.mil/OperationalEnvironment/Mid/OEFutureWarfareOntology#LowPolarSunSynchronousOrbits -->

    <owl:Class rdf:about="http://www.ontologylibrary.mil/OperationalEnvironment/Mid/OEFutureWarfareOntology#LowPolarSunSynchronousOrbits">
        <rdfs:subClassOf rdf:resource="http://www.ontologylibrary.mil/OperationalEnvironment/Mid/OEFutureWarfareOntology#SpaceEnvironmentControlledVocabulary"/>
        <obo:IAO_0000115>orbits with the altitude of 600 km to 800 km and the inclination of 85° to 97°</obo:IAO_0000115>
        <obo:IAO_0000119>International Organization for Standardization/International Electrotechnical Commission 17851:2016

Space systems -- Space environment simulation for material tests -- General principles and criteria

Publication Date: 2016-09

1st Edition</obo:IAO_0000119>
    </owl:Class>
    


    <!-- http://www.ontologylibrary.mil/OperationalEnvironment/Mid/OEFutureWarfareOntology#MachineLearning -->

    <owl:Class rdf:about="http://www.ontologylibrary.mil/OperationalEnvironment/Mid/OEFutureWarfareOntology#MachineLearning">
        <rdfs:subClassOf rdf:resource="http://www.ontologylibrary.mil/OperationalEnvironment/Mid/OEFutureWarfareOntology#ArtificialIntelligenceControlledVocabulary"/>
        <obo:IAO_0000115>A machine uses an automatic learning programme to solve problems from examples, enabling it to compare and classify data, and even recognize complex shapes. Before the advent of deep learning* in 2010, this type of programme needed to be overseen by humans – each image had to be explicitly designated as containing a human face, a cat’s head, etc., so that the machine could perform the requested recognition operation.</obo:IAO_0000115>
        <obo:IAO_0000119>United Nations Educational, Scientific, and Cultural Organization Courier 

March 2018

https://en.unesco.org/courier/2018-3/lexicon-artificial-intelligence</obo:IAO_0000119>
    </owl:Class>
    


    <!-- http://www.ontologylibrary.mil/OperationalEnvironment/Mid/OEFutureWarfareOntology#MacroeconomicPolicy -->

    <owl:Class rdf:about="http://www.ontologylibrary.mil/OperationalEnvironment/Mid/OEFutureWarfareOntology#MacroeconomicPolicy">
        <rdfs:subClassOf rdf:resource="http://www.ontologylibrary.mil/OperationalEnvironment/Mid/OEFutureWarfareOntology#EconomicsAndTrade"/>
        <obo:IAO_0000119>(1)

&quot;Macroeconomic Policy&quot;, The World Bank

December 22, 2014

http://www.worldbank.org/en/topic/macroeconomics/brief/macroeconomic-policy</obo:IAO_0000119>
        <obo:IAO_0000119>(2)

Robert Dolamore, &quot;The Tools of Macroeconomic Policy--A Short Primer&quot;, Paliament of Australia

March 21, 2019

https://www.aph.gov.au/About_Parliament/Parliamentary_Departments/Parliamentary_Library/pubs/BriefingBook44p/MacroeconomicPolicy</obo:IAO_0000119>
        <CommonCoreOntologies:definition>(1)

Macroeconomic policies include taxes, government spending and borrowing, exchange rate determinants, and monetary and credit rules.</CommonCoreOntologies:definition>
        <CommonCoreOntologies:definition>(2)

Macroeconomic policy aims to provide a stable economic environment that is conducive to fostering strong and sustainable economic growth. The key pillars of macroeconomic policy are fiscal policy, monetary policy and exchange rate policy.</CommonCoreOntologies:definition>
        <rdfs:label>Macroeconomic Policy</rdfs:label>
    </owl:Class>
    


    <!-- http://www.ontologylibrary.mil/OperationalEnvironment/Mid/OEFutureWarfareOntology#ManagementFabric -->

    <owl:Class rdf:about="http://www.ontologylibrary.mil/OperationalEnvironment/Mid/OEFutureWarfareOntology#ManagementFabric">
        <rdfs:subClassOf rdf:resource="http://www.ontologylibrary.mil/OperationalEnvironment/Mid/OEFutureWarfareOntology#BigDataRole"/>
        <obo:IAO_0000115>The Big Data characteristics of volume, velocity, variety, and variability demand a versatile system and software management platform for provisioning, software and package configuration and management, along with resource and performance monitoring and management. Big Data management involves system, data, security, and privacy considerations at scale, while maintaining a high level of data quality and secure accessibility.</obo:IAO_0000115>
        <obo:IAO_0000119>NIST Big Data Interoperability Framework: Volume 6, Reference Architecture

Final Version 1 

NIST Big Data Public Working Group (NBD-PWG) Reference Architecture Subgroup Information Technology Laboratory</obo:IAO_0000119>
    </owl:Class>
    


    <!-- http://www.ontologylibrary.mil/OperationalEnvironment/Mid/OEFutureWarfareOntology#ManagementSystem -->

    <owl:Class rdf:about="http://www.ontologylibrary.mil/OperationalEnvironment/Mid/OEFutureWarfareOntology#ManagementSystem">
        <rdfs:subClassOf rdf:resource="http://www.ontologylibrary.mil/OperationalEnvironment/Mid/OEFutureWarfareOntology#CyberSecurityControlledVocabulary"/>
        <obo:IAO_0000115>set of interrelated or interacting elements of an organization (3.50) to establish policies (3.53) and objectives (3.49) and processes (3.54) to achieve those objectives

Note 1 to entry: A management system can address a single discipline or several disciplines.

Note 2 to entry: The system elements include the organization’s structure, roles and responsibilities, planning and operation.

Note 3 to entry: The scope of a management system may include the whole of the organization, specific and identified functions of the organization, specific and identified sections of the organization, or one or more functions across a group of organizations.</obo:IAO_0000115>
        <obo:IAO_0000119>International Organization for Standardization/International Electrotechnical Commission 27000:2018

Security techniques — Information security management systems — Overview and vocabulary

Publication date : 2018-02

5th Edition</obo:IAO_0000119>
    </owl:Class>
    


    <!-- http://www.ontologylibrary.mil/OperationalEnvironment/Mid/OEFutureWarfareOntology#Manufacturing -->

    <owl:Class rdf:about="http://www.ontologylibrary.mil/OperationalEnvironment/Mid/OEFutureWarfareOntology#Manufacturing">
        <rdfs:subClassOf rdf:resource="http://www.ontologylibrary.mil/OperationalEnvironment/Mid/OEFutureWarfareOntology#EconomicActivity"/>
        <obo:IAO_0000119>&quot;Manufacturing&quot;, Wikipedia

March 14, 2019

https://en.wikipedia.org/wiki/Manufacturing</obo:IAO_0000119>
        <obo:IAO_0000119>(2)

Chelsea Levinson, &quot;Definition of the Manufacturing Industry&quot;, BIZFLUENT.COM

March 14, 2019

https://bizfluent.com/facts-6853113-definition-manufacturing-industry.html</obo:IAO_0000119>
        <obo:IAO_0000119>(3)

EconomyWatch, &quot;Manufacturing Industry&quot;, Economywatch.com

March 14, 2019

http://www.economywatch.com/world-industries/manufacturing</obo:IAO_0000119>
        <CommonCoreOntologies:definition>(1)

The term [&quot;manufacturing&quot;] is most commonly applied to industrial design, in which raw materials are transformed into finished goods on a large scale. Such finished goods may be sold to other manufacturers for the production of other, more complex products, such as aircraft, household appliances, furniture, sports equipment or automobiles, or sold to wholesalers, who in turn sell them to retailers, who then sell them to end users and consumers.

Manufacturing engineering or manufacturing process are the steps through which raw materials are transformed into a final product. The manufacturing process begins with the product design, and materials specification from which the product is made. These materials are then modified through manufacturing processes to become the required part.</CommonCoreOntologies:definition>
        <CommonCoreOntologies:definition>(2)

Manufacturers create physical goods. How these goods are created varies depending on the specific company and industry. However, most manufacturers use machinery and industrial equipment to produce goods for public consumption. The manufacturing process creates value, meaning companies can charge a premium for what they create.

...

Today’s advancement of computer technology allows manufacturers to do more with less time. Now, thousands of items can be manufactured within the space of minutes. Computer technology can be used to assemble, test and track production. Each year, technology continues to make manufacturing increasingly efficient, faster and more cost-effective. However, automation also eliminates many manufacturing jobs, leaving skilled employees without work.</CommonCoreOntologies:definition>
        <CommonCoreOntologies:definition>(3)

Manufacturing industries are broadly categorized into engineering industries, construction industries, electronics industries, chemical industries, energy industries, textile industries, food and beverage industries, metalworking industries, plastic industries, transport and telecommunication industries.</CommonCoreOntologies:definition>
        <rdfs:label>Manufacturing</rdfs:label>
    </owl:Class>
    


    <!-- http://www.ontologylibrary.mil/OperationalEnvironment/Mid/OEFutureWarfareOntology#MaximumContinuousRating -->

    <owl:Class rdf:about="http://www.ontologylibrary.mil/OperationalEnvironment/Mid/OEFutureWarfareOntology#MaximumContinuousRating">
        <rdfs:subClassOf rdf:resource="http://www.ontologylibrary.mil/OperationalEnvironment/Mid/OEFutureWarfareOntology#GasEnergyGeneration"/>
        <obo:IAO_0000115>International Organization for Standardization/International ISO 19859:2016

Technical Committee : ISO/TC 192  Gas turbines

ICS :  29.160.99  Other standards related to rotating machinery 27.040  Gas and steam turbines. Steam engines

Gas turbine applications -- Requirements for power generation

Publication date : 2016-08

1st Edition</obo:IAO_0000115>
        <obo:IAO_0000115>maximum continuous electrical output for the power generation package with the gas turbine package (3.8) operating at its maximum reference turbine control temperature [exhaust temperature, TIT (3.27) or RIT (3.20)] and its inlet guide vanes (where fitted) fully open</obo:IAO_0000115>
    </owl:Class>
    


    <!-- http://www.ontologylibrary.mil/OperationalEnvironment/Mid/OEFutureWarfareOntology#Measure -->

    <owl:Class rdf:about="http://www.ontologylibrary.mil/OperationalEnvironment/Mid/OEFutureWarfareOntology#Measure">
        <rdfs:subClassOf rdf:resource="http://www.ontologylibrary.mil/OperationalEnvironment/Mid/OEFutureWarfareOntology#CyberSecurityControlledVocabulary"/>
        <obo:IAO_0000115>variable to which a value is assigned as the result of measurement (3.43)</obo:IAO_0000115>
        <obo:IAO_0000119>International Organization for Standardization/International Electrotechnical Commission 27000:2018

Security techniques — Information security management systems — Overview and vocabulary

Publication date : 2018-02

5th Edition</obo:IAO_0000119>
    </owl:Class>
    


    <!-- http://www.ontologylibrary.mil/OperationalEnvironment/Mid/OEFutureWarfareOntology#Measurement -->

    <owl:Class rdf:about="http://www.ontologylibrary.mil/OperationalEnvironment/Mid/OEFutureWarfareOntology#Measurement">
        <rdfs:subClassOf rdf:resource="http://www.ontologylibrary.mil/OperationalEnvironment/Mid/OEFutureWarfareOntology#CyberSecurityControlledVocabulary"/>
        <obo:IAO_0000115>process (3.54) to determine a value</obo:IAO_0000115>
        <obo:IAO_0000119>International Organization for Standardization/International Electrotechnical Commission 27000:2018

Security techniques — Information security management systems — Overview and vocabulary

Publication date : 2018-02

5th Edition</obo:IAO_0000119>
    </owl:Class>
    


    <!-- http://www.ontologylibrary.mil/OperationalEnvironment/Mid/OEFutureWarfareOntology#MeasurementFunction -->

    <owl:Class rdf:about="http://www.ontologylibrary.mil/OperationalEnvironment/Mid/OEFutureWarfareOntology#MeasurementFunction">
        <rdfs:subClassOf rdf:resource="http://www.ontologylibrary.mil/OperationalEnvironment/Mid/OEFutureWarfareOntology#CyberSecurityControlledVocabulary"/>
        <obo:IAO_0000115>algorithm or calculation performed to combine two or more base measures (3.8)</obo:IAO_0000115>
        <obo:IAO_0000119>International Organization for Standardization/International Electrotechnical Commission 27000:2018

Security techniques — Information security management systems — Overview and vocabulary

Publication date : 2018-02

5th Edition</obo:IAO_0000119>
        <obo:IAO_0000119>[SOURCE: ISO/IEC/IEEE 15939:2017, 3.20]</obo:IAO_0000119>
    </owl:Class>
    


    <!-- http://www.ontologylibrary.mil/OperationalEnvironment/Mid/OEFutureWarfareOntology#MeasurementMethod -->

    <owl:Class rdf:about="http://www.ontologylibrary.mil/OperationalEnvironment/Mid/OEFutureWarfareOntology#MeasurementMethod">
        <rdfs:subClassOf rdf:resource="http://www.ontologylibrary.mil/OperationalEnvironment/Mid/OEFutureWarfareOntology#CyberSecurityControlledVocabulary"/>
        <obo:IAO_0000115>logical sequence of operations, described generically, used in quantifying an attribute with respect to a specified scale

Note 1 to entry: The type of measurement method depends on the nature of the operations used to quantify an attribute (3.4). Two types can be distinguished:

— subjective: quantification involving human judgment; and
— objective: quantification based on numerical rules.</obo:IAO_0000115>
        <obo:IAO_0000119>International Organization for Standardization/International Electrotechnical Commission 27000:2018

Security techniques — Information security management systems — Overview and vocabulary

Publication date : 2018-02

5th Edition</obo:IAO_0000119>
    </owl:Class>
    


    <!-- http://www.ontologylibrary.mil/OperationalEnvironment/Mid/OEFutureWarfareOntology#MechanismsOfSpaceEnvironmentEffectsOfMaterials -->

    <owl:Class rdf:about="http://www.ontologylibrary.mil/OperationalEnvironment/Mid/OEFutureWarfareOntology#MechanismsOfSpaceEnvironmentEffectsOfMaterials">
        <rdfs:subClassOf rdf:resource="http://www.ontologylibrary.mil/OperationalEnvironment/Mid/OEFutureWarfareOntology#SpaceEnvironmentControlledVocabulary"/>
        <obo:IAO_0000115>totality of physical and chemical phenomena causing the changes in material properties under the influence of primary and secondary space environment factors
— evaporation, sputtering, surface erosion
— surface contamination
— charge accumulation on the surface (surface charging)
— charge accumulation in the volume of dielectrics (bulk charging)
— formation of structural radiation defects</obo:IAO_0000115>
        <obo:IAO_0000119>International Organization for Standardization/International Electrotechnical Commission 17851:2016

Space systems -- Space environment simulation for material tests -- General principles and criteria

Publication Date: 2016-09

1st Edition</obo:IAO_0000119>
    </owl:Class>
    


    <!-- http://www.ontologylibrary.mil/OperationalEnvironment/Mid/OEFutureWarfareOntology#MedicalAdvancesInSyntheticBiology -->

    <owl:Class rdf:about="http://www.ontologylibrary.mil/OperationalEnvironment/Mid/OEFutureWarfareOntology#MedicalAdvancesInSyntheticBiology">
        <rdfs:subClassOf rdf:resource="http://www.ontologylibrary.mil/OperationalEnvironment/Mid/OEFutureWarfareOntology#SystemsThatSoldier"/>
        <obo:IAO_0000115>Synthetic Biology - Medical Advances: Enhance soldier survivability. [SOURCE: TRADOC G-2 Potential Game Changers, May 2018]</obo:IAO_0000115>
        <obo:IAO_0000119>Technology Environment of Ground Warfare in 2035-2050

Projections made in 2018 by ARL and TRADOC

[This is a draft outline of a potential document; prepared by Alexander Kott, the US Army Research Laboratory; July 2018]</obo:IAO_0000119>
    </owl:Class>
    


    <!-- http://www.ontologylibrary.mil/OperationalEnvironment/Mid/OEFutureWarfareOntology#Megacity -->

    <owl:Class rdf:about="http://www.ontologylibrary.mil/OperationalEnvironment/Mid/OEFutureWarfareOntology#Megacity">
        <rdfs:subClassOf rdf:resource="http://www.ontologylibrary.mil/OperationalEnvironment/Mid/OEFutureWarfareOntology#Urbanization"/>
        <obo:IAO_0000119>(1)

&quot;Megacity&quot;, Wikipedia

March 26, 2019

https://en.wikipedia.org/wiki/Megacity</obo:IAO_0000119>
        <obo:IAO_0000119>(2)

&quot;What Is a Megacity?&quot;, worldatlas.com

June 28, 2018

https://www.worldatlas.com/articles/what-is-a-megacity.html</obo:IAO_0000119>
        <CommonCoreOntologies:definition>(1)

A megacity is a very large city metropolitan area, typically with a population of more than 10 million people.

...

A megacity can be a single metropolitan area or two or more metropolitan areas that converge. The terms conurbation, metropolis, and metroplex are also applied to the latter. The term metacity has been used to describe metropolitan conurbations containing over 20 million people.</CommonCoreOntologies:definition>
        <CommonCoreOntologies:definition>(2)

Due to their high populations, megacities face several challenges. These challenges revolve around slums, crime, energy and material resources, homelessness, and traffic congestion. Slums are settlement areas which are characterized by improper housing facilities and poor sanitation. They have been caused by the rise in population and massive local and international immigration. Individuals who live in slums seldom receive access to proper education, healthcare, and housing. Slums are generally found in cities in developing countries. The rise of criminal activities due to discontentment of city residents is another limitation megacities face. A lack of fulfillment of basic needs such as food, water, and shelter can increase crime rates.

...

Megacities also face the challenge of managing limited energy and material resources such as electricity and water consumption, waste generation, transport energy, and steel production. There are many children and families who live on the streets in many megacities in spite of they many attempts by government and non-governmental organizations to end homelessness. The final challenge is traffic congestion which refers to transport delays that occur on the roads as a result of increase of use.</CommonCoreOntologies:definition>
        <rdfs:label>Megacity</rdfs:label>
    </owl:Class>
    


    <!-- http://www.ontologylibrary.mil/OperationalEnvironment/Mid/OEFutureWarfareOntology#Metadata -->

    <owl:Class rdf:about="http://www.ontologylibrary.mil/OperationalEnvironment/Mid/OEFutureWarfareOntology#Metadata">
        <rdfs:subClassOf rdf:resource="http://www.ontologylibrary.mil/OperationalEnvironment/Mid/OEFutureWarfareOntology#BigDataControlledVocabulary"/>
        <obo:IAO_0000115>data (3.1.5) about data or data elements, possibly including their data descriptions, and data about data ownership, access paths, access rights and data volatility</obo:IAO_0000115>
        <obo:IAO_0000119>Information technology — Big data — Overview and vocabulary

https://www.iso.org/jtc1</obo:IAO_0000119>
        <obo:IAO_0000119>[SOURCE: ISO/IEC 2382:2015, 17.06.05]</obo:IAO_0000119>
    </owl:Class>
    


    <!-- http://www.ontologylibrary.mil/OperationalEnvironment/Mid/OEFutureWarfareOntology#Meteoriod -->

    <owl:Class rdf:about="http://www.ontologylibrary.mil/OperationalEnvironment/Mid/OEFutureWarfareOntology#Meteoriod">
        <rdfs:subClassOf rdf:resource="http://www.ontologylibrary.mil/OperationalEnvironment/Mid/OEFutureWarfareOntology#SpaceSystems"/>
        <obo:IAO_0000115>particles of natural origin, resulting from the disintegration and fragmentation of comets and asteroids, which orbit the sun</obo:IAO_0000115>
        <obo:IAO_0000119>International Organization for Standardization/International Electrotechnical Commission 11227:2012

Space systems — Test procedure to evaluate spacecraft material ejecta upon hypervelocity impact

Publication Date: 2012-09

1st Edition</obo:IAO_0000119>
    </owl:Class>
    


    <!-- http://www.ontologylibrary.mil/OperationalEnvironment/Mid/OEFutureWarfareOntology#MidEarthOrbits -->

    <owl:Class rdf:about="http://www.ontologylibrary.mil/OperationalEnvironment/Mid/OEFutureWarfareOntology#MidEarthOrbits">
        <rdfs:subClassOf rdf:resource="http://www.ontologylibrary.mil/OperationalEnvironment/Mid/OEFutureWarfareOntology#SpaceEnvironmentControlledVocabulary"/>
        <obo:IAO_0000115>intermediate circular orbits with an altitude h = 2 000 km to 36 000 km:
— GPS orbit h = 20 200 km, inclination (i) = 55°
— GLONASS orbit h = 19 100 km, i = 64,8°
— GALILEO orbit h = 23 222 km, i = 56°
— BeiDou orbit h = 21 528 km, I = 55°</obo:IAO_0000115>
        <obo:IAO_0000119>International Organization for Standardization/International Electrotechnical Commission 17851:2016

Space systems -- Space environment simulation for material tests -- General principles and criteria

Publication Date: 2016-09

1st Edition</obo:IAO_0000119>
    </owl:Class>
    


    <!-- http://www.ontologylibrary.mil/OperationalEnvironment/Mid/OEFutureWarfareOntology#Migration -->

    <owl:Class rdf:about="http://www.ontologylibrary.mil/OperationalEnvironment/Mid/OEFutureWarfareOntology#Migration">
        <rdfs:subClassOf rdf:resource="http://www.ontologylibrary.mil/OperationalEnvironment/Mid/OEFutureWarfareOntology#Demographics"/>
        <obo:IAO_0000119>&quot;Migration&quot;, United Nations

March 25, 2019

http://www.un.org/en/sections/issues-depth/migration/index.html</obo:IAO_0000119>
        <CommonCoreOntologies:definition>Some people move in search of labour or economic opportunities, to join family, or to study. Others move to escape conflict, persecution, terrorism, or human rights violations. Still others move in response to the adverse effects of climate change, natural disasters, or other environmental factors.</CommonCoreOntologies:definition>
        <rdfs:label>Migration</rdfs:label>
    </owl:Class>
    


    <!-- http://www.ontologylibrary.mil/OperationalEnvironment/Mid/OEFutureWarfareOntology#MilleniumDevelopmentGoals -->

    <owl:Class rdf:about="http://www.ontologylibrary.mil/OperationalEnvironment/Mid/OEFutureWarfareOntology#MilleniumDevelopmentGoals">
        <rdfs:subClassOf rdf:resource="http://www.ontologylibrary.mil/OperationalEnvironment/Mid/OEFutureWarfareOntology#EconomicDevelopment"/>
        <obo:IAO_0000119>&quot;Millenium Development Goals&quot;, Wikipedia

March 19, 2019

https://en.wikipedia.org/wiki/Millennium_Development_Goals</obo:IAO_0000119>
        <CommonCoreOntologies:definition>To eradicate extreme poverty and hunger
    To achieve universal primary education
    To promote gender equality and empower women
    To reduce child mortality
    To improve maternal health
    To combat HIV/AIDS, malaria, and other diseases
    To ensure environmental sustainability
    To develop a global partnership for development</CommonCoreOntologies:definition>
        <rdfs:label>Millenium Development Goals</rdfs:label>
    </owl:Class>
    


    <!-- http://www.ontologylibrary.mil/OperationalEnvironment/Mid/OEFutureWarfareOntology#MindUploading -->

    <owl:Class rdf:about="http://www.ontologylibrary.mil/OperationalEnvironment/Mid/OEFutureWarfareOntology#MindUploading">
        <rdfs:subClassOf rdf:resource="http://www.ontologylibrary.mil/OperationalEnvironment/Mid/OEFutureWarfareOntology#ArtificialIntelligenceControlledVocabulary"/>
        <obo:IAO_0000115>According to transhumanists*, our sensations, thoughts and emotions can all be summed up as neural connections. Mind uploading is the transhumanist idea that the “contents” of the human brain can be reduced to a set of information that could be translated into binary computer code, and thus uploaded into a computer.</obo:IAO_0000115>
        <obo:IAO_0000119>United Nations Educational, Scientific, and Cultural Organization Courier 

March 2018

https://en.unesco.org/courier/2018-3/lexicon-artificial-intelligence</obo:IAO_0000119>
    </owl:Class>
    


    <!-- http://www.ontologylibrary.mil/OperationalEnvironment/Mid/OEFutureWarfareOntology#MinimumContinuousRating -->

    <owl:Class rdf:about="http://www.ontologylibrary.mil/OperationalEnvironment/Mid/OEFutureWarfareOntology#MinimumContinuousRating">
        <rdfs:subClassOf rdf:resource="http://www.ontologylibrary.mil/OperationalEnvironment/Mid/OEFutureWarfareOntology#GasEnergyGeneration"/>
        <obo:IAO_0000115>minimum continuous electrical output for the power generation package (3.14) without meeting emission limits and environmental constraints</obo:IAO_0000115>
        <obo:IAO_0000119>International Organization for Standardization/International ISO 19859:2016

Technical Committee : ISO/TC 192  Gas turbines

ICS :  29.160.99  Other standards related to rotating machinery 27.040  Gas and steam turbines. Steam engines

Gas turbine applications -- Requirements for power generation

Publication date : 2016-08

1st Edition</obo:IAO_0000119>
    </owl:Class>
    


    <!-- http://www.ontologylibrary.mil/OperationalEnvironment/Mid/OEFutureWarfareOntology#MinimumEnvironmentalLoad -->

    <owl:Class rdf:about="http://www.ontologylibrary.mil/OperationalEnvironment/Mid/OEFutureWarfareOntology#MinimumEnvironmentalLoad">
        <rdfs:subClassOf rdf:resource="http://www.ontologylibrary.mil/OperationalEnvironment/Mid/OEFutureWarfareOntology#GasEnergyGeneration"/>
        <obo:IAO_0000115>minimum continuous electrical output for the power generation package (3.14) while meeting all emission limits and environmental constraints</obo:IAO_0000115>
        <obo:IAO_0000119>International Organization for Standardization/International ISO 19859:2016

Technical Committee : ISO/TC 192  Gas turbines

ICS :  29.160.99  Other standards related to rotating machinery 27.040  Gas and steam turbines. Steam engines

Gas turbine applications -- Requirements for power generation

Publication date : 2016-08

1st Edition</obo:IAO_0000119>
    </owl:Class>
    


    <!-- http://www.ontologylibrary.mil/OperationalEnvironment/Mid/OEFutureWarfareOntology#Missiles -->

    <owl:Class rdf:about="http://www.ontologylibrary.mil/OperationalEnvironment/Mid/OEFutureWarfareOntology#Missiles">
        <rdfs:subClassOf rdf:resource="http://www.ontologylibrary.mil/OperationalEnvironment/Mid/OEFutureWarfareOntology#SystemsThatShoot"/>
        <obo:IAO_0000115>Developed for greater range and improved accuracy using inertial guidance. [SOURCE: TRADOC G-2 Potential Game Changers, May 2018]</obo:IAO_0000115>
        <obo:IAO_0000119>Technology Environment of Ground Warfare in 2035-2050

Projections made in 2018 by ARL and TRADOC

[This is a draft outline of a potential document; prepared by Alexander Kott, the US Army Research Laboratory; July 2018]</obo:IAO_0000119>
    </owl:Class>
    


    <!-- http://www.ontologylibrary.mil/OperationalEnvironment/Mid/OEFutureWarfareOntology#MonetaryPolicy -->

    <owl:Class rdf:about="http://www.ontologylibrary.mil/OperationalEnvironment/Mid/OEFutureWarfareOntology#MonetaryPolicy">
        <rdfs:subClassOf rdf:resource="http://www.ontologylibrary.mil/OperationalEnvironment/Mid/OEFutureWarfareOntology#MacroeconomicPolicy"/>
        <obo:IAO_0000119>&quot;Monetary Policy&quot;, Wikipedia

March 21, 2019

https://en.wikipedia.org/wiki/Monetary_policy</obo:IAO_0000119>
        <CommonCoreOntologies:definition>Monetary policy is the process by which the monetary authority of a country, typically the central bank or currency board, controls either the cost of very short-term borrowing or the money supply, often targeting an inflation rate or interest rate to ensure price stability and general trust in the currency.
Further goals of a monetary policy are usually to contribute to the stability of gross domestic product, to achieve and maintain low unemployment, and to maintain predictable exchange rates with other currencies.</CommonCoreOntologies:definition>
        <rdfs:label>Monetary Policy</rdfs:label>
    </owl:Class>
    


    <!-- http://www.ontologylibrary.mil/OperationalEnvironment/Mid/OEFutureWarfareOntology#Monitoring -->

    <owl:Class rdf:about="http://www.ontologylibrary.mil/OperationalEnvironment/Mid/OEFutureWarfareOntology#Monitoring">
        <rdfs:subClassOf rdf:resource="http://www.ontologylibrary.mil/OperationalEnvironment/Mid/OEFutureWarfareOntology#CyberSecurityControlledVocabulary"/>
        <obo:IAO_0000115>determining the status of a system, a process (3.54) or an activity

Note 1 to entry: To determine the status, there may be a need to check, supervise or critically observe.</obo:IAO_0000115>
        <obo:IAO_0000119>International Organization for Standardization/International Electrotechnical Commission 27000:2018

Security techniques — Information security management systems — Overview and vocabulary

Publication date : 2018-02

5th Edition</obo:IAO_0000119>
    </owl:Class>
    


    <!-- http://www.ontologylibrary.mil/OperationalEnvironment/Mid/OEFutureWarfareOntology#MultiFuelBasedHybridElectricEngines -->

    <owl:Class rdf:about="http://www.ontologylibrary.mil/OperationalEnvironment/Mid/OEFutureWarfareOntology#MultiFuelBasedHybridElectricEngines">
        <rdfs:subClassOf rdf:resource="http://www.ontologylibrary.mil/OperationalEnvironment/Mid/OEFutureWarfareOntology#SystemsThatMove"/>
    </owl:Class>
    


    <!-- http://www.ontologylibrary.mil/OperationalEnvironment/Mid/OEFutureWarfareOntology#MultifunctionalBatteries -->

    <owl:Class rdf:about="http://www.ontologylibrary.mil/OperationalEnvironment/Mid/OEFutureWarfareOntology#MultifunctionalBatteries">
        <rdfs:subClassOf rdf:resource="http://www.ontologylibrary.mil/OperationalEnvironment/Mid/OEFutureWarfareOntology#SystemsThatMove"/>
    </owl:Class>
    


    <!-- http://www.ontologylibrary.mil/OperationalEnvironment/Mid/OEFutureWarfareOntology#MultipartySystem -->

    <owl:Class rdf:about="http://www.ontologylibrary.mil/OperationalEnvironment/Mid/OEFutureWarfareOntology#MultipartySystem">
        <rdfs:subClassOf rdf:resource="http://www.ontologylibrary.mil/OperationalEnvironment/Mid/OEFutureWarfareOntology#PoliticalPartySystem"/>
        <obo:IAO_0000115>A multi-party system is a system in which multiple political parties across the political spectrum run for national election, and all have the capacity to gain control of government offices, separately or in coalition. Apart from one-party-dominant and two-party systems, multi-party systems tend to be more common in parliamentary systems than presidential systems and far more common in countries that use proportional representation compared to countries that use first-past-the-post elections.

First-past-the-post requires concentrated areas of support for large representation in the legislature whereas proportional representation better reflects the range of a population&apos;s views. Proportional systems may have multi-member districts with more than one representative elected from a given district to the same legislative body, and thus a greater number of viable parties.</obo:IAO_0000115>
        <obo:IAO_0000119>&quot;Multi-party System&quot;, Wikipedia

March 12, 2019

https://en.wikipedia.org/wiki/Multi-party_system</obo:IAO_0000119>
        <rdfs:label>Multiparty System</rdfs:label>
    </owl:Class>
    


    <!-- http://www.ontologylibrary.mil/OperationalEnvironment/Mid/OEFutureWarfareOntology#NanoMaterials -->

    <owl:Class rdf:about="http://www.ontologylibrary.mil/OperationalEnvironment/Mid/OEFutureWarfareOntology#NanoMaterials">
        <rdfs:subClassOf rdf:resource="http://www.ontologylibrary.mil/OperationalEnvironment/Mid/OEFutureWarfareOntology#SystemsThatShoot"/>
        <obo:IAO_0000115>Miniaturized power sources; reduce bulk, increase yield. [SOURCE: TRADOC G-2 Potential Game Changers, May 2018]</obo:IAO_0000115>
        <obo:IAO_0000119>Technology Environment of Ground Warfare in 2035-2050

Projections made in 2018 by ARL and TRADOC

[This is a draft outline of a potential document; prepared by Alexander Kott, the US Army Research Laboratory; July 2018]</obo:IAO_0000119>
    </owl:Class>
    


    <!-- http://www.ontologylibrary.mil/OperationalEnvironment/Mid/OEFutureWarfareOntology#Nationalism -->

    <owl:Class rdf:about="http://www.ontologylibrary.mil/OperationalEnvironment/Mid/OEFutureWarfareOntology#Nationalism">
        <rdfs:subClassOf rdf:resource="http://www.ontologylibrary.mil/OperationalEnvironment/Mid/OEFutureWarfareOntology#Identity"/>
    </owl:Class>
    


    <!-- http://www.ontologylibrary.mil/OperationalEnvironment/Mid/OEFutureWarfareOntology#Near-EarthSpace -->

    <owl:Class rdf:about="http://www.ontologylibrary.mil/OperationalEnvironment/Mid/OEFutureWarfareOntology#Near-EarthSpace">
        <rdfs:subClassOf rdf:resource="http://www.ontologylibrary.mil/OperationalEnvironment/Mid/OEFutureWarfareOntology#SpaceEnvironmentControlledVocabulary"/>
        <obo:IAO_0000115>region of space limited by sphere with radius equal to the average distance from the Moon to the Earth (380 000 km)</obo:IAO_0000115>
        <obo:IAO_0000119>International Organization for Standardization/International Electrotechnical Commission 17851:2016

Space systems -- Space environment simulation for material tests -- General principles and criteria

Publication Date: 2016-09

1st Edition</obo:IAO_0000119>
    </owl:Class>
    


    <!-- http://www.ontologylibrary.mil/OperationalEnvironment/Mid/OEFutureWarfareOntology#NeoConnectionism -->

    <owl:Class rdf:about="http://www.ontologylibrary.mil/OperationalEnvironment/Mid/OEFutureWarfareOntology#NeoConnectionism">
        <rdfs:subClassOf rdf:resource="http://www.ontologylibrary.mil/OperationalEnvironment/Mid/OEFutureWarfareOntology#ArtificialIntelligenceControlledVocabulary"/>
        <obo:IAO_0000115>A theory arising from the fields of cognitive science and neuroscience, neo-connectionism proposes to develop computer models that aim to simulate learning by formal neural networks*, the organization and functioning of which have been designed by analogy with physiological neural systems.</obo:IAO_0000115>
        <obo:IAO_0000119>United Nations Educational, Scientific, and Cultural Organization Courier 

March 2018

https://en.unesco.org/courier/2018-3/lexicon-artificial-intelligence</obo:IAO_0000119>
    </owl:Class>
    


    <!-- http://www.ontologylibrary.mil/OperationalEnvironment/Mid/OEFutureWarfareOntology#Non-tariffBarriers -->

    <owl:Class rdf:about="http://www.ontologylibrary.mil/OperationalEnvironment/Mid/OEFutureWarfareOntology#Non-tariffBarriers">
        <rdfs:subClassOf rdf:resource="http://www.ontologylibrary.mil/OperationalEnvironment/Mid/OEFutureWarfareOntology#InternationalTrade"/>
        <obo:IAO_0000119>&quot;Non-Tariff Barriers to Trade&quot;, Non-Tariff Barriers:  Reporting, Monitoring and Eliminating Mechanism

March 21, 2019

https://www.tradebarriers.org/ntb/non_tariff_barriers</obo:IAO_0000119>
        <CommonCoreOntologies:definition>Non-Tariff Barriers to trade can arise from:
        Import bans
        General or product-specific quotas
        Complex/discriminatory Rules of Origin
        Quality conditions imposed by the importing country on the exporting countries
        Unjustified Sanitary and Phyto-sanitary conditions
        Unreasonable/unjustified packaging, labelling, product standards
        Complex regulatory environment
        Determination of eligibility of an exporting country by the importing country
        Determination of eligibility of an exporting establishment (firm, company) by the importing country.
        Additional trade documents like Certificate of Origin, Certificate of Authenticity etc
        Occupational safety and health regulation
        Employment law
        Import licenses
        State subsidies, procurement, trading, state ownership
        Export subsidies
        Fixation of a minimum import price
        Product classification
        Quota shares
        Multiplicity and Controls of Foreign exchange market
        Inadequate infrastructure
        &quot;Buy national&quot; policy
        Over-valued currency
        Restrictive licenses
        Seasonal import regimes
        Corrupt and/or lengthy customs procedures</CommonCoreOntologies:definition>
        <rdfs:label>Non-tariff Barriers</rdfs:label>
    </owl:Class>
    


    <!-- http://www.ontologylibrary.mil/OperationalEnvironment/Mid/OEFutureWarfareOntology#NonAnthropogenicBioGenicGreenhouseGasEmission -->

    <owl:Class rdf:about="http://www.ontologylibrary.mil/OperationalEnvironment/Mid/OEFutureWarfareOntology#NonAnthropogenicBioGenicGreenhouseGasEmission">
        <rdfs:subClassOf rdf:resource="http://www.ontologylibrary.mil/OperationalEnvironment/Mid/OEFutureWarfareOntology#ClimateChangeAndResourceCompetitionControlledVocabulary"/>
        <obo:IAO_0000115>GHG emission (3.1.5) from biogenic material caused by natural disasters (e.g. wildfire or infestation by insects) or natural evolution (e.g. growth, decomposition)</obo:IAO_0000115>
        <obo:IAO_0000119>International Organization for Standardization/International Electrotechnical Commission 27000:2018

Technical Committee : ISO/TC 207/SC 7  Greenhouse gas management and related activities

ICS :  13.020.40  Pollution, pollution control and conservation

Greenhouse gases -- Part 1: Specification with guidance at the organization level for quantification and reporting of greenhouse gas emissions and removals 

Publication date : 2018-12

2nd Edition</obo:IAO_0000119>
    </owl:Class>
    


    <!-- http://www.ontologylibrary.mil/OperationalEnvironment/Mid/OEFutureWarfareOntology#NonRelationalDatabase -->

    <owl:Class rdf:about="http://www.ontologylibrary.mil/OperationalEnvironment/Mid/OEFutureWarfareOntology#NonRelationalDatabase">
        <rdfs:subClassOf rdf:resource="http://www.ontologylibrary.mil/OperationalEnvironment/Mid/OEFutureWarfareOntology#BigDataControlledVocabulary"/>
        <obo:IAO_0000115>In horizontally scaled systems, the data is distributed across the nodes of a cluster, while having a single logical structure. The new non-relational model database paradigms are typically referred to as NoSQL (Not Only SQL or No SQL) systems. The problem with identifying big data storage paradigms as NoSQL is, first, it describes the storage of data with respect to a set theory-based language for query and retrieval of data, and second, there is a growing capability in the application of the query languages similar to SQL against the new non-relational data repositories. While NoSQL is in such common usage that it will continue to refer to the new data models beyond the relational model, the term refers to databases that do not follow a relational model. Examples of non-relational database models include the column, sparse table, key-value, key-document, and graphical models.</obo:IAO_0000115>
        <obo:IAO_0000115>database (3.1.7) that does not follow a relational data model

Note 1 to entry: NoSQL, which is typically translated as “non SQL” or “not only SQL”, is the term in common usage to refer to databases that do not conform to a relational model.</obo:IAO_0000115>
        <obo:IAO_0000119>Information technology — Big data — Overview and vocabulary

https://www.iso.org/jtc1</obo:IAO_0000119>
    </owl:Class>
    


    <!-- http://www.ontologylibrary.mil/OperationalEnvironment/Mid/OEFutureWarfareOntology#NonRelationalModel -->

    <owl:Class rdf:about="http://www.ontologylibrary.mil/OperationalEnvironment/Mid/OEFutureWarfareOntology#NonRelationalModel">
        <rdfs:subClassOf rdf:resource="http://www.ontologylibrary.mil/OperationalEnvironment/Mid/OEFutureWarfareOntology#BigDataControlledVocabulary"/>
        <obo:IAO_0000115>logical data (3.1.5) model that does not follow a relational model for the storage and manipulation of data</obo:IAO_0000115>
        <obo:IAO_0000119>Information technology — Big data — Overview and vocabulary

https://www.iso.org/jtc1</obo:IAO_0000119>
    </owl:Class>
    


    <!-- http://www.ontologylibrary.mil/OperationalEnvironment/Mid/OEFutureWarfareOntology#NonRepudiation -->

    <owl:Class rdf:about="http://www.ontologylibrary.mil/OperationalEnvironment/Mid/OEFutureWarfareOntology#NonRepudiation">
        <rdfs:subClassOf rdf:resource="http://www.ontologylibrary.mil/OperationalEnvironment/Mid/OEFutureWarfareOntology#CyberSecurityControlledVocabulary"/>
        <obo:IAO_0000115>ability to prove the occurrence of a claimed event (3.21) or action and its originating entities</obo:IAO_0000115>
        <obo:IAO_0000119>International Organization for Standardization/International Electrotechnical Commission 27000:2018

Security techniques — Information security management systems — Overview and vocabulary

Publication date : 2018-02

5th Edition</obo:IAO_0000119>
    </owl:Class>
    


    <!-- http://www.ontologylibrary.mil/OperationalEnvironment/Mid/OEFutureWarfareOntology#Nonconformity -->

    <owl:Class rdf:about="http://www.ontologylibrary.mil/OperationalEnvironment/Mid/OEFutureWarfareOntology#Nonconformity">
        <rdfs:subClassOf rdf:resource="http://www.ontologylibrary.mil/OperationalEnvironment/Mid/OEFutureWarfareOntology#CyberSecurityControlledVocabulary"/>
        <obo:IAO_0000115>non-fulfilment of a requirement (3.56)</obo:IAO_0000115>
        <obo:IAO_0000119>International Organization for Standardization/International Electrotechnical Commission 27000:2018

Security techniques — Information security management systems — Overview and vocabulary

Publication date : 2018-02

5th Edition</obo:IAO_0000119>
    </owl:Class>
    


    <!-- http://www.ontologylibrary.mil/OperationalEnvironment/Mid/OEFutureWarfareOntology#Normalization -->

    <owl:Class rdf:about="http://www.ontologylibrary.mil/OperationalEnvironment/Mid/OEFutureWarfareOntology#Normalization">
        <rdfs:subClassOf rdf:resource="http://www.ontologylibrary.mil/OperationalEnvironment/Mid/OEFutureWarfareOntology#PowerGenerationAndStorageControlledVocabulary"/>
        <obo:IAO_0000115>modification of data to account for changes to enable comparison of energy performance (3.4.3) under equivalent conditions</obo:IAO_0000115>
        <obo:IAO_0000119>International Organization for Standardization/International ISO 50001:2018

Technical Committee : ISO/TC 301  Energy management and energy savings

ICS :  27.015  Energy efficiency. Energy conservation in general 03.100.70 Management systems

Energy management systems -- Requirements with guidance for use

Publication date : 2018-08

2nd Edition</obo:IAO_0000119>
    </owl:Class>
    


    <!-- http://www.ontologylibrary.mil/OperationalEnvironment/Mid/OEFutureWarfareOntology#Objective -->

    <owl:Class rdf:about="http://www.ontologylibrary.mil/OperationalEnvironment/Mid/OEFutureWarfareOntology#Objective">
        <rdfs:subClassOf rdf:resource="http://www.ontologylibrary.mil/OperationalEnvironment/Mid/OEFutureWarfareOntology#CyberSecurityControlledVocabulary"/>
        <obo:IAO_0000115>result to be achieved

Note 1 to entry: An objective can be strategic, tactical, or operational.

Note 2 to entry: Objectives can relate to different disciplines (such as financial, health and safety, and environmental goals) and can apply at different levels [such as strategic, organization-wide, project, product and process (3.54)].

Note 3 to entry: An objective can be expressed in other ways, e.g. as an intended outcome, a purpose, an operational criterion, as an information security objective or by the use of other words with similar meaning (e.g. aim, goal, or target).

Note 4 to entry: In the context of information security management systems, information security objectives are set by the organization, consistent with the information security policy, to achieve specific results.</obo:IAO_0000115>
        <obo:IAO_0000119>International Organization for Standardization/International Electrotechnical Commission 27000:2018

Security techniques — Information security management systems — Overview and vocabulary

Publication date : 2018-02

5th Edition</obo:IAO_0000119>
    </owl:Class>
    


    <!-- http://www.ontologylibrary.mil/OperationalEnvironment/Mid/OEFutureWarfareOntology#Obscurants -->

    <owl:Class rdf:about="http://www.ontologylibrary.mil/OperationalEnvironment/Mid/OEFutureWarfareOntology#Obscurants">
        <rdfs:subClassOf rdf:resource="http://www.ontologylibrary.mil/OperationalEnvironment/Mid/OEFutureWarfareOntology#SystemsThatProtect"/>
        <obo:IAO_0000115>Obscurants/Thermal Paint - Confuse sensors. [SOURCE: TRADOC G-2 Potential Game Changers, May 2018]</obo:IAO_0000115>
        <obo:IAO_0000119>Technology Environment of Ground Warfare in 2035-2050

Projections made in 2018 by ARL and TRADOC

[This is a draft outline of a potential document; prepared by Alexander Kott, the US Army Research Laboratory; July 2018]</obo:IAO_0000119>
    </owl:Class>
    


    <!-- http://www.ontologylibrary.mil/OperationalEnvironment/Mid/OEFutureWarfareOntology#One-partyRule -->

    <owl:Class rdf:about="http://www.ontologylibrary.mil/OperationalEnvironment/Mid/OEFutureWarfareOntology#One-partyRule">
        <rdfs:subClassOf rdf:resource="http://www.ontologylibrary.mil/OperationalEnvironment/Mid/OEFutureWarfareOntology#Authoritariansim"/>
        <obo:IAO_0000115>A one-party state, single-party state, one-party system, or single-party system is a type of state in which one political party has the right to form the government, usually based on the existing constitution. All other parties are either outlawed or allowed to take only a limited and controlled participation in elections. Sometimes the term de facto one-party state is used to describe a dominant-party system...[whose] existing practices or balance of political power effectively prevent the opposition from winning the elections.</obo:IAO_0000115>
        <obo:IAO_0000119>&quot;One-party State&quot;, Wikipedia

March 12, 2019

https://en.wikipedia.org/wiki/One-party_state</obo:IAO_0000119>
        <rdfs:label>One-party Rule</rdfs:label>
    </owl:Class>
    


    <!-- http://www.ontologylibrary.mil/OperationalEnvironment/Mid/OEFutureWarfareOntology#OperationalRelevance -->

    <owl:Class rdf:about="http://www.ontologylibrary.mil/OperationalEnvironment/Mid/OEFutureWarfareOntology#OperationalRelevance">
        <rdfs:subClassOf rdf:resource="http://www.ontologylibrary.mil/OperationalEnvironment/Mid/OEFutureWarfareOntology#FaultLineMethodology"/>
        <obo:IAO_0000119>Fault Lines Methodology Infographic</obo:IAO_0000119>
    </owl:Class>
    


    <!-- http://www.ontologylibrary.mil/OperationalEnvironment/Mid/OEFutureWarfareOntology#OptimizingHumanPerformance -->

    <owl:Class rdf:about="http://www.ontologylibrary.mil/OperationalEnvironment/Mid/OEFutureWarfareOntology#OptimizingHumanPerformance">
        <rdfs:subClassOf rdf:resource="http://www.ontologylibrary.mil/OperationalEnvironment/Mid/OEFutureWarfareOntology#SystemsThatSoldier"/>
        <rdfs:subClassOf>
            <owl:Restriction>
                <owl:onProperty rdf:resource="http://www.ontologylibrary.mil/OperationalEnvironment/Mid/OEFutureWarfareOntology#hasCombatApplication"/>
                <owl:someValuesFrom rdf:resource="http://www.ontologylibrary.mil/OperationalEnvironment/Mid/OEFutureWarfareOntology#SoldierCognitiveDomainEnhancement"/>
            </owl:Restriction>
        </rdfs:subClassOf>
        <rdfs:subClassOf>
            <owl:Restriction>
                <owl:onProperty rdf:resource="http://www.ontologylibrary.mil/OperationalEnvironment/Mid/OEFutureWarfareOntology#hasCombatApplication"/>
                <owl:someValuesFrom rdf:resource="http://www.ontologylibrary.mil/OperationalEnvironment/Mid/OEFutureWarfareOntology#SoldierPhysicalDomainEnhancement"/>
            </owl:Restriction>
        </rdfs:subClassOf>
        <rdfs:subClassOf>
            <owl:Restriction>
                <owl:onProperty rdf:resource="http://www.ontologylibrary.mil/OperationalEnvironment/Mid/OEFutureWarfareOntology#hasCombatApplication"/>
                <owl:someValuesFrom rdf:resource="http://www.ontologylibrary.mil/OperationalEnvironment/Mid/OEFutureWarfareOntology#SoldierPsychologicalDomainEnhancement"/>
            </owl:Restriction>
        </rdfs:subClassOf>
    </owl:Class>
    


    <!-- http://www.ontologylibrary.mil/OperationalEnvironment/Mid/OEFutureWarfareOntology#Organization -->

    <owl:Class rdf:about="http://www.ontologylibrary.mil/OperationalEnvironment/Mid/OEFutureWarfareOntology#Organization">
        <rdfs:subClassOf rdf:resource="http://www.ontologylibrary.mil/OperationalEnvironment/Mid/OEFutureWarfareOntology#CyberSecurityControlledVocabulary"/>
        <obo:IAO_0000115>person or group of people that has its own functions with responsibilities, authorities and relationships to achieve its objectives (3.49)

Note 1 to entry: The concept of organization includes but is not limited to sole-trader, company, corporation, firm, enterprise, authority, partnership, charity or institution, or part or combination thereof, whether incorporated or not, public or private.</obo:IAO_0000115>
        <obo:IAO_0000119>International Organization for Standardization/International Electrotechnical Commission 27000:2018

Security techniques — Information security management systems — Overview and vocabulary

Publication date : 2018-02

5th Edition</obo:IAO_0000119>
    </owl:Class>
    


    <!-- http://www.ontologylibrary.mil/OperationalEnvironment/Mid/OEFutureWarfareOntology#OrganizationalBoundary -->

    <owl:Class rdf:about="http://www.ontologylibrary.mil/OperationalEnvironment/Mid/OEFutureWarfareOntology#OrganizationalBoundary">
        <rdfs:subClassOf rdf:resource="http://www.ontologylibrary.mil/OperationalEnvironment/Mid/OEFutureWarfareOntology#ClimateChangeAndResourceCompetitionControlledVocabulary"/>
        <obo:IAO_0000115>grouping of activities or facilities in which an organization (3.4.2) exercises operational or financial control or has an equity share</obo:IAO_0000115>
        <obo:IAO_0000119>International Organization for Standardization/International Electrotechnical Commission 27000:2018

Technical Committee : ISO/TC 207/SC 7  Greenhouse gas management and related activities

ICS :  13.020.40  Pollution, pollution control and conservation

Greenhouse gases -- Part 1: Specification with guidance at the organization level for quantification and reporting of greenhouse gas emissions and removals 

Publication date : 2018-12

2nd Edition</obo:IAO_0000119>
    </owl:Class>
    


    <!-- http://www.ontologylibrary.mil/OperationalEnvironment/Mid/OEFutureWarfareOntology#Outsource -->

    <owl:Class rdf:about="http://www.ontologylibrary.mil/OperationalEnvironment/Mid/OEFutureWarfareOntology#Outsource">
        <rdfs:subClassOf rdf:resource="http://www.ontologylibrary.mil/OperationalEnvironment/Mid/OEFutureWarfareOntology#CyberSecurityControlledVocabulary"/>
        <obo:IAO_0000115>make an arrangement where an external organization (3.50) performs part of an organization’s function or process (3.54)

Note 1 to entry: An external organization is outside the scope of the management system (3.41), although the outsourced function or process is within the scope.</obo:IAO_0000115>
        <obo:IAO_0000119>International Organization for Standardization/International Electrotechnical Commission 27000:2018

Security techniques — Information security management systems — Overview and vocabulary

Publication date : 2018-02

5th Edition</obo:IAO_0000119>
    </owl:Class>
    


    <!-- http://www.ontologylibrary.mil/OperationalEnvironment/Mid/OEFutureWarfareOntology#Parallel -->

    <owl:Class rdf:about="http://www.ontologylibrary.mil/OperationalEnvironment/Mid/OEFutureWarfareOntology#Parallel">
        <rdfs:subClassOf rdf:resource="http://www.ontologylibrary.mil/OperationalEnvironment/Mid/OEFutureWarfareOntology#BigDataControlledVocabulary"/>
        <obo:IAO_0000115>pertaining to a process in which all events occur within the same interval of time, each one handled by a separate but similar functional unit

Note 1 to entry: Example: The parallel transmission of the bits of a computer word along the lines of an internal bus.</obo:IAO_0000115>
        <obo:IAO_0000119>Information technology — Big data — Overview and vocabulary

https://www.iso.org/jtc1</obo:IAO_0000119>
        <obo:IAO_0000119>[SOURCE: ISO/IEC 2382:2015, 03.02.01]</obo:IAO_0000119>
    </owl:Class>
    


    <!-- http://www.ontologylibrary.mil/OperationalEnvironment/Mid/OEFutureWarfareOntology#PartiallyStructuredData -->

    <owl:Class rdf:about="http://www.ontologylibrary.mil/OperationalEnvironment/Mid/OEFutureWarfareOntology#PartiallyStructuredData">
        <rdfs:subClassOf rdf:resource="http://www.ontologylibrary.mil/OperationalEnvironment/Mid/OEFutureWarfareOntology#BigDataControlledVocabulary"/>
        <obo:IAO_0000115>data (3.1.5) that has some organization

Note 1 to entry:  partially structured data is often referred to as semi-structured data by industry 

Note 2 to entry: examples of partially structured data are records with free text fields in addition to more structured fields.  Such data is frequently represented in computer interpretable/parsible formats such as XML or JSON.</obo:IAO_0000115>
        <obo:IAO_0000119>Information technology — Big data — Overview and vocabulary

https://www.iso.org/jtc1</obo:IAO_0000119>
    </owl:Class>
    


    <!-- http://www.ontologylibrary.mil/OperationalEnvironment/Mid/OEFutureWarfareOntology#Patronage -->

    <owl:Class rdf:about="http://www.ontologylibrary.mil/OperationalEnvironment/Mid/OEFutureWarfareOntology#Patronage">
        <rdfs:subClassOf rdf:resource="http://www.ontologylibrary.mil/OperationalEnvironment/Mid/OEFutureWarfareOntology#InformalInstitutions"/>
        <obo:IAO_0000115>In some countries the term [&quot;patronage&quot;] is used to describe political patronage, which is the use of state resources to reward individuals for their electoral support. Some patronage systems are legal, [such as a head of government&apos;s appointment powers]; in many cases, these appointments go to people who have supported the political party of the Prime Minister. As well, the term may refer to a type of corruption or favoritism in which a party in power rewards groups, families, ethnicities for their electoral support using illegal gifts or fraudulently awarded appointments or government contracts.</obo:IAO_0000115>
        <obo:IAO_0000119>&quot;Patronage&quot;, Wikipedia

March 12, 2019

https://en.wikipedia.org/wiki/Patronage</obo:IAO_0000119>
        <rdfs:label>Patronage</rdfs:label>
    </owl:Class>
    


    <!-- http://www.ontologylibrary.mil/OperationalEnvironment/Mid/OEFutureWarfareOntology#Pensions -->

    <owl:Class rdf:about="http://www.ontologylibrary.mil/OperationalEnvironment/Mid/OEFutureWarfareOntology#Pensions">
        <rdfs:subClassOf rdf:resource="http://www.ontologylibrary.mil/OperationalEnvironment/Mid/OEFutureWarfareOntology#WelfareState"/>
        <obo:IAO_0000119>&quot;Pension&quot;, Wikipedia

March 23, 2019

https://en.wikipedia.org/wiki/Pension</obo:IAO_0000119>
        <CommonCoreOntologies:definition>A pension...is a fund into which a sum of money is added during an employee&apos;s employment years, and from which payments are drawn to support the person&apos;s retirement from work in the form of periodic payments. A pension may be a &quot;defined benefit plan&quot; where a fixed sum is paid regularly to a person, or a &quot;defined contribution plan&quot; under which a fixed sum is invested and then becomes available at retirement age. Pensions should not be confused with severance pay; the former is usually paid in regular installments for life after retirement, while the latter is typically paid as a fixed amount after involuntary termination of employment prior to retirement.

The terms &quot;retirement plan&quot; and &quot;superannuation&quot; tend to refer to a pension granted upon retirement of the individual. Retirement plans may be set up by employers, insurance companies, the government or other institutions such as employer associations or trade unions.</CommonCoreOntologies:definition>
        <rdfs:label>Pensions</rdfs:label>
    </owl:Class>
    


    <!-- http://www.ontologylibrary.mil/OperationalEnvironment/Mid/OEFutureWarfareOntology#Perforation -->

    <owl:Class rdf:about="http://www.ontologylibrary.mil/OperationalEnvironment/Mid/OEFutureWarfareOntology#Perforation">
        <rdfs:subClassOf rdf:resource="http://www.ontologylibrary.mil/OperationalEnvironment/Mid/OEFutureWarfareOntology#SpaceSystems"/>
        <obo:IAO_0000115>hole created by an impact on a thin material in which there is no formation of a crater</obo:IAO_0000115>
        <obo:IAO_0000119>International Organization for Standardization/International Electrotechnical Commission 11227:2012

Space systems — Test procedure to evaluate spacecraft material ejecta upon hypervelocity impact

Publication Date: 2012-09

1st Edition</obo:IAO_0000119>
    </owl:Class>
    


    <!-- http://www.ontologylibrary.mil/OperationalEnvironment/Mid/OEFutureWarfareOntology#Performance -->

    <owl:Class rdf:about="http://www.ontologylibrary.mil/OperationalEnvironment/Mid/OEFutureWarfareOntology#Performance">
        <rdfs:subClassOf rdf:resource="http://www.ontologylibrary.mil/OperationalEnvironment/Mid/OEFutureWarfareOntology#CyberSecurityControlledVocabulary"/>
        <obo:IAO_0000115>measurable result

Note 1 to entry: Performance can relate either to quantitative or qualitative findings.

Note 2 to entry: Performance can relate to the management of activities, processes (3.54), products (including services), systems or organizations (3.50).</obo:IAO_0000115>
        <obo:IAO_0000119>International Organization for Standardization/International Electrotechnical Commission 27000:2018

Security techniques — Information security management systems — Overview and vocabulary

Publication date : 2018-02

5th Edition</obo:IAO_0000119>
    </owl:Class>
    


    <!-- http://www.ontologylibrary.mil/OperationalEnvironment/Mid/OEFutureWarfareOntology#PlasmaGun -->

    <owl:Class rdf:about="http://www.ontologylibrary.mil/OperationalEnvironment/Mid/OEFutureWarfareOntology#PlasmaGun">
        <rdfs:subClassOf rdf:resource="http://www.ontologylibrary.mil/OperationalEnvironment/Mid/OEFutureWarfareOntology#SpaceSystems"/>
        <obo:IAO_0000115>experimental device that produces an accelerated plasma flow, which is compressed in a coil and then drags a projectile up to hypervelocities</obo:IAO_0000115>
        <obo:IAO_0000119>International Organization for Standardization/International Electrotechnical Commission 11227:2012

Space systems — Test procedure to evaluate spacecraft material ejecta upon hypervelocity impact

Publication Date: 2012-09

1st Edition</obo:IAO_0000119>
    </owl:Class>
    


    <!-- http://www.ontologylibrary.mil/OperationalEnvironment/Mid/OEFutureWarfareOntology#PointAirDefenseSystems -->

    <owl:Class rdf:about="http://www.ontologylibrary.mil/OperationalEnvironment/Mid/OEFutureWarfareOntology#PointAirDefenseSystems">
        <rdfs:subClassOf rdf:resource="http://www.ontologylibrary.mil/OperationalEnvironment/Mid/OEFutureWarfareOntology#SystemsThatProtect"/>
        <obo:IAO_0000115>Point air defense systems defend against PGM. [SOURCE: TRADOC G-2 Potential Game Changers, May 2018]</obo:IAO_0000115>
        <obo:IAO_0000119>Technology Environment of Ground Warfare in 2035-2050

Projections made in 2018 by ARL and TRADOC

[This is a draft outline of a potential document; prepared by Alexander Kott, the US Army Research Laboratory; July 2018]</obo:IAO_0000119>
    </owl:Class>
    


    <!-- http://www.ontologylibrary.mil/OperationalEnvironment/Mid/OEFutureWarfareOntology#Policy -->

    <owl:Class rdf:about="http://www.ontologylibrary.mil/OperationalEnvironment/Mid/OEFutureWarfareOntology#Policy">
        <rdfs:subClassOf rdf:resource="http://www.ontologylibrary.mil/OperationalEnvironment/Mid/OEFutureWarfareOntology#CyberSecurityControlledVocabulary"/>
        <obo:IAO_0000115>intentions and direction of an organization (3.50), as formally expressed by its top management (3.75)</obo:IAO_0000115>
        <obo:IAO_0000119>International Organization for Standardization/International Electrotechnical Commission 27000:2018

Security techniques — Information security management systems — Overview and vocabulary

Publication date : 2018-02

5th Edition</obo:IAO_0000119>
    </owl:Class>
    


    <!-- http://www.ontologylibrary.mil/OperationalEnvironment/Mid/OEFutureWarfareOntology#PoliticalPartySystem -->

    <owl:Class rdf:about="http://www.ontologylibrary.mil/OperationalEnvironment/Mid/OEFutureWarfareOntology#PoliticalPartySystem">
        <rdfs:subClassOf rdf:resource="http://www.ontologylibrary.mil/OperationalEnvironment/Mid/OEFutureWarfareOntology#Democracy"/>
        <obo:IAO_0000115>A political party is an organized group of people, often with common views, who come together to contest elections and hold power in the government. The party agrees on some proposed policies and programmes, with a view to promoting the collective good or furthering their supporters&apos; interests.</obo:IAO_0000115>
        <obo:IAO_0000119>&quot;Political Party&quot;, Wikipedia

March 12, 2019

https://en.wikipedia.org/wiki/Political_party</obo:IAO_0000119>
        <rdfs:label>Political Party System</rdfs:label>
    </owl:Class>
    


    <!-- http://www.ontologylibrary.mil/OperationalEnvironment/Mid/OEFutureWarfareOntology#PovertyReduction -->

    <owl:Class rdf:about="http://www.ontologylibrary.mil/OperationalEnvironment/Mid/OEFutureWarfareOntology#PovertyReduction">
        <rdfs:subClassOf rdf:resource="http://www.ontologylibrary.mil/OperationalEnvironment/Mid/OEFutureWarfareOntology#WelfareState"/>
        <obo:IAO_0000119>&quot;Poverty Reduction&quot;, Wikipedia

March 22, 2019

https://en.wikipedia.org/wiki/Poverty_reduction</obo:IAO_0000119>
        <CommonCoreOntologies:definition>Aid in its simplest form is a basic income grant, a form of social security periodically providing citizens with money. 

...

Aid could also be rewarded based on doing certain requirements. Conditional Cash Transfers, widely credited as a successful anti-poverty program, is based on actions such as enrolling children in school or receiving vaccinations.

...

Welfare states have an effect on poverty reduction. Currently modern, expansive welfare states that ensure economic opportunity, independence and security in a near universal manner are still the exclusive domain of the developed nations.

...

Following his recommendations, international organizations...are working to help eradicate poverty worldwide with intervention in the areas of housing, food, education, basic health, agricultural inputs, safe drinking water, transportation and communications. 

...

There are several poverty targeting methods through which poor communities are identified and tracked for poverty reduction programmes. For instance, one common method of poverty targeting is &apos;means testing&apos; that uses a certain income or expenditure threshold for an individual or the a household to be considered as poor and eligible for support.</CommonCoreOntologies:definition>
        <rdfs:label>Poverty Reduction</rdfs:label>
    </owl:Class>
    


    <!-- http://www.ontologylibrary.mil/OperationalEnvironment/Mid/OEFutureWarfareOntology#PowerDistributionViaWireless -->

    <owl:Class rdf:about="http://www.ontologylibrary.mil/OperationalEnvironment/Mid/OEFutureWarfareOntology#PowerDistributionViaWireless">
        <rdfs:subClassOf rdf:resource="http://www.ontologylibrary.mil/OperationalEnvironment/Mid/OEFutureWarfareOntology#PowerSystems"/>
        <obo:IAO_0000115>Power and charging over the air (long distances). [SOURCE: TRADOC G-2 Potential Game Changers, May 2018]</obo:IAO_0000115>
        <obo:IAO_0000119>Technology Environment of Ground Warfare in 2035-2050

Projections made in 2018 by ARL and TRADOC

[This is a draft outline of a potential document; prepared by Alexander Kott, the US Army Research Laboratory; July 2018]</obo:IAO_0000119>
    </owl:Class>
    


    <!-- http://www.ontologylibrary.mil/OperationalEnvironment/Mid/OEFutureWarfareOntology#PowerGenerationAndStorageControlledVocabulary -->

    <owl:Class rdf:about="http://www.ontologylibrary.mil/OperationalEnvironment/Mid/OEFutureWarfareOntology#PowerGenerationAndStorageControlledVocabulary">
        <rdfs:subClassOf rdf:resource="http://www.ontologylibrary.mil/OperationalEnvironment/Mid/OEFutureWarfareOntology#ControlledVocabulary"/>
    </owl:Class>
    


    <!-- http://www.ontologylibrary.mil/OperationalEnvironment/Mid/OEFutureWarfareOntology#PowerPlant -->

    <owl:Class rdf:about="http://www.ontologylibrary.mil/OperationalEnvironment/Mid/OEFutureWarfareOntology#PowerPlant">
        <rdfs:subClassOf rdf:resource="http://www.ontologylibrary.mil/OperationalEnvironment/Mid/OEFutureWarfareOntology#GasEnergyGeneration"/>
        <obo:IAO_0000115>all main equipment and auxiliary equipment employed in producing electrical power at a site (3.23) and may include one or more power generation packages (3.14)</obo:IAO_0000115>
        <obo:IAO_0000119>International Organization for Standardization/International ISO 19859:2016

Technical Committee : ISO/TC 192  Gas turbines

ICS :  29.160.99  Other standards related to rotating machinery 27.040  Gas and steam turbines. Steam engines

Gas turbine applications -- Requirements for power generation

Publication date : 2016-08

1st Edition</obo:IAO_0000119>
    </owl:Class>
    


    <!-- http://www.ontologylibrary.mil/OperationalEnvironment/Mid/OEFutureWarfareOntology#PowerRating -->

    <owl:Class rdf:about="http://www.ontologylibrary.mil/OperationalEnvironment/Mid/OEFutureWarfareOntology#PowerRating">
        <rdfs:subClassOf rdf:resource="http://www.ontologylibrary.mil/OperationalEnvironment/Mid/OEFutureWarfareOntology#GasEnergyGeneration"/>
        <obo:IAO_0000115>net electrical power developed by the gas turbine when it is operated at a defined reference turbine control temperature [exhaust temperature, TIT (3.27) or RIT (3.20)] and standard reference conditions</obo:IAO_0000115>
        <obo:IAO_0000119>International Organization for Standardization/International ISO 19859:2016

Technical Committee : ISO/TC 192  Gas turbines

ICS :  29.160.99  Other standards related to rotating machinery 27.040  Gas and steam turbines. Steam engines

Gas turbine applications -- Requirements for power generation

Publication date : 2016-08

1st Edition</obo:IAO_0000119>
    </owl:Class>
    


    <!-- http://www.ontologylibrary.mil/OperationalEnvironment/Mid/OEFutureWarfareOntology#PowerStorageAndGenerationTrend -->

    <owl:Class rdf:about="http://www.ontologylibrary.mil/OperationalEnvironment/Mid/OEFutureWarfareOntology#PowerStorageAndGenerationTrend">
        <rdfs:subClassOf rdf:resource="http://www.ontologylibrary.mil/OperationalEnvironment/Mid/OEFutureWarfareOntology#Trend"/>
        <obo:IAO_0000115>Although more human beings stress available resources, population growth has also compounded the rate of innovation and technology development.  Human creativity is now clearly the most transformative force in the world, both enhancing human life, but also upending it, and – at times – precipitating catastrophic, disruptive events.  Information technology will continue to improve exponentially, and most of the developed world already is instrumented in some way.  Nearly every person on Earth has access to a connected, mobile device.  Advanced material capabilities have, and will continue to extend the trend of reduced size, weight, and power requirements, as nanomaterials, metamaterials, and bespoke structures allow multifunctional assemblies, vastly improving overall systems integration, reliability, and performance.  Advanced materials also foster increases in battery power and performance, allowing large amounts of power to be stored across a distributed grid, and miniaturized storage powers mobile robotics and vehicles of all types</obo:IAO_0000115>
        <obo:IAO_0000119>The Operational Environment and the Changing Character of Future Warfare</obo:IAO_0000119>
    </owl:Class>
    


    <!-- http://www.ontologylibrary.mil/OperationalEnvironment/Mid/OEFutureWarfareOntology#PowerSystems -->

    <owl:Class rdf:about="http://www.ontologylibrary.mil/OperationalEnvironment/Mid/OEFutureWarfareOntology#PowerSystems">
        <rdfs:subClassOf rdf:resource="http://www.ontologylibrary.mil/OperationalEnvironment/Mid/OEFutureWarfareOntology#SystemsThatMove"/>
    </owl:Class>
    


    <!-- http://www.ontologylibrary.mil/OperationalEnvironment/Mid/OEFutureWarfareOntology#President -->

    <owl:Class rdf:about="http://www.ontologylibrary.mil/OperationalEnvironment/Mid/OEFutureWarfareOntology#President">
        <rdfs:subClassOf rdf:resource="http://www.ontologylibrary.mil/OperationalEnvironment/Mid/OEFutureWarfareOntology#Executive"/>
        <obo:IAO_0000115>In almost all states with a presidential system of government, the president exercises the functions of head of state and head of government, i.e. the president directs the executive branch of government.</obo:IAO_0000115>
        <obo:IAO_0000119>&quot;President&quot;, Wikipedia

March 12, 2019

https://en.wikipedia.org/wiki/President#Presidential_systems</obo:IAO_0000119>
        <rdfs:label>President</rdfs:label>
    </owl:Class>
    


    <!-- http://www.ontologylibrary.mil/OperationalEnvironment/Mid/OEFutureWarfareOntology#PrimaryData -->

    <owl:Class rdf:about="http://www.ontologylibrary.mil/OperationalEnvironment/Mid/OEFutureWarfareOntology#PrimaryData">
        <rdfs:subClassOf rdf:resource="http://www.ontologylibrary.mil/OperationalEnvironment/Mid/OEFutureWarfareOntology#ClimateChangeAndResourceCompetitionControlledVocabulary"/>
        <obo:IAO_0000115>quantified value of a process or an activity obtained from a direct measurement or a calculation based on direct measurements

Note 1 to entry: Primary data can include greenhouse gas emission factors or greenhouse gas removal factors and/or greenhouse gas activity data</obo:IAO_0000115>
        <obo:IAO_0000119>International Organization for Standardization/International Electrotechnical Commission 27000:2018

Technical Committee : ISO/TC 207/SC 7  Greenhouse gas management and related activities

ICS :  13.020.40  Pollution, pollution control and conservation

Greenhouse gases -- Part 1: Specification with guidance at the organization level for quantification and reporting of greenhouse gas emissions and removals 

Publication date : 2018-12

2nd Edition</obo:IAO_0000119>
    </owl:Class>
    


    <!-- http://www.ontologylibrary.mil/OperationalEnvironment/Mid/OEFutureWarfareOntology#PrimaryFactors -->

    <owl:Class rdf:about="http://www.ontologylibrary.mil/OperationalEnvironment/Mid/OEFutureWarfareOntology#PrimaryFactors">
        <rdfs:subClassOf rdf:resource="http://www.ontologylibrary.mil/OperationalEnvironment/Mid/OEFutureWarfareOntology#SpaceEnvironmentControlledVocabulary"/>
        <obo:IAO_0000115>factors existing in space and affecting spacecraft (i.e. space environment components)
— vacuum
— neutral particles of the Earth’s upper atmosphere (including atomic oxygen)
— plasma (cold plasma with particle energy up to 10 eV, hot plasma with particle energy of 10 eV to 105 eV)
— solar electromagnetic radiation: X-rays, vacuum ultraviolet radiation, ultraviolet radiation, visible light, infrared radiation
— charged particles of high energy: Earth’s radiation belts, solar energetic particles, galactic cosmic rays
— meteoroids (micrometeoroids), ejecta (for Moon), lunar dust
— space debris (microparticles)</obo:IAO_0000115>
        <obo:IAO_0000119>International Organization for Standardization/International Electrotechnical Commission 17851:2016

Space systems -- Space environment simulation for material tests -- General principles and criteria

Publication Date: 2016-09

1st Edition</obo:IAO_0000119>
    </owl:Class>
    


    <!-- http://www.ontologylibrary.mil/OperationalEnvironment/Mid/OEFutureWarfareOntology#PrimeMinister -->

    <owl:Class rdf:about="http://www.ontologylibrary.mil/OperationalEnvironment/Mid/OEFutureWarfareOntology#PrimeMinister">
        <rdfs:subClassOf rdf:resource="http://www.ontologylibrary.mil/OperationalEnvironment/Mid/OEFutureWarfareOntology#Executive"/>
        <obo:IAO_0000115>A prime minister is the head of a cabinet and the leader of the ministers in the executive branch of government, often in a parliamentary or semi-presidential system.

...

In parliamentary systems fashioned after the Westminster system, the prime minister is the presiding and actual head of government and head of the executive branch.

...

In many systems, the prime minister selects and may dismiss other members of the cabinet, and allocates posts to members within the government. In most systems, the prime minister is the presiding member and chairman of the cabinet. 

The prime minister is often, but not always, a member of the Legislature or the Lower House thereof and is expected with other ministers to ensure the passage of bills through the legislature.</obo:IAO_0000115>
        <obo:IAO_0000119>&quot;Prime Minister&quot;, Wikipedia

March 12, 2019

https://en.wikipedia.org/wiki/Prime_minister</obo:IAO_0000119>
        <rdfs:label>Prime Mininster</rdfs:label>
    </owl:Class>
    


    <!-- http://www.ontologylibrary.mil/OperationalEnvironment/Mid/OEFutureWarfareOntology#Process -->

    <owl:Class rdf:about="http://www.ontologylibrary.mil/OperationalEnvironment/Mid/OEFutureWarfareOntology#Process">
        <rdfs:subClassOf rdf:resource="http://www.ontologylibrary.mil/OperationalEnvironment/Mid/OEFutureWarfareOntology#CyberSecurityControlledVocabulary"/>
        <obo:IAO_0000115>set of interrelated or interacting activities which transforms inputs into outputs</obo:IAO_0000115>
        <obo:IAO_0000119>International Organization for Standardization/International Electrotechnical Commission 27000:2018

Security techniques — Information security management systems — Overview and vocabulary

Publication date : 2018-02

5th Edition</obo:IAO_0000119>
    </owl:Class>
    


    <!-- http://www.ontologylibrary.mil/OperationalEnvironment/Mid/OEFutureWarfareOntology#Production -->

    <owl:Class rdf:about="http://www.ontologylibrary.mil/OperationalEnvironment/Mid/OEFutureWarfareOntology#Production">
        <rdfs:subClassOf rdf:resource="http://www.ontologylibrary.mil/OperationalEnvironment/Mid/OEFutureWarfareOntology#FaultLineMethodology"/>
        <obo:IAO_0000115>Transform the analysis into some kind of useable format for an intended audience. The fault line analysis, initially developed as an infographic, can formatted as a brief, a report, or simply be briefed orally. The strength of the analysis is amplified by combining discursive and visual descriptions into one format, accompanied with a clear and influential narrative.</obo:IAO_0000115>
        <obo:IAO_0000119>Fault Lines Methodology Infographic</obo:IAO_0000119>
    </owl:Class>
    


    <!-- http://www.ontologylibrary.mil/OperationalEnvironment/Mid/OEFutureWarfareOntology#Productivity -->

    <owl:Class rdf:about="http://www.ontologylibrary.mil/OperationalEnvironment/Mid/OEFutureWarfareOntology#Productivity">
        <rdfs:subClassOf rdf:resource="http://www.ontologylibrary.mil/OperationalEnvironment/Mid/OEFutureWarfareOntology#EconomicDevelopment"/>
        <obo:IAO_0000119>&quot;Productivity&quot;, Wikipedia

March 19, 2019

https://en.wikipedia.org/wiki/Productivity</obo:IAO_0000119>
        <CommonCoreOntologies:definition>Productivity describes various measures of the efficiency of production. A productivity measure is expressed as the ratio of output to inputs used in a production process, i.e. output per unit of input. Productivity is a crucial factor in production performance of firms and nations. Increasing national productivity can raise living standards because more real income improves people&apos;s ability to purchase goods and services, enjoy leisure, improve housing and education and contribute to social and environmental programs. Productivity growth can also help businesses to be more profitable.</CommonCoreOntologies:definition>
        <rdfs:label>Productivity</rdfs:label>
    </owl:Class>
    


    <!-- http://www.ontologylibrary.mil/OperationalEnvironment/Mid/OEFutureWarfareOntology#Proliferation -->

    <owl:Class rdf:about="http://www.ontologylibrary.mil/OperationalEnvironment/Mid/OEFutureWarfareOntology#Proliferation">
        <rdfs:subClassOf rdf:resource="http://www.ontologylibrary.mil/OperationalEnvironment/Mid/OEFutureWarfareOntology#Arms"/>
    </owl:Class>
    


    <!-- http://www.ontologylibrary.mil/OperationalEnvironment/Mid/OEFutureWarfareOntology#Propaganda -->

    <owl:Class rdf:about="http://www.ontologylibrary.mil/OperationalEnvironment/Mid/OEFutureWarfareOntology#Propaganda">
        <rdfs:subClassOf rdf:resource="http://www.ontologylibrary.mil/OperationalEnvironment/Mid/OEFutureWarfareOntology#Authoritariansim"/>
        <obo:IAO_0000115>Propaganda [is] dissemination of information—facts, arguments, rumours, half-truths, or lies—to influence public opinion.

Propaganda is the more or less systematic effort to manipulate other people’s beliefs, attitudes, or actions by means of symbols..... The propagandist...deliberately selects facts, arguments, and displays of symbols and presents them in ways he thinks will have the most effect. To maximize effect, he may omit pertinent facts or distort them, and he may try to divert the attention of the...people whom he is trying to sway...from everything but his own propaganda.</obo:IAO_0000115>
        <obo:IAO_0000119>Bruce Lannes Smith, &quot;Propaganda&quot;

March 12, 2019

https://www.britannica.com/topic/propaganda</obo:IAO_0000119>
        <rdfs:label>Propaganda</rdfs:label>
    </owl:Class>
    


    <!-- http://www.ontologylibrary.mil/OperationalEnvironment/Mid/OEFutureWarfareOntology#QuantumCommunications -->

    <owl:Class rdf:about="http://www.ontologylibrary.mil/OperationalEnvironment/Mid/OEFutureWarfareOntology#QuantumCommunications">
        <rdfs:subClassOf rdf:resource="http://www.ontologylibrary.mil/OperationalEnvironment/Mid/OEFutureWarfareOntology#CombatApplication"/>
    </owl:Class>
    


    <!-- http://www.ontologylibrary.mil/OperationalEnvironment/Mid/OEFutureWarfareOntology#QuantumComputing -->

    <owl:Class rdf:about="http://www.ontologylibrary.mil/OperationalEnvironment/Mid/OEFutureWarfareOntology#QuantumComputing">
        <rdfs:subClassOf rdf:resource="http://www.ontologylibrary.mil/OperationalEnvironment/Mid/OEFutureWarfareOntology#CombatApplication"/>
        <rdfs:subClassOf rdf:resource="http://www.ontologylibrary.mil/OperationalEnvironment/Mid/OEFutureWarfareOntology#SystemsThatSeeThinkCommunicate"/>
        <obo:IAO_0000115>From 1&amp;0 binary to quantum superpositions &amp; entanglement (e.g., 0 and 1 at same time)</obo:IAO_0000115>
        <obo:IAO_0000119>Potential Game Changers Infographic

7/11/2018</obo:IAO_0000119>
    </owl:Class>
    


    <!-- http://www.ontologylibrary.mil/OperationalEnvironment/Mid/OEFutureWarfareOntology#QuantumCryptography -->

    <owl:Class rdf:about="http://www.ontologylibrary.mil/OperationalEnvironment/Mid/OEFutureWarfareOntology#QuantumCryptography">
        <rdfs:subClassOf rdf:resource="http://www.ontologylibrary.mil/OperationalEnvironment/Mid/OEFutureWarfareOntology#CombatApplication"/>
    </owl:Class>
    


    <!-- http://www.ontologylibrary.mil/OperationalEnvironment/Mid/OEFutureWarfareOntology#QuantumNavigation -->

    <owl:Class rdf:about="http://www.ontologylibrary.mil/OperationalEnvironment/Mid/OEFutureWarfareOntology#QuantumNavigation">
        <rdfs:subClassOf rdf:resource="http://www.ontologylibrary.mil/OperationalEnvironment/Mid/OEFutureWarfareOntology#CombatApplication"/>
    </owl:Class>
    


    <!-- http://www.ontologylibrary.mil/OperationalEnvironment/Mid/OEFutureWarfareOntology#QuantumSensing -->

    <owl:Class rdf:about="http://www.ontologylibrary.mil/OperationalEnvironment/Mid/OEFutureWarfareOntology#QuantumSensing">
        <rdfs:subClassOf rdf:resource="http://www.ontologylibrary.mil/OperationalEnvironment/Mid/OEFutureWarfareOntology#CombatApplication"/>
    </owl:Class>
    


    <!-- http://www.ontologylibrary.mil/OperationalEnvironment/Mid/OEFutureWarfareOntology#RadarJammer -->

    <owl:Class rdf:about="http://www.ontologylibrary.mil/OperationalEnvironment/Mid/OEFutureWarfareOntology#RadarJammer">
        <rdfs:subClassOf rdf:resource="http://www.ontologylibrary.mil/OperationalEnvironment/Mid/OEFutureWarfareOntology#ActiveDenialSystems"/>
        <obo:IAO_0000115>Sophisticated noise or repeaters. Convergence of RF+Cyber through software defined radios. Controlled modulation can make signals look like noise to interceptors.</obo:IAO_0000115>
        <obo:IAO_0000119>Potential Game Changers Infographic

7/11/2018</obo:IAO_0000119>
    </owl:Class>
    


    <!-- http://www.ontologylibrary.mil/OperationalEnvironment/Mid/OEFutureWarfareOntology#RadioFrequencyWeapons -->

    <owl:Class rdf:about="http://www.ontologylibrary.mil/OperationalEnvironment/Mid/OEFutureWarfareOntology#RadioFrequencyWeapons">
        <rdfs:subClassOf rdf:resource="http://www.ontologylibrary.mil/OperationalEnvironment/Mid/OEFutureWarfareOntology#SystemsThatShoot"/>
        <obo:IAO_0000115>Attack targets across the frequency spectrum. Targets: Not just RF: Microwave weapons “cook targets,” people, electronics. [SOURCE: TRADOC G-2 Potential Game Changers, May 2018]</obo:IAO_0000115>
        <obo:IAO_0000119>Technology Environment of Ground Warfare in 2035-2050

Projections made in 2018 by ARL and TRADOC

[This is a draft outline of a potential document; prepared by Alexander Kott, the US Army Research Laboratory; July 2018]</obo:IAO_0000119>
    </owl:Class>
    


    <!-- http://www.ontologylibrary.mil/OperationalEnvironment/Mid/OEFutureWarfareOntology#RailGun -->

    <owl:Class rdf:about="http://www.ontologylibrary.mil/OperationalEnvironment/Mid/OEFutureWarfareOntology#RailGun">
        <rdfs:subClassOf rdf:resource="http://www.ontologylibrary.mil/OperationalEnvironment/Mid/OEFutureWarfareOntology#RailGunsAndEnhancedDirectedKineticEnergyWeapons"/>
        <obo:IAO_0000115>Electromagnetic projectile launchers: High velocity/energy and space (Mach 5 or higher). Not powered by explosive</obo:IAO_0000115>
        <obo:IAO_0000119>Potential Game Changers Infographic

7/11/2018</obo:IAO_0000119>
    </owl:Class>
    


    <!-- http://www.ontologylibrary.mil/OperationalEnvironment/Mid/OEFutureWarfareOntology#RailGunsAndEnhancedDirectedKineticEnergyWeapons -->

    <owl:Class rdf:about="http://www.ontologylibrary.mil/OperationalEnvironment/Mid/OEFutureWarfareOntology#RailGunsAndEnhancedDirectedKineticEnergyWeapons">
        <rdfs:subClassOf rdf:resource="http://www.ontologylibrary.mil/OperationalEnvironment/Mid/OEFutureWarfareOntology#SystemsThatShoot"/>
        <rdfs:subClassOf>
            <owl:Restriction>
                <owl:onProperty rdf:resource="http://www.ontologylibrary.mil/OperationalEnvironment/Mid/OEFutureWarfareOntology#hasCombatApplication"/>
                <owl:someValuesFrom rdf:resource="http://www.ontologylibrary.mil/OperationalEnvironment/Mid/OEFutureWarfareOntology#ElectroDynamicKineticEnergyWeaponsPrecisionWeaponPointDefense"/>
            </owl:Restriction>
        </rdfs:subClassOf>
        <rdfs:subClassOf>
            <owl:Restriction>
                <owl:onProperty rdf:resource="http://www.ontologylibrary.mil/OperationalEnvironment/Mid/OEFutureWarfareOntology#hasCombatApplication"/>
                <owl:someValuesFrom rdf:resource="http://www.ontologylibrary.mil/OperationalEnvironment/Mid/OEFutureWarfareOntology#HypersonicGlideVehicleDefense"/>
            </owl:Restriction>
        </rdfs:subClassOf>
        <rdfs:subClassOf>
            <owl:Restriction>
                <owl:onProperty rdf:resource="http://www.ontologylibrary.mil/OperationalEnvironment/Mid/OEFutureWarfareOntology#hasCombatApplication"/>
                <owl:someValuesFrom rdf:resource="http://www.ontologylibrary.mil/OperationalEnvironment/Mid/OEFutureWarfareOntology#LongRangePrecisionFires"/>
            </owl:Restriction>
        </rdfs:subClassOf>
    </owl:Class>
    


    <!-- http://www.ontologylibrary.mil/OperationalEnvironment/Mid/OEFutureWarfareOntology#RatedSpeed -->

    <owl:Class rdf:about="http://www.ontologylibrary.mil/OperationalEnvironment/Mid/OEFutureWarfareOntology#RatedSpeed">
        <rdfs:subClassOf rdf:resource="http://www.ontologylibrary.mil/OperationalEnvironment/Mid/OEFutureWarfareOntology#GasEnergyGeneration"/>
        <obo:IAO_0000115>speed expressed in revolutions per minute of the gas turbine core (3.5) output shaft required for generator synchronous speed</obo:IAO_0000115>
        <obo:IAO_0000119>International Organization for Standardization/International ISO 19859:2016

Technical Committee : ISO/TC 192  Gas turbines

ICS :  29.160.99  Other standards related to rotating machinery 27.040  Gas and steam turbines. Steam engines

Gas turbine applications -- Requirements for power generation

Publication date : 2016-08

1st Edition</obo:IAO_0000119>
    </owl:Class>
    


    <!-- http://www.ontologylibrary.mil/OperationalEnvironment/Mid/OEFutureWarfareOntology#RedirectedEnergy -->

    <owl:Class rdf:about="http://www.ontologylibrary.mil/OperationalEnvironment/Mid/OEFutureWarfareOntology#RedirectedEnergy">
        <rdfs:subClassOf rdf:resource="http://www.ontologylibrary.mil/OperationalEnvironment/Mid/OEFutureWarfareOntology#SystemsThatProtect"/>
        <obo:IAO_0000115>Hyper stealth invisibility, Electromagnetic illusion. [SOURCE: TRADOC G-2 Potential Game Changers, May 2018]</obo:IAO_0000115>
        <obo:IAO_0000119>Technology Environment of Ground Warfare in 2035-2050

Projections made in 2018 by ARL and TRADOC

[This is a draft outline of a potential document; prepared by Alexander Kott, the US Army Research Laboratory; July 2018]</obo:IAO_0000119>
    </owl:Class>
    


    <!-- http://www.ontologylibrary.mil/OperationalEnvironment/Mid/OEFutureWarfareOntology#RefugeesAndDisplacedPersons -->

    <owl:Class rdf:about="http://www.ontologylibrary.mil/OperationalEnvironment/Mid/OEFutureWarfareOntology#RefugeesAndDisplacedPersons">
        <rdfs:subClassOf rdf:resource="http://www.ontologylibrary.mil/OperationalEnvironment/Mid/OEFutureWarfareOntology#Migration"/>
        <obo:IAO_0000119>&quot;What Is a Refugee?&quot;, USA for UNHCR

March 25, 2019

https://www.unrefugees.org/refugee-facts/what-is-a-refugee/</obo:IAO_0000119>
        <CommonCoreOntologies:definition>Who is a refugee?

A refugee is someone who has been forced to flee his or her country because of persecution, war or violence. A refugee has a well-founded fear of persecution for reasons of race, religion, nationality, political opinion or membership in a particular social group. Most likely, they cannot return home or are afraid to do so. War and ethnic, tribal and religious violence are leading causes of refugees fleeing their countries.

Who is an internally displaced person?

An internally displaced person, or IDP, is someone who has been forced to flee their home but never cross an international border. These individuals seek safety anywhere they can find it—in nearby towns, schools, settlements, internal camps, even forests and fields. IDPs, which include people displaced by internal strife and natural disasters, are the largest group that UNHCR assists.</CommonCoreOntologies:definition>
        <rdfs:label>Refugees and Displaced Persons</rdfs:label>
    </owl:Class>
    


    <!-- http://www.ontologylibrary.mil/OperationalEnvironment/Mid/OEFutureWarfareOntology#RelationalAlgebra -->

    <owl:Class rdf:about="http://www.ontologylibrary.mil/OperationalEnvironment/Mid/OEFutureWarfareOntology#RelationalAlgebra">
        <rdfs:subClassOf rdf:resource="http://www.ontologylibrary.mil/OperationalEnvironment/Mid/OEFutureWarfareOntology#BigDataControlledVocabulary"/>
        <obo:IAO_0000115>algebra for expressing and manipulating relations</obo:IAO_0000115>
        <obo:IAO_0000119>Information technology — Big data — Overview and vocabulary

https://www.iso.org/jtc1</obo:IAO_0000119>
        <obo:IAO_0000119>[SOURCE: ISO/IEC 2382:2015, 17.04.08]</obo:IAO_0000119>
    </owl:Class>
    


    <!-- http://www.ontologylibrary.mil/OperationalEnvironment/Mid/OEFutureWarfareOntology#RelationalDatabase -->

    <owl:Class rdf:about="http://www.ontologylibrary.mil/OperationalEnvironment/Mid/OEFutureWarfareOntology#RelationalDatabase">
        <rdfs:subClassOf rdf:resource="http://www.ontologylibrary.mil/OperationalEnvironment/Mid/OEFutureWarfareOntology#BigDataControlledVocabulary"/>
        <obo:IAO_0000115>database (3.1.7) in which the data are organized according to a relational model</obo:IAO_0000115>
        <obo:IAO_0000119>Information technology — Big data — Overview and vocabulary

https://www.iso.org/jtc1</obo:IAO_0000119>
        <obo:IAO_0000119>[SOURCE: ISO/IEC 2382:2015, 17.04.05]</obo:IAO_0000119>
    </owl:Class>
    


    <!-- http://www.ontologylibrary.mil/OperationalEnvironment/Mid/OEFutureWarfareOntology#RelationalModel -->

    <owl:Class rdf:about="http://www.ontologylibrary.mil/OperationalEnvironment/Mid/OEFutureWarfareOntology#RelationalModel">
        <rdfs:subClassOf rdf:resource="http://www.ontologylibrary.mil/OperationalEnvironment/Mid/OEFutureWarfareOntology#BigDataControlledVocabulary"/>
        <obo:IAO_0000115>data model (3.1.9) whose structure is based on a set of relations</obo:IAO_0000115>
        <obo:IAO_0000119>Information technology — Big data — Overview and vocabulary

https://www.iso.org/jtc1</obo:IAO_0000119>
        <obo:IAO_0000119>[SOURCE: ISO/IEC 2382:2015, 17.04.04]</obo:IAO_0000119>
    </owl:Class>
    


    <!-- http://www.ontologylibrary.mil/OperationalEnvironment/Mid/OEFutureWarfareOntology#Reliability -->

    <owl:Class rdf:about="http://www.ontologylibrary.mil/OperationalEnvironment/Mid/OEFutureWarfareOntology#Reliability">
        <rdfs:subClassOf rdf:resource="http://www.ontologylibrary.mil/OperationalEnvironment/Mid/OEFutureWarfareOntology#CyberSecurityControlledVocabulary"/>
        <obo:IAO_0000115>property of consistent intended behaviour and results</obo:IAO_0000115>
        <obo:IAO_0000119>International Organization for Standardization/International Electrotechnical Commission 27000:2018

Security techniques — Information security management systems — Overview and vocabulary

Publication date : 2018-02

5th Edition</obo:IAO_0000119>
    </owl:Class>
    


    <!-- http://www.ontologylibrary.mil/OperationalEnvironment/Mid/OEFutureWarfareOntology#RenewableEnergy -->

    <owl:Class rdf:about="http://www.ontologylibrary.mil/OperationalEnvironment/Mid/OEFutureWarfareOntology#RenewableEnergy">
        <rdfs:subClassOf rdf:resource="http://www.ontologylibrary.mil/OperationalEnvironment/Mid/OEFutureWarfareOntology#PowerGenerationAndStorageControlledVocabulary"/>
        <obo:IAO_0000115>energy not depleted by extraction as it is naturally replenished at a rate faster than it is extracted

Note 1 to entry: Renewable energy excludes recovered or wasted energy.

Note 2 to entry: Organic fraction of municipal waste can be considered as a renewable energy.

Note 3 to entry: Whether the energy stored in a technical system is renewable or not depends upon the nature of the original energy.

Note 4 to entry: Criteria to categorize an energy as renewable can differ amongst jurisdictions, based on local environmental or other reasons.
[SOURCE: ISO/IEC 13273‑2:2015, 3.1.5, modified — The term “renewable energy source” has been replaced by “renewable energy”; the word “source” has been deleted after “energy” in the definition and in each of the Notes to entry; the verb “may” has been replaced by “can” in Note 2 to entry. The term “renewable energy” is defined differently in ISO/IEC 13273‑2:2015, 3.1.6.]</obo:IAO_0000115>
        <obo:IAO_0000119>International Organization for Standardization/International ISO 50007:2017

Technical Committee : ISO/TC 301  Energy management and energy savings

ICS :  27.015  Energy efficiency. Energy conservation in general

Energy services -- Guidelines for the assessment and improvement of the energy service to users

Publication date : 2017-06

1st Edition</obo:IAO_0000119>
    </owl:Class>
    


    <!-- http://www.ontologylibrary.mil/OperationalEnvironment/Mid/OEFutureWarfareOntology#ReportingBoundary -->

    <owl:Class rdf:about="http://www.ontologylibrary.mil/OperationalEnvironment/Mid/OEFutureWarfareOntology#ReportingBoundary">
        <rdfs:subClassOf rdf:resource="http://www.ontologylibrary.mil/OperationalEnvironment/Mid/OEFutureWarfareOntology#ClimateChangeAndResourceCompetitionControlledVocabulary"/>
        <obo:IAO_0000115>grouping of GHGemission (3.1.5) or GHGremovals (3.1.6) reported from within the organizational boundary (3.4.7), as well as those significant indirect emissions that are a consequence of the organization’s (3.4.2) operations and activities</obo:IAO_0000115>
        <obo:IAO_0000119>International Organization for Standardization/International Electrotechnical Commission 27000:2018

Technical Committee : ISO/TC 207/SC 7  Greenhouse gas management and related activities

ICS :  13.020.40  Pollution, pollution control and conservation

Greenhouse gases -- Part 1: Specification with guidance at the organization level for quantification and reporting of greenhouse gas emissions and removals 

Publication date : 2018-12

2nd Edition</obo:IAO_0000119>
    </owl:Class>
    


    <!-- http://www.ontologylibrary.mil/OperationalEnvironment/Mid/OEFutureWarfareOntology#Repression -->

    <owl:Class rdf:about="http://www.ontologylibrary.mil/OperationalEnvironment/Mid/OEFutureWarfareOntology#Repression">
        <rdfs:subClassOf rdf:resource="http://www.ontologylibrary.mil/OperationalEnvironment/Mid/OEFutureWarfareOntology#Authoritariansim"/>
        <obo:IAO_0000115>Political repression is the persecution of an individual or group within society for political reasons, particularly for the purpose of restricting or preventing their ability to take part in the political life of a society thereby reducing their standing among their fellow citizens.

...

It often is manifested through discriminatory policies, such as human rights violations, surveillance abuse, police brutality, imprisonment, involuntary settlement, stripping of citizen&apos;s rights, lustration and violent action or terror such as the murder, summary executions, torture, forced disappearance and other extrajudicial punishment of political activists, dissidents, or general population. Political repression can also be reinforced by means outside of written policy, such as by public and private media ownership and by self-censorship within the public.

Where political repression is sanctioned and organised by the state, it may constitute state terrorism, genocide, politicide or crimes against humanity. Systemic and violent political repression is a typical feature of dictatorships, totalitarian states and similar regimes. Acts of political repression may be carried out by secret police forces, army, paramilitary groups or death squads.</obo:IAO_0000115>
        <obo:IAO_0000119>&quot;Politiical Repression&quot;, Wikipedia

March 12, 2019

https://en.wikipedia.org/wiki/Political_repression</obo:IAO_0000119>
    </owl:Class>
    


    <!-- http://www.ontologylibrary.mil/OperationalEnvironment/Mid/OEFutureWarfareOntology#Requirement -->

    <owl:Class rdf:about="http://www.ontologylibrary.mil/OperationalEnvironment/Mid/OEFutureWarfareOntology#Requirement">
        <rdfs:subClassOf rdf:resource="http://www.ontologylibrary.mil/OperationalEnvironment/Mid/OEFutureWarfareOntology#CyberSecurityControlledVocabulary"/>
        <obo:IAO_0000115>need or expectation that is stated, generally implied or obligatory

Note 1 to entry: “Generally implied” means that it is custom or common practice for the organization and interested parties that the need or expectation under consideration is implied.

Note 2 to entry: A specified requirement is one that is stated, for example in documented information.</obo:IAO_0000115>
        <obo:IAO_0000119>International Organization for Standardization/International Electrotechnical Commission 27000:2018

Security techniques — Information security management systems — Overview and vocabulary

Publication date : 2018-02

5th Edition</obo:IAO_0000119>
    </owl:Class>
    


    <!-- http://www.ontologylibrary.mil/OperationalEnvironment/Mid/OEFutureWarfareOntology#ResidualRisk -->

    <owl:Class rdf:about="http://www.ontologylibrary.mil/OperationalEnvironment/Mid/OEFutureWarfareOntology#ResidualRisk">
        <rdfs:subClassOf rdf:resource="http://www.ontologylibrary.mil/OperationalEnvironment/Mid/OEFutureWarfareOntology#CyberSecurityControlledVocabulary"/>
        <obo:IAO_0000115>risk (3.61) remaining after risk treatment (3.72)

Note 1 to entry: Residual risk can contain unidentified risk.

Note 2 to entry: Residual risk can also be referred to as “retained risk”.</obo:IAO_0000115>
        <obo:IAO_0000119>International Organization for Standardization/International Electrotechnical Commission 27000:2018

Security techniques — Information security management systems — Overview and vocabulary

Publication date : 2018-02

5th Edition</obo:IAO_0000119>
    </owl:Class>
    


    <!-- http://www.ontologylibrary.mil/OperationalEnvironment/Mid/OEFutureWarfareOntology#ResourceExtraction -->

    <owl:Class rdf:about="http://www.ontologylibrary.mil/OperationalEnvironment/Mid/OEFutureWarfareOntology#ResourceExtraction">
        <rdfs:subClassOf rdf:resource="http://www.ontologylibrary.mil/OperationalEnvironment/Mid/OEFutureWarfareOntology#EconomicActivity"/>
        <obo:IAO_0000119>&quot;Natural Resource&quot;, Wikipedia

March 13, 2019

https://en.wikipedia.org/wiki/Natural_resource#Extraction</obo:IAO_0000119>
        <CommonCoreOntologies:definition>Extraction produces raw material, which is then processed to add value. Examples of extractive industries are hunting, trapping, mining, oil and gas drilling, and forestry. Natural resources can add substantial amounts to a country&apos;s wealth, however, a sudden inflow of money caused by a resource boom can create social problems including inflation harming other industries (&quot;Dutch disease&quot;) and corruption, leading to inequality and underdevelopment, this is known as the &quot;resource curse&quot;.</CommonCoreOntologies:definition>
        <rdfs:label>Resource Extraction</rdfs:label>
    </owl:Class>
    


    <!-- http://www.ontologylibrary.mil/OperationalEnvironment/Mid/OEFutureWarfareOntology#ResponsibleParty -->

    <owl:Class rdf:about="http://www.ontologylibrary.mil/OperationalEnvironment/Mid/OEFutureWarfareOntology#ResponsibleParty">
        <rdfs:subClassOf rdf:resource="http://www.ontologylibrary.mil/OperationalEnvironment/Mid/OEFutureWarfareOntology#ClimateChangeAndResourceCompetitionControlledVocabulary"/>
        <obo:IAO_0000115>person or persons responsible for the provision of the GHG statement (3.2.5) and the supporting GHG (3.1.1) information

Note 1 to entry: The responsible party can be either individuals or representatives of an organization (3.4.2) or project, and can be the party who engages the verifier (3.4.11) or validator (3.4.12).</obo:IAO_0000115>
        <obo:IAO_0000119>International Organization for Standardization/International Electrotechnical Commission 27000:2018

Technical Committee : ISO/TC 207/SC 7  Greenhouse gas management and related activities

ICS :  13.020.40  Pollution, pollution control and conservation

Greenhouse gases -- Part 1: Specification with guidance at the organization level for quantification and reporting of greenhouse gas emissions and removals 

Publication date : 2018-12

2nd Edition</obo:IAO_0000119>
    </owl:Class>
    


    <!-- http://www.ontologylibrary.mil/OperationalEnvironment/Mid/OEFutureWarfareOntology#Review -->

    <owl:Class rdf:about="http://www.ontologylibrary.mil/OperationalEnvironment/Mid/OEFutureWarfareOntology#Review">
        <rdfs:subClassOf rdf:resource="http://www.ontologylibrary.mil/OperationalEnvironment/Mid/OEFutureWarfareOntology#CyberSecurityControlledVocabulary"/>
        <obo:IAO_0000115>activity undertaken to determine the suitability, adequacy and effectiveness (3.20) of the subject matter to achieve established objectives (3.49)</obo:IAO_0000115>
        <obo:IAO_0000119>International Organization for Standardization/International Electrotechnical Commission 27000:2018

Security techniques — Information security management systems — Overview and vocabulary

Publication date : 2018-02

5th Edition</obo:IAO_0000119>
    </owl:Class>
    


    <!-- http://www.ontologylibrary.mil/OperationalEnvironment/Mid/OEFutureWarfareOntology#ReviewObject -->

    <owl:Class rdf:about="http://www.ontologylibrary.mil/OperationalEnvironment/Mid/OEFutureWarfareOntology#ReviewObject">
        <rdfs:subClassOf rdf:resource="http://www.ontologylibrary.mil/OperationalEnvironment/Mid/OEFutureWarfareOntology#CyberSecurityControlledVocabulary"/>
        <obo:IAO_0000115>specific item being reviewed</obo:IAO_0000115>
        <obo:IAO_0000119>International Organization for Standardization/International Electrotechnical Commission 27000:2018

Security techniques — Information security management systems — Overview and vocabulary

Publication date : 2018-02

5th Edition</obo:IAO_0000119>
    </owl:Class>
    


    <!-- http://www.ontologylibrary.mil/OperationalEnvironment/Mid/OEFutureWarfareOntology#ReviewObjective -->

    <owl:Class rdf:about="http://www.ontologylibrary.mil/OperationalEnvironment/Mid/OEFutureWarfareOntology#ReviewObjective">
        <rdfs:subClassOf rdf:resource="http://www.ontologylibrary.mil/OperationalEnvironment/Mid/OEFutureWarfareOntology#CyberSecurityControlledVocabulary"/>
        <obo:IAO_0000115>statement describing what is to be achieved as a result of a review (3.59)</obo:IAO_0000115>
        <obo:IAO_0000119>International Organization for Standardization/International Electrotechnical Commission 27000:2018

Security techniques — Information security management systems — Overview and vocabulary

Publication date : 2018-02

5th Edition</obo:IAO_0000119>
    </owl:Class>
    


    <!-- http://www.ontologylibrary.mil/OperationalEnvironment/Mid/OEFutureWarfareOntology#Risk -->

    <owl:Class rdf:about="http://www.ontologylibrary.mil/OperationalEnvironment/Mid/OEFutureWarfareOntology#Risk">
        <rdfs:subClassOf rdf:resource="http://www.ontologylibrary.mil/OperationalEnvironment/Mid/OEFutureWarfareOntology#CyberSecurityControlledVocabulary"/>
        <obo:IAO_0000115>effect of uncertainty on objectives (3.49)

Note 1 to entry: An effect is a deviation from the expected — positive or negative.

Note 2 to entry: Uncertainty is the state, even partial, of deficiency of information related to, understanding or knowledge of, an event, its consequence, or likelihood.

Note 3 to entry: Risk is often characterized by reference to potential “events” (as defined in ISO Guide 73:2009, 3.5.1.3) and “consequences” (as defined in ISO Guide 73:2009, 3.6.1.3), or a combination of these.

Note 4 to entry: Risk is often expressed in terms of a combination of the consequences of an event (including changes in circumstances) and the associated “likelihood” (as defined in ISO Guide 73:2009, 3.6.1.1) of occurrence.

Note 5 to entry: In the context of information security management systems, information security risks can be expressed as effect of uncertainty on information security objectives.

Note 6 to entry: Information security risk is associated with the potential that threats will exploit vulnerabilities of an information asset or group of information assets and thereby cause harm to an organization.</obo:IAO_0000115>
        <obo:IAO_0000119>International Organization for Standardization/International Electrotechnical Commission 27000:2018

Security techniques — Information security management systems — Overview and vocabulary

Publication date : 2018-02

5th Edition</obo:IAO_0000119>
    </owl:Class>
    


    <!-- http://www.ontologylibrary.mil/OperationalEnvironment/Mid/OEFutureWarfareOntology#RiskAcceptance -->

    <owl:Class rdf:about="http://www.ontologylibrary.mil/OperationalEnvironment/Mid/OEFutureWarfareOntology#RiskAcceptance">
        <rdfs:subClassOf rdf:resource="http://www.ontologylibrary.mil/OperationalEnvironment/Mid/OEFutureWarfareOntology#CyberSecurityControlledVocabulary"/>
        <obo:IAO_0000115>informed decision to take a particular risk (3.61)

Note 1 to entry: Risk acceptance can occur without risk treatment (3.72) or during the process (3.54) of risk treatment.

Note 2 to entry: Accepted risks are subject to monitoring (3.46) and review (3.58).</obo:IAO_0000115>
        <obo:IAO_0000119>International Organization for Standardization/International Electrotechnical Commission 27000:2018

Security techniques — Information security management systems — Overview and vocabulary

Publication date : 2018-02

5th Edition</obo:IAO_0000119>
        <obo:IAO_0000119>[SOURCE: ISO Guide 73:2009, 3.7.1.6]</obo:IAO_0000119>
    </owl:Class>
    


    <!-- http://www.ontologylibrary.mil/OperationalEnvironment/Mid/OEFutureWarfareOntology#RiskAnalysis -->

    <owl:Class rdf:about="http://www.ontologylibrary.mil/OperationalEnvironment/Mid/OEFutureWarfareOntology#RiskAnalysis">
        <rdfs:subClassOf rdf:resource="http://www.ontologylibrary.mil/OperationalEnvironment/Mid/OEFutureWarfareOntology#CyberSecurityControlledVocabulary"/>
        <obo:IAO_0000115>process (3.54) to comprehend the nature of risk (3.61) and to determine the level of risk (3.39)

Note 1 to entry: Risk analysis provides the basis for risk evaluation (3.67) and decisions about risk treatment (3.72).

Note 2 to entry: Risk analysis includes risk estimation.</obo:IAO_0000115>
        <obo:IAO_0000119>International Organization for Standardization/International Electrotechnical Commission 27000:2018

Security techniques — Information security management systems — Overview and vocabulary

Publication date : 2018-02

5th Edition</obo:IAO_0000119>
        <obo:IAO_0000119>[SOURCE: ISO Guide 73:2009, 3.6.1]</obo:IAO_0000119>
    </owl:Class>
    


    <!-- http://www.ontologylibrary.mil/OperationalEnvironment/Mid/OEFutureWarfareOntology#RiskAssessment -->

    <owl:Class rdf:about="http://www.ontologylibrary.mil/OperationalEnvironment/Mid/OEFutureWarfareOntology#RiskAssessment">
        <rdfs:subClassOf rdf:resource="http://www.ontologylibrary.mil/OperationalEnvironment/Mid/OEFutureWarfareOntology#CyberSecurityControlledVocabulary"/>
        <obo:IAO_0000115>overall process (3.54) of risk identification (3.68), risk analysis (3.63) and risk evaluation (3.67)</obo:IAO_0000115>
        <obo:IAO_0000119>International Organization for Standardization/International Electrotechnical Commission 27000:2018

Security techniques — Information security management systems — Overview and vocabulary

Publication date : 2018-02

5th Edition</obo:IAO_0000119>
        <obo:IAO_0000119>[SOURCE: ISO Guide 73:2009, 3.4.1]</obo:IAO_0000119>
    </owl:Class>
    


    <!-- http://www.ontologylibrary.mil/OperationalEnvironment/Mid/OEFutureWarfareOntology#RiskCommunicationAndConsultation -->

    <owl:Class rdf:about="http://www.ontologylibrary.mil/OperationalEnvironment/Mid/OEFutureWarfareOntology#RiskCommunicationAndConsultation">
        <rdfs:subClassOf rdf:resource="http://www.ontologylibrary.mil/OperationalEnvironment/Mid/OEFutureWarfareOntology#CyberSecurityControlledVocabulary"/>
        <obo:IAO_0000115>set of continual and iterative processes (3.54) that an organization conducts to provide, share or obtain information, and to engage in dialogue with stakeholders (3.37) regarding the management of risk (3.61)

Note 1 to entry: The information can relate to the existence, nature, form, likelihood (3.41), significance, evaluation, acceptability and treatment of risk.

Note 2 to entry: Consultation is a two-way process of informed communication between an organization (3.50) and its stakeholders on an issue prior to making a decision or determining a direction on that issue. Consultation is
— a process which impacts on a decision through influence rather than power; and
— an input to decision making, not joint decision making.</obo:IAO_0000115>
        <obo:IAO_0000119>International Organization for Standardization/International Electrotechnical Commission 27000:2018

Security techniques — Information security management systems — Overview and vocabulary

Publication date : 2018-02

5th Edition</obo:IAO_0000119>
    </owl:Class>
    


    <!-- http://www.ontologylibrary.mil/OperationalEnvironment/Mid/OEFutureWarfareOntology#RiskCriteria -->

    <owl:Class rdf:about="http://www.ontologylibrary.mil/OperationalEnvironment/Mid/OEFutureWarfareOntology#RiskCriteria">
        <rdfs:subClassOf rdf:resource="http://www.ontologylibrary.mil/OperationalEnvironment/Mid/OEFutureWarfareOntology#CyberSecurityControlledVocabulary"/>
        <obo:IAO_0000115>terms of reference against which the significance of risk (3.61) is evaluated

Note 1 to entry: Risk criteria are based on organizational objectives, and external context (3.22) and internal context (3.38).

Note 2 to entry: Risk criteria can be derived from standards, laws, policies (3.53) and other requirements (3.56).</obo:IAO_0000115>
        <obo:IAO_0000119>International Organization for Standardization/International Electrotechnical Commission 27000:2018

Security techniques — Information security management systems — Overview and vocabulary

Publication date : 2018-02

5th Edition</obo:IAO_0000119>
        <obo:IAO_0000119>[SOURCE: ISO Guide 73:2009, 3.3.1.3]</obo:IAO_0000119>
    </owl:Class>
    


    <!-- http://www.ontologylibrary.mil/OperationalEnvironment/Mid/OEFutureWarfareOntology#RiskEvaluation -->

    <owl:Class rdf:about="http://www.ontologylibrary.mil/OperationalEnvironment/Mid/OEFutureWarfareOntology#RiskEvaluation">
        <rdfs:subClassOf rdf:resource="http://www.ontologylibrary.mil/OperationalEnvironment/Mid/OEFutureWarfareOntology#CyberSecurityControlledVocabulary"/>
        <obo:IAO_0000115>process (3.54) of comparing the results of risk analysis (3.63) with risk criteria (3.66) to determine whether the risk (3.61) and/or its magnitude is acceptable or tolerable

Note 1 to entry: Risk evaluation assists in the decision about risk treatment (3.72).</obo:IAO_0000115>
        <obo:IAO_0000119>International Organization for Standardization/International Electrotechnical Commission 27000:2018

Security techniques — Information security management systems — Overview and vocabulary

Publication date : 2018-02

5th Edition</obo:IAO_0000119>
        <obo:IAO_0000119>[SOURCE: ISO Guide 73:2009, 3.7.1]</obo:IAO_0000119>
    </owl:Class>
    


    <!-- http://www.ontologylibrary.mil/OperationalEnvironment/Mid/OEFutureWarfareOntology#RiskIdentification -->

    <owl:Class rdf:about="http://www.ontologylibrary.mil/OperationalEnvironment/Mid/OEFutureWarfareOntology#RiskIdentification">
        <rdfs:subClassOf rdf:resource="http://www.ontologylibrary.mil/OperationalEnvironment/Mid/OEFutureWarfareOntology#CyberSecurityControlledVocabulary"/>
        <obo:IAO_0000115>process (3.54) of finding, recognizing and describing risks (3.61)

Note 1 to entry: Risk identification involves the identification of risk sources, events (3.21), their causes and their potential consequences (3.12).

Note 2 to entry: Risk identification can involve historical data, theoretical analysis, informed and expert opinions, and stakeholders’ (3.37) needs.</obo:IAO_0000115>
        <obo:IAO_0000119>International Organization for Standardization/International Electrotechnical Commission 27000:2018

Security techniques — Information security management systems — Overview and vocabulary

Publication date : 2018-02

5th Edition</obo:IAO_0000119>
        <obo:IAO_0000119>[SOURCE: ISO Guide 73:2009, 3.5.1]</obo:IAO_0000119>
    </owl:Class>
    


    <!-- http://www.ontologylibrary.mil/OperationalEnvironment/Mid/OEFutureWarfareOntology#RiskManagement -->

    <owl:Class rdf:about="http://www.ontologylibrary.mil/OperationalEnvironment/Mid/OEFutureWarfareOntology#RiskManagement">
        <rdfs:subClassOf rdf:resource="http://www.ontologylibrary.mil/OperationalEnvironment/Mid/OEFutureWarfareOntology#CyberSecurityControlledVocabulary"/>
        <obo:IAO_0000115>coordinated activities to direct and control an organization (3.50) with regard to risk (3.61)</obo:IAO_0000115>
        <obo:IAO_0000119>International Organization for Standardization/International Electrotechnical Commission 27000:2018

Security techniques — Information security management systems — Overview and vocabulary

Publication date : 2018-02

5th Edition</obo:IAO_0000119>
        <obo:IAO_0000119>[SOURCE: ISO Guide 73:2009, 2.1]</obo:IAO_0000119>
    </owl:Class>
    


    <!-- http://www.ontologylibrary.mil/OperationalEnvironment/Mid/OEFutureWarfareOntology#RiskManagementProcess -->

    <owl:Class rdf:about="http://www.ontologylibrary.mil/OperationalEnvironment/Mid/OEFutureWarfareOntology#RiskManagementProcess">
        <rdfs:subClassOf rdf:resource="http://www.ontologylibrary.mil/OperationalEnvironment/Mid/OEFutureWarfareOntology#CyberSecurityControlledVocabulary"/>
        <obo:IAO_0000115>systematic application of management policies (3.53), procedures and practices to the activities of communicating, consulting, establishing the context and identifying, analysing, evaluating, treating, monitoring and reviewing risk (3.61)

Note 1 to entry: ISO/IEC 27005 uses the term “process” (3.54) to describe risk management overall. The elements within the risk management (3.69) process are referred to as “activities”.</obo:IAO_0000115>
        <obo:IAO_0000119>International Organization for Standardization/International Electrotechnical Commission 27000:2018

Security techniques — Information security management systems — Overview and vocabulary

Publication date : 2018-02

5th Edition</obo:IAO_0000119>
    </owl:Class>
    


    <!-- http://www.ontologylibrary.mil/OperationalEnvironment/Mid/OEFutureWarfareOntology#RiskOwner -->

    <owl:Class rdf:about="http://www.ontologylibrary.mil/OperationalEnvironment/Mid/OEFutureWarfareOntology#RiskOwner">
        <rdfs:subClassOf rdf:resource="http://www.ontologylibrary.mil/OperationalEnvironment/Mid/OEFutureWarfareOntology#CyberSecurityControlledVocabulary"/>
        <obo:IAO_0000115>person or entity with the accountability and authority to manage a risk (3.61)</obo:IAO_0000115>
        <obo:IAO_0000119>International Organization for Standardization/International Electrotechnical Commission 27000:2018

Security techniques — Information security management systems — Overview and vocabulary

Publication date : 2018-02

5th Edition</obo:IAO_0000119>
        <obo:IAO_0000119>[SOURCE: ISO Guide 73:2009, 3.5.1.5]</obo:IAO_0000119>
    </owl:Class>
    


    <!-- http://www.ontologylibrary.mil/OperationalEnvironment/Mid/OEFutureWarfareOntology#RiskTreatment -->

    <owl:Class rdf:about="http://www.ontologylibrary.mil/OperationalEnvironment/Mid/OEFutureWarfareOntology#RiskTreatment">
        <rdfs:subClassOf rdf:resource="http://www.ontologylibrary.mil/OperationalEnvironment/Mid/OEFutureWarfareOntology#CyberSecurityControlledVocabulary"/>
        <obo:IAO_0000115>process (3.54) to modify risk (3.61)

Note 1 to entry: Risk treatment can involve:
— avoiding the risk by deciding not to start or continue with the activity that gives rise to the risk;
— taking or increasing risk in order to pursue an opportunity;
— removing the risk source;
— changing the likelihood (3.40);
— changing the consequences (3.12);
— sharing the risk with another party or parties (including contracts and risk financing);
— retaining the risk by informed choice.

Note 2 to entry: Risk treatments that deal with negative consequences are sometimes referred to as “risk mitigation”, “risk elimination”, “risk prevention” and “risk reduction”.

Note 3 to entry: Risk treatment can create new risks or modify existing risks.</obo:IAO_0000115>
        <obo:IAO_0000119>International Organization for Standardization/International Electrotechnical Commission 27000:2018

Security techniques — Information security management systems — Overview and vocabulary

Publication date : 2018-02

5th Edition</obo:IAO_0000119>
    </owl:Class>
    


    <!-- http://www.ontologylibrary.mil/OperationalEnvironment/Mid/OEFutureWarfareOntology#RoboticsControlledVocabulary -->

    <owl:Class rdf:about="http://www.ontologylibrary.mil/OperationalEnvironment/Mid/OEFutureWarfareOntology#RoboticsControlledVocabulary">
        <rdfs:subClassOf rdf:resource="http://www.ontologylibrary.mil/OperationalEnvironment/Mid/OEFutureWarfareOntology#ControlledVocabulary"/>
    </owl:Class>
    


    <!-- http://www.ontologylibrary.mil/OperationalEnvironment/Mid/OEFutureWarfareOntology#RoboticsTrend -->

    <owl:Class rdf:about="http://www.ontologylibrary.mil/OperationalEnvironment/Mid/OEFutureWarfareOntology#RoboticsTrend">
        <rdfs:subClassOf rdf:resource="http://www.ontologylibrary.mil/OperationalEnvironment/Mid/OEFutureWarfareOntology#Trend"/>
        <obo:IAO_0000115>Artificial Intelligence (AI) may be the most disruptive technology of our time: much of today’s “thought” is artificial, vice human.  Breakthroughs in AI and deep learning enable reasoning intelligent systems that, though not sentient, administer and optimize a great many aspects of modern life.  Advanced physio-mechanical interfaces enable humanmachine integration to include optimized searching of massive indexes of data, direct access to large-scale computing power, and life-like experiences through virtual reality. The revolutionary impact of “trans-humanism” challenges the very definition of “human” – with profound ethical dilemmas that remain unresolved. Big data techniques interrogate massive databases to discover hidden patterns and correlations that form the basis of modern advertising – and are continually leveraged for intelligence and security purposes by nation states and non-state entities alike.  Quantum computing, first applied to encryption functions, is now a key computing enabler, especially for artificial intelligence.9  A mature Internet of Things connects and integrates the devices of the information realm with formerly inert objects – structures, motors, or appliances -- of the physical realm.  Neuroscience has enhanced our understanding of brain function, including neural plasticity, and has enabled advanced techniques for human-machine interfacing. A better understanding of the machinery of the mind has found commercial application in the acceleration of speed and retention in learning.  In the most connected and wealthy parts of the world, cell phones and computers will all but disappear as physical, hand held devices.  Select individuals will directly connect to cyberspace through neural implants or augmented reality systems painted directly on a retina.  If we have not yet reached the “singularity”, where AI and machines are capable of outperforming the human mind, we will nonetheless have reached a point where AI, machines, and man-machine teaming open new possibilities in this realm.</obo:IAO_0000115>
        <obo:IAO_0000119>The Operational Environment and the Changing Character of Future Warfare</obo:IAO_0000119>
    </owl:Class>
    


    <!-- http://www.ontologylibrary.mil/OperationalEnvironment/Mid/OEFutureWarfareOntology#RotorInletTemperature -->

    <owl:Class rdf:about="http://www.ontologylibrary.mil/OperationalEnvironment/Mid/OEFutureWarfareOntology#RotorInletTemperature">
        <rdfs:subClassOf rdf:resource="http://www.ontologylibrary.mil/OperationalEnvironment/Mid/OEFutureWarfareOntology#GasEnergyGeneration"/>
        <obo:IAO_0000115>flow weighted mean total temperature of the working fluid relative to a stationary plane immediately upstream of the first rotating row of turbine blades
Note 1 to entry: Also known as the firing temperature.</obo:IAO_0000115>
        <obo:IAO_0000119>International Organization for Standardization/International ISO 19859:2016

Technical Committee : ISO/TC 192  Gas turbines

ICS :  29.160.99  Other standards related to rotating machinery 27.040  Gas and steam turbines. Steam engines

Gas turbine applications -- Requirements for power generation

Publication date : 2016-08

1st Edition</obo:IAO_0000119>
    </owl:Class>
    


    <!-- http://www.ontologylibrary.mil/OperationalEnvironment/Mid/OEFutureWarfareOntology#RuleOfLaw -->

    <owl:Class rdf:about="http://www.ontologylibrary.mil/OperationalEnvironment/Mid/OEFutureWarfareOntology#RuleOfLaw">
        <rdfs:subClassOf rdf:resource="http://www.ontologylibrary.mil/OperationalEnvironment/Mid/OEFutureWarfareOntology#JudicialSystem"/>
        <obo:IAO_0000115>(1)

In general, the rule of law implies that the creation of laws, their enforcement, and the relationships among legal rules are themselves legally regulated, so that no one—including the most highly placed official—is above the law. The legal constraint on rulers means that the government is subject to existing laws as much as its citizens are. Thus, a closely related notion is the idea of equality before the law, which holds that no “legal” person shall enjoy privileges that are not extended to all and that no person shall be immune from legal sanctions.</obo:IAO_0000115>
        <obo:IAO_0000115>(2)

Judicial independence means that judges are independent from political pressures and influences when they make their decisions. An independent judiciary is essential to maintaining the rule of law. Judges should not be pressured by a political party, a private interest, or popular opinion when they are called upon to determine what the law requires. Keeping the judiciary independent of these influences ensures that everyone has a fair chance to make their case in court and that judges will be impartial in making their decisions. Judges also must explain their decisions in public written opinions, and their decisions can be appealed to a higher court for review. These elements of judicial decision- making ensure that judges remain accountable to the rule of law.</obo:IAO_0000115>
        <obo:IAO_0000119>(1)

Naomi Choi, &quot;Rule of Law, Political Philosophy&quot;, Encyclopedia Britannica

March 12, 2019

https://www.britannica.com/topic/rule-of-law</obo:IAO_0000119>
        <obo:IAO_0000119>(2)

&quot;What Is the Rule of Law&quot;, American Bar Association Rule of Law Initiative

March 12, 2019

https://www.americanbar.org/advocacy/rule_of_law/what-is-the-rule-of-law/</obo:IAO_0000119>
        <rdfs:label>Rule of Law</rdfs:label>
    </owl:Class>
    


    <!-- http://www.ontologylibrary.mil/OperationalEnvironment/Mid/OEFutureWarfareOntology#Rural-urbanMigration -->

    <owl:Class rdf:about="http://www.ontologylibrary.mil/OperationalEnvironment/Mid/OEFutureWarfareOntology#Rural-urbanMigration">
        <rdfs:subClassOf rdf:resource="http://www.ontologylibrary.mil/OperationalEnvironment/Mid/OEFutureWarfareOntology#Migration"/>
        <obo:IAO_0000232>See the &quot;Urbanization&quot; class.  For a topic model that makes the sub-categories of &quot;Demographics&quot; topics in their own right, some or all of the vocabulary from &quot;Urbanization&quot;--at least, that pertaining to migration per se--would need to be duplicated here.</obo:IAO_0000232>
        <rdfs:label>Rural-urban Migration</rdfs:label>
    </owl:Class>
    


    <!-- http://www.ontologylibrary.mil/OperationalEnvironment/Mid/OEFutureWarfareOntology#SQL -->

    <owl:Class rdf:about="http://www.ontologylibrary.mil/OperationalEnvironment/Mid/OEFutureWarfareOntology#SQL">
        <rdfs:subClassOf rdf:resource="http://www.ontologylibrary.mil/OperationalEnvironment/Mid/OEFutureWarfareOntology#BigDataControlledVocabulary"/>
        <obo:IAO_0000115>database language specified by ISO/IEC 9075

Note 1 to entry: SQL is sometimes interpreted to stand for Structured Query Language, but that name is not used in ISO/IEC 9075.</obo:IAO_0000115>
        <obo:IAO_0000119>Information technology — Big data — Overview and vocabulary

https://www.iso.org/jtc1</obo:IAO_0000119>
    </owl:Class>
    


    <!-- http://www.ontologylibrary.mil/OperationalEnvironment/Mid/OEFutureWarfareOntology#Scaling -->

    <owl:Class rdf:about="http://www.ontologylibrary.mil/OperationalEnvironment/Mid/OEFutureWarfareOntology#Scaling">
        <rdfs:subClassOf rdf:resource="http://www.ontologylibrary.mil/OperationalEnvironment/Mid/OEFutureWarfareOntology#BigDataControlledVocabulary"/>
        <obo:IAO_0000115>Big data refers to the extensibility of data repositories and data processing across resources working in parallel, in the same way that the compute-intensive simulation community embraced massively parallel processing. By working out methods for communication among resources, the same scaling is now available to data-intensive applications. Vertical scaling implies increasing the system parameters of processing speed, storage, and memory for greater performance. This approach is limited by physical capabilities whose improvements have been described by Moore’s Law, requiring ever more sophisticated elements (e.g., hardware, software) that add time and expense to the implementation. The alternative method is to use horizontal scaling, to make use of distributed individual resources integrated to act as a single system. It is this horizontal scaling that is at the heart of the big data revolution. While the methods to achieve efficient scalability across resources will continually evolve, this paradigm shift (in analogy to the prior shift in the simulation community to parallel processing) is a one-time occurrence.</obo:IAO_0000115>
        <obo:IAO_0000119>Information technology — Big data — Overview and vocabulary

https://www.iso.org/jtc1</obo:IAO_0000119>
    </owl:Class>
    


    <!-- http://www.ontologylibrary.mil/OperationalEnvironment/Mid/OEFutureWarfareOntology#Scatter -->

    <owl:Class rdf:about="http://www.ontologylibrary.mil/OperationalEnvironment/Mid/OEFutureWarfareOntology#Scatter">
        <rdfs:subClassOf rdf:resource="http://www.ontologylibrary.mil/OperationalEnvironment/Mid/OEFutureWarfareOntology#BigDataControlledVocabulary"/>
        <obo:IAO_0000115>distribution of processing across multiple nodes in a cluster (3.1.4)</obo:IAO_0000115>
        <obo:IAO_0000119>Information technology — Big data — Overview and vocabulary

https://www.iso.org/jtc1</obo:IAO_0000119>
    </owl:Class>
    


    <!-- http://www.ontologylibrary.mil/OperationalEnvironment/Mid/OEFutureWarfareOntology#ScatterGather -->

    <owl:Class rdf:about="http://www.ontologylibrary.mil/OperationalEnvironment/Mid/OEFutureWarfareOntology#ScatterGather">
        <rdfs:subClassOf rdf:resource="http://www.ontologylibrary.mil/OperationalEnvironment/Mid/OEFutureWarfareOntology#BigDataControlledVocabulary"/>
        <obo:IAO_0000115>form of processing of large datasets (3.1.13) where the computation required is divided up and distributed across multiple nodes in a cluster and the overall result is combined from the results from each node

Note 1 to entry: Scatter-gather processing typically requires an algorithmic change to the processing software. An example of scatter-gather data processing is MapReduce.</obo:IAO_0000115>
        <obo:IAO_0000119>Information technology — Big data — Overview and vocabulary

https://www.iso.org/jtc1</obo:IAO_0000119>
    </owl:Class>
    


    <!-- http://www.ontologylibrary.mil/OperationalEnvironment/Mid/OEFutureWarfareOntology#Scope -->

    <owl:Class rdf:about="http://www.ontologylibrary.mil/OperationalEnvironment/Mid/OEFutureWarfareOntology#Scope">
        <rdfs:subClassOf rdf:resource="http://www.ontologylibrary.mil/OperationalEnvironment/Mid/OEFutureWarfareOntology#FaultLineMethodology"/>
        <obo:IAO_0000119>Fault Lines Methodology Infographic</obo:IAO_0000119>
        <CommonCoreOntologies:definition>SCOPE - Identify and outline the intent and outcome of the research. A scoping document provides the design and plan of research to fill an information requirement. The researcher provides the scoping document to the requestor for approval. The scoping document consists of the following sections: 

Background: 2-4 paragraphs outlining the nature of the project and a quick description of the OE. 

Justification/Purpose: A description of the knowledge gap/IR that the project intends to fill and the intended audience. 

Research question(s): Key assumptions and specific questions that the product will answer. Example research questions: What are the population’s grievances? What are the sources of instability? How might state and non-state actors exploit instability and grievances? 

Research method: The social science techniques used for data collection and analysis. Initial references: A list of potential sources of information for use in product development. 

Deliverable(s): A list of components that make up the final product (this could be one product). 

Point of contact: Who to contact with questions about the product. 

Timeline: A rough projection of the stages of development and timeline for deliverables. GCKN has a scoping document template to assist in this step.</CommonCoreOntologies:definition>
    </owl:Class>
    


    <!-- http://www.ontologylibrary.mil/OperationalEnvironment/Mid/OEFutureWarfareOntology#SecondaryData -->

    <owl:Class rdf:about="http://www.ontologylibrary.mil/OperationalEnvironment/Mid/OEFutureWarfareOntology#SecondaryData">
        <rdfs:subClassOf rdf:resource="http://www.ontologylibrary.mil/OperationalEnvironment/Mid/OEFutureWarfareOntology#ClimateChangeAndResourceCompetitionControlledVocabulary"/>
        <obo:IAO_0000115>data obtained from sources other than primary data (3.2.2)

Note 1 to entry: Such sources can include databases and published literature validated by competent authorities.</obo:IAO_0000115>
        <obo:IAO_0000119>International Organization for Standardization/International Electrotechnical Commission 27000:2018

Technical Committee : ISO/TC 207/SC 7  Greenhouse gas management and related activities

ICS :  13.020.40  Pollution, pollution control and conservation

Greenhouse gases -- Part 1: Specification with guidance at the organization level for quantification and reporting of greenhouse gas emissions and removals 

Publication date : 2018-12

2nd Edition</obo:IAO_0000119>
    </owl:Class>
    


    <!-- http://www.ontologylibrary.mil/OperationalEnvironment/Mid/OEFutureWarfareOntology#SecondaryFactors -->

    <owl:Class rdf:about="http://www.ontologylibrary.mil/OperationalEnvironment/Mid/OEFutureWarfareOntology#SecondaryFactors">
        <rdfs:subClassOf rdf:resource="http://www.ontologylibrary.mil/OperationalEnvironment/Mid/OEFutureWarfareOntology#SpaceEnvironmentControlledVocabulary"/>
        <obo:IAO_0000115>space factors appearing as a result of the impact of primary factors on materials but possessing of their own characteristics and physical mechanisms of the impact on materials
— spacecraft own atmosphere
— surface charging
— internal charging
— thermal cycling
— spacecraft operation factors: plasma sources (plasma contactors), electric propulsion engines and others</obo:IAO_0000115>
        <obo:IAO_0000119>International Organization for Standardization/International Electrotechnical Commission 17851:2016

Space systems -- Space environment simulation for material tests -- General principles and criteria

Publication Date: 2016-09

1st Edition</obo:IAO_0000119>
    </owl:Class>
    


    <!-- http://www.ontologylibrary.mil/OperationalEnvironment/Mid/OEFutureWarfareOntology#SecurityAndPrivacyFabric -->

    <owl:Class rdf:about="http://www.ontologylibrary.mil/OperationalEnvironment/Mid/OEFutureWarfareOntology#SecurityAndPrivacyFabric">
        <rdfs:subClassOf rdf:resource="http://www.ontologylibrary.mil/OperationalEnvironment/Mid/OEFutureWarfareOntology#BigDataRole"/>
        <obo:IAO_0000115>Security and privacy issues affect all other components of the NBDRA. The Security and Privacy Fabric interacts with the System Orchestrator for policy, requirements, and auditing and also with both the Big Data Application Provider and the Big Data Framework Provider for development, deployment, and operation. The NIST Big Data Interoperability Framework: Volume 4, Security and Privacy document discusses security and privacy topics.</obo:IAO_0000115>
        <obo:IAO_0000119>NIST Big Data Interoperability Framework: Volume 6, Reference Architecture

Final Version 1 

NIST Big Data Public Working Group (NBD-PWG) Reference Architecture Subgroup Information Technology Laboratory</obo:IAO_0000119>
    </owl:Class>
    


    <!-- http://www.ontologylibrary.mil/OperationalEnvironment/Mid/OEFutureWarfareOntology#SecurityAndViolentConflict -->

    <owl:Class rdf:about="http://www.ontologylibrary.mil/OperationalEnvironment/Mid/OEFutureWarfareOntology#SecurityAndViolentConflict">
        <rdfs:subClassOf rdf:resource="http://www.ontologylibrary.mil/OperationalEnvironment/Mid/OEFutureWarfareOntology#HumanFactorsControlledVocabulary"/>
        <rdfs:label>Security and Violent Conflict</rdfs:label>
    </owl:Class>
    


    <!-- http://www.ontologylibrary.mil/OperationalEnvironment/Mid/OEFutureWarfareOntology#SecurityImplementationStandard -->

    <owl:Class rdf:about="http://www.ontologylibrary.mil/OperationalEnvironment/Mid/OEFutureWarfareOntology#SecurityImplementationStandard">
        <rdfs:subClassOf rdf:resource="http://www.ontologylibrary.mil/OperationalEnvironment/Mid/OEFutureWarfareOntology#CyberSecurityControlledVocabulary"/>
        <obo:IAO_0000115>document specifying authorized ways for realizing security</obo:IAO_0000115>
        <obo:IAO_0000119>International Organization for Standardization/International Electrotechnical Commission 27000:2018

Security techniques — Information security management systems — Overview and vocabulary

Publication date : 2018-02

5th Edition</obo:IAO_0000119>
    </owl:Class>
    


    <!-- http://www.ontologylibrary.mil/OperationalEnvironment/Mid/OEFutureWarfareOntology#SemanticKnowledgeRepresentation -->

    <owl:Class rdf:about="http://www.ontologylibrary.mil/OperationalEnvironment/Mid/OEFutureWarfareOntology#SemanticKnowledgeRepresentation">
        <rdfs:subClassOf rdf:resource="http://www.ontologylibrary.mil/OperationalEnvironment/Mid/OEFutureWarfareOntology#ArtificialIntelligenceControlledVocabulary"/>
        <obo:IAO_0000115>Algorithms* to formulate a sentence written in any language (for example, “Paul takes the bus to Berlin”) in logical form, so that a computer is able to interpret it. The machine can then make logical inferences (like deductions) that enable it to classify words into different categories and analyse the sentences submitted to it.</obo:IAO_0000115>
        <obo:IAO_0000119>United Nations Educational, Scientific, and Cultural Organization Courier 

March 2018

https://en.unesco.org/courier/2018-3/lexicon-artificial-intelligence</obo:IAO_0000119>
    </owl:Class>
    


    <!-- http://www.ontologylibrary.mil/OperationalEnvironment/Mid/OEFutureWarfareOntology#SentientData -->

    <owl:Class rdf:about="http://www.ontologylibrary.mil/OperationalEnvironment/Mid/OEFutureWarfareOntology#SentientData">
        <rdfs:subClassOf rdf:resource="http://www.ontologylibrary.mil/OperationalEnvironment/Mid/OEFutureWarfareOntology#SystemsThatSeeThinkCommunicate"/>
        <obo:IAO_0000115>Pinpoints who can/cannot access and interact with, without human intervention. [SOURCE: TRADOC G-2 Potential Game Changers, May 2018]</obo:IAO_0000115>
        <obo:IAO_0000119>Technology Environment of Ground Warfare in 2035-2050

Projections made in 2018 by ARL and TRADOC

[This is a draft outline of a potential document; prepared by Alexander Kott, the US Army Research Laboratory; July 2018]</obo:IAO_0000119>
    </owl:Class>
    


    <!-- http://www.ontologylibrary.mil/OperationalEnvironment/Mid/OEFutureWarfareOntology#SequentialCombustion -->

    <owl:Class rdf:about="http://www.ontologylibrary.mil/OperationalEnvironment/Mid/OEFutureWarfareOntology#SequentialCombustion">
        <rdfs:subClassOf rdf:resource="http://www.ontologylibrary.mil/OperationalEnvironment/Mid/OEFutureWarfareOntology#GasEnergyGeneration"/>
        <obo:IAO_0000115>process created by a gas turbine that typically consists of two combustors, a high pressure combustor followed by a high pressure turbine and a low pressure combustor followed by a low pressure turbine</obo:IAO_0000115>
        <obo:IAO_0000119>International Organization for Standardization/International ISO 19859:2016

Technical Committee : ISO/TC 192  Gas turbines

ICS :  29.160.99  Other standards related to rotating machinery 27.040  Gas and steam turbines. Steam engines

Gas turbine applications -- Requirements for power generation

Publication date : 2016-08

1st Edition</obo:IAO_0000119>
    </owl:Class>
    


    <!-- http://www.ontologylibrary.mil/OperationalEnvironment/Mid/OEFutureWarfareOntology#ServiceSector -->

    <owl:Class rdf:about="http://www.ontologylibrary.mil/OperationalEnvironment/Mid/OEFutureWarfareOntology#ServiceSector">
        <rdfs:subClassOf rdf:resource="http://www.ontologylibrary.mil/OperationalEnvironment/Mid/OEFutureWarfareOntology#EconomicActivity"/>
        <obo:IAO_0000119>(1)

Editors of Encyclopaedia Britannica, &quot;Service Industry, Economics&quot;, Encyclodpaedia Britannica

March 14, 2019

https://www.britannica.com/topic/service-industry</obo:IAO_0000119>
        <obo:IAO_0000119>(2)

&quot;What is Service Sector&quot;, IGI Global

https://www.igi-global.com/dictionary/service-sector/47133</obo:IAO_0000119>
        <obo:IAO_0000119>(3)

Will Kenton, &quot;Service Sector&quot;, Investopedia

https://www.investopedia.com/terms/s/service-sector.asp</obo:IAO_0000119>
        <CommonCoreOntologies:definition>(1)

Service industries include everything else: banking, communications, wholesale and retail trade, all professional services such as engineering, computer software development, and medicine, nonprofit economic activity, all consumer services, and all government services, including defense and administration of justice.</CommonCoreOntologies:definition>
        <CommonCoreOntologies:definition>(2)

Activities in the service sector include retail, banks, hotels, real estate, education, health, social work, computer services, recreation, media, communications, electricity, gas and water supply.</CommonCoreOntologies:definition>
        <CommonCoreOntologies:definition>(3)

Technology, specifically information technology systems, is shaping the way businesses in the service sector operate. In nearly all industries within the sector, businesses institute technology to bolster production, increase speed and efficiency and cut down on the number of employees required for operation. This cuts down on costs and improves incoming revenue streams.</CommonCoreOntologies:definition>
        <rdfs:label>Service Sector</rdfs:label>
    </owl:Class>
    


    <!-- http://www.ontologylibrary.mil/OperationalEnvironment/Mid/OEFutureWarfareOntology#Sex-selectiveAbortion -->

    <owl:Class rdf:about="http://www.ontologylibrary.mil/OperationalEnvironment/Mid/OEFutureWarfareOntology#Sex-selectiveAbortion">
        <rdfs:subClassOf rdf:resource="http://www.ontologylibrary.mil/OperationalEnvironment/Mid/OEFutureWarfareOntology#SkewedSexRatio"/>
        <obo:IAO_0000119>&quot;Sex-selective Abortions During Past Three Decades May Explain Absence of Millions of Girls in India&quot;, International Perspectives on Sexual and Reproductive Health

September 27, 2011

https://www.guttmacher.org/journals/ipsrh/2011/09/sex-selective-abortions-during-past-three-decades-may-explain-absence</obo:IAO_0000119>
        <CommonCoreOntologies:definition>[The researchers] suggest that the increases in sex-selective abortion may be due to son preference combined with declines in fertility; the finding that selective abortion of females appears to be especially common among educated and wealthy women may reflect that these women are better able than others to afford ultrasound and abortion services.</CommonCoreOntologies:definition>
        <rdfs:label>Sex-selective Abortion</rdfs:label>
    </owl:Class>
    


    <!-- http://www.ontologylibrary.mil/OperationalEnvironment/Mid/OEFutureWarfareOntology#Shantytown -->

    <owl:Class rdf:about="http://www.ontologylibrary.mil/OperationalEnvironment/Mid/OEFutureWarfareOntology#Shantytown">
        <rdfs:subClassOf rdf:resource="http://www.ontologylibrary.mil/OperationalEnvironment/Mid/OEFutureWarfareOntology#Urbanization"/>
        <obo:IAO_0000119>&quot;Shanty Town&quot;, Wikipedia

March 26, 2019

https://en.wikipedia.org/wiki/Shanty_town</obo:IAO_0000119>
        <CommonCoreOntologies:definition>A shanty town or squatter area is a settlement of improvised housing which is known as shanties or shacks, made of plywood, corrugated metal, sheets of plastic, and cardboard boxes. Such settlements are usually found on the periphery of cities, in public parks, or near railroad tracks, rivers, lagoons or city trash dump sites. Sometimes called a squatter, or spontaneous settlement, a typical shanty town often lacks adequate infrastructure, including proper sanitation, safe water supply, electricity, hygienic streets, or other basic necessities to support human settlements.

Shanty towns are mostly found in developing nations....

Since construction is informal and unguided by urban planning, there is typically no formal street grid, house numbers, or named streets. Such settlements also lack some or all basic public services such as a sewage network, electricity, safe running water, rain water drainage, garbage removal, access to public transport, or insect and disease control services. Even if these resources are present, they are likely to be disorganized, unreliable, and poorly maintained. Shanty towns also tend to lack basic services present in more formally organized settlements, including policing, mail delivery, medical services, and fire fighting.</CommonCoreOntologies:definition>
        <rdfs:label>Shanty Town</rdfs:label>
        <rdfs:label>Shantytown</rdfs:label>
    </owl:Class>
    


    <!-- http://www.ontologylibrary.mil/OperationalEnvironment/Mid/OEFutureWarfareOntology#SignificantEnergyUse -->

    <owl:Class rdf:about="http://www.ontologylibrary.mil/OperationalEnvironment/Mid/OEFutureWarfareOntology#SignificantEnergyUse">
        <rdfs:subClassOf rdf:resource="http://www.ontologylibrary.mil/OperationalEnvironment/Mid/OEFutureWarfareOntology#PowerGenerationAndStorageControlledVocabulary"/>
        <obo:IAO_0000115>energy use (3.5.4) accounting for substantial energy consumption (3.5.2) and/or offering considerable potential for energy performance improvement (3.4.6)

Note 1 to entry: Significance criteria are determined by the organization (3.1.1).

Note 2 to entry: SEUs can be facilities, systems, processes, or equipment.</obo:IAO_0000115>
        <obo:IAO_0000119>International Organization for Standardization/International ISO 50001:2018

Technical Committee : ISO/TC 301  Energy management and energy savings

ICS :  27.015  Energy efficiency. Energy conservation in general 03.100.70 Management systems

Energy management systems -- Requirements with guidance for use

Publication date : 2018-08

2nd Edition</obo:IAO_0000119>
    </owl:Class>
    


    <!-- http://www.ontologylibrary.mil/OperationalEnvironment/Mid/OEFutureWarfareOntology#SignificantIndirectGreenhouseGasEmission -->

    <owl:Class rdf:about="http://www.ontologylibrary.mil/OperationalEnvironment/Mid/OEFutureWarfareOntology#SignificantIndirectGreenhouseGasEmission">
        <rdfs:subClassOf rdf:resource="http://www.ontologylibrary.mil/OperationalEnvironment/Mid/OEFutureWarfareOntology#ClimateChangeAndResourceCompetitionControlledVocabulary"/>
        <obo:IAO_0000115>organization’s (3.4.2) quantified and reported GHGemissions (3.1.5) complying with the significance criteria set by the organization</obo:IAO_0000115>
        <obo:IAO_0000119>International Organization for Standardization/International Electrotechnical Commission 27000:2018

Technical Committee : ISO/TC 207/SC 7  Greenhouse gas management and related activities

ICS :  13.020.40  Pollution, pollution control and conservation

Greenhouse gases -- Part 1: Specification with guidance at the organization level for quantification and reporting of greenhouse gas emissions and removals 

Publication date : 2018-12

2nd Edition</obo:IAO_0000119>
    </owl:Class>
    


    <!-- http://www.ontologylibrary.mil/OperationalEnvironment/Mid/OEFutureWarfareOntology#SilicaAerogel -->

    <owl:Class rdf:about="http://www.ontologylibrary.mil/OperationalEnvironment/Mid/OEFutureWarfareOntology#SilicaAerogel">
        <rdfs:subClassOf rdf:resource="http://www.ontologylibrary.mil/OperationalEnvironment/Mid/OEFutureWarfareOntology#SpaceSystems"/>
        <obo:IAO_0000115>low-density solid material, made with a porous, silica-based structure, used for the retrieval of ejecta fragments in impact experiments</obo:IAO_0000115>
        <obo:IAO_0000119>International Organization for Standardization/International Electrotechnical Commission 11227:2012

Space systems — Test procedure to evaluate spacecraft material ejecta upon hypervelocity impact

Publication Date: 2012-09

1st Edition</obo:IAO_0000119>
    </owl:Class>
    


    <!-- http://www.ontologylibrary.mil/OperationalEnvironment/Mid/OEFutureWarfareOntology#SiteSpecificData -->

    <owl:Class rdf:about="http://www.ontologylibrary.mil/OperationalEnvironment/Mid/OEFutureWarfareOntology#SiteSpecificData">
        <rdfs:subClassOf rdf:resource="http://www.ontologylibrary.mil/OperationalEnvironment/Mid/OEFutureWarfareOntology#ClimateChangeAndResourceCompetitionControlledVocabulary"/>
        <obo:IAO_0000115>primary data (3.2.2) obtained within the organizational boundary (3.4.7)

Note 1 to entry: All site-specific data are primary data, but not all primary data are site-specific data.</obo:IAO_0000115>
        <obo:IAO_0000119>International Organization for Standardization/International Electrotechnical Commission 27000:2018

Technical Committee : ISO/TC 207/SC 7  Greenhouse gas management and related activities

ICS :  13.020.40  Pollution, pollution control and conservation

Greenhouse gases -- Part 1: Specification with guidance at the organization level for quantification and reporting of greenhouse gas emissions and removals 

Publication date : 2018-12

2nd Edition</obo:IAO_0000119>
    </owl:Class>
    


    <!-- http://www.ontologylibrary.mil/OperationalEnvironment/Mid/OEFutureWarfareOntology#SkewedSexRatio -->

    <owl:Class rdf:about="http://www.ontologylibrary.mil/OperationalEnvironment/Mid/OEFutureWarfareOntology#SkewedSexRatio">
        <rdfs:subClassOf rdf:resource="http://www.ontologylibrary.mil/OperationalEnvironment/Mid/OEFutureWarfareOntology#Demographics"/>
        <obo:IAO_0000119>(1)

Jospeh Chamie, &quot;Six Asian Nations Lead in Seriously Skewed Sex Ratios as Birth&quot;, PassBlue

September 28, 2016

https://www.passblue.com/2016/09/28/six-asian-nations-lead-in-seriously-skewed-sex-ratios-at-birth/</obo:IAO_0000119>
        <obo:IAO_0000119>(2)

Simon Denyer &amp; Annie Gowen, &quot;Too Many Men:  China and India Battle with the Consequences of Gender Imbalance&quot;

April 24, 2018

https://www.scmp.com/magazines/post-magazine/long-reads/article/2142658/too-many-men-china-and-india-battle-consequences</obo:IAO_0000119>
        <CommonCoreOntologies:definition>(1)

[S]ex imbalances at birth are primarily a result of a combination of three important factors: a strong preference of couples for sons over daughters; fetal-sex determination followed by abortions of female fetuses; and rapid declines in the number of children per couple to comparatively low levels.</CommonCoreOntologies:definition>
        <CommonCoreOntologies:definition>(2)

The consequences of having too many men, now coming of age, are far-reaching: beyond an epidemic of loneliness, the imbalance distorts labour markets, drives up savings rates...and drives down consumption, artificially inflates certain property values and parallels increases in violent crime, trafficking or prostitution in a growing number of locations.</CommonCoreOntologies:definition>
        <rdfs:label>Skewed Sex Ratio</rdfs:label>
    </owl:Class>
    


    <!-- http://www.ontologylibrary.mil/OperationalEnvironment/Mid/OEFutureWarfareOntology#SoldierCognitiveDomainEnhancement -->

    <owl:Class rdf:about="http://www.ontologylibrary.mil/OperationalEnvironment/Mid/OEFutureWarfareOntology#SoldierCognitiveDomainEnhancement">
        <rdfs:subClassOf rdf:resource="http://www.ontologylibrary.mil/OperationalEnvironment/Mid/OEFutureWarfareOntology#CombatApplication"/>
        <rdfs:subClassOf>
            <owl:Restriction>
                <owl:onProperty rdf:resource="http://www.ontologylibrary.mil/OperationalEnvironment/Mid/OEFutureWarfareOntology#hasCategoryOfEffort"/>
                <owl:someValuesFrom rdf:resource="http://www.ontologylibrary.mil/OperationalEnvironment/Mid/OEFutureWarfareOntology#SystemsThatSoldier"/>
            </owl:Restriction>
        </rdfs:subClassOf>
        <obo:IAO_0000115>Soldiers operate in environments that are highly dynamic, increasingly complex, and physically demanding. Therefore, both their physical and cognitive burden must be mitigated while maintaining overmatch. ARL&apos;s research in the area of augmentation aims to reduce the effects of burden and exploit technological and scientific advances in the field of capability enhancement while ensuring that the augmentation adapts to the Soldier instead of requiring the Soldier to adapt to the augmentation. Augmentation focuses on enabling superhuman performance and increasing resilience during sustained activities in both training and operational domains. Though interconnected, performance enhancement and resilience enhancement are distinct areas of research. Innovations in cognitive and physical augmentation systems that are matched to individual capabilities and accommodate the operational environment are expected to significantly impact warfighter situational awareness, physical prowess and decision making. Innovations are also expected to enhance warfighter physical capabilities by balancing load and improving protection and performance.</obo:IAO_0000115>
        <obo:IAO_0000119>Army Research Laboratory

https://www.arl.army.mil/www/default.cfm?page=2645</obo:IAO_0000119>
    </owl:Class>
    


    <!-- http://www.ontologylibrary.mil/OperationalEnvironment/Mid/OEFutureWarfareOntology#SoldierPhysicalDomainEnhancement -->

    <owl:Class rdf:about="http://www.ontologylibrary.mil/OperationalEnvironment/Mid/OEFutureWarfareOntology#SoldierPhysicalDomainEnhancement">
        <rdfs:subClassOf rdf:resource="http://www.ontologylibrary.mil/OperationalEnvironment/Mid/OEFutureWarfareOntology#CombatApplication"/>
        <rdfs:subClassOf>
            <owl:Restriction>
                <owl:onProperty rdf:resource="http://www.ontologylibrary.mil/OperationalEnvironment/Mid/OEFutureWarfareOntology#hasCategoryOfEffort"/>
                <owl:someValuesFrom rdf:resource="http://www.ontologylibrary.mil/OperationalEnvironment/Mid/OEFutureWarfareOntology#SystemsThatSoldier"/>
            </owl:Restriction>
        </rdfs:subClassOf>
        <obo:IAO_0000115>Soldiers operate in environments that are highly dynamic, increasingly complex, and physically demanding. Therefore, both their physical and cognitive burden must be mitigated while maintaining overmatch. ARL&apos;s research in the area of augmentation aims to reduce the effects of burden and exploit technological and scientific advances in the field of capability enhancement while ensuring that the augmentation adapts to the Soldier instead of requiring the Soldier to adapt to the augmentation. Augmentation focuses on enabling superhuman performance and increasing resilience during sustained activities in both training and operational domains. Though interconnected, performance enhancement and resilience enhancement are distinct areas of research. Innovations in cognitive and physical augmentation systems that are matched to individual capabilities and accommodate the operational environment are expected to significantly impact warfighter situational awareness, physical prowess and decision making. Innovations are also expected to enhance warfighter physical capabilities by balancing load and improving protection and performance.</obo:IAO_0000115>
        <obo:IAO_0000119>Army Research Laboratory

https://www.arl.army.mil/www/default.cfm?page=2645</obo:IAO_0000119>
    </owl:Class>
    


    <!-- http://www.ontologylibrary.mil/OperationalEnvironment/Mid/OEFutureWarfareOntology#SoldierPsychologicalDomainEnhancement -->

    <owl:Class rdf:about="http://www.ontologylibrary.mil/OperationalEnvironment/Mid/OEFutureWarfareOntology#SoldierPsychologicalDomainEnhancement">
        <rdfs:subClassOf rdf:resource="http://www.ontologylibrary.mil/OperationalEnvironment/Mid/OEFutureWarfareOntology#CombatApplication"/>
        <rdfs:subClassOf>
            <owl:Restriction>
                <owl:onProperty rdf:resource="http://www.ontologylibrary.mil/OperationalEnvironment/Mid/OEFutureWarfareOntology#hasCategoryOfEffort"/>
                <owl:someValuesFrom rdf:resource="http://www.ontologylibrary.mil/OperationalEnvironment/Mid/OEFutureWarfareOntology#SystemsThatSoldier"/>
            </owl:Restriction>
        </rdfs:subClassOf>
        <obo:IAO_0000115>Soldiers operate in environments that are highly dynamic, increasingly complex, and physically demanding. Therefore, both their physical and cognitive burden must be mitigated while maintaining overmatch. ARL&apos;s research in the area of augmentation aims to reduce the effects of burden and exploit technological and scientific advances in the field of capability enhancement while ensuring that the augmentation adapts to the Soldier instead of requiring the Soldier to adapt to the augmentation. Augmentation focuses on enabling superhuman performance and increasing resilience during sustained activities in both training and operational domains. Though interconnected, performance enhancement and resilience enhancement are distinct areas of research. Innovations in cognitive and physical augmentation systems that are matched to individual capabilities and accommodate the operational environment are expected to significantly impact warfighter situational awareness, physical prowess and decision making. Innovations are also expected to enhance warfighter physical capabilities by balancing load and improving protection and performance.</obo:IAO_0000115>
        <obo:IAO_0000119>Army Research Laboratory

https://www.arl.army.mil/www/default.cfm?page=2645</obo:IAO_0000119>
    </owl:Class>
    


    <!-- http://www.ontologylibrary.mil/OperationalEnvironment/Mid/OEFutureWarfareOntology#SoldierWearableInterface -->

    <owl:Class rdf:about="http://www.ontologylibrary.mil/OperationalEnvironment/Mid/OEFutureWarfareOntology#SoldierWearableInterface">
        <rdfs:subClassOf rdf:resource="http://www.ontologylibrary.mil/OperationalEnvironment/Mid/OEFutureWarfareOntology#SystemsThatSoldier"/>
        <obo:IAO_0000115>Soldier-wearable interface for immersive training, including AI-based “virtual coach” Soldier interface that: - Functions pervasively to provide relevant feedback for real-world learning - Recognizes and exploits similarities across Soldier tasks to speed learning - Applies augmentation approaches to optimize cognitive and affective states for learning [SOURCE: ARL ERP documents]</obo:IAO_0000115>
        <obo:IAO_0000119>Technology Environment of Ground Warfare in 2035-2050

Projections made in 2018 by ARL and TRADOC

[This is a draft outline of a potential document; prepared by Alexander Kott, the US Army Research Laboratory; July 2018]</obo:IAO_0000119>
    </owl:Class>
    


    <!-- http://www.ontologylibrary.mil/OperationalEnvironment/Mid/OEFutureWarfareOntology#SpaceEnvironmentControlledVocabulary -->

    <owl:Class rdf:about="http://www.ontologylibrary.mil/OperationalEnvironment/Mid/OEFutureWarfareOntology#SpaceEnvironmentControlledVocabulary">
        <rdfs:subClassOf rdf:resource="http://www.ontologylibrary.mil/OperationalEnvironment/Mid/OEFutureWarfareOntology#CyberAndSpaceControlledVocabulary"/>
    </owl:Class>
    


    <!-- http://www.ontologylibrary.mil/OperationalEnvironment/Mid/OEFutureWarfareOntology#SpaceSystems -->

    <owl:Class rdf:about="http://www.ontologylibrary.mil/OperationalEnvironment/Mid/OEFutureWarfareOntology#SpaceSystems">
        <rdfs:subClassOf rdf:resource="http://www.ontologylibrary.mil/OperationalEnvironment/Mid/OEFutureWarfareOntology#SpaceEnvironmentControlledVocabulary"/>
    </owl:Class>
    


    <!-- http://www.ontologylibrary.mil/OperationalEnvironment/Mid/OEFutureWarfareOntology#Spall -->

    <owl:Class rdf:about="http://www.ontologylibrary.mil/OperationalEnvironment/Mid/OEFutureWarfareOntology#Spall">
        <rdfs:subClassOf rdf:resource="http://www.ontologylibrary.mil/OperationalEnvironment/Mid/OEFutureWarfareOntology#SpaceSystems"/>
        <obo:IAO_0000115>piece of material broken and ejected upon high-velocity impact, usually by stress waves, mainly on brittle material

Note 1 to entry: If the resulting tensile stress caused by the reflection of the compression wave on the surface (front or back) exceeds the tensile strength of the material, a thin sheet of material separates from the target and is ejected.</obo:IAO_0000115>
        <obo:IAO_0000119>International Organization for Standardization/International Electrotechnical Commission 11227:2012

Space systems — Test procedure to evaluate spacecraft material ejecta upon hypervelocity impact

Publication Date: 2012-09

1st Edition</obo:IAO_0000119>
    </owl:Class>
    


    <!-- http://www.ontologylibrary.mil/OperationalEnvironment/Mid/OEFutureWarfareOntology#Specimen -->

    <owl:Class rdf:about="http://www.ontologylibrary.mil/OperationalEnvironment/Mid/OEFutureWarfareOntology#Specimen">
        <rdfs:subClassOf rdf:resource="http://www.ontologylibrary.mil/OperationalEnvironment/Mid/OEFutureWarfareOntology#SpaceSystems"/>
        <obo:IAO_0000115>target representative sample of a spacecraft material that is used in impact experiments</obo:IAO_0000115>
        <obo:IAO_0000119>International Organization for Standardization/International Electrotechnical Commission 11227:2012

Space systems — Test procedure to evaluate spacecraft material ejecta upon hypervelocity impact

Publication Date: 2012-09

1st Edition</obo:IAO_0000119>
    </owl:Class>
    


    <!-- http://www.ontologylibrary.mil/OperationalEnvironment/Mid/OEFutureWarfareOntology#StaticFactor -->

    <owl:Class rdf:about="http://www.ontologylibrary.mil/OperationalEnvironment/Mid/OEFutureWarfareOntology#StaticFactor">
        <rdfs:subClassOf rdf:resource="http://www.ontologylibrary.mil/OperationalEnvironment/Mid/OEFutureWarfareOntology#PowerGenerationAndStorageControlledVocabulary"/>
        <obo:IAO_0000115>identified factor that significantly impacts energy performance (3.4.3) and does not routinely change

Note 1 to entry: Significance criteria are determined by the organization (3.1.1).

EXAMPLE:Facility size; design of installed equipment; number of weekly shifts; range of products.

[SOURCE: ISO 50015:2014, 3.22, modified — Note 1 to entry and EXAMPLE 1 have been modified and EXAMPLE 2 has been deleted.]</obo:IAO_0000115>
        <obo:IAO_0000119>International Organization for Standardization/International ISO 50001:2018

Technical Committee : ISO/TC 301  Energy management and energy savings

ICS :  27.015  Energy efficiency. Energy conservation in general 03.100.70 Management systems

Energy management systems -- Requirements with guidance for use

Publication date : 2018-08

2nd Edition</obo:IAO_0000119>
    </owl:Class>
    


    <!-- http://www.ontologylibrary.mil/OperationalEnvironment/Mid/OEFutureWarfareOntology#StealthCommunications -->

    <owl:Class rdf:about="http://www.ontologylibrary.mil/OperationalEnvironment/Mid/OEFutureWarfareOntology#StealthCommunications">
        <rdfs:subClassOf rdf:resource="http://www.ontologylibrary.mil/OperationalEnvironment/Mid/OEFutureWarfareOntology#SystemsThatProtect"/>
        <obo:IAO_0000115>Stealth communications, nearly undetectable by the adversary based on novel physical principles such as quantum [SOURCE: ARL ERP documents]</obo:IAO_0000115>
        <obo:IAO_0000119>Technology Environment of Ground Warfare in 2035-2050

Projections made in 2018 by ARL and TRADOC

[This is a draft outline of a potential document; prepared by Alexander Kott, the US Army Research Laboratory; July 2018]</obo:IAO_0000119>
    </owl:Class>
    


    <!-- http://www.ontologylibrary.mil/OperationalEnvironment/Mid/OEFutureWarfareOntology#StreamingData -->

    <owl:Class rdf:about="http://www.ontologylibrary.mil/OperationalEnvironment/Mid/OEFutureWarfareOntology#StreamingData">
        <rdfs:subClassOf rdf:resource="http://www.ontologylibrary.mil/OperationalEnvironment/Mid/OEFutureWarfareOntology#BigDataControlledVocabulary"/>
        <obo:IAO_0000115>data (3.1.5) passing across an interface from a source that is operating continuously</obo:IAO_0000115>
        <obo:IAO_0000119>Information technology — Big data — Overview and vocabulary

https://www.iso.org/jtc1</obo:IAO_0000119>
        <obo:IAO_0000119>[SOURCE: ISO/IEC 19784 4:2011, 4.4]</obo:IAO_0000119>
    </owl:Class>
    


    <!-- http://www.ontologylibrary.mil/OperationalEnvironment/Mid/OEFutureWarfareOntology#Stress -->

    <owl:Class rdf:about="http://www.ontologylibrary.mil/OperationalEnvironment/Mid/OEFutureWarfareOntology#Stress">
        <rdfs:subClassOf rdf:resource="http://www.ontologylibrary.mil/OperationalEnvironment/Mid/OEFutureWarfareOntology#SpaceSystems"/>
        <obo:IAO_0000115>force exerted on a body that tends to strain or to deform its shape.</obo:IAO_0000115>
        <obo:IAO_0000119>International Organization for Standardization/International Electrotechnical Commission 11227:2012

Space systems — Test procedure to evaluate spacecraft material ejecta upon hypervelocity impact

Publication Date: 2012-09

1st Edition</obo:IAO_0000119>
    </owl:Class>
    


    <!-- http://www.ontologylibrary.mil/OperationalEnvironment/Mid/OEFutureWarfareOntology#StrongAI -->

    <owl:Class rdf:about="http://www.ontologylibrary.mil/OperationalEnvironment/Mid/OEFutureWarfareOntology#StrongAI">
        <rdfs:subClassOf rdf:resource="http://www.ontologylibrary.mil/OperationalEnvironment/Mid/OEFutureWarfareOntology#ArtificialIntelligenceControlledVocabulary"/>
        <obo:IAO_0000115>Strong AI or AGI would be a machine that has consciousness and feelings, and is capable of providing  solutions for any kind of problem – that is pure fiction, for now.</obo:IAO_0000115>
        <obo:IAO_0000119>United Nations Educational, Scientific, and Cultural Organization Courier 

March 2018

https://en.unesco.org/courier/2018-3/lexicon-artificial-intelligence</obo:IAO_0000119>
    </owl:Class>
    


    <!-- http://www.ontologylibrary.mil/OperationalEnvironment/Mid/OEFutureWarfareOntology#StructuredData -->

    <owl:Class rdf:about="http://www.ontologylibrary.mil/OperationalEnvironment/Mid/OEFutureWarfareOntology#StructuredData">
        <rdfs:subClassOf rdf:resource="http://www.ontologylibrary.mil/OperationalEnvironment/Mid/OEFutureWarfareOntology#BigDataControlledVocabulary"/>
        <obo:IAO_0000115>data (3.1.5) which are characterized by not having any structure apart from that record or file level”

Note 1 to entry: On the whole unstructured data is not composed of data elements.

Example: An example of unstructured data is free text.</obo:IAO_0000115>
        <obo:IAO_0000119>Information technology — Big data — Overview and vocabulary

https://www.iso.org/jtc1</obo:IAO_0000119>
    </owl:Class>
    


    <!-- http://www.ontologylibrary.mil/OperationalEnvironment/Mid/OEFutureWarfareOntology#SubjectMatterExpertChecks -->

    <owl:Class rdf:about="http://www.ontologylibrary.mil/OperationalEnvironment/Mid/OEFutureWarfareOntology#SubjectMatterExpertChecks">
        <rdfs:subClassOf rdf:resource="http://www.ontologylibrary.mil/OperationalEnvironment/Mid/OEFutureWarfareOntology#FaultLineMethodology"/>
        <obo:IAO_0000115>Improve the accuracy, credibility, and validity of the analysis. Present the fault lines analysis to the initial group of SMEs once it is fully formed for feedback as to the product’s ability to fully answer the research question accurately.  GCKN can also serve as an expert check both in the quality of the product as well as with the format and delivery of the product.</obo:IAO_0000115>
        <obo:IAO_0000119>Fault Lines Methodology Infographic</obo:IAO_0000119>
    </owl:Class>
    


    <!-- http://www.ontologylibrary.mil/OperationalEnvironment/Mid/OEFutureWarfareOntology#SubstateConflict -->

    <owl:Class rdf:about="http://www.ontologylibrary.mil/OperationalEnvironment/Mid/OEFutureWarfareOntology#SubstateConflict">
        <rdfs:subClassOf rdf:resource="http://www.ontologylibrary.mil/OperationalEnvironment/Mid/OEFutureWarfareOntology#SecurityAndViolentConflict"/>
    </owl:Class>
    


    <!-- http://www.ontologylibrary.mil/OperationalEnvironment/Mid/OEFutureWarfareOntology#SupranationalOrganization -->

    <owl:Class rdf:about="http://www.ontologylibrary.mil/OperationalEnvironment/Mid/OEFutureWarfareOntology#SupranationalOrganization">
        <rdfs:subClassOf rdf:resource="http://www.ontologylibrary.mil/OperationalEnvironment/Mid/OEFutureWarfareOntology#InternationalSystem"/>
        <obo:IAO_0000115>(1)

A supranational union is a type of multinational political union where negotiated power is delegated to an authority by governments of member states.</obo:IAO_0000115>
        <obo:IAO_0000115>(2)

In addition to basic trade, supranational organizations may be involved in other activities designed to promote international standards. This can include activities related to food production, such as agriculture and fisheries, and those concerning the environment or energy production.

Supranational organizations may also be involved in education and forms of foreign aid or assistance to countries. Certain organizations are involved in areas with significant political impact on the member nations, including arms, the acceptable treatment of prisoners of war, nuclear power, and other nuclear-development capabilities.</obo:IAO_0000115>
        <obo:IAO_0000119>(1)

&quot;Supranational Union&quot;, Wikipedia

March 13, 2019

https://en.wikipedia.org/wiki/Supranational_union</obo:IAO_0000119>
        <obo:IAO_0000119>(2)

Marshall Hargrave, &quot;Supranational&quot;, Investopedia

March 13, 2019

https://www.investopedia.com/terms/s/supranational.asp</obo:IAO_0000119>
        <rdfs:label>Supranational Organization</rdfs:label>
    </owl:Class>
    


    <!-- http://www.ontologylibrary.mil/OperationalEnvironment/Mid/OEFutureWarfareOntology#SurfaceImpactFactors -->

    <owl:Class rdf:about="http://www.ontologylibrary.mil/OperationalEnvironment/Mid/OEFutureWarfareOntology#SurfaceImpactFactors">
        <rdfs:subClassOf rdf:resource="http://www.ontologylibrary.mil/OperationalEnvironment/Mid/OEFutureWarfareOntology#SpaceEnvironmentControlledVocabulary"/>
        <obo:IAO_0000112>EXAMPLE:Plasma, ultraviolet (UV) and vacuum ultraviolet (VUV), and hard microparticles.</obo:IAO_0000112>
        <obo:IAO_0000115>space factors which impact changes in the characteristics or properties of near-surface layers of materials (with depth of less than ~100 μm)</obo:IAO_0000115>
        <obo:IAO_0000119>International Organization for Standardization/International Electrotechnical Commission 17851:2016

Space systems -- Space environment simulation for material tests -- General principles and criteria

Publication Date: 2016-09

1st Edition</obo:IAO_0000119>
    </owl:Class>
    


    <!-- http://www.ontologylibrary.mil/OperationalEnvironment/Mid/OEFutureWarfareOntology#SustainableDevelopment -->

    <owl:Class rdf:about="http://www.ontologylibrary.mil/OperationalEnvironment/Mid/OEFutureWarfareOntology#SustainableDevelopment">
        <rdfs:subClassOf rdf:resource="http://www.ontologylibrary.mil/OperationalEnvironment/Mid/OEFutureWarfareOntology#PowerGenerationAndStorageControlledVocabulary"/>
        <obo:IAO_0000115>development that meets the needs of the present generation without compromising the ability of future generations to meet their own needs

Note 1 to entry: A key component of sustainability is continually increasing reductions in greenhouse gas emissions.</obo:IAO_0000115>
        <obo:IAO_0000119>International Organization for Standardization/International ISO 50007:2017

Technical Committee : ISO/TC 301  Energy management and energy savings

ICS :  27.015  Energy efficiency. Energy conservation in general

Energy services -- Guidelines for the assessment and improvement of the energy service to users

Publication date : 2017-06

1st Edition</obo:IAO_0000119>
    </owl:Class>
    


    <!-- http://www.ontologylibrary.mil/OperationalEnvironment/Mid/OEFutureWarfareOntology#SynergisticEffects -->

    <owl:Class rdf:about="http://www.ontologylibrary.mil/OperationalEnvironment/Mid/OEFutureWarfareOntology#SynergisticEffects">
        <rdfs:subClassOf rdf:resource="http://www.ontologylibrary.mil/OperationalEnvironment/Mid/OEFutureWarfareOntology#SpaceEnvironmentControlledVocabulary"/>
        <obo:IAO_0000115>effects appearing with the simultaneous or sequential impact of several space environment factors when the final effect is not equal to the sum of the effects from the individual factors</obo:IAO_0000115>
        <obo:IAO_0000119>International Organization for Standardization/International Electrotechnical Commission 17851:2016

Space systems -- Space environment simulation for material tests -- General principles and criteria

Publication Date: 2016-09

1st Edition</obo:IAO_0000119>
    </owl:Class>
    


    <!-- http://www.ontologylibrary.mil/OperationalEnvironment/Mid/OEFutureWarfareOntology#SyntheticBiology -->

    <owl:Class rdf:about="http://www.ontologylibrary.mil/OperationalEnvironment/Mid/OEFutureWarfareOntology#SyntheticBiology">
        <rdfs:subClassOf rdf:resource="http://www.ontologylibrary.mil/OperationalEnvironment/Mid/OEFutureWarfareOntology#CombatApplication"/>
        <obo:IAO_0000115>Engineering/modification of biological entities.

-Increased Crop Yield: Potential to reduce food scarcity

-Weaponization: Potential for micro-targeting, seek &amp; destroy microbes that can target DNA. Potentially accessible to super-empowered individuals.

-Medical Advances: Enhance soldier survivability

-Genetic Modification: Disease resistant, potentially designer babies and super athletes/soldiers. Synthetic DNA stores digital data. Data can be used for micro-targeting.

CRISPR: Genome Editing</obo:IAO_0000115>
        <obo:IAO_0000119>Potential Game Changers Infographic

7/11/2018</obo:IAO_0000119>
    </owl:Class>
    


    <!-- http://www.ontologylibrary.mil/OperationalEnvironment/Mid/OEFutureWarfareOntology#System -->

    <owl:Class rdf:about="http://www.ontologylibrary.mil/OperationalEnvironment/Mid/OEFutureWarfareOntology#System">
        <rdfs:subClassOf rdf:resource="http://purl.obolibrary.org/obo/BFO_0000141"/>
    </owl:Class>
    


    <!-- http://www.ontologylibrary.mil/OperationalEnvironment/Mid/OEFutureWarfareOntology#SystemOrchestrator -->

    <owl:Class rdf:about="http://www.ontologylibrary.mil/OperationalEnvironment/Mid/OEFutureWarfareOntology#SystemOrchestrator">
        <rdfs:subClassOf rdf:resource="http://www.ontologylibrary.mil/OperationalEnvironment/Mid/OEFutureWarfareOntology#BigDataRole"/>
        <obo:IAO_0000115>The System Orchestrator provides the overarching requirements that the system must fulfill, including policy, governance, architecture, resources, and business requirements, as well as monitoring or auditing activities to ensure that the system complies with those requirements. The System Orchestrator role provides system requirements, high-level design, and monitoring for the data system. While the role predates Big Data systems, some related design activities have changed within the Big Data paradigm.

The System Orchestrator role includes defining and integrating the required data application activities into an operational vertical system. Typically, the System Orchestrator involves a collection of more specific roles, performed by one or more actors, which manage and orchestrate the operation of the Big Data system. These actors may be human components, software components, or some combination of the two. The function of the System Orchestrator is to configure and manage the other components of the Big Data architecture to implement one or more workloads that the architecture is designed to execute. The workloads managed by the System Orchestrator may be assigning/provisioning framework components to individual physical or virtual nodes at the lower level, or providing a graphical user interface that supports the specification of workflows linking together multiple applications and components at the higher level. The System Orchestrator may also, through the Management Fabric, monitor the workloads and system to confirm that specific quality of service requirements are met for each workload, and may actually elastically assign and provision additional physical or virtual resources to meet workload requirements resulting from changes/surges in the data or number of users/transactions.</obo:IAO_0000115>
        <obo:IAO_0000119>NIST Big Data Interoperability Framework: Volume 6, Reference Architecture

Final Version 1 

NIST Big Data Public Working Group (NBD-PWG) Reference Architecture Subgroup Information Technology Laboratory</obo:IAO_0000119>
    </owl:Class>
    


    <!-- http://www.ontologylibrary.mil/OperationalEnvironment/Mid/OEFutureWarfareOntology#SystemsThatMove -->

    <owl:Class rdf:about="http://www.ontologylibrary.mil/OperationalEnvironment/Mid/OEFutureWarfareOntology#SystemsThatMove">
        <rdfs:subClassOf rdf:resource="http://www.ontologylibrary.mil/OperationalEnvironment/Mid/OEFutureWarfareOntology#FunctionalSystem"/>
        <obo:IAO_0000115>While most ground vehicles will continue to use the proven wheeled and tracked locomotion, a growing fraction of vehicles, especially the ground robots intended for operations in highly cluttered, broken terrain such as urban rubble and forests, will use legged locomotion. The advances of legged locomotion in the last decade have been remarkable and are likely to continue so; by 2050 it will be a fully proven, robust technology.</obo:IAO_0000115>
        <obo:IAO_0000119>Ground Warfare in 2050: How It Might Look 
 
by Alexander Kott 

Office of the Director, ARL 

US Army Research Laboratory</obo:IAO_0000119>
    </owl:Class>
    


    <!-- http://www.ontologylibrary.mil/OperationalEnvironment/Mid/OEFutureWarfareOntology#SystemsThatProtect -->

    <owl:Class rdf:about="http://www.ontologylibrary.mil/OperationalEnvironment/Mid/OEFutureWarfareOntology#SystemsThatProtect">
        <rdfs:subClassOf rdf:resource="http://www.ontologylibrary.mil/OperationalEnvironment/Mid/OEFutureWarfareOntology#FunctionalSystem"/>
    </owl:Class>
    


    <!-- http://www.ontologylibrary.mil/OperationalEnvironment/Mid/OEFutureWarfareOntology#SystemsThatSeeThinkCommunicate -->

    <owl:Class rdf:about="http://www.ontologylibrary.mil/OperationalEnvironment/Mid/OEFutureWarfareOntology#SystemsThatSeeThinkCommunicate">
        <rdfs:subClassOf rdf:resource="http://www.ontologylibrary.mil/OperationalEnvironment/Mid/OEFutureWarfareOntology#FunctionalSystem"/>
    </owl:Class>
    


    <!-- http://www.ontologylibrary.mil/OperationalEnvironment/Mid/OEFutureWarfareOntology#SystemsThatShoot -->

    <owl:Class rdf:about="http://www.ontologylibrary.mil/OperationalEnvironment/Mid/OEFutureWarfareOntology#SystemsThatShoot">
        <rdfs:subClassOf rdf:resource="http://www.ontologylibrary.mil/OperationalEnvironment/Mid/OEFutureWarfareOntology#FunctionalSystem"/>
    </owl:Class>
    


    <!-- http://www.ontologylibrary.mil/OperationalEnvironment/Mid/OEFutureWarfareOntology#SystemsThatSoldier -->

    <owl:Class rdf:about="http://www.ontologylibrary.mil/OperationalEnvironment/Mid/OEFutureWarfareOntology#SystemsThatSoldier">
        <rdfs:subClassOf rdf:resource="http://www.ontologylibrary.mil/OperationalEnvironment/Mid/OEFutureWarfareOntology#FunctionalSystem"/>
    </owl:Class>
    


    <!-- http://www.ontologylibrary.mil/OperationalEnvironment/Mid/OEFutureWarfareOntology#SystemsThatSupply -->

    <owl:Class rdf:about="http://www.ontologylibrary.mil/OperationalEnvironment/Mid/OEFutureWarfareOntology#SystemsThatSupply">
        <rdfs:subClassOf rdf:resource="http://www.ontologylibrary.mil/OperationalEnvironment/Mid/OEFutureWarfareOntology#FunctionalSystem"/>
    </owl:Class>
    


    <!-- http://www.ontologylibrary.mil/OperationalEnvironment/Mid/OEFutureWarfareOntology#SystemsThatUseQuantumEntanglement -->

    <owl:Class rdf:about="http://www.ontologylibrary.mil/OperationalEnvironment/Mid/OEFutureWarfareOntology#SystemsThatUseQuantumEntanglement">
        <rdfs:subClassOf rdf:resource="http://www.ontologylibrary.mil/OperationalEnvironment/Mid/OEFutureWarfareOntology#SystemsThatSeeThinkCommunicate"/>
        <obo:IAO_0000119>Projected breakthroughs in ways to measure, distribute, and exploit quantum entanglement will enable ultra-precise timing and time distribution, improved sensing, faster information processing, and new security in communications that are impossible by any other means. [SOURCE: ARL-TR-8283]</obo:IAO_0000119>
        <obo:IAO_0000119>Technology Environment of Ground Warfare in 2035-2050

Projections made in 2018 by ARL and TRADOC

[This is a draft outline of a potential document; prepared by Alexander Kott, the US Army Research Laboratory; July 2018]</obo:IAO_0000119>
    </owl:Class>
    


    <!-- http://www.ontologylibrary.mil/OperationalEnvironment/Mid/OEFutureWarfareOntology#Tariffs -->

    <owl:Class rdf:about="http://www.ontologylibrary.mil/OperationalEnvironment/Mid/OEFutureWarfareOntology#Tariffs">
        <rdfs:subClassOf rdf:resource="http://www.ontologylibrary.mil/OperationalEnvironment/Mid/OEFutureWarfareOntology#InternationalTrade"/>
        <obo:IAO_0000119>(1)

&quot;Tariffs&quot;, World Trade Organization

March 21, 2019

https://www.wto.org/english/tratop_e/tariffs_e/tariffs_e.htm</obo:IAO_0000119>
        <obo:IAO_0000119>(2)

Will Kenton, &quot;Tariff&quot;, Investopedia

February 16, 2019

https://www.investopedia.com/terms/t/tariff.asp</obo:IAO_0000119>
        <CommonCoreOntologies:definition>(1)

Customs duties on merchandise imports are called tariffs. Tariffs give a price advantage to locally-produced goods over similar goods which are imported, and they raise revenues for governments.</CommonCoreOntologies:definition>
        <CommonCoreOntologies:definition>(2)

Governments may impose tariffs to raise revenue or to protect domestic industries – particularly nascent ones – from foreign competition. By making foreign-produced goods more expensive, tariffs can make domestic-produced ones more attractive. By protecting these industries, governments can also protect jobs.</CommonCoreOntologies:definition>
        <rdfs:label>Tariffs</rdfs:label>
    </owl:Class>
    


    <!-- http://www.ontologylibrary.mil/OperationalEnvironment/Mid/OEFutureWarfareOntology#TechnologyEngineeringAndManufacturingControlledVocabulary -->

    <owl:Class rdf:about="http://www.ontologylibrary.mil/OperationalEnvironment/Mid/OEFutureWarfareOntology#TechnologyEngineeringAndManufacturingControlledVocabulary">
        <rdfs:subClassOf rdf:resource="http://www.ontologylibrary.mil/OperationalEnvironment/Mid/OEFutureWarfareOntology#ControlledVocabulary"/>
    </owl:Class>
    


    <!-- http://www.ontologylibrary.mil/OperationalEnvironment/Mid/OEFutureWarfareOntology#TechnologyEngineeringAndManufacturingTrend -->

    <owl:Class rdf:about="http://www.ontologylibrary.mil/OperationalEnvironment/Mid/OEFutureWarfareOntology#TechnologyEngineeringAndManufacturingTrend">
        <rdfs:subClassOf rdf:resource="http://www.ontologylibrary.mil/OperationalEnvironment/Mid/OEFutureWarfareOntology#Trend"/>
        <obo:IAO_0000115>The impact of the development of so many new and potential revolutionary technologies is made all the more disruptive by the convergence phenomenon.  Virtually every new technology is connected and intersecting to other new technologies and advances.  The example of the contemporary “smart phone”, which connects advances in cellular telephones with a camera, gaming, miniaturized computing and the Internet has completely transformed, and in many ways disrupted contemporary life.   Future convergences between various technological advances are likely to be equally disruptive and equally unpredictable, but the areas in which we foresee the most likely convergences are: 

 Biology and bio-engineering, to include optimizing human performance 

 Neurologic enhancement 

 Nanotechnology 

 Advanced Material Sciences 

 Quantum Computing 

 Artificial Intelligence 

 Robotics 

 Additive Manufacturing</obo:IAO_0000115>
        <obo:IAO_0000119>The Operational Environment and the Changing Character of Future Warfare</obo:IAO_0000119>
    </owl:Class>
    


    <!-- http://www.ontologylibrary.mil/OperationalEnvironment/Mid/OEFutureWarfareOntology#TensileStrength -->

    <owl:Class rdf:about="http://www.ontologylibrary.mil/OperationalEnvironment/Mid/OEFutureWarfareOntology#TensileStrength">
        <rdfs:subClassOf rdf:resource="http://www.ontologylibrary.mil/OperationalEnvironment/Mid/OEFutureWarfareOntology#SpaceSystems"/>
        <obo:IAO_0000115>power to resist tensile stress

Note 1 to entry: The tensile strength of brittle materials is about two orders of magnitude less than the tensile strength of metals.</obo:IAO_0000115>
        <obo:IAO_0000119>International Organization for Standardization/International Electrotechnical Commission 11227:2012

Space systems — Test procedure to evaluate spacecraft material ejecta upon hypervelocity impact

Publication Date: 2012-09

1st Edition</obo:IAO_0000119>
    </owl:Class>
    


    <!-- http://www.ontologylibrary.mil/OperationalEnvironment/Mid/OEFutureWarfareOntology#TensileStress -->

    <owl:Class rdf:about="http://www.ontologylibrary.mil/OperationalEnvironment/Mid/OEFutureWarfareOntology#TensileStress">
        <rdfs:subClassOf rdf:resource="http://www.ontologylibrary.mil/OperationalEnvironment/Mid/OEFutureWarfareOntology#SpaceSystems"/>
        <obo:IAO_0000115>stress on a material produced by pulling forces along an axis, which tends to extend or break the material</obo:IAO_0000115>
        <obo:IAO_0000119>International Organization for Standardization/International Electrotechnical Commission 11227:2012

Space systems — Test procedure to evaluate spacecraft material ejecta upon hypervelocity impact

Publication Date: 2012-09

1st Edition</obo:IAO_0000119>
    </owl:Class>
    


    <!-- http://www.ontologylibrary.mil/OperationalEnvironment/Mid/OEFutureWarfareOntology#Terrorism -->

    <owl:Class rdf:about="http://www.ontologylibrary.mil/OperationalEnvironment/Mid/OEFutureWarfareOntology#Terrorism">
        <rdfs:subClassOf rdf:resource="http://www.ontologylibrary.mil/OperationalEnvironment/Mid/OEFutureWarfareOntology#SecurityAndViolentConflict"/>
    </owl:Class>
    


    <!-- http://www.ontologylibrary.mil/OperationalEnvironment/Mid/OEFutureWarfareOntology#TheEraOfAcceleratedHumanProgress -->

    <owl:Class rdf:about="http://www.ontologylibrary.mil/OperationalEnvironment/Mid/OEFutureWarfareOntology#TheEraOfAcceleratedHumanProgress">
        <rdfs:subClassOf rdf:resource="http://purl.obolibrary.org/obo/BFO_0000038"/>
        <obo:IAO_0000115>The timeframe of 2017-2035, which relates to a period where our adversaries can take advantage of new technologies, involves new doctrine and revised strategic concepts to effectively challenge U.S. military forces across multiple domains. Our adversaries in some cases will have superior, or near equal capabilities bolstered by advantages in time, space, and perception, and when employed effectively – often in a hybrid and multidomain fashion – they can prevail over a U.S.-led force.  The Era of Accelerated Human Progress represents an evolutionary movement rooted in the present, but clearly advancing to a new state of affairs.</obo:IAO_0000115>
        <obo:IAO_0000119>The Operational Environment and the Changing Character of Future Warfare</obo:IAO_0000119>
    </owl:Class>
    


    <!-- http://www.ontologylibrary.mil/OperationalEnvironment/Mid/OEFutureWarfareOntology#TheEraOfContestedEquality -->

    <owl:Class rdf:about="http://www.ontologylibrary.mil/OperationalEnvironment/Mid/OEFutureWarfareOntology#TheEraOfContestedEquality">
        <rdfs:subClassOf rdf:resource="http://purl.obolibrary.org/obo/BFO_0000038"/>
        <obo:IAO_0000115>The timeframe of 2035-2050 is a period marked by significant breakthroughs in technology and convergences in terms of capabilities, which lead to significant changes in the character of warfare.  During this period, traditional aspects of warfare undergo dramatic, almost revolutionary changes which at the end of this timeframe may even challenge the very nature of warfare itself. In this era, no one actor is likely to have any long-term strategic or technological advantage, with aggregate power between the U.S. and its peer and near-peer rivals being equivalent, but not necessarily symmetric.  Prevailing in this period will depend on an ability to synchronize multi-domain capabilities against an artificial intelligence-enhanced adversary with an overarching capability to visualize and understand the battlespace at even greater ranges and velocities.</obo:IAO_0000115>
        <obo:IAO_0000119>The Operational Environment and the Changing Character of Future Warfare</obo:IAO_0000119>
    </owl:Class>
    


    <!-- http://www.ontologylibrary.mil/OperationalEnvironment/Mid/OEFutureWarfareOntology#ThinSupercapacitors -->

    <owl:Class rdf:about="http://www.ontologylibrary.mil/OperationalEnvironment/Mid/OEFutureWarfareOntology#ThinSupercapacitors">
        <rdfs:subClassOf rdf:resource="http://www.ontologylibrary.mil/OperationalEnvironment/Mid/OEFutureWarfareOntology#PowerSystems"/>
        <obo:IAO_0000115>Store exponentially more energy and recharge faster. [SOURCE: TRADOC G-2 Potential Game Changers, May 2018]</obo:IAO_0000115>
        <obo:IAO_0000119>Technology Environment of Ground Warfare in 2035-2050

Projections made in 2018 by ARL and TRADOC

[This is a draft outline of a potential document; prepared by Alexander Kott, the US Army Research Laboratory; July 2018]</obo:IAO_0000119>
    </owl:Class>
    


    <!-- http://www.ontologylibrary.mil/OperationalEnvironment/Mid/OEFutureWarfareOntology#Threat -->

    <owl:Class rdf:about="http://www.ontologylibrary.mil/OperationalEnvironment/Mid/OEFutureWarfareOntology#Threat">
        <rdfs:subClassOf rdf:resource="http://www.ontologylibrary.mil/OperationalEnvironment/Mid/OEFutureWarfareOntology#CyberSecurityControlledVocabulary"/>
        <obo:IAO_0000115>potential cause of an unwanted incident, which can result in harm to a system or organization (3.50)</obo:IAO_0000115>
        <obo:IAO_0000119>International Organization for Standardization/International Electrotechnical Commission 27000:2018

Security techniques — Information security management systems — Overview and vocabulary

Publication date : 2018-02

5th Edition</obo:IAO_0000119>
    </owl:Class>
    


    <!-- http://www.ontologylibrary.mil/OperationalEnvironment/Mid/OEFutureWarfareOntology#TopManagement -->

    <owl:Class rdf:about="http://www.ontologylibrary.mil/OperationalEnvironment/Mid/OEFutureWarfareOntology#TopManagement">
        <rdfs:subClassOf rdf:resource="http://www.ontologylibrary.mil/OperationalEnvironment/Mid/OEFutureWarfareOntology#CyberSecurityControlledVocabulary"/>
        <obo:IAO_0000115>person or group of people who directs and controls an organization (3.50) at the highest level

Note 1 to entry: Top management has the power to delegate authority and provide resources within the organization.

Note 2 to entry: If the scope of the management system (3.41) covers only part of an organization, then top management refers to those who direct and control that part of the organization.

Note 3 to entry: Top management is sometimes called executive management and can include Chief Executive Officers, Chief Financial Officers, Chief Information Officers, and similar roles.</obo:IAO_0000115>
        <obo:IAO_0000119>International Organization for Standardization/International Electrotechnical Commission 27000:2018

Security techniques — Information security management systems — Overview and vocabulary

Publication date : 2018-02

5th Edition</obo:IAO_0000119>
    </owl:Class>
    


    <!-- http://www.ontologylibrary.mil/OperationalEnvironment/Mid/OEFutureWarfareOntology#TradeAgreement -->

    <owl:Class rdf:about="http://www.ontologylibrary.mil/OperationalEnvironment/Mid/OEFutureWarfareOntology#TradeAgreement">
        <rdfs:subClassOf rdf:resource="http://www.ontologylibrary.mil/OperationalEnvironment/Mid/OEFutureWarfareOntology#InternationalTrade"/>
        <obo:IAO_0000119>Letricia Dixon &amp; Editors of Encyclopaedia Britannica, &quot;Trade Agreement&quot;, Encyclopaedia Britannica

March 21, 2019

https://www.britannica.com/topic/trade-agreement</obo:IAO_0000119>
        <CommonCoreOntologies:definition>Trade agreements are one way to reduce [trade] barriers, thereby opening all parties to the benefits of increased trade.

...

Even without the constraints imposed by most-favoured-nation and national treatment clauses, sometimes general multilateral agreements are easier to reach than separate bilateral agreements. In many cases the possible loss from a concession to one country is almost as great as that which would result from a similar concession to many countries. The gains that the most efficient producers realize from worldwide tariff reductions are large enough to warrant substantial concessions.</CommonCoreOntologies:definition>
        <rdfs:label>Trade Agreement</rdfs:label>
    </owl:Class>
    


    <!-- http://www.ontologylibrary.mil/OperationalEnvironment/Mid/OEFutureWarfareOntology#Transhumanism -->

    <owl:Class rdf:about="http://www.ontologylibrary.mil/OperationalEnvironment/Mid/OEFutureWarfareOntology#Transhumanism">
        <rdfs:subClassOf rdf:resource="http://www.ontologylibrary.mil/OperationalEnvironment/Mid/OEFutureWarfareOntology#ArtificialIntelligenceControlledVocabulary"/>
        <obo:IAO_0000115>A movement whose followers want to reach the “post-human” condition by eliminating disabilities, suffering, illness, ageing and death, through the “NBIC convergence” (the convergence of nanotechnology, biotechnology, information technology and cognitive science). They promote the use of human cloning, virtual reality*, hybridization between humans and machines and mind uploading*. Their opponents accuse them of excessive speculation, of founding a new mystical order which idolizes technology, and of fantasizing about a “superhuman” with eugenicist overtones.</obo:IAO_0000115>
        <obo:IAO_0000119>United Nations Educational, Scientific, and Cultural Organization Courier 

March 2018

https://en.unesco.org/courier/2018-3/lexicon-artificial-intelligence</obo:IAO_0000119>
    </owl:Class>
    


    <!-- http://www.ontologylibrary.mil/OperationalEnvironment/Mid/OEFutureWarfareOntology#Trend -->

    <owl:Class rdf:about="http://www.ontologylibrary.mil/OperationalEnvironment/Mid/OEFutureWarfareOntology#Trend">
        <rdfs:subClassOf rdf:resource="http://purl.obolibrary.org/obo/BFO_0000015"/>
    </owl:Class>
    


    <!-- http://www.ontologylibrary.mil/OperationalEnvironment/Mid/OEFutureWarfareOntology#TrustedInformationCommunicationEntity -->

    <owl:Class rdf:about="http://www.ontologylibrary.mil/OperationalEnvironment/Mid/OEFutureWarfareOntology#TrustedInformationCommunicationEntity">
        <rdfs:subClassOf rdf:resource="http://www.ontologylibrary.mil/OperationalEnvironment/Mid/OEFutureWarfareOntology#CyberSecurityControlledVocabulary"/>
        <obo:IAO_0000115>autonomous organization (3.50) supporting information exchange within an information sharing community (3.34)</obo:IAO_0000115>
        <obo:IAO_0000119>International Organization for Standardization/International Electrotechnical Commission 27000:2018

Security techniques — Information security management systems — Overview and vocabulary

Publication date : 2018-02

5th Edition</obo:IAO_0000119>
    </owl:Class>
    


    <!-- http://www.ontologylibrary.mil/OperationalEnvironment/Mid/OEFutureWarfareOntology#TurbineInletTemperature -->

    <owl:Class rdf:about="http://www.ontologylibrary.mil/OperationalEnvironment/Mid/OEFutureWarfareOntology#TurbineInletTemperature">
        <rdfs:subClassOf rdf:resource="http://www.ontologylibrary.mil/OperationalEnvironment/Mid/OEFutureWarfareOntology#GasEnergyGeneration"/>
        <obo:IAO_0000115>mean temperature of the working fluid upstream of the first stage turbine stator blades</obo:IAO_0000115>
        <obo:IAO_0000119>International Organization for Standardization/International ISO 19859:2016

Technical Committee : ISO/TC 192  Gas turbines

ICS :  29.160.99  Other standards related to rotating machinery 27.040  Gas and steam turbines. Steam engines

Gas turbine applications -- Requirements for power generation

Publication date : 2016-08

1st Edition</obo:IAO_0000119>
    </owl:Class>
    


    <!-- http://www.ontologylibrary.mil/OperationalEnvironment/Mid/OEFutureWarfareOntology#Two-partySystem -->

    <owl:Class rdf:about="http://www.ontologylibrary.mil/OperationalEnvironment/Mid/OEFutureWarfareOntology#Two-partySystem">
        <rdfs:subClassOf rdf:resource="http://www.ontologylibrary.mil/OperationalEnvironment/Mid/OEFutureWarfareOntology#PoliticalPartySystem"/>
        <obo:IAO_0000115>A two-party system is a party system where two major political parties dominate the government. One of the two parties typically holds a majority in the legislature and is usually referred to as the majority or governing party while the other is the minority or opposition party. Around the world, the term has different senses. [In some countries], the sense of two-party system describes an arrangement in which all or nearly all elected officials belong to one of the only two major parties, and third parties rarely win any seats in the legislature. In such arrangements, two-party systems are thought to result from various factors like winner-takes-all election rules. In such systems, while chances for third-party candidates winning election to major national office are remote, it is possible for groups within the larger parties, or in opposition to one or both of them, to exert influence on the two major parties. In contrast, in [some] parliamentary systems and elsewhere, the term two-party system is sometimes used to indicate an arrangement in which two major parties dominate elections but in which there are viable third parties which do win seats in the legislature, and in which the two major parties exert proportionately greater influence than their percentage of votes would suggest.</obo:IAO_0000115>
        <obo:IAO_0000119>&quot;Two-party System&quot;, Wikipedia

March 12, 2019

https://en.wikipedia.org/wiki/Two-party_system</obo:IAO_0000119>
        <rdfs:label>Two-party System</rdfs:label>
    </owl:Class>
    


    <!-- http://www.ontologylibrary.mil/OperationalEnvironment/Mid/OEFutureWarfareOntology#Uncertainty -->

    <owl:Class rdf:about="http://www.ontologylibrary.mil/OperationalEnvironment/Mid/OEFutureWarfareOntology#Uncertainty">
        <rdfs:subClassOf rdf:resource="http://www.ontologylibrary.mil/OperationalEnvironment/Mid/OEFutureWarfareOntology#ClimateChangeAndResourceCompetitionControlledVocabulary"/>
        <obo:IAO_0000115>parameter associated with the result of quantification that characterizes the dispersion of the values that could be reasonably attributed to the quantified amount

Note 1 to entry: Uncertainty information typically specifies quantitative estimates of the likely dispersion of values and a qualitative description of the likely causes of the dispersion.</obo:IAO_0000115>
        <obo:IAO_0000119>International Organization for Standardization/International Electrotechnical Commission 27000:2018

Technical Committee : ISO/TC 207/SC 7  Greenhouse gas management and related activities

ICS :  13.020.40  Pollution, pollution control and conservation

Greenhouse gases -- Part 1: Specification with guidance at the organization level for quantification and reporting of greenhouse gas emissions and removals 

Publication date : 2018-12

2nd Edition</obo:IAO_0000119>
    </owl:Class>
    


    <!-- http://www.ontologylibrary.mil/OperationalEnvironment/Mid/OEFutureWarfareOntology#UnemploymentBenefits -->

    <owl:Class rdf:about="http://www.ontologylibrary.mil/OperationalEnvironment/Mid/OEFutureWarfareOntology#UnemploymentBenefits">
        <rdfs:subClassOf rdf:resource="http://www.ontologylibrary.mil/OperationalEnvironment/Mid/OEFutureWarfareOntology#WelfareState"/>
        <obo:IAO_0000119>Julia Kagan, &quot;Unemployment Compensatin&quot;, Investopedia

Feb 23, 2018

https://www.investopedia.com/terms/u/unemployment-compensation.asp</obo:IAO_0000119>
        <CommonCoreOntologies:definition>Unemployment compensation is paid by the state to unemployed workers who have lost their jobs due to layoffs or retrenchment. Unemployment compensation is meant to provide a source of income for jobless workers until they can find employment. In order to be eligible for it, certain criteria must be satisfied by an unemployed worker, such as having worked for a minimum stipulated period and actively looking for employment. Unemployment compensation provides partial income replacement..... It&apos;s also known as unemployment insurance or unemployment benefits.</CommonCoreOntologies:definition>
        <rdfs:label>Unemployment Benefits</rdfs:label>
    </owl:Class>
    


    <!-- http://www.ontologylibrary.mil/OperationalEnvironment/Mid/OEFutureWarfareOntology#UnmannedAirVehicles -->

    <owl:Class rdf:about="http://www.ontologylibrary.mil/OperationalEnvironment/Mid/OEFutureWarfareOntology#UnmannedAirVehicles">
        <rdfs:subClassOf rdf:resource="http://www.ontologylibrary.mil/OperationalEnvironment/Mid/OEFutureWarfareOntology#SystemsThatMove"/>
        <obo:IAO_0000115>Multiple combat vehicles will generate collaborative real-time AI-generated courses of action; with explanations, 90% understood by Soldier teams; with rationale provided by AI agents to improve Soldier decisions 80% of the time [SOURCE: ARL ERP documents]</obo:IAO_0000115>
        <obo:IAO_0000119>Technology Environment of Ground Warfare in 2035-2050

Projections made in 2018 by ARL and TRADOC

[This is a draft outline of a potential document; prepared by Alexander Kott, the US Army Research Laboratory; July 2018]</obo:IAO_0000119>
    </owl:Class>
    


    <!-- http://www.ontologylibrary.mil/OperationalEnvironment/Mid/OEFutureWarfareOntology#UnmannedGroundVehicles -->

    <owl:Class rdf:about="http://www.ontologylibrary.mil/OperationalEnvironment/Mid/OEFutureWarfareOntology#UnmannedGroundVehicles">
        <rdfs:subClassOf rdf:resource="http://www.ontologylibrary.mil/OperationalEnvironment/Mid/OEFutureWarfareOntology#SystemsThatMove"/>
        <obo:IAO_0000115>Multiple combat vehicles will generate collaborative real-time AI-generated courses of action; with explanations, 90% understood by Soldier teams; with rationale provided by AI agents to improve Soldier decisions 80% of the time [SOURCE: ARL ERP documents]</obo:IAO_0000115>
        <obo:IAO_0000119>Technology Environment of Ground Warfare in 2035-2050

Projections made in 2018 by ARL and TRADOC

[This is a draft outline of a potential document; prepared by Alexander Kott, the US Army Research Laboratory; July 2018]</obo:IAO_0000119>
    </owl:Class>
    


    <!-- http://www.ontologylibrary.mil/OperationalEnvironment/Mid/OEFutureWarfareOntology#UnstructuredData -->

    <owl:Class rdf:about="http://www.ontologylibrary.mil/OperationalEnvironment/Mid/OEFutureWarfareOntology#UnstructuredData">
        <rdfs:subClassOf rdf:resource="http://www.ontologylibrary.mil/OperationalEnvironment/Mid/OEFutureWarfareOntology#BigDataControlledVocabulary"/>
        <obo:IAO_0000115>Unstructured data has been increasing in both volume and prominence. While relational databases tend to have support for these types of data elements, their ability to directly analyse, index, and process them has tended to be both limited and accessed via non-standard SQL extensions. The need to analyse unstructured data has been present for many years. However, the big data paradigm shift has increased the emphasis on the value of unstructured data. Unstructured data also places an emphasis on new and different engineering methods that can analyse such data more efficiently.</obo:IAO_0000115>
        <obo:IAO_0000115>data (3.1.5) which are characterized by not having any structure apart from that record or file level”</obo:IAO_0000115>
        <obo:IAO_0000119>Information technology — Big data — Overview and vocabulary

https://www.iso.org/jtc1</obo:IAO_0000119>
    </owl:Class>
    


    <!-- http://www.ontologylibrary.mil/OperationalEnvironment/Mid/OEFutureWarfareOntology#UrbanSprawl -->

    <owl:Class rdf:about="http://www.ontologylibrary.mil/OperationalEnvironment/Mid/OEFutureWarfareOntology#UrbanSprawl">
        <rdfs:subClassOf rdf:resource="http://www.ontologylibrary.mil/OperationalEnvironment/Mid/OEFutureWarfareOntology#Urbanization"/>
        <obo:IAO_0000119>&quot;What Is Urban Sprawl?&quot;, Conserve Energy Future

March 26, 2019

https://www.conserve-energy-future.com/causes-and-effects-of-urban-sprawl.php</obo:IAO_0000119>
        <CommonCoreOntologies:definition>[Urban sprawl] refers to the migration of a population from populated towns and cities to low density residential development over more and more rural land.
 ...

...[Urban] sprawl is defined as low density residential and commercial development on undeveloped land.</CommonCoreOntologies:definition>
        <rdfs:label>Urban Sprawl</rdfs:label>
    </owl:Class>
    


    <!-- http://www.ontologylibrary.mil/OperationalEnvironment/Mid/OEFutureWarfareOntology#Urbanization -->

    <owl:Class rdf:about="http://www.ontologylibrary.mil/OperationalEnvironment/Mid/OEFutureWarfareOntology#Urbanization">
        <rdfs:subClassOf rdf:resource="http://www.ontologylibrary.mil/OperationalEnvironment/Mid/OEFutureWarfareOntology#Demographics"/>
        <obo:IAO_0000119>Josy O&apos;Donnel, &quot;What is Urbanization and What are the Positive and Negative Effects?, Conservation Institute

April 30, 2018

https://www.conservationinstitute.org/what-is-urbanization/</obo:IAO_0000119>
        <CommonCoreOntologies:definition>Urbanization is when people move from rural farmland to cities and towns. Rural areas are more densely packed and offer greater opportunities to their residents in the form of higher paying jobs and a larger variety of job opportunities.

Most developing countries experience the process of urbanization, especially once they start becoming industrialized. Cities and towns become hubs of trade and culture, and more people start moving out of the country to gain access to some of these social and financial benefits.

Urbanization is a natural part of developing society, but it has its downside as well. As populations in cities and towns rise, they expand and eventually invade rural areas. We need to strike a balance with urbanization if we want to flourish as a society.

...

Urban areas have more jobs to offer and can lure people out of rural areas with the promise of a better life and a higher-paying salary. People find more jobs in virtually every industry while looking in cities and towns than they do searching rural locations.

There are more people in urban areas, which means there is more demand. The increased demand opens the door to employment opportunities for a lot of people who can’t find a job in their rural hometown.</CommonCoreOntologies:definition>
        <rdfs:label>Urbanization</rdfs:label>
    </owl:Class>
    


    <!-- http://www.ontologylibrary.mil/OperationalEnvironment/Mid/OEFutureWarfareOntology#Validation -->

    <owl:Class rdf:about="http://www.ontologylibrary.mil/OperationalEnvironment/Mid/OEFutureWarfareOntology#Validation">
        <rdfs:subClassOf rdf:resource="http://www.ontologylibrary.mil/OperationalEnvironment/Mid/OEFutureWarfareOntology#ClimateChangeAndResourceCompetitionControlledVocabulary"/>
        <obo:IAO_0000115>process for evaluating the reasonableness of the assumptions, limitations and methods that support a statement about the outcome of future activities</obo:IAO_0000115>
        <obo:IAO_0000119>International Organization for Standardization/International Electrotechnical Commission 27000:2018

Technical Committee : ISO/TC 207/SC 7  Greenhouse gas management and related activities

ICS :  13.020.40  Pollution, pollution control and conservation

Greenhouse gases -- Part 1: Specification with guidance at the organization level for quantification and reporting of greenhouse gas emissions and removals 

Publication date : 2018-12

2nd Edition</obo:IAO_0000119>
    </owl:Class>
    


    <!-- http://www.ontologylibrary.mil/OperationalEnvironment/Mid/OEFutureWarfareOntology#Validator -->

    <owl:Class rdf:about="http://www.ontologylibrary.mil/OperationalEnvironment/Mid/OEFutureWarfareOntology#Validator">
        <rdfs:subClassOf rdf:resource="http://www.ontologylibrary.mil/OperationalEnvironment/Mid/OEFutureWarfareOntology#ClimateChangeAndResourceCompetitionControlledVocabulary"/>
        <obo:IAO_0000115>competent and impartial person with responsibility for performing and reporting on a validation (3.4.10)</obo:IAO_0000115>
        <obo:IAO_0000119>International Organization for Standardization/International Electrotechnical Commission 27000:2018

Technical Committee : ISO/TC 207/SC 7  Greenhouse gas management and related activities

ICS :  13.020.40  Pollution, pollution control and conservation

Greenhouse gases -- Part 1: Specification with guidance at the organization level for quantification and reporting of greenhouse gas emissions and removals 

Publication date : 2018-12

2nd Edition</obo:IAO_0000119>
    </owl:Class>
    


    <!-- http://www.ontologylibrary.mil/OperationalEnvironment/Mid/OEFutureWarfareOntology#Verification -->

    <owl:Class rdf:about="http://www.ontologylibrary.mil/OperationalEnvironment/Mid/OEFutureWarfareOntology#Verification">
        <rdfs:subClassOf rdf:resource="http://www.ontologylibrary.mil/OperationalEnvironment/Mid/OEFutureWarfareOntology#ClimateChangeAndResourceCompetitionControlledVocabulary"/>
        <obo:IAO_0000115>process for evaluating a statement of historical data and information to determine if the statement is materially correct and conforms to criteria</obo:IAO_0000115>
        <obo:IAO_0000119>International Organization for Standardization/International Electrotechnical Commission 27000:2018

Technical Committee : ISO/TC 207/SC 7  Greenhouse gas management and related activities

ICS :  13.020.40  Pollution, pollution control and conservation

Greenhouse gases -- Part 1: Specification with guidance at the organization level for quantification and reporting of greenhouse gas emissions and removals 

Publication date : 2018-12

2nd Edition</obo:IAO_0000119>
    </owl:Class>
    


    <!-- http://www.ontologylibrary.mil/OperationalEnvironment/Mid/OEFutureWarfareOntology#Verifier -->

    <owl:Class rdf:about="http://www.ontologylibrary.mil/OperationalEnvironment/Mid/OEFutureWarfareOntology#Verifier">
        <rdfs:subClassOf rdf:resource="http://www.ontologylibrary.mil/OperationalEnvironment/Mid/OEFutureWarfareOntology#ClimateChangeAndResourceCompetitionControlledVocabulary"/>
        <obo:IAO_0000115>competent and impartial person with responsibility for performing and reporting on a verification (3.4.9)</obo:IAO_0000115>
        <obo:IAO_0000119>International Organization for Standardization/International Electrotechnical Commission 27000:2018

Technical Committee : ISO/TC 207/SC 7  Greenhouse gas management and related activities

ICS :  13.020.40  Pollution, pollution control and conservation

Greenhouse gases -- Part 1: Specification with guidance at the organization level for quantification and reporting of greenhouse gas emissions and removals 

Publication date : 2018-12

2nd Edition</obo:IAO_0000119>
    </owl:Class>
    


    <!-- http://www.ontologylibrary.mil/OperationalEnvironment/Mid/OEFutureWarfareOntology#VerticalScaling -->

    <owl:Class rdf:about="http://www.ontologylibrary.mil/OperationalEnvironment/Mid/OEFutureWarfareOntology#VerticalScaling">
        <rdfs:subClassOf rdf:resource="http://www.ontologylibrary.mil/OperationalEnvironment/Mid/OEFutureWarfareOntology#BigDataControlledVocabulary"/>
        <obo:IAO_0000115>act of increasing the performance of data processing through improvements to processors, memory, storage, or connectivity

Note 1 to entry: Vertical scaling for increasing performance is also referred to as scale-up.</obo:IAO_0000115>
        <obo:IAO_0000119>Information technology — Big data — Overview and vocabulary

https://www.iso.org/jtc1</obo:IAO_0000119>
    </owl:Class>
    


    <!-- http://www.ontologylibrary.mil/OperationalEnvironment/Mid/OEFutureWarfareOntology#ViolentProtest -->

    <owl:Class rdf:about="http://www.ontologylibrary.mil/OperationalEnvironment/Mid/OEFutureWarfareOntology#ViolentProtest">
        <rdfs:subClassOf rdf:resource="http://www.ontologylibrary.mil/OperationalEnvironment/Mid/OEFutureWarfareOntology#SubstateConflict"/>
    </owl:Class>
    


    <!-- http://www.ontologylibrary.mil/OperationalEnvironment/Mid/OEFutureWarfareOntology#VolumeImpactFactors -->

    <owl:Class rdf:about="http://www.ontologylibrary.mil/OperationalEnvironment/Mid/OEFutureWarfareOntology#VolumeImpactFactors">
        <rdfs:subClassOf rdf:resource="http://www.ontologylibrary.mil/OperationalEnvironment/Mid/OEFutureWarfareOntology#SpaceEnvironmentControlledVocabulary"/>
        <obo:IAO_0000112>EXAMPLE:Particles of Earth’s radiation belts, galactic cosmic rays, solar energetic particles, meteoroids and others.</obo:IAO_0000112>
        <obo:IAO_0000115>space factors causing changes in bulk materials (in depths more than 0,1 mm to 1 mm)</obo:IAO_0000115>
        <obo:IAO_0000119>International Organization for Standardization/International Electrotechnical Commission 17851:2016

Space systems -- Space environment simulation for material tests -- General principles and criteria

Publication Date: 2016-09

1st Edition</obo:IAO_0000119>
    </owl:Class>
    


    <!-- http://www.ontologylibrary.mil/OperationalEnvironment/Mid/OEFutureWarfareOntology#Vulnerability -->

    <owl:Class rdf:about="http://www.ontologylibrary.mil/OperationalEnvironment/Mid/OEFutureWarfareOntology#Vulnerability">
        <rdfs:subClassOf rdf:resource="http://www.ontologylibrary.mil/OperationalEnvironment/Mid/OEFutureWarfareOntology#CyberSecurityControlledVocabulary"/>
        <obo:IAO_0000115>weakness of an asset or control (3.14) that can be exploited by one or more threats (3.74)</obo:IAO_0000115>
        <obo:IAO_0000119>International Organization for Standardization/International Electrotechnical Commission 27000:2018

Security techniques — Information security management systems — Overview and vocabulary

Publication date : 2018-02

5th Edition</obo:IAO_0000119>
    </owl:Class>
    


    <!-- http://www.ontologylibrary.mil/OperationalEnvironment/Mid/OEFutureWarfareOntology#WeakAI -->

    <owl:Class rdf:about="http://www.ontologylibrary.mil/OperationalEnvironment/Mid/OEFutureWarfareOntology#WeakAI">
        <rdfs:subClassOf rdf:resource="http://www.ontologylibrary.mil/OperationalEnvironment/Mid/OEFutureWarfareOntology#ArtificialIntelligenceControlledVocabulary"/>
        <obo:IAO_0000115>Weak AI or Artificial Narrow Intelligence (ANI) is the only form of AI that humanity has achieved so far – machines that are capable of performing certain precise tasks autonomously but without consciousness, within a framework defined by humans and following decisions taken by humans alone.</obo:IAO_0000115>
        <obo:IAO_0000119>United Nations Educational, Scientific, and Cultural Organization Courier 

March 2018

https://en.unesco.org/courier/2018-3/lexicon-artificial-intelligence</obo:IAO_0000119>
    </owl:Class>
    


    <!-- http://www.ontologylibrary.mil/OperationalEnvironment/Mid/OEFutureWarfareOntology#WeaponizationOfSyntheticBiology -->

    <owl:Class rdf:about="http://www.ontologylibrary.mil/OperationalEnvironment/Mid/OEFutureWarfareOntology#WeaponizationOfSyntheticBiology">
        <rdfs:subClassOf rdf:resource="http://www.ontologylibrary.mil/OperationalEnvironment/Mid/OEFutureWarfareOntology#SystemsThatSoldier"/>
        <obo:IAO_0000115>Synthetic Biology - Weaponization: Potential for micro-targeting, Seek &amp; destroy microbes that can target DNA. Potentially accessible to super-empowered individuals. [SOURCE: TRADOC G-2 Potential Game Changers, May 2018]</obo:IAO_0000115>
        <obo:IAO_0000119>Technology Environment of Ground Warfare in 2035-2050

Projections made in 2018 by ARL and TRADOC

[This is a draft outline of a potential document; prepared by Alexander Kott, the US Army Research Laboratory; July 2018]</obo:IAO_0000119>
    </owl:Class>
    


    <!-- http://www.ontologylibrary.mil/OperationalEnvironment/Mid/OEFutureWarfareOntology#WelfareState -->

    <owl:Class rdf:about="http://www.ontologylibrary.mil/OperationalEnvironment/Mid/OEFutureWarfareOntology#WelfareState">
        <rdfs:subClassOf rdf:resource="http://www.ontologylibrary.mil/OperationalEnvironment/Mid/OEFutureWarfareOntology#EconomicsAndTrade"/>
        <obo:IAO_0000119>Peter Bondarenko &amp; Editors of Encyclopaedia Britannica, &quot;Welfare State&quot;, Encyclopaedia Britannica

March 22, 2019

https://www.britannica.com/topic/welfare-state</obo:IAO_0000119>
        <CommonCoreOntologies:definition>Welfare state, concept of government in which the state or a well-established network of social institutions plays a key role in the protection and promotion of the economic and social well-being of citizens. It is based on the principles of equality of opportunity, equitable distribution of wealth, and public responsibility for those unable to avail themselves of the minimal provisions for a good life. The general term may cover a variety of forms of economic and social organization.

A fundamental feature of the welfare state is social insurance, a provision common to most advanced industrialized countries.... Such insurance is usually financed by compulsory contributions and is intended to provide benefits to persons and families during periods of greatest need. It is widely recognized, however, that in practice the cash benefits fall considerably short of the levels intended by the designers of the plans.

The welfare state also usually includes public provision of basic education, health services, and housing (in some cases at low cost or without charge).

...

Antipoverty programs and the system of personal taxation may also be regarded as aspects of the welfare state. Personal taxation falls into this category insofar as its progressivity is used to achieve greater justice in income distribution (rather than merely to raise revenue) and also insofar as it used to finance social insurance payments and other benefits not completely financed by compulsory contributions. In socialist countries the welfare state also covers employment and administration of consumer prices.</CommonCoreOntologies:definition>
        <rdfs:label>Welfare State</rdfs:label>
    </owl:Class>
    


    <!-- http://www.ontologylibrary.mil/OperationalEnvironment/Mid/OEFutureWarfareOntology#WitnessPlate -->

    <owl:Class rdf:about="http://www.ontologylibrary.mil/OperationalEnvironment/Mid/OEFutureWarfareOntology#WitnessPlate">
        <rdfs:subClassOf rdf:resource="http://www.ontologylibrary.mil/OperationalEnvironment/Mid/OEFutureWarfareOntology#SpaceSystems"/>
        <obo:IAO_0000115>flat sheet of ductile material used in impact experiments to capture ejecta and characterize the resulting damage</obo:IAO_0000115>
        <obo:IAO_0000119>International Organization for Standardization/International Electrotechnical Commission 11227:2012

Space systems — Test procedure to evaluate spacecraft material ejecta upon hypervelocity impact

Publication Date: 2012-09

1st Edition</obo:IAO_0000119>
    </owl:Class>
    


    <!-- http://www.ontologylibrary.mil/OperationalEnvironment/Mid/OEFutureWarfareOntology#Research&amp;Analysis -->

    <owl:Class rdf:about="http://www.ontologylibrary.mil/OperationalEnvironment/Mid/OEFutureWarfareOntology#Research&amp;Analysis">
        <rdfs:subClassOf rdf:resource="http://www.ontologylibrary.mil/OperationalEnvironment/Mid/OEFutureWarfareOntology#FaultLineMethodology"/>
        <obo:IAO_0000115>Fault Lines Analysis provides the command with an understanding of the most exploitable sources of instability in the OE. The Fault Lines Analysis Methodology is based on co-created analysis:  research and analysis conducted as a team. There are 3 distinct stages to the team research and analysis process:  Analysis 1 (A1), Analysis (A2), and Analysis 3 (A3). A1 reviews and develops categories from source text by assigning relevant words, phrases or labels to significant portions of the text.  These categories become the foundation for early analysis.  A2 organizes the categories around themes based on the relationship of ideas developed from the comparisons and analytic memos. A3 generates plausible explanations and responses to the research question (becoming assumptions or hypotheses tested in the next stage).  Each analysis stage builds on the analysis of the previous stage(s). The evolution of sound analytic explanation occurs through a systematic and defensible inductive research process. The independent stages are inductively generated to be later deductively tested by a pool of SMEs in an OE.  GCKN is available to assist with the research process.</obo:IAO_0000115>
        <obo:IAO_0000119>Fault Lines Methodology Infographic</obo:IAO_0000119>
    </owl:Class>
    


    <!-- http://www.ontologyrepository.com/CommonCoreOntologies/Algorithm -->

    <owl:Class rdf:about="http://www.ontologyrepository.com/CommonCoreOntologies/Algorithm">
        <rdfs:subClassOf rdf:resource="http://www.ontologylibrary.mil/OperationalEnvironment/Mid/OEFutureWarfareOntology#ArtificialIntelligenceControlledVocabulary"/>
    </owl:Class>
    


    <!-- http://www.ontologyrepository.com/CommonCoreOntologies/DescriptiveInformationContentEntity -->

    <owl:Class rdf:about="http://www.ontologyrepository.com/CommonCoreOntologies/DescriptiveInformationContentEntity"/>
</rdf:RDF>



<!-- Generated by the OWL API (version 4.5.7.2018-12-02T02:23:35Z) https://github.com/owlcs/owlapi -->

